<?xml version="1.0" encoding="UTF-8"?>
<!DOCTYPE rdf:RDF [
	<!ENTITY xsd "http://www.w3.org/2001/XMLSchema#">
	<!ENTITY owl "http://www.w3.org/2002/07/owl#">
	<!ENTITY rdf "http://www.w3.org/1999/02/22-rdf-syntax-ns#">
	<!ENTITY rdfs "http://www.w3.org/2000/01/rdf-schema#">
	<!ENTITY	xs "http://www.w3.org/2001/XMLSchema#">
	<!ENTITY	mei "http://www.music-encoding.org/ns/mei">
	<!ENTITY	xlink "http://www.w3.org/1999/xlink#">
	<!ENTITY	xml "http://www.w3.org/XML/1998/namespace#">
]>
<rdf:RDF xmlns:xs="http://www.w3.org/2001/XMLSchema#" xmlns:mei="http://www.music-encoding.org/ns/mei" xmlns:xlink="http://www.w3.org/1999/xlink#"  xmlns:owl="&owl;" xmlns:rdf="&rdf;" xmlns:rdfs="&rdfs;" >
	<owl:Ontology rdf:about="">
		<!--	#################################################################################################################	-->
		<!--	The imported and included files in the xsd follow - Should be double-checked for existence and if they should be imported using owl:imports.	-->
		<!--	#################################################################################################################	-->
		<!--	<import namespace="http://www.w3.org/1999/xlink" schemaLocation="xlink.xsd"/>	-->
		<!--	<import namespace="http://www.w3.org/XML/1998/namespace" schemaLocation="http://www.w3.org/2004/10/xml.xsd"/>	-->
		<!--	#####################################################################################	-->
		<!--	In the "datatypes" entity, we refer to the file with the simple datatypes produced from the original schema.	-->
		<!--	#####################################################################################	-->
		</owl:Ontology>
	<!--	Datatype Definitions	-->
		<rdfs:Datatype rdf:about="&xsd;ID">
		<rdfs:isDefinedBy rdf:resource="&xsd;"/>
		<rdfs:label>ID</rdfs:label>
	</rdfs:Datatype>
	<rdfs:Datatype rdf:about="&xsd;IDREF">
		<rdfs:isDefinedBy rdf:resource="&xsd;"/>
		<rdfs:label>IDREF</rdfs:label>
	</rdfs:Datatype>
	<rdfs:Datatype rdf:about="&xsd;IDREFS">
		<rdfs:isDefinedBy rdf:resource="&xsd;"/>
		<rdfs:label>IDREFS</rdfs:label>
	</rdfs:Datatype>
	<rdfs:Datatype rdf:ID="data.ACCIDENTAL.EXPLICIT">
		<owl:equivalentClass><rdfs:Datatype>
		<owl:onDatatype rdf:resource="&xs;token"/><owl:withRestrictions rdf:parseType="Collection"><rdf:Description><xs:enumeration>s</xs:enumeration></rdf:Description><rdf:Description><xs:enumeration>f</xs:enumeration></rdf:Description><rdf:Description><xs:enumeration>ss</xs:enumeration></rdf:Description><rdf:Description><xs:enumeration>x</xs:enumeration></rdf:Description><rdf:Description><xs:enumeration>ff</xs:enumeration></rdf:Description><rdf:Description><xs:enumeration>xs</xs:enumeration></rdf:Description><rdf:Description><xs:enumeration>sx</xs:enumeration></rdf:Description><rdf:Description><xs:enumeration>ts</xs:enumeration></rdf:Description><rdf:Description><xs:enumeration>tf</xs:enumeration></rdf:Description><rdf:Description><xs:enumeration>n</xs:enumeration></rdf:Description><rdf:Description><xs:enumeration>nf</xs:enumeration></rdf:Description><rdf:Description><xs:enumeration>ns</xs:enumeration></rdf:Description><rdf:Description><xs:enumeration>su</xs:enumeration></rdf:Description><rdf:Description><xs:enumeration>sd</xs:enumeration></rdf:Description><rdf:Description><xs:enumeration>fu</xs:enumeration></rdf:Description><rdf:Description><xs:enumeration>fd</xs:enumeration></rdf:Description><rdf:Description><xs:enumeration>nu</xs:enumeration></rdf:Description><rdf:Description><xs:enumeration>nd</xs:enumeration></rdf:Description><rdf:Description><xs:enumeration>1qf</xs:enumeration></rdf:Description><rdf:Description><xs:enumeration>3qf</xs:enumeration></rdf:Description><rdf:Description><xs:enumeration>1qs</xs:enumeration></rdf:Description><rdf:Description><xs:enumeration>3qs</xs:enumeration></rdf:Description></owl:withRestrictions></rdfs:Datatype></owl:equivalentClass></rdfs:Datatype>
	<rdfs:Datatype rdf:ID="data.ACCIDENTAL.IMPLICIT">
		<owl:equivalentClass><rdfs:Datatype>
		<owl:onDatatype rdf:resource="&xs;token"/><owl:withRestrictions rdf:parseType="Collection"><rdf:Description><xs:enumeration>s</xs:enumeration></rdf:Description><rdf:Description><xs:enumeration>f</xs:enumeration></rdf:Description><rdf:Description><xs:enumeration>ss</xs:enumeration></rdf:Description><rdf:Description><xs:enumeration>ff</xs:enumeration></rdf:Description><rdf:Description><xs:enumeration>n</xs:enumeration></rdf:Description><rdf:Description><xs:enumeration>su</xs:enumeration></rdf:Description><rdf:Description><xs:enumeration>sd</xs:enumeration></rdf:Description><rdf:Description><xs:enumeration>fu</xs:enumeration></rdf:Description><rdf:Description><xs:enumeration>fd</xs:enumeration></rdf:Description></owl:withRestrictions></rdfs:Datatype></owl:equivalentClass></rdfs:Datatype>
	<rdfs:Datatype rdf:ID="data.ARTICULATION">
		<owl:equivalentClass><rdfs:Datatype>
		<owl:onDatatype rdf:resource="&xs;token"/><owl:withRestrictions rdf:parseType="Collection"><rdf:Description><xs:enumeration>acc</xs:enumeration></rdf:Description><rdf:Description><xs:enumeration>stacc</xs:enumeration></rdf:Description><rdf:Description><xs:enumeration>ten</xs:enumeration></rdf:Description><rdf:Description><xs:enumeration>stacciss</xs:enumeration></rdf:Description><rdf:Description><xs:enumeration>marc</xs:enumeration></rdf:Description><rdf:Description><xs:enumeration>marc-stacc</xs:enumeration></rdf:Description><rdf:Description><xs:enumeration>spicc</xs:enumeration></rdf:Description><rdf:Description><xs:enumeration>doit</xs:enumeration></rdf:Description><rdf:Description><xs:enumeration>scoop</xs:enumeration></rdf:Description><rdf:Description><xs:enumeration>rip</xs:enumeration></rdf:Description><rdf:Description><xs:enumeration>plop</xs:enumeration></rdf:Description><rdf:Description><xs:enumeration>fall</xs:enumeration></rdf:Description><rdf:Description><xs:enumeration>longfall</xs:enumeration></rdf:Description><rdf:Description><xs:enumeration>bend</xs:enumeration></rdf:Description><rdf:Description><xs:enumeration>flip</xs:enumeration></rdf:Description><rdf:Description><xs:enumeration>smear</xs:enumeration></rdf:Description><rdf:Description><xs:enumeration>shake</xs:enumeration></rdf:Description><rdf:Description><xs:enumeration>dnbow</xs:enumeration></rdf:Description><rdf:Description><xs:enumeration>upbow</xs:enumeration></rdf:Description><rdf:Description><xs:enumeration>harm</xs:enumeration></rdf:Description><rdf:Description><xs:enumeration>snap</xs:enumeration></rdf:Description><rdf:Description><xs:enumeration>fingernail</xs:enumeration></rdf:Description><rdf:Description><xs:enumeration>ten-stacc</xs:enumeration></rdf:Description><rdf:Description><xs:enumeration>damp</xs:enumeration></rdf:Description><rdf:Description><xs:enumeration>dampall</xs:enumeration></rdf:Description><rdf:Description><xs:enumeration>open</xs:enumeration></rdf:Description><rdf:Description><xs:enumeration>stop</xs:enumeration></rdf:Description><rdf:Description><xs:enumeration>dbltongue</xs:enumeration></rdf:Description><rdf:Description><xs:enumeration>trpltongue</xs:enumeration></rdf:Description><rdf:Description><xs:enumeration>heel</xs:enumeration></rdf:Description><rdf:Description><xs:enumeration>toe</xs:enumeration></rdf:Description><rdf:Description><xs:enumeration>tap</xs:enumeration></rdf:Description><rdf:Description><xs:enumeration>lhpizz</xs:enumeration></rdf:Description><rdf:Description><xs:enumeration>dot</xs:enumeration></rdf:Description><rdf:Description><xs:enumeration>stroke</xs:enumeration></rdf:Description></owl:withRestrictions></rdfs:Datatype></owl:equivalentClass></rdfs:Datatype>
	<rdfs:Datatype rdf:ID="data.AUGMENTDOT">
		<owl:equivalentClass><rdfs:Datatype>
		<owl:onDatatype rdf:resource="&xs;nonNegativeInteger"/><owl:withRestrictions rdf:parseType="Collection"><rdf:Description><xs:maxInclusive>4</xs:maxInclusive></rdf:Description></owl:withRestrictions></rdfs:Datatype></owl:equivalentClass></rdfs:Datatype>
	<rdfs:Datatype rdf:ID="data.BARPLACE">
		<owl:equivalentClass><rdfs:Datatype>
		<owl:onDatatype rdf:resource="&xs;token"/><owl:withRestrictions rdf:parseType="Collection"><rdf:Description><xs:enumeration>mensur</xs:enumeration></rdf:Description><rdf:Description><xs:enumeration>staff</xs:enumeration></rdf:Description><rdf:Description><xs:enumeration>takt</xs:enumeration></rdf:Description></owl:withRestrictions></rdfs:Datatype></owl:equivalentClass></rdfs:Datatype>
	<rdfs:Datatype rdf:ID="data.BARRENDITION">
		<owl:equivalentClass><rdfs:Datatype>
		<owl:onDatatype rdf:resource="&xs;token"/><owl:withRestrictions rdf:parseType="Collection"><rdf:Description><xs:enumeration>dashed</xs:enumeration></rdf:Description><rdf:Description><xs:enumeration>dotted</xs:enumeration></rdf:Description><rdf:Description><xs:enumeration>dbl</xs:enumeration></rdf:Description><rdf:Description><xs:enumeration>dbldashed</xs:enumeration></rdf:Description><rdf:Description><xs:enumeration>dbldotted</xs:enumeration></rdf:Description><rdf:Description><xs:enumeration>end</xs:enumeration></rdf:Description><rdf:Description><xs:enumeration>invis</xs:enumeration></rdf:Description><rdf:Description><xs:enumeration>rptstart</xs:enumeration></rdf:Description><rdf:Description><xs:enumeration>rptboth</xs:enumeration></rdf:Description><rdf:Description><xs:enumeration>rptend</xs:enumeration></rdf:Description><rdf:Description><xs:enumeration>single</xs:enumeration></rdf:Description></owl:withRestrictions></rdfs:Datatype></owl:equivalentClass></rdfs:Datatype>
	<rdfs:Datatype rdf:ID="data.BEAM">
		<owl:equivalentClass><rdfs:Datatype>
		<owl:onDatatype rdf:resource="&xs;token"/><owl:withRestrictions rdf:parseType="Collection"><rdf:Description><xs:pattern>[i|m|t][1-6]</xs:pattern></rdf:Description></owl:withRestrictions></rdfs:Datatype></owl:equivalentClass></rdfs:Datatype>
	<rdfs:Datatype rdf:ID="data.BEAT">
		<owl:equivalentClass><rdfs:Datatype>
		<owl:onDatatype rdf:resource="&xs;decimal"/><owl:withRestrictions rdf:parseType="Collection"><rdf:Description><xs:minInclusive>0</xs:minInclusive></rdf:Description></owl:withRestrictions></rdfs:Datatype></owl:equivalentClass></rdfs:Datatype>
	<rdfs:Datatype rdf:ID="data.BEATRPT.REND">
		<owl:equivalentClass><rdfs:Datatype>
		<owl:unionOf rdf:parseType="Collection"><rdf:Description rdf:about="NS_data.BEATRPT.REND_UNType_1"/><rdf:Description rdf:about="NS_data.BEATRPT.REND_UNType_2"/></owl:unionOf></rdfs:Datatype></owl:equivalentClass></rdfs:Datatype>
	<rdfs:Datatype rdf:ID="NS_data.BEATRPT.REND_UNType_1">
		<owl:equivalentClass><rdfs:Datatype>
		<owl:onDatatype rdf:resource="&xs;positiveInteger"/><owl:withRestrictions rdf:parseType="Collection"><rdf:Description><xs:pattern>4|8|16|32|64|128</xs:pattern></rdf:Description></owl:withRestrictions></rdfs:Datatype></owl:equivalentClass></rdfs:Datatype>
	<rdfs:Datatype rdf:ID="NS_data.BEATRPT.REND_UNType_2">
		<owl:equivalentClass><rdfs:Datatype>
		<owl:onDatatype rdf:resource="&xs;token"/><owl:withRestrictions rdf:parseType="Collection"><rdf:Description><xs:pattern>mixed</xs:pattern></rdf:Description></owl:withRestrictions></rdfs:Datatype></owl:equivalentClass></rdfs:Datatype>
	<rdfs:Datatype rdf:ID="data.BEND.AMOUNT">
		<owl:equivalentClass><rdfs:Datatype>
		<owl:unionOf rdf:parseType="Collection"><rdf:Description rdf:about="NS_data.BEND.AMOUNT_UNType_1"/><rdf:Description rdf:about="NS_data.BEND.AMOUNT_UNType_2"/><rdf:Description rdf:about="NS_data.BEND.AMOUNT_UNType_3"/></owl:unionOf></rdfs:Datatype></owl:equivalentClass></rdfs:Datatype>
	<rdfs:Datatype rdf:ID="NS_data.BEND.AMOUNT_UNType_1">
		<owl:equivalentClass><rdfs:Datatype>
		<owl:onDatatype rdf:resource="&xs;decimal"/><owl:withRestrictions rdf:parseType="Collection"><rdf:Description><xs:pattern>\.25|\.5|\.75</xs:pattern></rdf:Description></owl:withRestrictions></rdfs:Datatype></owl:equivalentClass></rdfs:Datatype>
	<rdfs:Datatype rdf:ID="NS_data.BEND.AMOUNT_UNType_2">
		<owl:equivalentClass><rdfs:Datatype>
		<owl:onDatatype rdf:resource="&xs;decimal"/><owl:withRestrictions rdf:parseType="Collection"><rdf:Description><xs:pattern>[0-9](\.25|\.5|\.75)?</xs:pattern></rdf:Description></owl:withRestrictions></rdfs:Datatype></owl:equivalentClass></rdfs:Datatype>
	<rdfs:Datatype rdf:ID="NS_data.BEND.AMOUNT_UNType_3">
		<owl:equivalentClass><rdfs:Datatype>
		<owl:onDatatype rdf:resource="&xs;token"/><owl:withRestrictions rdf:parseType="Collection"><rdf:Description><xs:pattern>full</xs:pattern></rdf:Description></owl:withRestrictions></rdfs:Datatype></owl:equivalentClass></rdfs:Datatype>
	<rdfs:Datatype rdf:ID="data.BOOLEAN">
		<owl:equivalentClass><rdfs:Datatype>
		<owl:onDatatype rdf:resource="&xs;token"/><owl:withRestrictions rdf:parseType="Collection"><rdf:Description><xs:enumeration>true</xs:enumeration></rdf:Description><rdf:Description><xs:enumeration>false</xs:enumeration></rdf:Description></owl:withRestrictions></rdfs:Datatype></owl:equivalentClass></rdfs:Datatype>
	<rdfs:Datatype rdf:ID="data.CERTAINTY">
		<owl:equivalentClass><rdfs:Datatype>
		<owl:onDatatype rdf:resource="&xs;token"/><owl:withRestrictions rdf:parseType="Collection"><rdf:Description><xs:enumeration>high</xs:enumeration></rdf:Description><rdf:Description><xs:enumeration>medium</xs:enumeration></rdf:Description><rdf:Description><xs:enumeration>low</xs:enumeration></rdf:Description><rdf:Description><xs:enumeration>unknown</xs:enumeration></rdf:Description></owl:withRestrictions></rdfs:Datatype></owl:equivalentClass></rdfs:Datatype>
	<rdfs:Datatype rdf:ID="data.CLEFLINE">
		<owl:equivalentClass><rdfs:Datatype>
		<owl:onDatatype rdf:resource="&xs;positiveInteger"/><owl:withRestrictions rdf:parseType="Collection"></owl:withRestrictions></rdfs:Datatype></owl:equivalentClass></rdfs:Datatype>
	<rdfs:Datatype rdf:ID="data.CLEFSHAPE">
		<owl:equivalentClass><rdfs:Datatype>
		<owl:onDatatype rdf:resource="&xs;token"/><owl:withRestrictions rdf:parseType="Collection"><rdf:Description><xs:enumeration>G</xs:enumeration></rdf:Description><rdf:Description><xs:enumeration>GG</xs:enumeration></rdf:Description><rdf:Description><xs:enumeration>F</xs:enumeration></rdf:Description><rdf:Description><xs:enumeration>C</xs:enumeration></rdf:Description><rdf:Description><xs:enumeration>perc</xs:enumeration></rdf:Description><rdf:Description><xs:enumeration>TAB</xs:enumeration></rdf:Description></owl:withRestrictions></rdfs:Datatype></owl:equivalentClass></rdfs:Datatype>
	<rdfs:Datatype rdf:ID="data.CLUSTER">
		<owl:equivalentClass><rdfs:Datatype>
		<owl:onDatatype rdf:resource="&xs;token"/><owl:withRestrictions rdf:parseType="Collection"><rdf:Description><xs:enumeration>white</xs:enumeration></rdf:Description><rdf:Description><xs:enumeration>black</xs:enumeration></rdf:Description><rdf:Description><xs:enumeration>chromatic</xs:enumeration></rdf:Description></owl:withRestrictions></rdfs:Datatype></owl:equivalentClass></rdfs:Datatype>
	<rdfs:Datatype rdf:ID="data.COLORNAMES">
		<owl:equivalentClass><rdfs:Datatype>
		<owl:onDatatype rdf:resource="&xs;token"/><owl:withRestrictions rdf:parseType="Collection"><rdf:Description><xs:enumeration>aqua</xs:enumeration></rdf:Description><rdf:Description><xs:enumeration>black</xs:enumeration></rdf:Description><rdf:Description><xs:enumeration>blue</xs:enumeration></rdf:Description><rdf:Description><xs:enumeration>fuchsia</xs:enumeration></rdf:Description><rdf:Description><xs:enumeration>gray</xs:enumeration></rdf:Description><rdf:Description><xs:enumeration>green</xs:enumeration></rdf:Description><rdf:Description><xs:enumeration>lime</xs:enumeration></rdf:Description><rdf:Description><xs:enumeration>maroon</xs:enumeration></rdf:Description><rdf:Description><xs:enumeration>navy</xs:enumeration></rdf:Description><rdf:Description><xs:enumeration>olive</xs:enumeration></rdf:Description><rdf:Description><xs:enumeration>purple</xs:enumeration></rdf:Description><rdf:Description><xs:enumeration>red</xs:enumeration></rdf:Description><rdf:Description><xs:enumeration>silver</xs:enumeration></rdf:Description><rdf:Description><xs:enumeration>teal</xs:enumeration></rdf:Description><rdf:Description><xs:enumeration>white</xs:enumeration></rdf:Description><rdf:Description><xs:enumeration>yellow</xs:enumeration></rdf:Description></owl:withRestrictions></rdfs:Datatype></owl:equivalentClass></rdfs:Datatype>
	<rdfs:Datatype rdf:ID="data.COLORVALUES">
		<owl:equivalentClass><rdfs:Datatype>
		<owl:unionOf rdf:parseType="Collection"><rdf:Description rdf:about="NS_data.COLORVALUES_UNType_1"/><rdf:Description rdf:about="NS_data.COLORVALUES_UNType_2"/><rdf:Description rdf:about="NS_data.COLORVALUES_UNType_3"/><rdf:Description rdf:about="NS_data.COLORVALUES_UNType_4"/><rdf:Description rdf:about="NS_data.COLORVALUES_UNType_5"/><rdf:Description rdf:about="NS_data.COLORVALUES_UNType_6"/></owl:unionOf></rdfs:Datatype></owl:equivalentClass></rdfs:Datatype>
	<rdfs:Datatype rdf:ID="NS_data.COLORVALUES_UNType_1">
		<owl:equivalentClass><rdfs:Datatype>
		<owl:onDatatype rdf:resource="&xs;token"/><owl:withRestrictions rdf:parseType="Collection"><rdf:Description><xs:pattern>#[0-9A-Fa-f]{6,6}</xs:pattern></rdf:Description></owl:withRestrictions></rdfs:Datatype></owl:equivalentClass></rdfs:Datatype>
	<rdfs:Datatype rdf:ID="NS_data.COLORVALUES_UNType_2">
		<owl:equivalentClass><rdfs:Datatype>
		<owl:onDatatype rdf:resource="&xs;token"/><owl:withRestrictions rdf:parseType="Collection"><rdf:Description><xs:pattern>#[0-9A-Fa-f]{8,8}</xs:pattern></rdf:Description></owl:withRestrictions></rdfs:Datatype></owl:equivalentClass></rdfs:Datatype>
	<rdfs:Datatype rdf:ID="NS_data.COLORVALUES_UNType_3">
		<owl:equivalentClass><rdfs:Datatype>
		<owl:onDatatype rdf:resource="&xs;token"/><owl:withRestrictions rdf:parseType="Collection"><rdf:Description><xs:pattern>rgb\((\s*(([01]?[0-9]?[0-9])|2[0-4][0-9]|25[0-5])\s*,\s*){2}([01]?[0-9]?[0-9]|2[0-4][0-9]|25[0-5])\s*\)</xs:pattern></rdf:Description></owl:withRestrictions></rdfs:Datatype></owl:equivalentClass></rdfs:Datatype>
	<rdfs:Datatype rdf:ID="NS_data.COLORVALUES_UNType_4">
		<owl:equivalentClass><rdfs:Datatype>
		<owl:onDatatype rdf:resource="&xs;token"/><owl:withRestrictions rdf:parseType="Collection"><rdf:Description><xs:pattern>rgba\(\s*(([01]?[0-9]?[0-9]|2[0-4][0-9]|25[0-5])\s*,\s*){3}(0(\.\d+)?|1(\.0+)?)\s*\)|rgba\(\s*(((\d{1,2})?%|100%)\s*,\s*){2}(\d{1,2}%|100%)\s*,\s*(0(\.\d+)?|1(\.0+)?)\s*\)</xs:pattern></rdf:Description></owl:withRestrictions></rdfs:Datatype></owl:equivalentClass></rdfs:Datatype>
	<rdfs:Datatype rdf:ID="NS_data.COLORVALUES_UNType_5">
		<owl:equivalentClass><rdfs:Datatype>
		<owl:onDatatype rdf:resource="&xs;token"/><owl:withRestrictions rdf:parseType="Collection"><rdf:Description><xs:pattern>hsl\(\s*((\d{1,2})|[12]\d{2}|3[0-5]\d|360)\s*,\s*(\d{1,2}%|100%)\s*,\s*(\d{1,2}%|100%)\s*\)</xs:pattern></rdf:Description></owl:withRestrictions></rdfs:Datatype></owl:equivalentClass></rdfs:Datatype>
	<rdfs:Datatype rdf:ID="NS_data.COLORVALUES_UNType_6">
		<owl:equivalentClass><rdfs:Datatype>
		<owl:onDatatype rdf:resource="&xs;token"/><owl:withRestrictions rdf:parseType="Collection"><rdf:Description><xs:pattern>hsla\(\s*(\d{1,2}|[12]\d{2}|3[0-5]\d|360)\s*,\s*(\d{1,2}%|100%)\s*,\s*(\d{1,2}%|100%)\s*,\s*(0(\.\d+)?|1(\.0+)?)\s*\)</xs:pattern></rdf:Description></owl:withRestrictions></rdfs:Datatype></owl:equivalentClass></rdfs:Datatype>
	<rdfs:Datatype rdf:ID="data.COLOR">
		<owl:equivalentClass><rdfs:Datatype>
		<owl:unionOf rdf:parseType="Collection"><rdf:Description rdf:about="mei:data.COLORNAMES"/><rdf:Description rdf:about="mei:data.COLORVALUES"/></owl:unionOf></rdfs:Datatype></owl:equivalentClass></rdfs:Datatype>
	<rdfs:Datatype rdf:ID="data.DEGREES">
		<owl:equivalentClass><rdfs:Datatype>
		<owl:onDatatype rdf:resource="&xs;decimal"/><owl:withRestrictions rdf:parseType="Collection"><rdf:Description><xs:maxInclusive>360.0</xs:maxInclusive></rdf:Description><rdf:Description><xs:minInclusive>-360.0</xs:minInclusive></rdf:Description></owl:withRestrictions></rdfs:Datatype></owl:equivalentClass></rdfs:Datatype>
	<rdfs:Datatype rdf:ID="data.DURATION">
		<owl:equivalentClass><rdfs:Datatype>
		<owl:unionOf rdf:parseType="Collection"><rdf:Description rdf:about="mei:data.DURATION.cmn"/><rdf:Description rdf:about="mei:data.DURATION.mensural"/></owl:unionOf></rdfs:Datatype></owl:equivalentClass></rdfs:Datatype>
	<rdfs:Datatype rdf:ID="data.DURATION.additive">
		<owl:equivalentClass><rdfs:Datatype>
		<owl:onDatatype rdf:resource="&xs;token"/><owl:withRestrictions rdf:parseType="Collection"><rdf:Description><xs:pattern>(long|breve|1|2|4|8|16|32|64|128|256|1024|2048)(\.)*</xs:pattern></rdf:Description></owl:withRestrictions></rdfs:Datatype></owl:equivalentClass></rdfs:Datatype>
	<rdfs:Datatype rdf:ID="data.DURATION.gestural.prop">
		<owl:equivalentClass><rdfs:Datatype>
		<owl:onDatatype rdf:resource="&xs;token"/><owl:withRestrictions rdf:parseType="Collection"><rdf:Description><xs:pattern>[0-9]+(\.)*r</xs:pattern></rdf:Description></owl:withRestrictions></rdfs:Datatype></owl:equivalentClass></rdfs:Datatype>
	<rdfs:Datatype rdf:ID="data.DURATION.gestural.pat">
		<owl:equivalentClass><rdfs:Datatype>
		<owl:onDatatype rdf:resource="&xs;token"/><owl:withRestrictions rdf:parseType="Collection"><rdf:Description><xs:pattern>[0-9]+(p|(\.[0-9]+)?(b|s))</xs:pattern></rdf:Description></owl:withRestrictions></rdfs:Datatype></owl:equivalentClass></rdfs:Datatype>
	<rdfs:Datatype rdf:ID="data.DURATION.gestural">
		<owl:equivalentClass><rdfs:Datatype>
		<owl:unionOf rdf:parseType="Collection"><rdf:Description rdf:about="mei:data.DURATION.gestural.prop"/><rdf:Description rdf:about="mei:data.DURATION.gestural.pat"/><rdf:Description rdf:about="mei:data.DURATION.mensural"/></owl:unionOf></rdfs:Datatype></owl:equivalentClass></rdfs:Datatype>
	<rdfs:Datatype rdf:ID="data.ENCLOSURE">
		<owl:equivalentClass><rdfs:Datatype>
		<owl:onDatatype rdf:resource="&xs;token"/><owl:withRestrictions rdf:parseType="Collection"><rdf:Description><xs:enumeration>paren</xs:enumeration></rdf:Description><rdf:Description><xs:enumeration>brack</xs:enumeration></rdf:Description></owl:withRestrictions></rdfs:Datatype></owl:equivalentClass></rdfs:Datatype>
	<rdfs:Datatype rdf:ID="data.FILL">
		<owl:equivalentClass><rdfs:Datatype>
		<owl:onDatatype rdf:resource="&xs;token"/><owl:withRestrictions rdf:parseType="Collection"><rdf:Description><xs:enumeration>void</xs:enumeration></rdf:Description><rdf:Description><xs:enumeration>solid</xs:enumeration></rdf:Description><rdf:Description><xs:enumeration>top</xs:enumeration></rdf:Description><rdf:Description><xs:enumeration>bottom</xs:enumeration></rdf:Description><rdf:Description><xs:enumeration>left</xs:enumeration></rdf:Description><rdf:Description><xs:enumeration>right</xs:enumeration></rdf:Description></owl:withRestrictions></rdfs:Datatype></owl:equivalentClass></rdfs:Datatype>
	<rdfs:Datatype rdf:ID="data.FINGER.FRET">
		<owl:equivalentClass><rdfs:Datatype>
		<owl:unionOf rdf:parseType="Collection"><rdf:Description rdf:about="NS_data.FINGER.FRET_UNType_1"/><rdf:Description rdf:about="NS_data.FINGER.FRET_UNType_2"/></owl:unionOf></rdfs:Datatype></owl:equivalentClass></rdfs:Datatype>
	<rdfs:Datatype rdf:ID="NS_data.FINGER.FRET_UNType_1">
		<owl:equivalentClass><rdfs:Datatype>
		<owl:onDatatype rdf:resource="&xs;positiveInteger"/><owl:withRestrictions rdf:parseType="Collection"><rdf:Description><xs:minInclusive>1</xs:minInclusive></rdf:Description><rdf:Description><xs:maxInclusive>4</xs:maxInclusive></rdf:Description></owl:withRestrictions></rdfs:Datatype></owl:equivalentClass></rdfs:Datatype>
	<rdfs:Datatype rdf:ID="NS_data.FINGER.FRET_UNType_2">
		<owl:equivalentClass><rdfs:Datatype>
		<owl:onDatatype rdf:resource="&xs;token"/><owl:withRestrictions rdf:parseType="Collection"><rdf:Description><xs:pattern>x|o|t</xs:pattern></rdf:Description></owl:withRestrictions></rdfs:Datatype></owl:equivalentClass></rdfs:Datatype>
	<rdfs:Datatype rdf:ID="data.FONTFAMILY">
		<owl:equivalentClass><rdfs:Datatype>
		<owl:onDatatype rdf:resource="&xs;token"/><owl:withRestrictions rdf:parseType="Collection"></owl:withRestrictions></rdfs:Datatype></owl:equivalentClass></rdfs:Datatype>
	<rdfs:Datatype rdf:ID="data.FONTNAME">
		<owl:equivalentClass><rdfs:Datatype>
		<owl:onDatatype rdf:resource="&xs;token"/><owl:withRestrictions rdf:parseType="Collection"></owl:withRestrictions></rdfs:Datatype></owl:equivalentClass></rdfs:Datatype>
	<rdfs:Datatype rdf:ID="data.FONTSIZE">
		<owl:equivalentClass><rdfs:Datatype>
		<owl:unionOf rdf:parseType="Collection"><rdf:Description rdf:about="mei:data.FONTSIZENUMERIC"/><rdf:Description rdf:about="mei:data.FONTSIZETERM"/><rdf:Description rdf:about="mei:data.PERCENT"/></owl:unionOf></rdfs:Datatype></owl:equivalentClass></rdfs:Datatype>
	<rdfs:Datatype rdf:ID="data.FONTSIZENUMERIC">
		<owl:equivalentClass><rdfs:Datatype>
		<owl:onDatatype rdf:resource="&xs;token"/><owl:withRestrictions rdf:parseType="Collection"><rdf:Description><xs:pattern>\d*(\.\d+)?(pt)?</xs:pattern></rdf:Description></owl:withRestrictions></rdfs:Datatype></owl:equivalentClass></rdfs:Datatype>
	<rdfs:Datatype rdf:ID="data.FONTSIZETERM">
		<owl:equivalentClass><rdfs:Datatype>
		<owl:onDatatype rdf:resource="&xs;token"/><owl:withRestrictions rdf:parseType="Collection"><rdf:Description><xs:enumeration>xx-small</xs:enumeration></rdf:Description><rdf:Description><xs:enumeration>x-small</xs:enumeration></rdf:Description><rdf:Description><xs:enumeration>small</xs:enumeration></rdf:Description><rdf:Description><xs:enumeration>medium</xs:enumeration></rdf:Description><rdf:Description><xs:enumeration>large</xs:enumeration></rdf:Description><rdf:Description><xs:enumeration>x-large</xs:enumeration></rdf:Description><rdf:Description><xs:enumeration>xx-large</xs:enumeration></rdf:Description><rdf:Description><xs:enumeration>smaller</xs:enumeration></rdf:Description><rdf:Description><xs:enumeration>larger</xs:enumeration></rdf:Description></owl:withRestrictions></rdfs:Datatype></owl:equivalentClass></rdfs:Datatype>
	<rdfs:Datatype rdf:ID="data.FONTSTYLE">
		<owl:equivalentClass><rdfs:Datatype>
		<owl:onDatatype rdf:resource="&xs;token"/><owl:withRestrictions rdf:parseType="Collection"><rdf:Description><xs:enumeration>italic</xs:enumeration></rdf:Description><rdf:Description><xs:enumeration>normal</xs:enumeration></rdf:Description><rdf:Description><xs:enumeration>oblique</xs:enumeration></rdf:Description></owl:withRestrictions></rdfs:Datatype></owl:equivalentClass></rdfs:Datatype>
	<rdfs:Datatype rdf:ID="data.FONTWEIGHT">
		<owl:equivalentClass><rdfs:Datatype>
		<owl:onDatatype rdf:resource="&xs;token"/><owl:withRestrictions rdf:parseType="Collection"><rdf:Description><xs:enumeration>bold</xs:enumeration></rdf:Description><rdf:Description><xs:enumeration>normal</xs:enumeration></rdf:Description></owl:withRestrictions></rdfs:Datatype></owl:equivalentClass></rdfs:Datatype>
	<rdfs:Datatype rdf:ID="data.FRET">
		<owl:equivalentClass><rdfs:Datatype>
		<owl:onDatatype rdf:resource="&xs;positiveInteger"/><owl:withRestrictions rdf:parseType="Collection"><rdf:Description><xs:minInclusive>1</xs:minInclusive></rdf:Description><rdf:Description><xs:maxInclusive>5</xs:maxInclusive></rdf:Description></owl:withRestrictions></rdfs:Datatype></owl:equivalentClass></rdfs:Datatype>
	<rdfs:Datatype rdf:ID="data.FRETNUMBER">
		<owl:equivalentClass><rdfs:Datatype>
		<owl:onDatatype rdf:resource="&xs;nonNegativeInteger"/><owl:withRestrictions rdf:parseType="Collection"></owl:withRestrictions></rdfs:Datatype></owl:equivalentClass></rdfs:Datatype>
	<rdfs:Datatype rdf:ID="data.GLISSANDO">
		<owl:equivalentClass><rdfs:Datatype>
		<owl:onDatatype rdf:resource="&xs;token"/><owl:withRestrictions rdf:parseType="Collection"><rdf:Description><xs:enumeration>i</xs:enumeration></rdf:Description><rdf:Description><xs:enumeration>m</xs:enumeration></rdf:Description><rdf:Description><xs:enumeration>t</xs:enumeration></rdf:Description></owl:withRestrictions></rdfs:Datatype></owl:equivalentClass></rdfs:Datatype>
	<rdfs:Datatype rdf:ID="data.GRACE">
		<owl:equivalentClass><rdfs:Datatype>
		<owl:onDatatype rdf:resource="&xs;token"/><owl:withRestrictions rdf:parseType="Collection"><rdf:Description><xs:enumeration>acc</xs:enumeration></rdf:Description><rdf:Description><xs:enumeration>unacc</xs:enumeration></rdf:Description><rdf:Description><xs:enumeration>unknown</xs:enumeration></rdf:Description></owl:withRestrictions></rdfs:Datatype></owl:equivalentClass></rdfs:Datatype>
	<rdfs:Datatype rdf:ID="data.HEADSHAPE">
		<owl:equivalentClass><rdfs:Datatype>
		<owl:unionOf rdf:parseType="Collection"><rdf:Description rdf:about="mei:data.HEADSHAPE.list"/><rdf:Description rdf:about="mei:data.NMTOKEN"/></owl:unionOf></rdfs:Datatype></owl:equivalentClass></rdfs:Datatype>
	<rdfs:Datatype rdf:ID="data.HEADSHAPE.list">
		<owl:equivalentClass><rdfs:Datatype>
		<owl:onDatatype rdf:resource="&xs;token"/><owl:withRestrictions rdf:parseType="Collection"><rdf:Description><xs:enumeration>quarter</xs:enumeration></rdf:Description><rdf:Description><xs:enumeration>half</xs:enumeration></rdf:Description><rdf:Description><xs:enumeration>whole</xs:enumeration></rdf:Description><rdf:Description><xs:enumeration>backslash</xs:enumeration></rdf:Description><rdf:Description><xs:enumeration>circle</xs:enumeration></rdf:Description><rdf:Description><xs:enumeration>+</xs:enumeration></rdf:Description><rdf:Description><xs:enumeration>diamond</xs:enumeration></rdf:Description><rdf:Description><xs:enumeration>isotriangle</xs:enumeration></rdf:Description><rdf:Description><xs:enumeration>oval</xs:enumeration></rdf:Description><rdf:Description><xs:enumeration>piewedge</xs:enumeration></rdf:Description><rdf:Description><xs:enumeration>rectangle</xs:enumeration></rdf:Description><rdf:Description><xs:enumeration>rtriangle</xs:enumeration></rdf:Description><rdf:Description><xs:enumeration>semicircle</xs:enumeration></rdf:Description><rdf:Description><xs:enumeration>slash</xs:enumeration></rdf:Description><rdf:Description><xs:enumeration>square</xs:enumeration></rdf:Description><rdf:Description><xs:enumeration>x</xs:enumeration></rdf:Description></owl:withRestrictions></rdfs:Datatype></owl:equivalentClass></rdfs:Datatype>
	<rdfs:Datatype rdf:ID="data.HORIZONTALALIGNMENT">
		<owl:equivalentClass><rdfs:Datatype>
		<owl:onDatatype rdf:resource="&xs;token"/><owl:withRestrictions rdf:parseType="Collection"><rdf:Description><xs:enumeration>left</xs:enumeration></rdf:Description><rdf:Description><xs:enumeration>right</xs:enumeration></rdf:Description><rdf:Description><xs:enumeration>center</xs:enumeration></rdf:Description><rdf:Description><xs:enumeration>justify</xs:enumeration></rdf:Description></owl:withRestrictions></rdfs:Datatype></owl:equivalentClass></rdfs:Datatype>
	<rdfs:Datatype rdf:ID="data.INEUMEFORM">
		<owl:equivalentClass><rdfs:Datatype>
		<owl:onDatatype rdf:resource="&xs;token"/><owl:withRestrictions rdf:parseType="Collection"><rdf:Description><xs:enumeration>liquescent1</xs:enumeration></rdf:Description><rdf:Description><xs:enumeration>liquescent2</xs:enumeration></rdf:Description><rdf:Description><xs:enumeration>tied</xs:enumeration></rdf:Description><rdf:Description><xs:enumeration>tiedliquescent1</xs:enumeration></rdf:Description><rdf:Description><xs:enumeration>tiedliquescent2</xs:enumeration></rdf:Description></owl:withRestrictions></rdfs:Datatype></owl:equivalentClass></rdfs:Datatype>
	<rdfs:Datatype rdf:ID="data.INEUMENAME">
		<owl:equivalentClass><rdfs:Datatype>
		<owl:onDatatype rdf:resource="&xs;token"/><owl:withRestrictions rdf:parseType="Collection"><rdf:Description><xs:enumeration>pessubpunctis</xs:enumeration></rdf:Description><rdf:Description><xs:enumeration>climacus</xs:enumeration></rdf:Description><rdf:Description><xs:enumeration>scandicus</xs:enumeration></rdf:Description><rdf:Description><xs:enumeration>bistropha</xs:enumeration></rdf:Description><rdf:Description><xs:enumeration>tristropha</xs:enumeration></rdf:Description><rdf:Description><xs:enumeration>pressusminor</xs:enumeration></rdf:Description><rdf:Description><xs:enumeration>pressusmaior</xs:enumeration></rdf:Description></owl:withRestrictions></rdfs:Datatype></owl:equivalentClass></rdfs:Datatype>
	<rdfs:Datatype rdf:ID="data.INTERVAL.HARMONIC">
		<owl:equivalentClass><rdfs:Datatype>
		<owl:onDatatype rdf:resource="&xs;token"/><owl:withRestrictions rdf:parseType="Collection"><rdf:Description><xs:pattern>[AdMmP][0-9]+</xs:pattern></rdf:Description></owl:withRestrictions></rdfs:Datatype></owl:equivalentClass></rdfs:Datatype>
	<rdfs:Datatype rdf:ID="data.INTERVAL.MELODIC">
		<owl:equivalentClass><rdfs:Datatype>
		<owl:unionOf rdf:parseType="Collection"><rdf:Description rdf:about="xs:decimal"/></owl:unionOf></rdfs:Datatype></owl:equivalentClass></rdfs:Datatype>
	<rdfs:Datatype rdf:ID="data.ISODATE">
		<owl:equivalentClass><rdfs:Datatype>
		<owl:unionOf rdf:parseType="Collection"><rdf:Description rdf:about="xs:date"/><rdf:Description rdf:about="xs:gYear"/><rdf:Description rdf:about="xs:gMonth"/><rdf:Description rdf:about="xs:gDay"/><rdf:Description rdf:about="xs:gYearMonth"/><rdf:Description rdf:about="xs:gMonthDay"/><rdf:Description rdf:about="xs:time"/><rdf:Description rdf:about="xs:dateTime"/></owl:unionOf></rdfs:Datatype></owl:equivalentClass></rdfs:Datatype>
	<rdfs:Datatype rdf:ID="data.ISOTIME">
		<owl:equivalentClass><rdfs:Datatype>
		<owl:onDatatype rdf:resource="&xs;time"/><owl:withRestrictions rdf:parseType="Collection"></owl:withRestrictions></rdfs:Datatype></owl:equivalentClass></rdfs:Datatype>
	<rdfs:Datatype rdf:ID="data.KEYSIGNATURE">
		<owl:equivalentClass><rdfs:Datatype>
		<owl:onDatatype rdf:resource="&xs;token"/><owl:withRestrictions rdf:parseType="Collection"><rdf:Description><xs:pattern>mixed|0|([1-9]|1[0-2])[f|s]</xs:pattern></rdf:Description></owl:withRestrictions></rdfs:Datatype></owl:equivalentClass></rdfs:Datatype>
	<rdfs:Datatype rdf:ID="data.KEYSIGTOKEN">
		<owl:equivalentClass><rdfs:Datatype>
		<owl:onDatatype rdf:resource="&xs;token"/><owl:withRestrictions rdf:parseType="Collection"><rdf:Description><xs:pattern>[a-g][0-9](s|f|ss|x|ff|xs|sx|ts|tf|n|nf|ns|su|sd|fu|fd|nu|nd|1qf|3qf|1qs|3qs)</xs:pattern></rdf:Description></owl:withRestrictions></rdfs:Datatype></owl:equivalentClass></rdfs:Datatype>
	<rdfs:Datatype rdf:ID="data.LAYERSCHEME">
		<owl:equivalentClass><rdfs:Datatype>
		<owl:onDatatype rdf:resource="&xs;token"/><owl:withRestrictions rdf:parseType="Collection"><rdf:Description><xs:enumeration>1</xs:enumeration></rdf:Description><rdf:Description><xs:enumeration>2o</xs:enumeration></rdf:Description><rdf:Description><xs:enumeration>2f</xs:enumeration></rdf:Description><rdf:Description><xs:enumeration>3o</xs:enumeration></rdf:Description><rdf:Description><xs:enumeration>3f</xs:enumeration></rdf:Description></owl:withRestrictions></rdfs:Datatype></owl:equivalentClass></rdfs:Datatype>
	<rdfs:Datatype rdf:ID="data.LIGATUREFORM">
		<owl:equivalentClass><rdfs:Datatype>
		<owl:onDatatype rdf:resource="&xs;token"/><owl:withRestrictions rdf:parseType="Collection"><rdf:Description><xs:enumeration>recta</xs:enumeration></rdf:Description><rdf:Description><xs:enumeration>obliqua</xs:enumeration></rdf:Description></owl:withRestrictions></rdfs:Datatype></owl:equivalentClass></rdfs:Datatype>
	<rdfs:Datatype rdf:ID="data.LINEFORM">
		<owl:equivalentClass><rdfs:Datatype>
		<owl:onDatatype rdf:resource="&xs;token"/><owl:withRestrictions rdf:parseType="Collection"><rdf:Description><xs:enumeration>dashed</xs:enumeration></rdf:Description><rdf:Description><xs:enumeration>dotted</xs:enumeration></rdf:Description><rdf:Description><xs:enumeration>solid</xs:enumeration></rdf:Description><rdf:Description><xs:enumeration>wavy</xs:enumeration></rdf:Description></owl:withRestrictions></rdfs:Datatype></owl:equivalentClass></rdfs:Datatype>
	<rdfs:Datatype rdf:ID="data.LINESTARTENDSYMBOL">
		<owl:equivalentClass><rdfs:Datatype>
		<owl:onDatatype rdf:resource="&xs;token"/><owl:withRestrictions rdf:parseType="Collection"><rdf:Description><xs:enumeration>angledown</xs:enumeration></rdf:Description><rdf:Description><xs:enumeration>angleup</xs:enumeration></rdf:Description><rdf:Description><xs:enumeration>angleright</xs:enumeration></rdf:Description><rdf:Description><xs:enumeration>angleleft</xs:enumeration></rdf:Description><rdf:Description><xs:enumeration>arrow</xs:enumeration></rdf:Description><rdf:Description><xs:enumeration>arrowopen</xs:enumeration></rdf:Description><rdf:Description><xs:enumeration>arrowwhite</xs:enumeration></rdf:Description><rdf:Description><xs:enumeration>harpoonleft</xs:enumeration></rdf:Description><rdf:Description><xs:enumeration>harpoonright</xs:enumeration></rdf:Description><rdf:Description><xs:enumeration>none</xs:enumeration></rdf:Description></owl:withRestrictions></rdfs:Datatype></owl:equivalentClass></rdfs:Datatype>
	<rdfs:Datatype rdf:ID="data.LINESTARTENDSYMBOLSIZE">
		<owl:equivalentClass><rdfs:Datatype>
		<owl:onDatatype rdf:resource="&xs;positiveInteger"/><owl:withRestrictions rdf:parseType="Collection"><rdf:Description><xs:minInclusive>1</xs:minInclusive></rdf:Description><rdf:Description><xs:maxInclusive>9</xs:maxInclusive></rdf:Description></owl:withRestrictions></rdfs:Datatype></owl:equivalentClass></rdfs:Datatype>
	<rdfs:Datatype rdf:ID="data.LINEWIDTH">
		<owl:equivalentClass><rdfs:Datatype>
		<owl:unionOf rdf:parseType="Collection"><rdf:Description rdf:about="mei:data.LINEWIDTHTERM"/><rdf:Description rdf:about="mei:data.MEASUREMENTABS"/></owl:unionOf></rdfs:Datatype></owl:equivalentClass></rdfs:Datatype>
	<rdfs:Datatype rdf:ID="data.LINEWIDTHTERM">
		<owl:equivalentClass><rdfs:Datatype>
		<owl:onDatatype rdf:resource="&xs;token"/><owl:withRestrictions rdf:parseType="Collection"><rdf:Description><xs:enumeration>narrow</xs:enumeration></rdf:Description><rdf:Description><xs:enumeration>medium</xs:enumeration></rdf:Description><rdf:Description><xs:enumeration>wide</xs:enumeration></rdf:Description></owl:withRestrictions></rdfs:Datatype></owl:equivalentClass></rdfs:Datatype>
	<rdfs:Datatype rdf:ID="data.MEASUREBEAT">
		<owl:equivalentClass><rdfs:Datatype>
		<owl:onDatatype rdf:resource="&xs;token"/><owl:withRestrictions rdf:parseType="Collection"><rdf:Description><xs:pattern>([0-9]+m\s*\+\s*)?[0-9]+(\.?[0-9]*)?</xs:pattern></rdf:Description></owl:withRestrictions></rdfs:Datatype></owl:equivalentClass></rdfs:Datatype>
	<rdfs:Datatype rdf:ID="data.MEASUREBEATOFFSET">
		<owl:equivalentClass><rdfs:Datatype>
		<owl:onDatatype rdf:resource="&xs;token"/><owl:withRestrictions rdf:parseType="Collection"><rdf:Description><xs:pattern>(\+|-)?[0-9]+m\+[0-9]+(\.[0-9]*)?</xs:pattern></rdf:Description></owl:withRestrictions></rdfs:Datatype></owl:equivalentClass></rdfs:Datatype>
	<rdfs:Datatype rdf:ID="data.MEASUREMENTABS">
		<owl:equivalentClass><rdfs:Datatype>
		<owl:onDatatype rdf:resource="&xs;token"/><owl:withRestrictions rdf:parseType="Collection"><rdf:Description><xs:pattern>(\+)?\d+(\.\d+)?(cm|mm|in|pt|pc|px|vu)?</xs:pattern></rdf:Description></owl:withRestrictions></rdfs:Datatype></owl:equivalentClass></rdfs:Datatype>
	<rdfs:Datatype rdf:ID="data.MEASUREMENTREL">
		<owl:equivalentClass><rdfs:Datatype>
		<owl:onDatatype rdf:resource="&xs;token"/><owl:withRestrictions rdf:parseType="Collection"><rdf:Description><xs:pattern>(\+|-)?\d+(\.\d+)?(cm|mm|in|pt|pc|px|vu)?</xs:pattern></rdf:Description></owl:withRestrictions></rdfs:Datatype></owl:equivalentClass></rdfs:Datatype>
	<rdfs:Datatype rdf:ID="data.MELODICFUNCTION">
		<owl:equivalentClass><rdfs:Datatype>
		<owl:onDatatype rdf:resource="&xs;token"/><owl:withRestrictions rdf:parseType="Collection"><rdf:Description><xs:enumeration>aln</xs:enumeration></rdf:Description><rdf:Description><xs:enumeration>ant</xs:enumeration></rdf:Description><rdf:Description><xs:enumeration>app</xs:enumeration></rdf:Description><rdf:Description><xs:enumeration>apt</xs:enumeration></rdf:Description><rdf:Description><xs:enumeration>arp</xs:enumeration></rdf:Description><rdf:Description><xs:enumeration>arp7</xs:enumeration></rdf:Description><rdf:Description><xs:enumeration>aun</xs:enumeration></rdf:Description><rdf:Description><xs:enumeration>chg</xs:enumeration></rdf:Description><rdf:Description><xs:enumeration>cln</xs:enumeration></rdf:Description><rdf:Description><xs:enumeration>ct</xs:enumeration></rdf:Description><rdf:Description><xs:enumeration>ct7</xs:enumeration></rdf:Description><rdf:Description><xs:enumeration>cun</xs:enumeration></rdf:Description><rdf:Description><xs:enumeration>cup</xs:enumeration></rdf:Description><rdf:Description><xs:enumeration>et</xs:enumeration></rdf:Description><rdf:Description><xs:enumeration>ln</xs:enumeration></rdf:Description><rdf:Description><xs:enumeration>ped</xs:enumeration></rdf:Description><rdf:Description><xs:enumeration>rep</xs:enumeration></rdf:Description><rdf:Description><xs:enumeration>ret</xs:enumeration></rdf:Description><rdf:Description><xs:enumeration>23ret</xs:enumeration></rdf:Description><rdf:Description><xs:enumeration>78ret</xs:enumeration></rdf:Description><rdf:Description><xs:enumeration>sus</xs:enumeration></rdf:Description><rdf:Description><xs:enumeration>43sus</xs:enumeration></rdf:Description><rdf:Description><xs:enumeration>98sus</xs:enumeration></rdf:Description><rdf:Description><xs:enumeration>76sus</xs:enumeration></rdf:Description><rdf:Description><xs:enumeration>un</xs:enumeration></rdf:Description><rdf:Description><xs:enumeration>un7</xs:enumeration></rdf:Description><rdf:Description><xs:enumeration>upt</xs:enumeration></rdf:Description><rdf:Description><xs:enumeration>upt7</xs:enumeration></rdf:Description></owl:withRestrictions></rdfs:Datatype></owl:equivalentClass></rdfs:Datatype>
	<rdfs:Datatype rdf:ID="data.MENSURATIONSIGN">
		<owl:equivalentClass><rdfs:Datatype>
		<owl:onDatatype rdf:resource="&xs;token"/><owl:withRestrictions rdf:parseType="Collection"><rdf:Description><xs:enumeration>C</xs:enumeration></rdf:Description><rdf:Description><xs:enumeration>O</xs:enumeration></rdf:Description></owl:withRestrictions></rdfs:Datatype></owl:equivalentClass></rdfs:Datatype>
	<rdfs:Datatype rdf:ID="data.METERSIGN">
		<owl:equivalentClass><rdfs:Datatype>
		<owl:onDatatype rdf:resource="&xs;token"/><owl:withRestrictions rdf:parseType="Collection"><rdf:Description><xs:enumeration>common</xs:enumeration></rdf:Description><rdf:Description><xs:enumeration>cut</xs:enumeration></rdf:Description></owl:withRestrictions></rdfs:Datatype></owl:equivalentClass></rdfs:Datatype>
	<rdfs:Datatype rdf:ID="data.MIDICHANNEL">
		<owl:equivalentClass><rdfs:Datatype>
		<owl:onDatatype rdf:resource="&xs;positiveInteger"/><owl:withRestrictions rdf:parseType="Collection"><rdf:Description><xs:maxInclusive>16</xs:maxInclusive></rdf:Description></owl:withRestrictions></rdfs:Datatype></owl:equivalentClass></rdfs:Datatype>
	<rdfs:Datatype rdf:ID="data.MIDIBPM">
		<owl:equivalentClass><rdfs:Datatype>
		<owl:onDatatype rdf:resource="&xs;positiveInteger"/><owl:withRestrictions rdf:parseType="Collection"></owl:withRestrictions></rdfs:Datatype></owl:equivalentClass></rdfs:Datatype>
	<rdfs:Datatype rdf:ID="data.MIDIMSPB">
		<owl:equivalentClass><rdfs:Datatype>
		<owl:onDatatype rdf:resource="&xs;positiveInteger"/><owl:withRestrictions rdf:parseType="Collection"></owl:withRestrictions></rdfs:Datatype></owl:equivalentClass></rdfs:Datatype>
	<rdfs:Datatype rdf:ID="data.MIDINAMES">
		<owl:equivalentClass><rdfs:Datatype>
		<owl:onDatatype rdf:resource="&xs;token"/><owl:withRestrictions rdf:parseType="Collection"><rdf:Description><xs:enumeration>Acoustic_Grand_Piano</xs:enumeration></rdf:Description><rdf:Description><xs:enumeration>Bright_Acoustic_Piano</xs:enumeration></rdf:Description><rdf:Description><xs:enumeration>Electric_Grand_Piano</xs:enumeration></rdf:Description><rdf:Description><xs:enumeration>Honky-tonk_Piano</xs:enumeration></rdf:Description><rdf:Description><xs:enumeration>Electric_Piano_1</xs:enumeration></rdf:Description><rdf:Description><xs:enumeration>Electric_Piano_2</xs:enumeration></rdf:Description><rdf:Description><xs:enumeration>Harpsichord</xs:enumeration></rdf:Description><rdf:Description><xs:enumeration>Clavi</xs:enumeration></rdf:Description><rdf:Description><xs:enumeration>Celesta</xs:enumeration></rdf:Description><rdf:Description><xs:enumeration>Glockenspiel</xs:enumeration></rdf:Description><rdf:Description><xs:enumeration>Music_Box</xs:enumeration></rdf:Description><rdf:Description><xs:enumeration>Vibraphone</xs:enumeration></rdf:Description><rdf:Description><xs:enumeration>Marimba</xs:enumeration></rdf:Description><rdf:Description><xs:enumeration>Xylophone</xs:enumeration></rdf:Description><rdf:Description><xs:enumeration>Tubular_Bells</xs:enumeration></rdf:Description><rdf:Description><xs:enumeration>Dulcimer</xs:enumeration></rdf:Description><rdf:Description><xs:enumeration>Drawbar_Organ</xs:enumeration></rdf:Description><rdf:Description><xs:enumeration>Percussive_Organ</xs:enumeration></rdf:Description><rdf:Description><xs:enumeration>Rock_Organ</xs:enumeration></rdf:Description><rdf:Description><xs:enumeration>Church_Organ</xs:enumeration></rdf:Description><rdf:Description><xs:enumeration>Reed_Organ</xs:enumeration></rdf:Description><rdf:Description><xs:enumeration>Accordion</xs:enumeration></rdf:Description><rdf:Description><xs:enumeration>Harmonica</xs:enumeration></rdf:Description><rdf:Description><xs:enumeration>Tango_Accordion</xs:enumeration></rdf:Description><rdf:Description><xs:enumeration>Acoustic_Guitar_nylon</xs:enumeration></rdf:Description><rdf:Description><xs:enumeration>Acoustic_Guitar_steel</xs:enumeration></rdf:Description><rdf:Description><xs:enumeration>Electric_Guitar_jazz</xs:enumeration></rdf:Description><rdf:Description><xs:enumeration>Electric_Guitar_clean</xs:enumeration></rdf:Description><rdf:Description><xs:enumeration>Electric_Guitar_muted</xs:enumeration></rdf:Description><rdf:Description><xs:enumeration>Overdriven_Guitar</xs:enumeration></rdf:Description><rdf:Description><xs:enumeration>Distortion_Guitar</xs:enumeration></rdf:Description><rdf:Description><xs:enumeration>Guitar_harmonics</xs:enumeration></rdf:Description><rdf:Description><xs:enumeration>Acoustic_Bass</xs:enumeration></rdf:Description><rdf:Description><xs:enumeration>Electric_Bass_finger</xs:enumeration></rdf:Description><rdf:Description><xs:enumeration>Electric_Bass_pick</xs:enumeration></rdf:Description><rdf:Description><xs:enumeration>Fretless_Bass</xs:enumeration></rdf:Description><rdf:Description><xs:enumeration>Slap_Bass_1</xs:enumeration></rdf:Description><rdf:Description><xs:enumeration>Slap_Bass_2</xs:enumeration></rdf:Description><rdf:Description><xs:enumeration>Synth_Bass_1</xs:enumeration></rdf:Description><rdf:Description><xs:enumeration>Synth_Bass_2</xs:enumeration></rdf:Description><rdf:Description><xs:enumeration>Violin</xs:enumeration></rdf:Description><rdf:Description><xs:enumeration>Viola</xs:enumeration></rdf:Description><rdf:Description><xs:enumeration>Cello</xs:enumeration></rdf:Description><rdf:Description><xs:enumeration>Contrabass</xs:enumeration></rdf:Description><rdf:Description><xs:enumeration>Tremolo_Strings</xs:enumeration></rdf:Description><rdf:Description><xs:enumeration>Pizzicato_Strings</xs:enumeration></rdf:Description><rdf:Description><xs:enumeration>Orchestral_Harp</xs:enumeration></rdf:Description><rdf:Description><xs:enumeration>Timpani</xs:enumeration></rdf:Description><rdf:Description><xs:enumeration>String_Ensemble_1</xs:enumeration></rdf:Description><rdf:Description><xs:enumeration>String_Ensemble_2</xs:enumeration></rdf:Description><rdf:Description><xs:enumeration>SynthStrings_1</xs:enumeration></rdf:Description><rdf:Description><xs:enumeration>SynthStrings_2</xs:enumeration></rdf:Description><rdf:Description><xs:enumeration>Choir_Aahs</xs:enumeration></rdf:Description><rdf:Description><xs:enumeration>Voice_Oohs</xs:enumeration></rdf:Description><rdf:Description><xs:enumeration>Synth_Voice</xs:enumeration></rdf:Description><rdf:Description><xs:enumeration>Orchestra_Hit</xs:enumeration></rdf:Description><rdf:Description><xs:enumeration>Trumpet</xs:enumeration></rdf:Description><rdf:Description><xs:enumeration>Trombone</xs:enumeration></rdf:Description><rdf:Description><xs:enumeration>Tuba</xs:enumeration></rdf:Description><rdf:Description><xs:enumeration>Muted_Trumpet</xs:enumeration></rdf:Description><rdf:Description><xs:enumeration>French_Horn</xs:enumeration></rdf:Description><rdf:Description><xs:enumeration>Brass_Section</xs:enumeration></rdf:Description><rdf:Description><xs:enumeration>SynthBrass_1</xs:enumeration></rdf:Description><rdf:Description><xs:enumeration>SynthBrass_2</xs:enumeration></rdf:Description><rdf:Description><xs:enumeration>Soprano_Sax</xs:enumeration></rdf:Description><rdf:Description><xs:enumeration>Alto_Sax</xs:enumeration></rdf:Description><rdf:Description><xs:enumeration>Tenor_Sax</xs:enumeration></rdf:Description><rdf:Description><xs:enumeration>Baritone_Sax</xs:enumeration></rdf:Description><rdf:Description><xs:enumeration>Oboe</xs:enumeration></rdf:Description><rdf:Description><xs:enumeration>English_Horn</xs:enumeration></rdf:Description><rdf:Description><xs:enumeration>Bassoon</xs:enumeration></rdf:Description><rdf:Description><xs:enumeration>Clarinet</xs:enumeration></rdf:Description><rdf:Description><xs:enumeration>Piccolo</xs:enumeration></rdf:Description><rdf:Description><xs:enumeration>Flute</xs:enumeration></rdf:Description><rdf:Description><xs:enumeration>Recorder</xs:enumeration></rdf:Description><rdf:Description><xs:enumeration>Pan_Flute</xs:enumeration></rdf:Description><rdf:Description><xs:enumeration>Blown_Bottle</xs:enumeration></rdf:Description><rdf:Description><xs:enumeration>Shakuhachi</xs:enumeration></rdf:Description><rdf:Description><xs:enumeration>Whistle</xs:enumeration></rdf:Description><rdf:Description><xs:enumeration>Ocarina</xs:enumeration></rdf:Description><rdf:Description><xs:enumeration>Lead_1_square</xs:enumeration></rdf:Description><rdf:Description><xs:enumeration>Lead_2_sawtooth</xs:enumeration></rdf:Description><rdf:Description><xs:enumeration>Lead_3_calliope</xs:enumeration></rdf:Description><rdf:Description><xs:enumeration>Lead_4_chiff</xs:enumeration></rdf:Description><rdf:Description><xs:enumeration>Lead_5_charang</xs:enumeration></rdf:Description><rdf:Description><xs:enumeration>Lead_6_voice</xs:enumeration></rdf:Description><rdf:Description><xs:enumeration>Lead_7_fifths</xs:enumeration></rdf:Description><rdf:Description><xs:enumeration>Lead_8_bass_and_lead</xs:enumeration></rdf:Description><rdf:Description><xs:enumeration>Pad_1_new_age</xs:enumeration></rdf:Description><rdf:Description><xs:enumeration>Pad_2_warm</xs:enumeration></rdf:Description><rdf:Description><xs:enumeration>Pad_3_polysynth</xs:enumeration></rdf:Description><rdf:Description><xs:enumeration>Pad_4_choir</xs:enumeration></rdf:Description><rdf:Description><xs:enumeration>Pad_5_bowed</xs:enumeration></rdf:Description><rdf:Description><xs:enumeration>Pad_6_metallic</xs:enumeration></rdf:Description><rdf:Description><xs:enumeration>Pad_7_halo</xs:enumeration></rdf:Description><rdf:Description><xs:enumeration>Pad_8_sweep</xs:enumeration></rdf:Description><rdf:Description><xs:enumeration>FX_1_rain</xs:enumeration></rdf:Description><rdf:Description><xs:enumeration>FX_2_soundtrack</xs:enumeration></rdf:Description><rdf:Description><xs:enumeration>FX_3_crystal</xs:enumeration></rdf:Description><rdf:Description><xs:enumeration>FX_4_atmosphere</xs:enumeration></rdf:Description><rdf:Description><xs:enumeration>FX_5_brightness</xs:enumeration></rdf:Description><rdf:Description><xs:enumeration>FX_6_goblins</xs:enumeration></rdf:Description><rdf:Description><xs:enumeration>FX_7_echoes</xs:enumeration></rdf:Description><rdf:Description><xs:enumeration>FX_8_sci-fi</xs:enumeration></rdf:Description><rdf:Description><xs:enumeration>Sitar</xs:enumeration></rdf:Description><rdf:Description><xs:enumeration>Banjo</xs:enumeration></rdf:Description><rdf:Description><xs:enumeration>Shamisen</xs:enumeration></rdf:Description><rdf:Description><xs:enumeration>Koto</xs:enumeration></rdf:Description><rdf:Description><xs:enumeration>Kalimba</xs:enumeration></rdf:Description><rdf:Description><xs:enumeration>Bagpipe</xs:enumeration></rdf:Description><rdf:Description><xs:enumeration>Fiddle</xs:enumeration></rdf:Description><rdf:Description><xs:enumeration>Shanai</xs:enumeration></rdf:Description><rdf:Description><xs:enumeration>Tinkle_Bell</xs:enumeration></rdf:Description><rdf:Description><xs:enumeration>Agogo</xs:enumeration></rdf:Description><rdf:Description><xs:enumeration>Steel_Drums</xs:enumeration></rdf:Description><rdf:Description><xs:enumeration>Woodblock</xs:enumeration></rdf:Description><rdf:Description><xs:enumeration>Taiko_Drum</xs:enumeration></rdf:Description><rdf:Description><xs:enumeration>Melodic_Tom</xs:enumeration></rdf:Description><rdf:Description><xs:enumeration>Synth_Drum</xs:enumeration></rdf:Description><rdf:Description><xs:enumeration>Reverse_Cymbal</xs:enumeration></rdf:Description><rdf:Description><xs:enumeration>Guitar_Fret_Noise</xs:enumeration></rdf:Description><rdf:Description><xs:enumeration>Breath_Noise</xs:enumeration></rdf:Description><rdf:Description><xs:enumeration>Seashore</xs:enumeration></rdf:Description><rdf:Description><xs:enumeration>Bird_Tweet</xs:enumeration></rdf:Description><rdf:Description><xs:enumeration>Telephone_Ring</xs:enumeration></rdf:Description><rdf:Description><xs:enumeration>Helicopter</xs:enumeration></rdf:Description><rdf:Description><xs:enumeration>Applause</xs:enumeration></rdf:Description><rdf:Description><xs:enumeration>Gunshot</xs:enumeration></rdf:Description><rdf:Description><xs:enumeration>Acoustic_Bass_Drum</xs:enumeration></rdf:Description><rdf:Description><xs:enumeration>Bass_Drum_1</xs:enumeration></rdf:Description><rdf:Description><xs:enumeration>Side_Stick</xs:enumeration></rdf:Description><rdf:Description><xs:enumeration>Acoustic_Snare</xs:enumeration></rdf:Description><rdf:Description><xs:enumeration>Hand_Clap</xs:enumeration></rdf:Description><rdf:Description><xs:enumeration>Electric_Snare</xs:enumeration></rdf:Description><rdf:Description><xs:enumeration>Low_Floor_Tom</xs:enumeration></rdf:Description><rdf:Description><xs:enumeration>Closed_Hi_Hat</xs:enumeration></rdf:Description><rdf:Description><xs:enumeration>High_Floor_Tom</xs:enumeration></rdf:Description><rdf:Description><xs:enumeration>Pedal_Hi-Hat</xs:enumeration></rdf:Description><rdf:Description><xs:enumeration>Low_Tom</xs:enumeration></rdf:Description><rdf:Description><xs:enumeration>Open_Hi-Hat</xs:enumeration></rdf:Description><rdf:Description><xs:enumeration>Low-Mid_Tom</xs:enumeration></rdf:Description><rdf:Description><xs:enumeration>Hi-Mid_Tom</xs:enumeration></rdf:Description><rdf:Description><xs:enumeration>Crash_Cymbal_1</xs:enumeration></rdf:Description><rdf:Description><xs:enumeration>High_Tom</xs:enumeration></rdf:Description><rdf:Description><xs:enumeration>Ride_Cymbal_1</xs:enumeration></rdf:Description><rdf:Description><xs:enumeration>Chinese_Cymbal</xs:enumeration></rdf:Description><rdf:Description><xs:enumeration>Ride_Bell</xs:enumeration></rdf:Description><rdf:Description><xs:enumeration>Tambourine</xs:enumeration></rdf:Description><rdf:Description><xs:enumeration>Splash_Cymbal</xs:enumeration></rdf:Description><rdf:Description><xs:enumeration>Cowbell</xs:enumeration></rdf:Description><rdf:Description><xs:enumeration>Crash_Cymbal_2</xs:enumeration></rdf:Description><rdf:Description><xs:enumeration>Vibraslap</xs:enumeration></rdf:Description><rdf:Description><xs:enumeration>Ride_Cymbal_2</xs:enumeration></rdf:Description><rdf:Description><xs:enumeration>Hi_Bongo</xs:enumeration></rdf:Description><rdf:Description><xs:enumeration>Low_Bongo</xs:enumeration></rdf:Description><rdf:Description><xs:enumeration>Mute_Hi_Conga</xs:enumeration></rdf:Description><rdf:Description><xs:enumeration>Open_Hi_Conga</xs:enumeration></rdf:Description><rdf:Description><xs:enumeration>Low_Conga</xs:enumeration></rdf:Description><rdf:Description><xs:enumeration>High_Timbale</xs:enumeration></rdf:Description><rdf:Description><xs:enumeration>Low_Timbale</xs:enumeration></rdf:Description><rdf:Description><xs:enumeration>High_Agogo</xs:enumeration></rdf:Description><rdf:Description><xs:enumeration>Low_Agogo</xs:enumeration></rdf:Description><rdf:Description><xs:enumeration>Cabasa</xs:enumeration></rdf:Description><rdf:Description><xs:enumeration>Maracas</xs:enumeration></rdf:Description><rdf:Description><xs:enumeration>Short_Whistle</xs:enumeration></rdf:Description><rdf:Description><xs:enumeration>Long_Whistle</xs:enumeration></rdf:Description><rdf:Description><xs:enumeration>Short_Guiro</xs:enumeration></rdf:Description><rdf:Description><xs:enumeration>Long_Guiro</xs:enumeration></rdf:Description><rdf:Description><xs:enumeration>Claves</xs:enumeration></rdf:Description><rdf:Description><xs:enumeration>Hi_Wood_Block</xs:enumeration></rdf:Description><rdf:Description><xs:enumeration>Low_Wood_Block</xs:enumeration></rdf:Description><rdf:Description><xs:enumeration>Mute_Cuica</xs:enumeration></rdf:Description><rdf:Description><xs:enumeration>Open_Cuica</xs:enumeration></rdf:Description><rdf:Description><xs:enumeration>Mute_Triangle</xs:enumeration></rdf:Description><rdf:Description><xs:enumeration>Open_Triangle</xs:enumeration></rdf:Description></owl:withRestrictions></rdfs:Datatype></owl:equivalentClass></rdfs:Datatype>
	<rdfs:Datatype rdf:ID="data.MIDIVALUE">
		<owl:equivalentClass><rdfs:Datatype>
		<owl:onDatatype rdf:resource="&xs;nonNegativeInteger"/><owl:withRestrictions rdf:parseType="Collection"><rdf:Description><xs:maxInclusive>127</xs:maxInclusive></rdf:Description></owl:withRestrictions></rdfs:Datatype></owl:equivalentClass></rdfs:Datatype>
	<rdfs:Datatype rdf:ID="data.MODE">
		<owl:equivalentClass><rdfs:Datatype>
		<owl:onDatatype rdf:resource="&xs;token"/><owl:withRestrictions rdf:parseType="Collection"><rdf:Description><xs:enumeration>major</xs:enumeration></rdf:Description><rdf:Description><xs:enumeration>minor</xs:enumeration></rdf:Description><rdf:Description><xs:enumeration>dorian</xs:enumeration></rdf:Description><rdf:Description><xs:enumeration>phrygian</xs:enumeration></rdf:Description><rdf:Description><xs:enumeration>lydian</xs:enumeration></rdf:Description><rdf:Description><xs:enumeration>mixolydian</xs:enumeration></rdf:Description><rdf:Description><xs:enumeration>aeolian</xs:enumeration></rdf:Description><rdf:Description><xs:enumeration>locrian</xs:enumeration></rdf:Description></owl:withRestrictions></rdfs:Datatype></owl:equivalentClass></rdfs:Datatype>
	<rdfs:Datatype rdf:ID="data.MODUSMAIOR">
		<owl:equivalentClass><rdfs:Datatype>
		<owl:onDatatype rdf:resource="&xs;positiveInteger"/><owl:withRestrictions rdf:parseType="Collection"><rdf:Description><xs:minInclusive>2</xs:minInclusive></rdf:Description><rdf:Description><xs:maxInclusive>3</xs:maxInclusive></rdf:Description></owl:withRestrictions></rdfs:Datatype></owl:equivalentClass></rdfs:Datatype>
	<rdfs:Datatype rdf:ID="data.MODUSMINOR">
		<owl:equivalentClass><rdfs:Datatype>
		<owl:onDatatype rdf:resource="&xs;positiveInteger"/><owl:withRestrictions rdf:parseType="Collection"><rdf:Description><xs:minInclusive>2</xs:minInclusive></rdf:Description><rdf:Description><xs:maxInclusive>3</xs:maxInclusive></rdf:Description></owl:withRestrictions></rdfs:Datatype></owl:equivalentClass></rdfs:Datatype>
	<rdfs:Datatype rdf:ID="data.MUSICFONT">
		<owl:equivalentClass><rdfs:Datatype>
		<owl:onDatatype rdf:resource="&xs;token"/><owl:withRestrictions rdf:parseType="Collection"></owl:withRestrictions></rdfs:Datatype></owl:equivalentClass></rdfs:Datatype>
	<rdfs:Datatype rdf:ID="data.NMTOKEN">
		<owl:equivalentClass><rdfs:Datatype>
		<owl:onDatatype rdf:resource="&xs;NMTOKEN"/><owl:withRestrictions rdf:parseType="Collection"></owl:withRestrictions></rdfs:Datatype></owl:equivalentClass></rdfs:Datatype>
	<rdfs:Datatype rdf:ID="data.NOTATIONTYPE">
		<owl:equivalentClass><rdfs:Datatype>
		<owl:onDatatype rdf:resource="&xs;token"/><owl:withRestrictions rdf:parseType="Collection"><rdf:Description><xs:enumeration>cmn</xs:enumeration></rdf:Description><rdf:Description><xs:enumeration>mensural</xs:enumeration></rdf:Description><rdf:Description><xs:enumeration>mensural.black</xs:enumeration></rdf:Description><rdf:Description><xs:enumeration>mensural.white</xs:enumeration></rdf:Description><rdf:Description><xs:enumeration>neume</xs:enumeration></rdf:Description><rdf:Description><xs:enumeration>tab</xs:enumeration></rdf:Description></owl:withRestrictions></rdfs:Datatype></owl:equivalentClass></rdfs:Datatype>
	<rdfs:Datatype rdf:ID="data.NOTEHEADMODIFIER">
		<owl:equivalentClass><rdfs:Datatype>
		<owl:unionOf rdf:parseType="Collection"><rdf:Description rdf:about="mei:data.NOTEHEADMODIFIER.list"/><rdf:Description rdf:about="mei:data.NOTEHEADMODIFIER.pat"/></owl:unionOf></rdfs:Datatype></owl:equivalentClass></rdfs:Datatype>
	<rdfs:Datatype rdf:ID="data.NOTEHEADMODIFIER.list">
		<owl:equivalentClass><rdfs:Datatype>
		<owl:onDatatype rdf:resource="&xs;token"/><owl:withRestrictions rdf:parseType="Collection"><rdf:Description><xs:enumeration>slash</xs:enumeration></rdf:Description><rdf:Description><xs:enumeration>backslash</xs:enumeration></rdf:Description><rdf:Description><xs:enumeration>vline</xs:enumeration></rdf:Description><rdf:Description><xs:enumeration>hline</xs:enumeration></rdf:Description><rdf:Description><xs:enumeration>centerdot</xs:enumeration></rdf:Description><rdf:Description><xs:enumeration>paren</xs:enumeration></rdf:Description><rdf:Description><xs:enumeration>brack</xs:enumeration></rdf:Description><rdf:Description><xs:enumeration>box</xs:enumeration></rdf:Description><rdf:Description><xs:enumeration>circle</xs:enumeration></rdf:Description><rdf:Description><xs:enumeration>dblwhole</xs:enumeration></rdf:Description></owl:withRestrictions></rdfs:Datatype></owl:equivalentClass></rdfs:Datatype>
	<rdfs:Datatype rdf:ID="data.NOTEHEADMODIFIER.pat">
		<owl:equivalentClass><rdfs:Datatype>
		<owl:unionOf rdf:parseType="Collection"><rdf:Description rdf:about="NS_data.NOTEHEADMODIFIER.pat_UNType_1"/><rdf:Description rdf:about="NS_data.NOTEHEADMODIFIER.pat_UNType_2"/></owl:unionOf></rdfs:Datatype></owl:equivalentClass></rdfs:Datatype>
	<rdfs:Datatype rdf:ID="NS_data.NOTEHEADMODIFIER.pat_UNType_1">
		<owl:equivalentClass><rdfs:Datatype>
		<owl:onDatatype rdf:resource="&xs;string"/><owl:withRestrictions rdf:parseType="Collection"><rdf:Description><xs:pattern>centertext\((A|B|C|D|E|F|G)(f|♭|n|♮|s|♯)?\)</xs:pattern></rdf:Description></owl:withRestrictions></rdfs:Datatype></owl:equivalentClass></rdfs:Datatype>
	<rdfs:Datatype rdf:ID="NS_data.NOTEHEADMODIFIER.pat_UNType_2">
		<owl:equivalentClass><rdfs:Datatype>
		<owl:onDatatype rdf:resource="&xs;string"/><owl:withRestrictions rdf:parseType="Collection"><rdf:Description><xs:pattern>centertext\(H(s|♯)?\)</xs:pattern></rdf:Description></owl:withRestrictions></rdfs:Datatype></owl:equivalentClass></rdfs:Datatype>
	<rdfs:Datatype rdf:ID="data.OCTAVE">
		<owl:equivalentClass><rdfs:Datatype>
		<owl:onDatatype rdf:resource="&xs;nonNegativeInteger"/><owl:withRestrictions rdf:parseType="Collection"><rdf:Description><xs:maxInclusive>9</xs:maxInclusive></rdf:Description></owl:withRestrictions></rdfs:Datatype></owl:equivalentClass></rdfs:Datatype>
	<rdfs:Datatype rdf:ID="data.OCTAVE.DIS">
		<owl:equivalentClass><rdfs:Datatype>
		<owl:onDatatype rdf:resource="&xs;positiveInteger"/><owl:withRestrictions rdf:parseType="Collection"><rdf:Description><xs:pattern>8|15|22</xs:pattern></rdf:Description></owl:withRestrictions></rdfs:Datatype></owl:equivalentClass></rdfs:Datatype>
	<rdfs:Datatype rdf:ID="data.ORIENTATION">
		<owl:equivalentClass><rdfs:Datatype>
		<owl:onDatatype rdf:resource="&xs;token"/><owl:withRestrictions rdf:parseType="Collection"><rdf:Description><xs:pattern>reversed|90CW|90CCW</xs:pattern></rdf:Description></owl:withRestrictions></rdfs:Datatype></owl:equivalentClass></rdfs:Datatype>
	<rdfs:Datatype rdf:ID="data.OTHERSTAFF">
		<owl:equivalentClass><rdfs:Datatype>
		<owl:onDatatype rdf:resource="&xs;token"/><owl:withRestrictions rdf:parseType="Collection"><rdf:Description><xs:enumeration>above</xs:enumeration></rdf:Description><rdf:Description><xs:enumeration>below</xs:enumeration></rdf:Description></owl:withRestrictions></rdfs:Datatype></owl:equivalentClass></rdfs:Datatype>
	<rdfs:Datatype rdf:ID="data.PAGE.PANELS">
		<owl:equivalentClass><rdfs:Datatype>
		<owl:onDatatype rdf:resource="&xs;positiveInteger"/><owl:withRestrictions rdf:parseType="Collection"><rdf:Description><xs:minInclusive>1</xs:minInclusive></rdf:Description><rdf:Description><xs:maxInclusive>2</xs:maxInclusive></rdf:Description></owl:withRestrictions></rdfs:Datatype></owl:equivalentClass></rdfs:Datatype>
	<rdfs:Datatype rdf:ID="data.PERCENT">
		<owl:equivalentClass><rdfs:Datatype>
		<owl:onDatatype rdf:resource="&xs;token"/><owl:withRestrictions rdf:parseType="Collection"><rdf:Description><xs:pattern>[0-9]+(\.?[0-9]*)?%</xs:pattern></rdf:Description></owl:withRestrictions></rdfs:Datatype></owl:equivalentClass></rdfs:Datatype>
	<rdfs:Datatype rdf:ID="data.PGSCALE">
		<owl:equivalentClass><rdfs:Datatype>
		<owl:onDatatype rdf:resource="&mei;data.PERCENT"/><owl:withRestrictions rdf:parseType="Collection"></owl:withRestrictions></rdfs:Datatype></owl:equivalentClass></rdfs:Datatype>
	<rdfs:Datatype rdf:ID="data.PITCHCLASS">
		<owl:equivalentClass><rdfs:Datatype>
		<owl:onDatatype rdf:resource="&xs;nonNegativeInteger"/><owl:withRestrictions rdf:parseType="Collection"><rdf:Description><xs:maxInclusive>11</xs:maxInclusive></rdf:Description></owl:withRestrictions></rdfs:Datatype></owl:equivalentClass></rdfs:Datatype>
	<rdfs:Datatype rdf:ID="data.PITCHNAME">
		<owl:equivalentClass><rdfs:Datatype>
		<owl:onDatatype rdf:resource="&xs;token"/><owl:withRestrictions rdf:parseType="Collection"><rdf:Description><xs:pattern>[a-g]</xs:pattern></rdf:Description></owl:withRestrictions></rdfs:Datatype></owl:equivalentClass></rdfs:Datatype>
	<rdfs:Datatype rdf:ID="data.PITCHNAME.GES">
		<owl:equivalentClass><rdfs:Datatype>
		<owl:onDatatype rdf:resource="&xs;token"/><owl:withRestrictions rdf:parseType="Collection"><rdf:Description><xs:pattern>[a-g]|none</xs:pattern></rdf:Description></owl:withRestrictions></rdfs:Datatype></owl:equivalentClass></rdfs:Datatype>
	<rdfs:Datatype rdf:ID="data.PITCHNUMBER">
		<owl:equivalentClass><rdfs:Datatype>
		<owl:onDatatype rdf:resource="&xs;nonNegativeInteger"/><owl:withRestrictions rdf:parseType="Collection"></owl:withRestrictions></rdfs:Datatype></owl:equivalentClass></rdfs:Datatype>
	<rdfs:Datatype rdf:ID="data.PLACE">
		<owl:equivalentClass><rdfs:Datatype>
		<owl:onDatatype rdf:resource="&xs;token"/><owl:withRestrictions rdf:parseType="Collection"><rdf:Description><xs:enumeration>above</xs:enumeration></rdf:Description><rdf:Description><xs:enumeration>below</xs:enumeration></rdf:Description></owl:withRestrictions></rdfs:Datatype></owl:equivalentClass></rdfs:Datatype>
	<rdfs:Datatype rdf:ID="data.PROLATIO">
		<owl:equivalentClass><rdfs:Datatype>
		<owl:onDatatype rdf:resource="&xs;positiveInteger"/><owl:withRestrictions rdf:parseType="Collection"><rdf:Description><xs:minInclusive>2</xs:minInclusive></rdf:Description><rdf:Description><xs:maxInclusive>3</xs:maxInclusive></rdf:Description></owl:withRestrictions></rdfs:Datatype></owl:equivalentClass></rdfs:Datatype>
	<rdfs:Datatype rdf:ID="data.ROTATION">
		<owl:equivalentClass><rdfs:Datatype>
		<owl:unionOf rdf:parseType="Collection"><rdf:Description rdf:about="mei:data.DEGREES"/><rdf:Description rdf:about="mei:data.ROTATIONDIRECTION"/></owl:unionOf></rdfs:Datatype></owl:equivalentClass></rdfs:Datatype>
	<rdfs:Datatype rdf:ID="data.ROTATIONDIRECTION">
		<owl:equivalentClass><rdfs:Datatype>
		<owl:onDatatype rdf:resource="&xs;token"/><owl:withRestrictions rdf:parseType="Collection"><rdf:Description><xs:enumeration>none</xs:enumeration></rdf:Description><rdf:Description><xs:enumeration>down</xs:enumeration></rdf:Description><rdf:Description><xs:enumeration>left</xs:enumeration></rdf:Description><rdf:Description><xs:enumeration>ne</xs:enumeration></rdf:Description><rdf:Description><xs:enumeration>nw</xs:enumeration></rdf:Description><rdf:Description><xs:enumeration>se</xs:enumeration></rdf:Description><rdf:Description><xs:enumeration>sw</xs:enumeration></rdf:Description></owl:withRestrictions></rdfs:Datatype></owl:equivalentClass></rdfs:Datatype>
	<rdfs:Datatype rdf:ID="data.SCALEDEGREE">
		<owl:equivalentClass><rdfs:Datatype>
		<owl:onDatatype rdf:resource="&xs;token"/><owl:withRestrictions rdf:parseType="Collection"><rdf:Description><xs:pattern>(\^|v)?[1-7](\+|\-)?</xs:pattern></rdf:Description></owl:withRestrictions></rdfs:Datatype></owl:equivalentClass></rdfs:Datatype>
	<rdfs:Datatype rdf:ID="data.SIZE">
		<owl:equivalentClass><rdfs:Datatype>
		<owl:onDatatype rdf:resource="&xs;token"/><owl:withRestrictions rdf:parseType="Collection"><rdf:Description><xs:enumeration>normal</xs:enumeration></rdf:Description><rdf:Description><xs:enumeration>cue</xs:enumeration></rdf:Description></owl:withRestrictions></rdfs:Datatype></owl:equivalentClass></rdfs:Datatype>
	<rdfs:Datatype rdf:ID="data.SLASH">
		<owl:equivalentClass><rdfs:Datatype>
		<owl:onDatatype rdf:resource="&xs;positiveInteger"/><owl:withRestrictions rdf:parseType="Collection"><rdf:Description><xs:minInclusive>1</xs:minInclusive></rdf:Description><rdf:Description><xs:maxInclusive>6</xs:maxInclusive></rdf:Description></owl:withRestrictions></rdfs:Datatype></owl:equivalentClass></rdfs:Datatype>
	<rdfs:Datatype rdf:ID="data.SLUR">
		<owl:equivalentClass><rdfs:Datatype>
		<owl:onDatatype rdf:resource="&xs;token"/><owl:withRestrictions rdf:parseType="Collection"><rdf:Description><xs:pattern>[i|m|t][1-6]</xs:pattern></rdf:Description></owl:withRestrictions></rdfs:Datatype></owl:equivalentClass></rdfs:Datatype>
	<rdfs:Datatype rdf:ID="data.STAFFLOC">
		<owl:equivalentClass><rdfs:Datatype>
		<owl:onDatatype rdf:resource="&xs;integer"/><owl:withRestrictions rdf:parseType="Collection"></owl:withRestrictions></rdfs:Datatype></owl:equivalentClass></rdfs:Datatype>
	<rdfs:Datatype rdf:ID="data.STAFFREL">
		<owl:equivalentClass><rdfs:Datatype>
		<owl:onDatatype rdf:resource="&xs;token"/><owl:withRestrictions rdf:parseType="Collection"><rdf:Description><xs:enumeration>above</xs:enumeration></rdf:Description><rdf:Description><xs:enumeration>below</xs:enumeration></rdf:Description><rdf:Description><xs:enumeration>within</xs:enumeration></rdf:Description></owl:withRestrictions></rdfs:Datatype></owl:equivalentClass></rdfs:Datatype>
	<rdfs:Datatype rdf:ID="data.STEMDIRECTION">
		<owl:equivalentClass><rdfs:Datatype>
		<owl:unionOf rdf:parseType="Collection"><rdf:Description rdf:about="mei:data.STEMDIRECTION.basic"/><rdf:Description rdf:about="mei:data.STEMDIRECTION.extended"/></owl:unionOf></rdfs:Datatype></owl:equivalentClass></rdfs:Datatype>
	<rdfs:Datatype rdf:ID="data.STEMDIRECTION.basic">
		<owl:equivalentClass><rdfs:Datatype>
		<owl:onDatatype rdf:resource="&xs;token"/><owl:withRestrictions rdf:parseType="Collection"><rdf:Description><xs:enumeration>up</xs:enumeration></rdf:Description><rdf:Description><xs:enumeration>down</xs:enumeration></rdf:Description></owl:withRestrictions></rdfs:Datatype></owl:equivalentClass></rdfs:Datatype>
	<rdfs:Datatype rdf:ID="data.STEMDIRECTION.extended">
		<owl:equivalentClass><rdfs:Datatype>
		<owl:onDatatype rdf:resource="&xs;token"/><owl:withRestrictions rdf:parseType="Collection"><rdf:Description><xs:enumeration>left</xs:enumeration></rdf:Description><rdf:Description><xs:enumeration>right</xs:enumeration></rdf:Description><rdf:Description><xs:enumeration>ne</xs:enumeration></rdf:Description><rdf:Description><xs:enumeration>se</xs:enumeration></rdf:Description><rdf:Description><xs:enumeration>nw</xs:enumeration></rdf:Description><rdf:Description><xs:enumeration>sw</xs:enumeration></rdf:Description></owl:withRestrictions></rdfs:Datatype></owl:equivalentClass></rdfs:Datatype>
	<rdfs:Datatype rdf:ID="data.STEMMODIFIER">
		<owl:equivalentClass><rdfs:Datatype>
		<owl:onDatatype rdf:resource="&xs;token"/><owl:withRestrictions rdf:parseType="Collection"><rdf:Description><xs:enumeration>none</xs:enumeration></rdf:Description><rdf:Description><xs:enumeration>1slash</xs:enumeration></rdf:Description><rdf:Description><xs:enumeration>2slash</xs:enumeration></rdf:Description><rdf:Description><xs:enumeration>3slash</xs:enumeration></rdf:Description><rdf:Description><xs:enumeration>4slash</xs:enumeration></rdf:Description><rdf:Description><xs:enumeration>5slash</xs:enumeration></rdf:Description><rdf:Description><xs:enumeration>6slash</xs:enumeration></rdf:Description><rdf:Description><xs:enumeration>sprech</xs:enumeration></rdf:Description><rdf:Description><xs:enumeration>z</xs:enumeration></rdf:Description></owl:withRestrictions></rdfs:Datatype></owl:equivalentClass></rdfs:Datatype>
	<rdfs:Datatype rdf:ID="data.STEMPOSITION">
		<owl:equivalentClass><rdfs:Datatype>
		<owl:onDatatype rdf:resource="&xs;token"/><owl:withRestrictions rdf:parseType="Collection"><rdf:Description><xs:enumeration>left</xs:enumeration></rdf:Description><rdf:Description><xs:enumeration>right</xs:enumeration></rdf:Description><rdf:Description><xs:enumeration>center</xs:enumeration></rdf:Description></owl:withRestrictions></rdfs:Datatype></owl:equivalentClass></rdfs:Datatype>
	<rdfs:Datatype rdf:ID="data.STRINGNUMBER">
		<owl:equivalentClass><rdfs:Datatype>
		<owl:onDatatype rdf:resource="&xs;positiveInteger"/><owl:withRestrictions rdf:parseType="Collection"></owl:withRestrictions></rdfs:Datatype></owl:equivalentClass></rdfs:Datatype>
	<rdfs:Datatype rdf:ID="data.TEMPERAMENT">
		<owl:equivalentClass><rdfs:Datatype>
		<owl:onDatatype rdf:resource="&xs;token"/><owl:withRestrictions rdf:parseType="Collection"><rdf:Description><xs:enumeration>equal</xs:enumeration></rdf:Description><rdf:Description><xs:enumeration>just</xs:enumeration></rdf:Description><rdf:Description><xs:enumeration>mean</xs:enumeration></rdf:Description><rdf:Description><xs:enumeration>pythagorean</xs:enumeration></rdf:Description></owl:withRestrictions></rdfs:Datatype></owl:equivalentClass></rdfs:Datatype>
	<rdfs:Datatype rdf:ID="data.TEMPOVALUE">
		<owl:equivalentClass><rdfs:Datatype>
		<owl:onDatatype rdf:resource="&xs;decimal"/><owl:withRestrictions rdf:parseType="Collection"></owl:withRestrictions></rdfs:Datatype></owl:equivalentClass></rdfs:Datatype>
	<rdfs:Datatype rdf:ID="data.TEMPUS">
		<owl:equivalentClass><rdfs:Datatype>
		<owl:onDatatype rdf:resource="&xs;positiveInteger"/><owl:withRestrictions rdf:parseType="Collection"><rdf:Description><xs:minInclusive>2</xs:minInclusive></rdf:Description><rdf:Description><xs:maxInclusive>3</xs:maxInclusive></rdf:Description></owl:withRestrictions></rdfs:Datatype></owl:equivalentClass></rdfs:Datatype>
	<rdfs:Datatype rdf:ID="data.TEXTRENDITIONLIST">
		<owl:equivalentClass><rdfs:Datatype>
		<owl:onDatatype rdf:resource="&xs;token"/><owl:withRestrictions rdf:parseType="Collection"><rdf:Description><xs:enumeration>italic</xs:enumeration></rdf:Description><rdf:Description><xs:enumeration>oblique</xs:enumeration></rdf:Description><rdf:Description><xs:enumeration>smcaps</xs:enumeration></rdf:Description><rdf:Description><xs:enumeration>bold</xs:enumeration></rdf:Description><rdf:Description><xs:enumeration>bolder</xs:enumeration></rdf:Description><rdf:Description><xs:enumeration>lighter</xs:enumeration></rdf:Description><rdf:Description><xs:enumeration>box</xs:enumeration></rdf:Description><rdf:Description><xs:enumeration>circle</xs:enumeration></rdf:Description><rdf:Description><xs:enumeration>dbox</xs:enumeration></rdf:Description><rdf:Description><xs:enumeration>tbox</xs:enumeration></rdf:Description><rdf:Description><xs:enumeration>bslash</xs:enumeration></rdf:Description><rdf:Description><xs:enumeration>fslash</xs:enumeration></rdf:Description><rdf:Description><xs:enumeration>line-through</xs:enumeration></rdf:Description><rdf:Description><xs:enumeration>none</xs:enumeration></rdf:Description><rdf:Description><xs:enumeration>overline</xs:enumeration></rdf:Description><rdf:Description><xs:enumeration>overstrike</xs:enumeration></rdf:Description><rdf:Description><xs:enumeration>strike</xs:enumeration></rdf:Description><rdf:Description><xs:enumeration>sub</xs:enumeration></rdf:Description><rdf:Description><xs:enumeration>sup</xs:enumeration></rdf:Description><rdf:Description><xs:enumeration>underline</xs:enumeration></rdf:Description><rdf:Description><xs:enumeration>ltr</xs:enumeration></rdf:Description><rdf:Description><xs:enumeration>rtl</xs:enumeration></rdf:Description><rdf:Description><xs:enumeration>lro</xs:enumeration></rdf:Description><rdf:Description><xs:enumeration>rlo</xs:enumeration></rdf:Description></owl:withRestrictions></rdfs:Datatype></owl:equivalentClass></rdfs:Datatype>
	<rdfs:Datatype rdf:ID="data.TEXTRENDITIONPAR">
		<owl:equivalentClass><rdfs:Datatype>
		<owl:unionOf rdf:parseType="Collection"><rdf:Description rdf:about="NS_data.TEXTRENDITIONPAR_UNType_1"/><rdf:Description rdf:about="NS_data.TEXTRENDITIONPAR_UNType_2"/></owl:unionOf></rdfs:Datatype></owl:equivalentClass></rdfs:Datatype>
	<rdfs:Datatype rdf:ID="NS_data.TEXTRENDITIONPAR_UNType_1">
		<owl:equivalentClass><rdfs:Datatype>
		<owl:onDatatype rdf:resource="&xs;string"/><owl:withRestrictions rdf:parseType="Collection"><rdf:Description><xs:pattern>(underline|overline|line-through|strike)\(\d+\)</xs:pattern></rdf:Description></owl:withRestrictions></rdfs:Datatype></owl:equivalentClass></rdfs:Datatype>
	<rdfs:Datatype rdf:ID="NS_data.TEXTRENDITIONPAR_UNType_2">
		<owl:equivalentClass><rdfs:Datatype>
		<owl:onDatatype rdf:resource="&xs;string"/><owl:withRestrictions rdf:parseType="Collection"><rdf:Description><xs:pattern>(letter-spacing|line-height)\((\+|-)?\d+(\.\d+)?%?\)</xs:pattern></rdf:Description></owl:withRestrictions></rdfs:Datatype></owl:equivalentClass></rdfs:Datatype>
	<rdfs:Datatype rdf:ID="data.TEXTRENDITION">
		<owl:equivalentClass><rdfs:Datatype>
		<owl:unionOf rdf:parseType="Collection"><rdf:Description rdf:about="mei:data.TEXTRENDITIONLIST"/><rdf:Description rdf:about="mei:data.TEXTRENDITIONPAR"/></owl:unionOf></rdfs:Datatype></owl:equivalentClass></rdfs:Datatype>
	<rdfs:Datatype rdf:ID="data.TIE">
		<owl:equivalentClass><rdfs:Datatype>
		<owl:onDatatype rdf:resource="&xs;token"/><owl:withRestrictions rdf:parseType="Collection"><rdf:Description><xs:pattern>[i|m|t]</xs:pattern></rdf:Description></owl:withRestrictions></rdfs:Datatype></owl:equivalentClass></rdfs:Datatype>
	<rdfs:Datatype rdf:ID="data.TSTAMPOFFSET">
		<owl:equivalentClass><rdfs:Datatype>
		<owl:onDatatype rdf:resource="&xs;decimal"/><owl:withRestrictions rdf:parseType="Collection"></owl:withRestrictions></rdfs:Datatype></owl:equivalentClass></rdfs:Datatype>
	<rdfs:Datatype rdf:ID="data.TUPLET">
		<owl:equivalentClass><rdfs:Datatype>
		<owl:onDatatype rdf:resource="&xs;token"/><owl:withRestrictions rdf:parseType="Collection"><rdf:Description><xs:pattern>[i|m|t][1-6]</xs:pattern></rdf:Description></owl:withRestrictions></rdfs:Datatype></owl:equivalentClass></rdfs:Datatype>
	<rdfs:Datatype rdf:ID="data.UNEUMEFORM">
		<owl:equivalentClass><rdfs:Datatype>
		<owl:onDatatype rdf:resource="&xs;token"/><owl:withRestrictions rdf:parseType="Collection"><rdf:Description><xs:enumeration>liquescent1</xs:enumeration></rdf:Description><rdf:Description><xs:enumeration>liquescent2</xs:enumeration></rdf:Description><rdf:Description><xs:enumeration>liquescent3</xs:enumeration></rdf:Description><rdf:Description><xs:enumeration>quilismatic</xs:enumeration></rdf:Description><rdf:Description><xs:enumeration>rectangular</xs:enumeration></rdf:Description><rdf:Description><xs:enumeration>rhombic</xs:enumeration></rdf:Description><rdf:Description><xs:enumeration>tied</xs:enumeration></rdf:Description></owl:withRestrictions></rdfs:Datatype></owl:equivalentClass></rdfs:Datatype>
	<rdfs:Datatype rdf:ID="data.UNEUMENAME">
		<owl:equivalentClass><rdfs:Datatype>
		<owl:onDatatype rdf:resource="&xs;token"/><owl:withRestrictions rdf:parseType="Collection"><rdf:Description><xs:enumeration>punctum</xs:enumeration></rdf:Description><rdf:Description><xs:enumeration>virga</xs:enumeration></rdf:Description><rdf:Description><xs:enumeration>pes</xs:enumeration></rdf:Description><rdf:Description><xs:enumeration>clivis</xs:enumeration></rdf:Description><rdf:Description><xs:enumeration>torculus</xs:enumeration></rdf:Description><rdf:Description><xs:enumeration>torculusresupinus</xs:enumeration></rdf:Description><rdf:Description><xs:enumeration>porrectus</xs:enumeration></rdf:Description><rdf:Description><xs:enumeration>porrectusflexus</xs:enumeration></rdf:Description><rdf:Description><xs:enumeration>apostropha</xs:enumeration></rdf:Description><rdf:Description><xs:enumeration>oriscus</xs:enumeration></rdf:Description><rdf:Description><xs:enumeration>pressusmaior</xs:enumeration></rdf:Description><rdf:Description><xs:enumeration>pressusminor</xs:enumeration></rdf:Description><rdf:Description><xs:enumeration>virgastrata</xs:enumeration></rdf:Description></owl:withRestrictions></rdfs:Datatype></owl:equivalentClass></rdfs:Datatype>
	<rdfs:Datatype rdf:ID="data.URI">
		<owl:equivalentClass><rdfs:Datatype>
		<owl:onDatatype rdf:resource="&xs;anyURI"/><owl:withRestrictions rdf:parseType="Collection"></owl:withRestrictions></rdfs:Datatype></owl:equivalentClass></rdfs:Datatype>
	<rdfs:Datatype rdf:ID="data.BETYPE">
		<owl:equivalentClass><rdfs:Datatype>
		<owl:onDatatype rdf:resource="&xs;token"/><owl:withRestrictions rdf:parseType="Collection"><rdf:Description><xs:enumeration>byte</xs:enumeration></rdf:Description><rdf:Description><xs:enumeration>smil</xs:enumeration></rdf:Description><rdf:Description><xs:enumeration>midi</xs:enumeration></rdf:Description><rdf:Description><xs:enumeration>mmc</xs:enumeration></rdf:Description><rdf:Description><xs:enumeration>mtc</xs:enumeration></rdf:Description><rdf:Description><xs:enumeration>smpte-25</xs:enumeration></rdf:Description><rdf:Description><xs:enumeration>smpte-24</xs:enumeration></rdf:Description><rdf:Description><xs:enumeration>smpte-df30</xs:enumeration></rdf:Description><rdf:Description><xs:enumeration>smpte-ndf30</xs:enumeration></rdf:Description><rdf:Description><xs:enumeration>smpte-df29.97</xs:enumeration></rdf:Description><rdf:Description><xs:enumeration>smpte-ndf29.97</xs:enumeration></rdf:Description><rdf:Description><xs:enumeration>tcf</xs:enumeration></rdf:Description><rdf:Description><xs:enumeration>time</xs:enumeration></rdf:Description></owl:withRestrictions></rdfs:Datatype></owl:equivalentClass></rdfs:Datatype>
	<rdfs:Datatype rdf:ID="data.DURATION.cmn">
		<owl:equivalentClass><rdfs:Datatype>
		<owl:onDatatype rdf:resource="&xs;token"/><owl:withRestrictions rdf:parseType="Collection"><rdf:Description><xs:enumeration>long</xs:enumeration></rdf:Description><rdf:Description><xs:enumeration>breve</xs:enumeration></rdf:Description><rdf:Description><xs:enumeration>1</xs:enumeration></rdf:Description><rdf:Description><xs:enumeration>2</xs:enumeration></rdf:Description><rdf:Description><xs:enumeration>4</xs:enumeration></rdf:Description><rdf:Description><xs:enumeration>8</xs:enumeration></rdf:Description><rdf:Description><xs:enumeration>16</xs:enumeration></rdf:Description><rdf:Description><xs:enumeration>32</xs:enumeration></rdf:Description><rdf:Description><xs:enumeration>64</xs:enumeration></rdf:Description><rdf:Description><xs:enumeration>128</xs:enumeration></rdf:Description><rdf:Description><xs:enumeration>256</xs:enumeration></rdf:Description><rdf:Description><xs:enumeration>512</xs:enumeration></rdf:Description><rdf:Description><xs:enumeration>1024</xs:enumeration></rdf:Description><rdf:Description><xs:enumeration>2048</xs:enumeration></rdf:Description></owl:withRestrictions></rdfs:Datatype></owl:equivalentClass></rdfs:Datatype>
	<rdfs:Datatype rdf:ID="data.DURATION.mensural">
		<owl:equivalentClass><rdfs:Datatype>
		<owl:onDatatype rdf:resource="&xs;token"/><owl:withRestrictions rdf:parseType="Collection"><rdf:Description><xs:enumeration>maxima</xs:enumeration></rdf:Description><rdf:Description><xs:enumeration>longa</xs:enumeration></rdf:Description><rdf:Description><xs:enumeration>brevis</xs:enumeration></rdf:Description><rdf:Description><xs:enumeration>semibrevis</xs:enumeration></rdf:Description><rdf:Description><xs:enumeration>minima</xs:enumeration></rdf:Description><rdf:Description><xs:enumeration>semiminima</xs:enumeration></rdf:Description><rdf:Description><xs:enumeration>fusa</xs:enumeration></rdf:Description><rdf:Description><xs:enumeration>semifusa</xs:enumeration></rdf:Description></owl:withRestrictions></rdfs:Datatype></owl:equivalentClass></rdfs:Datatype>
	<rdfs:Datatype rdf:ID="data.ORNAM.cmn">
		<owl:equivalentClass><rdfs:Datatype>
		<owl:onDatatype rdf:resource="&xs;token"/><owl:withRestrictions rdf:parseType="Collection"><rdf:Description><xs:pattern>[A|a|b|I|i|K|k|M|m|N|n|S|s|T|t|O]|(A|a|S|s|K|k)?(T|t|M|m)(I|i|S|s)?</xs:pattern></rdf:Description></owl:withRestrictions></rdfs:Datatype></owl:equivalentClass></rdfs:Datatype>
	<!--	Class Definitions	-->
		<owl:DatatypeProperty rdf:ID="subtype__xs_NMTOKEN">
		<rdfs:range rdf:resource="&xs;NMTOKEN"/>
		<rdfs:label>subtype</rdfs:label>
	<rdfs:comment>Provide any sub-classification for the element, additional to that given by its type attribute.</rdfs:comment>
	</owl:DatatypeProperty>
	<owl:DatatypeProperty rdf:ID="n__xs_nonNegativeInteger">
		<rdfs:range rdf:resource="&xs;nonNegativeInteger"/>
		<rdfs:label>n</rdfs:label>
	<rdfs:comment>A non-negative integer value functioning as a &quot;name&quot;.</rdfs:comment>
	</owl:DatatypeProperty>
	<owl:DatatypeProperty rdf:ID="value__xs_decimal">
		<rdfs:range rdf:resource="&xs;decimal"/>
		<rdfs:label>value</rdfs:label>
	<rdfs:comment>Numeric value capturing a measurement or count. Can only be interpreted in combination with the unit attribute.</rdfs:comment>
	</owl:DatatypeProperty>
	<owl:DatatypeProperty rdf:ID="halign__mei_data.HORIZONTALALIGNMENT">
		<rdfs:range rdf:resource="&datatypes;data.HORIZONTALALIGNMENT"/>
		<rdfs:label>halign</rdfs:label>
	<rdfs:comment>Records horizontal alignment of the page footer.</rdfs:comment>
	</owl:DatatypeProperty>
	<owl:DatatypeProperty rdf:ID="rotation__mei_data.DEGREES">
		<rdfs:range rdf:resource="&datatypes;data.DEGREES"/>
		<rdfs:label>rotation</rdfs:label>
	<rdfs:comment>A positive value for rotation rotates the text in a counter-clockwise fashion, while negative values produce clockwise rotation.</rdfs:comment>
	</owl:DatatypeProperty>
	<owl:DatatypeProperty rdf:ID="delim__xs_string">
		<rdfs:range rdf:resource="&xs;string"/>
		<rdfs:label>delim</rdfs:label>
	<rdfs:comment>Indicates the delimiter used to mark the portions of text that are to be stacked.</rdfs:comment>
	</owl:DatatypeProperty>
	<owl:DatatypeProperty rdf:ID="mainLang__xs_language">
		<rdfs:range rdf:resource="&xs;language"/>
		<rdfs:label>mainLang</rdfs:label>
	<rdfs:comment>(main language) supplies a code which identifies the chief language used in the bibliographic work.</rdfs:comment>
	</owl:DatatypeProperty>
	<owl:DatatypeProperty rdf:ID="version__xs_NMTOKEN">
		<rdfs:range rdf:resource="&xs;NMTOKEN"/>
		<rdfs:label>version</rdfs:label>
	<rdfs:comment>Supplies a version number for an application, independent of its identifier or display name.</rdfs:comment>
	</owl:DatatypeProperty>
	<owl:DatatypeProperty rdf:ID="initial__mei_data.BOOLEAN">
		<rdfs:range rdf:resource="&datatypes;data.BOOLEAN"/>
		<rdfs:label>initial</rdfs:label>
	<rdfs:comment>Marks this hand as the first one of the document.</rdfs:comment>
	</owl:DatatypeProperty>
	<owl:DatatypeProperty rdf:ID="isodur__xs_duration">
		<rdfs:range rdf:resource="&xs;duration"/>
		<rdfs:label>isodur</rdfs:label>
	<rdfs:comment>Holds a W3C duration value, e.g., &quot;PT2H34M45.67S&quot;.</rdfs:comment>
	</owl:DatatypeProperty>
	<owl:DatatypeProperty rdf:ID="count__xs_positiveInteger">
		<rdfs:range rdf:resource="&xs;positiveInteger"/>
		<rdfs:label>count</rdfs:label>
	<rdfs:comment>Indicates the number of performers.</rdfs:comment>
	</owl:DatatypeProperty>
	<owl:DatatypeProperty rdf:ID="solo__mei_data.BOOLEAN">
		<rdfs:range rdf:resource="&datatypes;data.BOOLEAN"/>
		<rdfs:label>solo</rdfs:label>
	<rdfs:comment>Marks this instrument or vocal part as a soloist. Do not use this attribute for a solo instrument which is not accompanied.</rdfs:comment>
	</owl:DatatypeProperty>
	<owl:DatatypeProperty rdf:ID="currency__xs_NMTOKEN">
		<rdfs:range rdf:resource="&xs;NMTOKEN"/>
		<rdfs:label>currency</rdfs:label>
	<rdfs:comment>Monetary unit.</rdfs:comment>
	</owl:DatatypeProperty>
	<owl:DatatypeProperty rdf:ID="num__xs_positiveInteger">
		<rdfs:range rdf:resource="&xs;positiveInteger"/>
		<rdfs:label>num</rdfs:label>
	<rdfs:comment>Records the channel configuration in numeric form.</rdfs:comment>
	</owl:DatatypeProperty>
	<owl:DatatypeProperty rdf:ID="num__mei_data.MIDICHANNEL">
		<rdfs:range rdf:resource="&datatypes;data.MIDICHANNEL"/>
		<rdfs:label>num</rdfs:label>
	<rdfs:comment>MIDI number in the range set by data.MIDICHANNEL.</rdfs:comment>
	</owl:DatatypeProperty>
	<owl:DatatypeProperty rdf:ID="expan__xs_string">
		<rdfs:range rdf:resource="&xs;string"/>
		<rdfs:label>expan</rdfs:label>
	<rdfs:comment>Records the expansion of a text abbreviation.</rdfs:comment>
	</owl:DatatypeProperty>
	<owl:DatatypeProperty rdf:ID="degree__xs_string">
		<rdfs:range rdf:resource="&xs;string"/>
		<rdfs:label>degree</rdfs:label>
	<rdfs:comment>Records the degree of damage.</rdfs:comment>
	</owl:DatatypeProperty>
	<owl:DatatypeProperty rdf:ID="abbr__xs_string">
		<rdfs:range rdf:resource="&xs;string"/>
		<rdfs:label>abbr</rdfs:label>
	<rdfs:comment>Captures the abbreviated form of the text.</rdfs:comment>
	</owl:DatatypeProperty>
	<owl:DatatypeProperty rdf:ID="new__mei_data.URI">
		<rdfs:range rdf:resource="&datatypes;data.URI"/>
		<rdfs:label>new</rdfs:label>
	<rdfs:comment>Identifies the new hand. The value must contain the ID of a hand element given elsewhere in the document.</rdfs:comment>
	</owl:DatatypeProperty>
	<owl:DatatypeProperty rdf:ID="old__mei_data.URI">
		<rdfs:range rdf:resource="&datatypes;data.URI"/>
		<rdfs:label>old</rdfs:label>
	<rdfs:comment>Identifies the old hand. The value must contain the ID of a hand element given elsewhere in the document.</rdfs:comment>
	</owl:DatatypeProperty>
	<owl:DatatypeProperty rdf:ID="desc__xs_string">
		<rdfs:range rdf:resource="&xs;string"/>
		<rdfs:label>desc</rdfs:label>
	<rdfs:comment>Provides a description of the means of restoration, 'stet' or 'strike-down', for example.</rdfs:comment>
	</owl:DatatypeProperty>
	<owl:DatatypeProperty rdf:ID="ulx__xs_nonNegativeInteger">
		<rdfs:range rdf:resource="&xs;nonNegativeInteger"/>
		<rdfs:label>ulx</rdfs:label>
	<rdfs:comment>Indicates the upper-left corner x coordinate.</rdfs:comment>
	</owl:DatatypeProperty>
	<owl:DatatypeProperty rdf:ID="uly__xs_nonNegativeInteger">
		<rdfs:range rdf:resource="&xs;nonNegativeInteger"/>
		<rdfs:label>uly</rdfs:label>
	<rdfs:comment>Indicates the upper-left corner y coordinate.</rdfs:comment>
	</owl:DatatypeProperty>
	<owl:DatatypeProperty rdf:ID="pos__xs_positiveInteger">
		<rdfs:range rdf:resource="&xs;positiveInteger"/>
		<rdfs:label>pos</rdfs:label>
	<rdfs:comment>Records the fret position at which the chord tablature is to be played.</rdfs:comment>
	</owl:DatatypeProperty>
	<owl:DatatypeProperty rdf:ID="fing__mei_data.FINGER.FRET">
		<rdfs:range rdf:resource="&datatypes;data.FINGER.FRET"/>
		<rdfs:label>fing</rdfs:label>
	<rdfs:comment>Indicates which finger, if any, should be used to play an individual string. The index, middle, ring, and little fingers are represented by the values 1-4, while 't' is for the thumb. The values 'x' and 'o' indicate muffled and open strings, respectively.</rdfs:comment>
	</owl:DatatypeProperty>
	<owl:DatatypeProperty rdf:ID="abstype__mei_data.BETYPE">
		<rdfs:range rdf:resource="&datatypes;data.BETYPE"/>
		<rdfs:label>abstype</rdfs:label>
	<rdfs:comment>Specifies the kind of values used in the absolute attribute.</rdfs:comment>
	</owl:DatatypeProperty>
	<owl:DatatypeProperty rdf:ID="inttype__mei_data.BETYPE">
		<rdfs:range rdf:resource="&datatypes;data.BETYPE"/>
		<rdfs:label>inttype</rdfs:label>
	<rdfs:comment>Specifies the kind of values used in the interval attribute.</rdfs:comment>
	</owl:DatatypeProperty>
	<owl:DatatypeProperty rdf:ID="since__mei_data.URI">
		<rdfs:range rdf:resource="&datatypes;data.URI"/>
		<rdfs:label>since</rdfs:label>
	<rdfs:comment>Identifies the reference point for determining the time of the current when element, which is obtained by adding the interval to the time of the reference point. The value should be the ID of another when element within the same parent element. If the since attribute is omitted and the absolute attribute is not specified, then the reference point is understood to be the immediately preceding when element.</rdfs:comment>
	</owl:DatatypeProperty>
	<owl:Class rdf:ID="macro.metaLike.page">
		<rdfs:subClassOf>
			<owl:Class>
				<owl:intersectionOf rdf:parseType="Collection">
				<owl:Restriction>
				<owl:onProperty rdf:resource="&mei;pgHead"/>
				<owl:maxCardinality rdf:datatype="&xsd;nonNegativeInteger">1</owl:maxCardinality>
			</owl:Restriction>
		<owl:Restriction>
				<owl:onProperty rdf:resource="&mei;pgFoot"/>
				<owl:maxCardinality rdf:datatype="&xsd;nonNegativeInteger">1</owl:maxCardinality>
			</owl:Restriction>
		<owl:Restriction>
				<owl:onProperty rdf:resource="&mei;pgDesc"/>
				<owl:maxCardinality rdf:datatype="&xsd;nonNegativeInteger">1</owl:maxCardinality>
			</owl:Restriction>
		</owl:intersectionOf>
	</owl:Class>
	</rdfs:subClassOf>
		<rdfs:label>macro.metaLike.page</rdfs:label>
	</owl:Class>
	<owl:DatatypeProperty rdf:about="#&mei;pgHead">
		<rdfs:domain rdf:resource="#macro.metaLike.page"/>
		 </owl:DatatypeProperty>
	<owl:DatatypeProperty rdf:about="#&mei;pgFoot">
		<rdfs:domain rdf:resource="#macro.metaLike.page"/>
		 </owl:DatatypeProperty>
	<owl:DatatypeProperty rdf:about="#&mei;pgDesc">
		<rdfs:domain rdf:resource="#macro.metaLike.page"/>
		 </owl:DatatypeProperty>
	<owl:Class rdf:ID="macro.availabilityPart">
		<rdfs:label>macro.availabilityPart</rdfs:label>
	</owl:Class>
	<owl:DatatypeProperty rdf:about="#&mei;accessRestrict">
		<rdfs:domain rdf:resource="#macro.availabilityPart"/>
		 </owl:DatatypeProperty>
	<owl:DatatypeProperty rdf:about="#&mei;distributor">
		<rdfs:domain rdf:resource="#macro.availabilityPart"/>
		 </owl:DatatypeProperty>
	<owl:DatatypeProperty rdf:about="#&mei;price">
		<rdfs:domain rdf:resource="#macro.availabilityPart"/>
		 </owl:DatatypeProperty>
	<owl:DatatypeProperty rdf:about="#&mei;sysReq">
		<rdfs:domain rdf:resource="#macro.availabilityPart"/>
		 </owl:DatatypeProperty>
	<owl:DatatypeProperty rdf:about="#&mei;useRestrict">
		<rdfs:domain rdf:resource="#macro.availabilityPart"/>
		 </owl:DatatypeProperty>
	<owl:DatatypeProperty rdf:ID="accid__NS_accid_UNType">
		<rdfs:label>accid</rdfs:label>
	<rdfs:comment>(accidental) – Records a temporary alteration to the pitch of a note.</rdfs:comment>
	</owl:DatatypeProperty>
	<owl:DatatypeProperty rdf:ID="actor__NS_actor_UNType">
		<rdfs:label>actor</rdfs:label>
	<rdfs:comment>Name of an actor appearing within a cast list.</rdfs:comment>
	</owl:DatatypeProperty>
	<owl:DatatypeProperty rdf:ID="address__NS_address_UNType">
		<rdfs:label>address</rdfs:label>
	<rdfs:comment>Contains a postal address, for example of a publisher, an organization, or an individual.</rdfs:comment>
	</owl:DatatypeProperty>
	<owl:DatatypeProperty rdf:ID="addrLine__NS_addrLine_UNType">
		<rdfs:label>addrLine</rdfs:label>
	<rdfs:comment>(address line) – Single line of a postal address.</rdfs:comment>
	</owl:DatatypeProperty>
	<owl:DatatypeProperty rdf:ID="annot__NS_annot_UNType">
		<rdfs:label>annot</rdfs:label>
	<rdfs:comment>(annotation) – Provides a short statement explaining the text or indicating the basis for an assertion.</rdfs:comment>
	</owl:DatatypeProperty>
	<owl:DatatypeProperty rdf:ID="arranger__NS_arranger_UNType">
		<rdfs:label>arranger</rdfs:label>
	<rdfs:comment>A person or organization who transcribes a musical composition, usually for a different medium from that of the original; in an arrangement the musical substance remains essentially unchanged.</rdfs:comment>
	</owl:DatatypeProperty>
	<owl:DatatypeProperty rdf:ID="artic__NS_artic_UNType">
		<rdfs:label>artic</rdfs:label>
	<rdfs:comment>(articulation) – An indication of how to play a note or chord.</rdfs:comment>
	</owl:DatatypeProperty>
	<owl:DatatypeProperty rdf:ID="author__NS_author_UNType">
		<rdfs:label>author</rdfs:label>
	<rdfs:comment>The name of the creator of the intellectual content of a non-musical, literary work.</rdfs:comment>
	</owl:DatatypeProperty>
	<owl:DatatypeProperty rdf:ID="barLine__NS_barLine_UNType">
		<rdfs:label>barLine</rdfs:label>
	<rdfs:comment>Vertical line drawn through one or more staves that divides musical notation into metrical units.</rdfs:comment>
	</owl:DatatypeProperty>
	<owl:DatatypeProperty rdf:ID="bibl__NS_bibl_UNType">
		<rdfs:label>bibl</rdfs:label>
	<rdfs:comment>(bibliographic reference) – Provides a loosely-structured bibliographic citation in which the sub-components may or may not be explicitly marked.</rdfs:comment>
	</owl:DatatypeProperty>
	<owl:DatatypeProperty rdf:ID="biblList__NS_biblList_UNType">
		<rdfs:label>biblList</rdfs:label>
	<rdfs:comment>List of bibliographic references.</rdfs:comment>
	</owl:DatatypeProperty>
	<owl:DatatypeProperty rdf:ID="biblScope__NS_biblScope_UNType">
		<rdfs:label>biblScope</rdfs:label>
	<rdfs:comment>(scope of citation) – Defines the scope of a bibliographic reference, for example as a list of page numbers, or a named subdivision of a larger work.</rdfs:comment>
	</owl:DatatypeProperty>
	<owl:DatatypeProperty rdf:ID="body__NS_body_UNType">
		<rdfs:label>body</rdfs:label>
	<rdfs:comment>Contains the whole of a single musical text, excluding any front or back matter.</rdfs:comment>
	</owl:DatatypeProperty>
	<owl:DatatypeProperty rdf:ID="caption__NS_caption_UNType">
		<rdfs:label>caption</rdfs:label>
	<rdfs:comment>A label which accompanies an illustration or a table.</rdfs:comment>
	</owl:DatatypeProperty>
	<owl:DatatypeProperty rdf:ID="castGrp__NS_castGrp_UNType">
		<rdfs:label>castGrp</rdfs:label>
	<rdfs:comment>(cast group) – Groups one or more individual castItem elements within a cast list.</rdfs:comment>
	</owl:DatatypeProperty>
	<owl:DatatypeProperty rdf:ID="castItem__NS_castItem_UNType">
		<rdfs:label>castItem</rdfs:label>
	<rdfs:comment>Contains a single entry within a cast list, describing either a single role or a list of non-speaking roles.</rdfs:comment>
	</owl:DatatypeProperty>
	<owl:DatatypeProperty rdf:ID="castList__NS_castList_UNType">
		<rdfs:label>castList</rdfs:label>
	<rdfs:comment>Contains a single cast list or dramatis personae.</rdfs:comment>
	</owl:DatatypeProperty>
	<owl:DatatypeProperty rdf:ID="chord__NS_chord_UNType">
		<rdfs:label>chord</rdfs:label>
	<rdfs:comment>A simultaneous sounding of two or more notes in the same layer *with the same duration*.</rdfs:comment>
	</owl:DatatypeProperty>
	<owl:DatatypeProperty rdf:ID="clef__NS_clef_UNType">
		<rdfs:label>clef</rdfs:label>
	<rdfs:comment>Indication of the exact location of a particular note on the staff and, therefore, the other notes as well.</rdfs:comment>
	</owl:DatatypeProperty>
	<owl:DatatypeProperty rdf:ID="clefGrp__NS_clefGrp_UNType">
		<rdfs:label>clefGrp</rdfs:label>
	<rdfs:comment>(clef group) – A set of simultaneously-occurring clefs.</rdfs:comment>
	</owl:DatatypeProperty>
	<owl:DatatypeProperty rdf:ID="composer__NS_composer_UNType">
		<rdfs:label>composer</rdfs:label>
	<rdfs:comment>The name of the creator of the intellectual content of a musical work.</rdfs:comment>
	</owl:DatatypeProperty>
	<owl:DatatypeProperty rdf:ID="creation__NS_creation_UNType">
		<rdfs:label>creation</rdfs:label>
	<rdfs:comment>Non-bibliographic details of the creation of an intellectual entity, in narrative form, such as the date, place, and circumstances of its composition. More detailed information may be captured within the history element.</rdfs:comment>
	</owl:DatatypeProperty>
	<owl:DatatypeProperty rdf:ID="custos__NS_custos_UNType">
		<rdfs:label>custos</rdfs:label>
	<rdfs:comment>Symbol placed at the end of a line of music to indicate the first note of the next line. Sometimes called a &quot;direct&quot;.</rdfs:comment>
	</owl:DatatypeProperty>
	<owl:DatatypeProperty rdf:ID="date__NS_date_UNType">
		<rdfs:label>date</rdfs:label>
	<rdfs:comment>A string identifying a point in time or the time period between two such points.</rdfs:comment>
	</owl:DatatypeProperty>
	<owl:DatatypeProperty rdf:ID="depth__NS_depth_UNType">
		<rdfs:label>depth</rdfs:label>
	<rdfs:comment>Description of a measurement taken through a three-dimensional object.</rdfs:comment>
	</owl:DatatypeProperty>
	<owl:DatatypeProperty rdf:ID="desc__NS_desc_UNType">
		<rdfs:label>desc</rdfs:label>
	<rdfs:comment>(description) – Container for text that briefly describes the feature to which it is attached, including its intended usage, purpose, or application as appropriate.</rdfs:comment>
	</owl:DatatypeProperty>
	<owl:DatatypeProperty rdf:ID="dir__NS_dir_UNType">
		<rdfs:label>dir</rdfs:label>
	<rdfs:comment>(directive) – An instruction expressed as a combination of text and symbols — such as segno and coda symbols, fermatas over a bar line, etc., typically above, below, or between staves, but not on the staff — that is not encoded elsewhere in more specific elements, like &lt;tempo&gt; or &lt;dynam&gt;.</rdfs:comment>
	</owl:DatatypeProperty>
	<owl:DatatypeProperty rdf:ID="distributor__NS_distributor_UNType">
		<rdfs:label>distributor</rdfs:label>
	<rdfs:comment>Person or agency, other than a publisher, from which access (including electronic access) to a bibliographic entity may be obtained.</rdfs:comment>
	</owl:DatatypeProperty>
	<owl:DatatypeProperty rdf:ID="div__NS_div_UNType">
		<rdfs:label>div</rdfs:label>
	<rdfs:comment>(division) – Major structural division of text, such as a preface, chapter or section.</rdfs:comment>
	</owl:DatatypeProperty>
	<owl:DatatypeProperty rdf:ID="dot__NS_dot_UNType">
		<rdfs:label>dot</rdfs:label>
	<rdfs:comment>Dot of augmentation or division.</rdfs:comment>
	</owl:DatatypeProperty>
	<owl:DatatypeProperty rdf:ID="dynam__NS_dynam_UNType">
		<rdfs:label>dynam</rdfs:label>
	<rdfs:comment>(dynamic) – Indication of the volume of a note, phrase, or section of music.</rdfs:comment>
	</owl:DatatypeProperty>
	<owl:DatatypeProperty rdf:ID="edition__NS_edition_UNType">
		<rdfs:label>edition</rdfs:label>
	<rdfs:comment>(edition designation) – A word or text phrase that indicates a difference in either content or form between the item being described and a related item previously issued by the same publisher/distributor (e.g. 2nd edition, version 2.0, etc.), or simultaneously issued by either the same publisher/distributor or another publisher/distributor (e.g. large print edition, British edition, etc.).</rdfs:comment>
	</owl:DatatypeProperty>
	<owl:DatatypeProperty rdf:ID="editor__NS_editor_UNType">
		<rdfs:label>editor</rdfs:label>
	<rdfs:comment>The name of the individual(s), institution(s) or organization(s) acting in an editorial capacity.</rdfs:comment>
	</owl:DatatypeProperty>
	<owl:DatatypeProperty rdf:ID="ending__NS_ending_UNType">
		<rdfs:label>ending</rdfs:label>
	<rdfs:comment>Alternative ending for a repeated passage of music; i.e., prima volta, seconda volta, etc.</rdfs:comment>
	</owl:DatatypeProperty>
	<owl:DatatypeProperty rdf:ID="event__NS_event_UNType">
		<rdfs:label>event</rdfs:label>
	<rdfs:comment>Contains a free-text event description.</rdfs:comment>
	</owl:DatatypeProperty>
	<owl:DatatypeProperty rdf:ID="eventList__NS_eventList_UNType">
		<rdfs:label>eventList</rdfs:label>
	<rdfs:comment>Contains historical information given as a sequence of significant past events.</rdfs:comment>
	</owl:DatatypeProperty>
	<owl:DatatypeProperty rdf:ID="expansion__NS_expansion_UNType">
		<rdfs:label>expansion</rdfs:label>
	<rdfs:comment>Indicates how a section may be programmatically expanded into its 'through-composed' form.</rdfs:comment>
	</owl:DatatypeProperty>
	<owl:DatatypeProperty rdf:ID="extent__NS_extent_UNType">
		<rdfs:label>extent</rdfs:label>
	<rdfs:comment>Used to express size in terms other than physical dimensions, such as number of pages, number of records in file, number of bytes, performance duration for music, audio recordings and visual projections, etc.</rdfs:comment>
	</owl:DatatypeProperty>
	<owl:DatatypeProperty rdf:ID="funder__NS_funder_UNType">
		<rdfs:label>funder</rdfs:label>
	<rdfs:comment>Names of individuals, institutions, or organizations responsible for funding. Funders provide financial support for a project; they are distinct from sponsors, who provide intellectual support and authority.</rdfs:comment>
	</owl:DatatypeProperty>
	<owl:DatatypeProperty rdf:ID="genre__NS_genre_UNType">
		<rdfs:label>genre</rdfs:label>
	<rdfs:comment>Term or terms that designate a category characterizing a particular style, form, or content.</rdfs:comment>
	</owl:DatatypeProperty>
	<owl:DatatypeProperty rdf:ID="group__NS_group_UNType">
		<rdfs:label>group</rdfs:label>
	<rdfs:comment>Contains a composite musical text, grouping together a sequence of distinct musical texts (or groups of such musical texts) which are regarded as a unit for some purpose, for example, the collected works of a composer.</rdfs:comment>
	</owl:DatatypeProperty>
	<owl:DatatypeProperty rdf:ID="grpSym__NS_grpSym_UNType">
		<rdfs:label>grpSym</rdfs:label>
	<rdfs:comment>(group symbol) – A brace or bracket used to group two or more staves of a score or part.</rdfs:comment>
	</owl:DatatypeProperty>
	<owl:DatatypeProperty rdf:ID="head__NS_head_UNType">
		<rdfs:label>head</rdfs:label>
	<rdfs:comment>(heading) – Contains any heading, for example, the title of a section of text, or the heading of a list.</rdfs:comment>
	</owl:DatatypeProperty>
	<owl:DatatypeProperty rdf:ID="height__NS_height_UNType">
		<rdfs:label>height</rdfs:label>
	<rdfs:comment>Description of the vertical size of an object.</rdfs:comment>
	</owl:DatatypeProperty>
	<owl:DatatypeProperty rdf:ID="identifier__NS_identifier_UNType">
		<rdfs:label>identifier</rdfs:label>
	<rdfs:comment>An alpha-numeric string that establishes the identity of the described material.</rdfs:comment>
	</owl:DatatypeProperty>
	<owl:DatatypeProperty rdf:ID="imprint__NS_imprint_UNType">
		<rdfs:label>imprint</rdfs:label>
	<rdfs:comment>Information relating to the publication or distribution of a bibliographic item.</rdfs:comment>
	</owl:DatatypeProperty>
	<owl:DatatypeProperty rdf:ID="incip__NS_incip_UNType">
		<rdfs:label>incip</rdfs:label>
	<rdfs:comment>(incipit) – The opening music and/or words of a composition.</rdfs:comment>
	</owl:DatatypeProperty>
	<owl:DatatypeProperty rdf:ID="keyAccid__NS_keyAccid_UNType">
		<rdfs:label>keyAccid</rdfs:label>
	<rdfs:comment>(key accidental) – Accidental in a key signature.</rdfs:comment>
	</owl:DatatypeProperty>
	<owl:DatatypeProperty rdf:ID="keySig__NS_keySig_UNType">
		<rdfs:label>keySig</rdfs:label>
	<rdfs:comment>(key signature) – Written key signature.</rdfs:comment>
	</owl:DatatypeProperty>
	<owl:DatatypeProperty rdf:ID="label__NS_label_UNType">
		<rdfs:label>label</rdfs:label>
	<rdfs:comment>A container for text that identifies the feature to which it is attached.</rdfs:comment>
	</owl:DatatypeProperty>
	<owl:DatatypeProperty rdf:ID="layer__NS_layer_UNType">
		<rdfs:label>layer</rdfs:label>
	<rdfs:comment>An independent stream of events on a staff.</rdfs:comment>
	</owl:DatatypeProperty>
	<owl:DatatypeProperty rdf:ID="layerDef__NS_layerDef_UNType">
		<rdfs:label>layerDef</rdfs:label>
	<rdfs:comment>(layer definition) – Container for layer meta-information.</rdfs:comment>
	</owl:DatatypeProperty>
	<owl:DatatypeProperty rdf:ID="lb__NS_lb_UNType">
		<rdfs:label>lb</rdfs:label>
	<rdfs:comment>(line break) – An empty formatting element that forces text to begin on a new line.</rdfs:comment>
	</owl:DatatypeProperty>
	<owl:DatatypeProperty rdf:ID="librettist__NS_librettist_UNType">
		<rdfs:label>librettist</rdfs:label>
	<rdfs:comment>Person or organization who is a writer of the text of an opera, oratorio, etc.</rdfs:comment>
	</owl:DatatypeProperty>
	<owl:DatatypeProperty rdf:ID="lyricist__NS_lyricist_UNType">
		<rdfs:label>lyricist</rdfs:label>
	<rdfs:comment>Person or organization who is a writer of the text of a song.</rdfs:comment>
	</owl:DatatypeProperty>
	<owl:DatatypeProperty rdf:ID="mdiv__NS_mdiv_UNType">
		<rdfs:label>mdiv</rdfs:label>
	<rdfs:comment>(musical division) – Contains a subdivision of the body of a musical text.</rdfs:comment>
	</owl:DatatypeProperty>
	<owl:DatatypeProperty rdf:ID="mei__NS_mei_UNType">
		<rdfs:label>mei</rdfs:label>
	<rdfs:comment>Contains a single MEI-conformant document, consisting of an MEI header and a musical text, either in isolation or as part of an meiCorpus element.</rdfs:comment>
	</owl:DatatypeProperty>
	<owl:DatatypeProperty rdf:ID="music__NS_music_UNType">
		<rdfs:label>music</rdfs:label>
	<rdfs:comment>Contains a single musical text of any kind, whether unitary or composite, for example, an etude, opera, song cycle, symphony, or anthology of piano solos.</rdfs:comment>
	</owl:DatatypeProperty>
	<owl:DatatypeProperty rdf:ID="name__NS_name_UNType">
		<rdfs:label>name</rdfs:label>
	<rdfs:comment>Proper noun or noun phrase.</rdfs:comment>
	</owl:DatatypeProperty>
	<owl:DatatypeProperty rdf:ID="note__NS_note_UNType">
		<rdfs:label>note</rdfs:label>
	<rdfs:comment>A single pitched event. </rdfs:comment>
	</owl:DatatypeProperty>
	<owl:DatatypeProperty rdf:ID="num__NS_num_UNType">
		<rdfs:label>num</rdfs:label>
	<rdfs:comment>(number) – Numeric information in any form.</rdfs:comment>
	</owl:DatatypeProperty>
	<owl:DatatypeProperty rdf:ID="ornam__NS_ornam_UNType">
		<rdfs:label>ornam</rdfs:label>
	<rdfs:comment>An element indicating an ornament that is not a mordent, turn, or trill. </rdfs:comment>
	</owl:DatatypeProperty>
	<owl:DatatypeProperty rdf:ID="p__NS_p_UNType">
		<rdfs:label>p</rdfs:label>
	<rdfs:comment>(paragraph) – One or more text phrases that form a logical prose passage.</rdfs:comment>
	</owl:DatatypeProperty>
	<owl:DatatypeProperty rdf:ID="pad__NS_pad_UNType">
		<rdfs:label>pad</rdfs:label>
	<rdfs:comment>(padding) – An indication of extra visual space between notational elements.</rdfs:comment>
	</owl:DatatypeProperty>
	<owl:DatatypeProperty rdf:ID="part__NS_part_UNType">
		<rdfs:label>part</rdfs:label>
	<rdfs:comment>An alternative visual rendition of the score from the point of view of a particular performer (or group of performers).</rdfs:comment>
	</owl:DatatypeProperty>
	<owl:DatatypeProperty rdf:ID="parts__NS_parts_UNType">
		<rdfs:label>parts</rdfs:label>
	<rdfs:comment>Provides a container for performers' parts.</rdfs:comment>
	</owl:DatatypeProperty>
	<owl:DatatypeProperty rdf:ID="pb__NS_pb_UNType">
		<rdfs:label>pb</rdfs:label>
	<rdfs:comment>(page break) – An empty formatting element that forces text to begin on a new page.</rdfs:comment>
	</owl:DatatypeProperty>
	<owl:DatatypeProperty rdf:ID="pgDesc__NS_pgDesc_UNType">
		<rdfs:label>pgDesc</rdfs:label>
	<rdfs:comment>(page description) – Contains a brief prose description of the appearance or description of the content of a physical page.</rdfs:comment>
	</owl:DatatypeProperty>
	<owl:DatatypeProperty rdf:ID="pgFoot__NS_pgFoot_UNType">
		<rdfs:label>pgFoot</rdfs:label>
	<rdfs:comment>(page footer) – A running footer on the first page. Also, used to temporarily override a running footer on individual pages.</rdfs:comment>
	</owl:DatatypeProperty>
	<owl:DatatypeProperty rdf:ID="pgFoot2__NS_pgFoot2_UNType">
		<rdfs:label>pgFoot2</rdfs:label>
	<rdfs:comment>(page footer 2) – A running footer on the pages following the first.</rdfs:comment>
	</owl:DatatypeProperty>
	<owl:DatatypeProperty rdf:ID="pgHead__NS_pgHead_UNType">
		<rdfs:label>pgHead</rdfs:label>
	<rdfs:comment>(page header) – A running header on the first page. Also, used to temporarily override a running header on individual pages.</rdfs:comment>
	</owl:DatatypeProperty>
	<owl:DatatypeProperty rdf:ID="pgHead2__NS_pgHead2_UNType">
		<rdfs:label>pgHead2</rdfs:label>
	<rdfs:comment>(page header 2) – A running header on the pages following the first.</rdfs:comment>
	</owl:DatatypeProperty>
	<owl:DatatypeProperty rdf:ID="phrase__NS_phrase_UNType">
		<rdfs:label>phrase</rdfs:label>
	<rdfs:comment>Indication of 1) a &quot;unified melodic idea&quot; or 2) performance technique.</rdfs:comment>
	</owl:DatatypeProperty>
	<owl:DatatypeProperty rdf:ID="physLoc__NS_physLoc_UNType">
		<rdfs:label>physLoc</rdfs:label>
	<rdfs:comment>(physical location) – Groups information about the current physical location of a bibliographic item, such as the repository in which it is located and its shelf mark(s), and its previous locations.</rdfs:comment>
	</owl:DatatypeProperty>
	<owl:DatatypeProperty rdf:ID="publisher__NS_publisher_UNType">
		<rdfs:label>publisher</rdfs:label>
	<rdfs:comment>Name of the organization responsible for the publication of a bibliographic item.</rdfs:comment>
	</owl:DatatypeProperty>
	<owl:DatatypeProperty rdf:ID="pubPlace__NS_pubPlace_UNType">
		<rdfs:label>pubPlace</rdfs:label>
	<rdfs:comment>(publication place) – Name of the place where a bibliographic item was published.</rdfs:comment>
	</owl:DatatypeProperty>
	<owl:DatatypeProperty rdf:ID="recipient__NS_recipient_UNType">
		<rdfs:label>recipient</rdfs:label>
	<rdfs:comment>The name of the individual(s), institution(s) or organization(s) receiving correspondence.</rdfs:comment>
	</owl:DatatypeProperty>
	<owl:DatatypeProperty rdf:ID="relatedItem__NS_relatedItem_UNType">
		<rdfs:label>relatedItem</rdfs:label>
	<rdfs:comment>(related item) – Contains or references another bibliographic item which is related to the present one.</rdfs:comment>
	</owl:DatatypeProperty>
	<owl:DatatypeProperty rdf:ID="rend__NS_rend_UNType">
		<rdfs:label>rend</rdfs:label>
	<rdfs:comment>(render) – A formatting element indicating special visual rendering, e.g., bold or italicized, of a text word or phrase.</rdfs:comment>
	</owl:DatatypeProperty>
	<owl:DatatypeProperty rdf:ID="repository__NS_repository_UNType">
		<rdfs:label>repository</rdfs:label>
	<rdfs:comment>Institution, agency, or individual which holds a bibliographic item.</rdfs:comment>
	</owl:DatatypeProperty>
	<owl:DatatypeProperty rdf:ID="resp__NS_resp_UNType">
		<rdfs:label>resp</rdfs:label>
	<rdfs:comment>(responsibility) – A phrase describing the nature of intellectual responsibility.</rdfs:comment>
	</owl:DatatypeProperty>
	<owl:DatatypeProperty rdf:ID="respStmt__NS_respStmt_UNType">
		<rdfs:label>respStmt</rdfs:label>
	<rdfs:comment>(responsibility statement) – Names one or more individuals, groups, or in rare cases, mechanical processes, responsible for creation or realization of the intellectual or artistic content.</rdfs:comment>
	</owl:DatatypeProperty>
	<owl:DatatypeProperty rdf:ID="rest__NS_rest_UNType">
		<rdfs:label>rest</rdfs:label>
	<rdfs:comment>A non-sounding event found in the source being transcribed.</rdfs:comment>
	</owl:DatatypeProperty>
	<owl:DatatypeProperty rdf:ID="role__NS_role_UNType">
		<rdfs:label>role</rdfs:label>
	<rdfs:comment>Name of a dramatic role, as given in a cast list.</rdfs:comment>
	</owl:DatatypeProperty>
	<owl:DatatypeProperty rdf:ID="roleDesc__NS_roleDesc_UNType">
		<rdfs:label>roleDesc</rdfs:label>
	<rdfs:comment>(role description) – Describes a character's role in a drama.</rdfs:comment>
	</owl:DatatypeProperty>
	<owl:DatatypeProperty rdf:ID="sb__NS_sb_UNType">
		<rdfs:label>sb</rdfs:label>
	<rdfs:comment>(system break) – An empty formatting element that forces musical notation to begin on a new line.</rdfs:comment>
	</owl:DatatypeProperty>
	<owl:DatatypeProperty rdf:ID="score__NS_score_UNType">
		<rdfs:label>score</rdfs:label>
	<rdfs:comment>Full score view of the musical content.</rdfs:comment>
	</owl:DatatypeProperty>
	<owl:DatatypeProperty rdf:ID="scoreDef__NS_scoreDef_UNType">
		<rdfs:label>scoreDef</rdfs:label>
	<rdfs:comment>(score definition) – Container for score meta-information.</rdfs:comment>
	</owl:DatatypeProperty>
	<owl:DatatypeProperty rdf:ID="section__NS_section_UNType">
		<rdfs:label>section</rdfs:label>
	<rdfs:comment>Segment of music data.</rdfs:comment>
	</owl:DatatypeProperty>
	<owl:DatatypeProperty rdf:ID="series__NS_series_UNType">
		<rdfs:label>series</rdfs:label>
	<rdfs:comment>Contains information about the serial publication in which a bibliographic item has appeared.</rdfs:comment>
	</owl:DatatypeProperty>
	<owl:DatatypeProperty rdf:ID="space__NS_space_UNType">
		<rdfs:label>space</rdfs:label>
	<rdfs:comment>A placeholder used to fill an incomplete measure, layer, etc. most often so that the combined duration of the events equals the number of beats in the measure.</rdfs:comment>
	</owl:DatatypeProperty>
	<owl:DatatypeProperty rdf:ID="sponsor__NS_sponsor_UNType">
		<rdfs:label>sponsor</rdfs:label>
	<rdfs:comment>Names of sponsoring individuals, organizations or institutions. Sponsors give their intellectual authority to a project; they are to be distinguished from funders, who provide the funding but do not necessarily take intellectual responsibility.</rdfs:comment>
	</owl:DatatypeProperty>
	<owl:DatatypeProperty rdf:ID="stack__NS_stack_UNType">
		<rdfs:label>stack</rdfs:label>
	<rdfs:comment>(stacked text) – An inline table with a single column.</rdfs:comment>
	</owl:DatatypeProperty>
	<owl:DatatypeProperty rdf:ID="staff__NS_staff_UNType">
		<rdfs:label>staff</rdfs:label>
	<rdfs:comment>A group of equidistant horizontal lines on which notes are placed in order to represent pitch or a grouping element for individual 'strands' of notes, rests, etc. that may or may not actually be rendered on staff lines; that is, both diastematic and non-diastematic signs.</rdfs:comment>
	</owl:DatatypeProperty>
	<owl:DatatypeProperty rdf:ID="staffDef__NS_staffDef_UNType">
		<rdfs:label>staffDef</rdfs:label>
	<rdfs:comment>(staff definition) – Container for staff meta-information.</rdfs:comment>
	</owl:DatatypeProperty>
	<owl:DatatypeProperty rdf:ID="staffGrp__NS_staffGrp_UNType">
		<rdfs:label>staffGrp</rdfs:label>
	<rdfs:comment>(staff group) – A group of bracketed or braced staves.</rdfs:comment>
	</owl:DatatypeProperty>
	<owl:DatatypeProperty rdf:ID="syl__NS_syl_UNType">
		<rdfs:label>syl</rdfs:label>
	<rdfs:comment>(syllable) – Individual lyric syllable.</rdfs:comment>
	</owl:DatatypeProperty>
	<owl:DatatypeProperty rdf:ID="tempo__NS_tempo_UNType">
		<rdfs:label>tempo</rdfs:label>
	<rdfs:comment>Text and symbols descriptive of tempo, mood, or style, e.g., &quot;allarg.&quot;, &quot;a tempo&quot;, &quot;cantabile&quot;, &quot;Moderato&quot;, &quot;♩=60&quot;, &quot;Moderato ♩ =60&quot;).</rdfs:comment>
	</owl:DatatypeProperty>
	<owl:DatatypeProperty rdf:ID="textLang__NS_textLang_UNType">
		<rdfs:label>textLang</rdfs:label>
	<rdfs:comment>(text language) – Identifies the languages and writing systems within the work described by a bibliographic description, not the language of the description.</rdfs:comment>
	</owl:DatatypeProperty>
	<owl:DatatypeProperty rdf:ID="title__NS_title_UNType">
		<rdfs:label>title</rdfs:label>
	<rdfs:comment>Title of a bibliographic entity.</rdfs:comment>
	</owl:DatatypeProperty>
	<owl:DatatypeProperty rdf:ID="titlePage__NS_titlePage_UNType">
		<rdfs:label>titlePage</rdfs:label>
	<rdfs:comment>Contains a transcription of the title page of a text.</rdfs:comment>
	</owl:DatatypeProperty>
	<owl:DatatypeProperty rdf:ID="width__NS_width_UNType">
		<rdfs:label>width</rdfs:label>
	<rdfs:comment>Description of the horizontal size of an object.</rdfs:comment>
	</owl:DatatypeProperty>
	<owl:DatatypeProperty rdf:ID="accessRestrict__NS_accessRestrict_UNType">
		<rdfs:label>accessRestrict</rdfs:label>
	<rdfs:comment>(access restriction) – Describes the conditions that affect the accessibility of material.</rdfs:comment>
	</owl:DatatypeProperty>
	<owl:DatatypeProperty rdf:ID="altId__NS_altId_UNType">
		<rdfs:label>altId</rdfs:label>
	<rdfs:comment>(alternative identifier) – May contain a bibliographic identifier that does not fit within the meiHead element's id attribute, for example because the identifier does not fit the definition of an XML id or because multiple identifiers are needed.</rdfs:comment>
	</owl:DatatypeProperty>
	<owl:DatatypeProperty rdf:ID="appInfo__NS_appInfo_UNType">
		<rdfs:label>appInfo</rdfs:label>
	<rdfs:comment>(application information) – Groups information about applications which have acted upon the MEI file.</rdfs:comment>
	</owl:DatatypeProperty>
	<owl:DatatypeProperty rdf:ID="application__NS_application_UNType">
		<rdfs:label>application</rdfs:label>
	<rdfs:comment>Provides information about an application which has acted upon the current document.</rdfs:comment>
	</owl:DatatypeProperty>
	<owl:DatatypeProperty rdf:ID="audience__NS_audience_UNType">
		<rdfs:label>audience</rdfs:label>
	<rdfs:comment>Defines the class of user for which the work is intended, as defined by age group (e.g., children, young adults, adults, etc.), educational level (e.g., primary, secondary, etc.), or other categorization.</rdfs:comment>
	</owl:DatatypeProperty>
	<owl:DatatypeProperty rdf:ID="availability__NS_availability_UNType">
		<rdfs:label>availability</rdfs:label>
	<rdfs:comment>Groups elements that describe the availability of and access to a bibliographic item, including an MEI-encoded document.</rdfs:comment>
	</owl:DatatypeProperty>
	<owl:DatatypeProperty rdf:ID="byline__NS_byline_UNType">
		<rdfs:label>byline</rdfs:label>
	<rdfs:comment>Contains the primary statement of responsibility given for a work on its title page.</rdfs:comment>
	</owl:DatatypeProperty>
	<owl:DatatypeProperty rdf:ID="captureMode__NS_captureMode_UNType">
		<rdfs:label>captureMode</rdfs:label>
	<rdfs:comment>(capture mode) – The means used to record notation, sound, or images in the production of a source/manifestation (e.g., analogue, acoustic, electric, digital, optical etc.).</rdfs:comment>
	</owl:DatatypeProperty>
	<owl:DatatypeProperty rdf:ID="carrierForm__NS_carrierForm_UNType">
		<rdfs:label>carrierForm</rdfs:label>
	<rdfs:comment>(carrier form) – The specific class of material to which the physical carrier of the source/manifestation belongs (e.g., sound cassette, videodisc, microfilm cartridge, transparency, etc.). The carrier for a manifestation comprising multiple physical components may include more than one form (e.g., a filmstrip with an accompanying booklet, a separate sound disc carrying the sound track for a film, etc.).</rdfs:comment>
	</owl:DatatypeProperty>
	<owl:DatatypeProperty rdf:ID="change__NS_change_UNType">
		<rdfs:label>change</rdfs:label>
	<rdfs:comment>Individual change within the revision description.</rdfs:comment>
	</owl:DatatypeProperty>
	<owl:DatatypeProperty rdf:ID="changeDesc__NS_changeDesc_UNType">
		<rdfs:label>changeDesc</rdfs:label>
	<rdfs:comment>(change description) – Description of a revision of the MEI file.</rdfs:comment>
	</owl:DatatypeProperty>
	<owl:DatatypeProperty rdf:ID="classCode__NS_classCode_UNType">
		<rdfs:label>classCode</rdfs:label>
	<rdfs:comment>(classification code) – Holds a citation to the source of controlled-vocabulary terms used in the &lt;termList&gt; element; for example, Library of Congress Subject Headings (LCSH), Library of Congress Classification (LCC), Library of Congress Name Authority File (LCNAF), or other thesaurus or ontology.</rdfs:comment>
	</owl:DatatypeProperty>
	<owl:DatatypeProperty rdf:ID="classification__NS_classification_UNType">
		<rdfs:label>classification</rdfs:label>
	<rdfs:comment>Groups information which describes the nature or topic of an entity.</rdfs:comment>
	</owl:DatatypeProperty>
	<owl:DatatypeProperty rdf:ID="condition__NS_condition_UNType">
		<rdfs:label>condition</rdfs:label>
	<rdfs:comment>The physical condition of an item, particularly any variances between the physical make-up of the item and that of other copies of the same item (e.g., missing pages or plates, brittleness, faded images, etc.).</rdfs:comment>
	</owl:DatatypeProperty>
	<owl:DatatypeProperty rdf:ID="contentItem__NS_contentItem_UNType">
		<rdfs:label>contentItem</rdfs:label>
	<rdfs:comment>Contains a single entry within a content description element.</rdfs:comment>
	</owl:DatatypeProperty>
	<owl:DatatypeProperty rdf:ID="contents__NS_contents_UNType">
		<rdfs:label>contents</rdfs:label>
	<rdfs:comment>Description of the material contained within a resource.</rdfs:comment>
	</owl:DatatypeProperty>
	<owl:DatatypeProperty rdf:ID="context__NS_context_UNType">
		<rdfs:label>context</rdfs:label>
	<rdfs:comment>The historical, social, intellectual, artistic, or other context within which the work was originally conceived (e.g., the 17th century restoration of the monarchy in England, the aesthetic movement of the late 19th century, etc.) or the historical, social, intellectual, artistic, or other context within which the expression was realized.</rdfs:comment>
	</owl:DatatypeProperty>
	<owl:DatatypeProperty rdf:ID="correction__NS_correction_UNType">
		<rdfs:label>correction</rdfs:label>
	<rdfs:comment>States how and under what circumstances corrections have been made in the text.</rdfs:comment>
	</owl:DatatypeProperty>
	<owl:DatatypeProperty rdf:ID="dimensions__NS_dimensions_UNType">
		<rdfs:label>dimensions</rdfs:label>
	<rdfs:comment>Information about the physical size of a bibliographic source; usually includes numerical data.</rdfs:comment>
	</owl:DatatypeProperty>
	<owl:DatatypeProperty rdf:ID="editionStmt__NS_editionStmt_UNType">
		<rdfs:label>editionStmt</rdfs:label>
	<rdfs:comment>(edition statement) – Container for meta-data pertaining to a particular edition of the material being described.</rdfs:comment>
	</owl:DatatypeProperty>
	<owl:DatatypeProperty rdf:ID="editorialDecl__NS_editorialDecl_UNType">
		<rdfs:label>editorialDecl</rdfs:label>
	<rdfs:comment>(editorial declaration) – Used to provide details of editorial principles and practices applied during the encoding of musical text.</rdfs:comment>
	</owl:DatatypeProperty>
	<owl:DatatypeProperty rdf:ID="encodingDesc__NS_encodingDesc_UNType">
		<rdfs:label>encodingDesc</rdfs:label>
	<rdfs:comment>(encoding description) – Documents the relationship between an electronic file and the source or sources from which it was derived as well as applications used in the encoding/editing process.</rdfs:comment>
	</owl:DatatypeProperty>
	<owl:DatatypeProperty rdf:ID="exhibHist__NS_exhibHist_UNType">
		<rdfs:label>exhibHist</rdfs:label>
	<rdfs:comment>(exhibition history) – A record of public exhibitions, including dates, venues, etc.</rdfs:comment>
	</owl:DatatypeProperty>
	<owl:DatatypeProperty rdf:ID="extMeta__NS_extMeta_UNType">
		<rdfs:label>extMeta</rdfs:label>
	<rdfs:comment>(extended metadata) – Provides a container element for non-MEI metadata formats.</rdfs:comment>
	</owl:DatatypeProperty>
	<owl:DatatypeProperty rdf:ID="fileChar__NS_fileChar_UNType">
		<rdfs:label>fileChar</rdfs:label>
	<rdfs:comment>(file characteristics) – Standards or schemes used to encode the file (e.g., ASCII, SGML, etc.), physical characteristics of the file (e.g., recording density, parity, blocking, etc.), and other characteristics that have a bearing on how the file can be processed.</rdfs:comment>
	</owl:DatatypeProperty>
	<owl:DatatypeProperty rdf:ID="fileDesc__NS_fileDesc_UNType">
		<rdfs:label>fileDesc</rdfs:label>
	<rdfs:comment>(file description) – Contains a full bibliographic description of the MEI file.</rdfs:comment>
	</owl:DatatypeProperty>
	<owl:DatatypeProperty rdf:ID="fingerprint__NS_fingerprint_UNType">
		<rdfs:label>fingerprint</rdfs:label>
	<rdfs:comment>Contains a string that uniquely identifies an item, such as those constructed by combining groups of characters transcribed from specified pages of a printed item or a file's checksum.</rdfs:comment>
	</owl:DatatypeProperty>
	<owl:DatatypeProperty rdf:ID="hand__NS_hand_UNType">
		<rdfs:label>hand</rdfs:label>
	<rdfs:comment>Defines a distinct scribe or handwriting style.</rdfs:comment>
	</owl:DatatypeProperty>
	<owl:DatatypeProperty rdf:ID="handList__NS_handList_UNType">
		<rdfs:label>handList</rdfs:label>
	<rdfs:comment>Container for one or more hand elements.</rdfs:comment>
	</owl:DatatypeProperty>
	<owl:DatatypeProperty rdf:ID="history__NS_history_UNType">
		<rdfs:label>history</rdfs:label>
	<rdfs:comment>Provides a container for information about the history of a resource. To facilitate efficient data interchange, basic information about the circumstances surrounding the creation of bibliographic resources should be recorded within the creation element.</rdfs:comment>
	</owl:DatatypeProperty>
	<owl:DatatypeProperty rdf:ID="incipCode__NS_incipCode_UNType">
		<rdfs:label>incipCode</rdfs:label>
	<rdfs:comment>Incipit coded in a non-XML, plain text format, such as Plaine &amp; Easie Code.</rdfs:comment>
	</owl:DatatypeProperty>
	<owl:DatatypeProperty rdf:ID="incipText__NS_incipText_UNType">
		<rdfs:label>incipText</rdfs:label>
	<rdfs:comment>Opening words of a musical composition.</rdfs:comment>
	</owl:DatatypeProperty>
	<owl:DatatypeProperty rdf:ID="inscription__NS_inscription_UNType">
		<rdfs:label>inscription</rdfs:label>
	<rdfs:comment>An inscription added to an item, such as a bookplate, a note designating the item as a gift, and/or the author's signature.</rdfs:comment>
	</owl:DatatypeProperty>
	<owl:DatatypeProperty rdf:ID="interpretation__NS_interpretation_UNType">
		<rdfs:label>interpretation</rdfs:label>
	<rdfs:comment>Describes the scope of any analytic or interpretive information added to the transcription of the music.</rdfs:comment>
	</owl:DatatypeProperty>
	<owl:DatatypeProperty rdf:ID="key__NS_key_UNType">
		<rdfs:label>key</rdfs:label>
	<rdfs:comment>Key captures information about tonal center and mode.</rdfs:comment>
	</owl:DatatypeProperty>
	<owl:DatatypeProperty rdf:ID="language__NS_language_UNType">
		<rdfs:label>language</rdfs:label>
	<rdfs:comment>Description of a language used in the document.</rdfs:comment>
	</owl:DatatypeProperty>
	<owl:DatatypeProperty rdf:ID="langUsage__NS_langUsage_UNType">
		<rdfs:label>langUsage</rdfs:label>
	<rdfs:comment>(language usage) – Groups elements describing the languages, sub-languages, dialects, etc., represented within the encoded resource.</rdfs:comment>
	</owl:DatatypeProperty>
	<owl:DatatypeProperty rdf:ID="meiHead__NS_meiHead_UNType">
		<rdfs:label>meiHead</rdfs:label>
	<rdfs:comment>(MEI header) – Supplies the descriptive and declarative metadata prefixed to every MEI-conformant text.</rdfs:comment>
	</owl:DatatypeProperty>
	<owl:DatatypeProperty rdf:ID="mensuration__NS_mensuration_UNType">
		<rdfs:label>mensuration</rdfs:label>
	<rdfs:comment>Captures information about mensuration within bibliographic descriptions.</rdfs:comment>
	</owl:DatatypeProperty>
	<owl:DatatypeProperty rdf:ID="meter__NS_meter_UNType">
		<rdfs:label>meter</rdfs:label>
	<rdfs:comment>Captures information about the time signature within bibliographic descriptions.</rdfs:comment>
	</owl:DatatypeProperty>
	<owl:DatatypeProperty rdf:ID="normalization__NS_normalization_UNType">
		<rdfs:label>normalization</rdfs:label>
	<rdfs:comment>Indicates the extent of normalization or regularization of the original source carried out in converting it to electronic form.</rdfs:comment>
	</owl:DatatypeProperty>
	<owl:DatatypeProperty rdf:ID="notesStmt__NS_notesStmt_UNType">
		<rdfs:label>notesStmt</rdfs:label>
	<rdfs:comment>(notes statement)– Collects any notes providing information about a text additional to that recorded in other parts of the bibliographic description.</rdfs:comment>
	</owl:DatatypeProperty>
	<owl:DatatypeProperty rdf:ID="otherChar__NS_otherChar_UNType">
		<rdfs:label>otherChar</rdfs:label>
	<rdfs:comment>(other distinguishing characteristic) – Any characteristic that serves to differentiate a work or expression from another.</rdfs:comment>
	</owl:DatatypeProperty>
	<owl:DatatypeProperty rdf:ID="perfDuration__NS_perfDuration_UNType">
		<rdfs:label>perfDuration</rdfs:label>
	<rdfs:comment>(performance duration) – Used to express the duration of performance of printed or manuscript music or the playing time for a sound recording, videorecording, etc.</rdfs:comment>
	</owl:DatatypeProperty>
	<owl:DatatypeProperty rdf:ID="perfMedium__NS_perfMedium_UNType">
		<rdfs:label>perfMedium</rdfs:label>
	<rdfs:comment>(performance medium) – Indicates the number and character of the performing forces used in a musical composition.</rdfs:comment>
	</owl:DatatypeProperty>
	<owl:DatatypeProperty rdf:ID="perfRes__NS_perfRes_UNType">
		<rdfs:label>perfRes</rdfs:label>
	<rdfs:comment>(performance resource) – Name of an instrument on which a performer plays, a performer's voice range, or a standard performing ensemble designation.</rdfs:comment>
	</owl:DatatypeProperty>
	<owl:DatatypeProperty rdf:ID="perfResList__NS_perfResList_UNType">
		<rdfs:label>perfResList</rdfs:label>
	<rdfs:comment>Several instrumental or vocal resources treated as a group.</rdfs:comment>
	</owl:DatatypeProperty>
	<owl:DatatypeProperty rdf:ID="physDesc__NS_physDesc_UNType">
		<rdfs:label>physDesc</rdfs:label>
	<rdfs:comment>(physical description) – Container for information about the appearance, construction, or handling of physical materials, such as their dimension, quantity, color, style, and technique of creation.</rdfs:comment>
	</owl:DatatypeProperty>
	<owl:DatatypeProperty rdf:ID="physMedium__NS_physMedium_UNType">
		<rdfs:label>physMedium</rdfs:label>
	<rdfs:comment>(physical medium) – Records the physical materials used in the source, such as ink and paper.</rdfs:comment>
	</owl:DatatypeProperty>
	<owl:DatatypeProperty rdf:ID="plateNum__NS_plateNum_UNType">
		<rdfs:label>plateNum</rdfs:label>
	<rdfs:comment>(plate number) – Designation assigned to a resource by a music publisher, usually printed at the bottom of each page, and sometimes appearing also on the title page.</rdfs:comment>
	</owl:DatatypeProperty>
	<owl:DatatypeProperty rdf:ID="playingSpeed__NS_playingSpeed_UNType">
		<rdfs:label>playingSpeed</rdfs:label>
	<rdfs:comment>Playing speed for a sound recording is the speed at which the carrier must be operated to produce the sound intended (e.g., 33 1/3 rpm, 19 cm/s, etc.).</rdfs:comment>
	</owl:DatatypeProperty>
	<owl:DatatypeProperty rdf:ID="price__NS_price_UNType">
		<rdfs:label>price</rdfs:label>
	<rdfs:comment>The cost of access to a bibliographic item.</rdfs:comment>
	</owl:DatatypeProperty>
	<owl:DatatypeProperty rdf:ID="projectDesc__NS_projectDesc_UNType">
		<rdfs:label>projectDesc</rdfs:label>
	<rdfs:comment>(project description) – Project-level meta-data describing the aim or purpose for which the electronic file was encoded, funding agencies, etc. together with any other relevant information concerning the process by which it was assembled or collected.</rdfs:comment>
	</owl:DatatypeProperty>
	<owl:DatatypeProperty rdf:ID="provenance__NS_provenance_UNType">
		<rdfs:label>provenance</rdfs:label>
	<rdfs:comment>The record of ownership or custodianship of an item.</rdfs:comment>
	</owl:DatatypeProperty>
	<owl:DatatypeProperty rdf:ID="pubStmt__NS_pubStmt_UNType">
		<rdfs:label>pubStmt</rdfs:label>
	<rdfs:comment>(publication statement) – Container for information regarding the publication or distribution of a bibliographic item, including the publisher's name and address, the date of publication, and other relevant details.</rdfs:comment>
	</owl:DatatypeProperty>
	<owl:DatatypeProperty rdf:ID="revisionDesc__NS_revisionDesc_UNType">
		<rdfs:label>revisionDesc</rdfs:label>
	<rdfs:comment>(revision description) – Container for information about alterations that have been made to an MEI file.</rdfs:comment>
	</owl:DatatypeProperty>
	<owl:DatatypeProperty rdf:ID="samplingDecl__NS_samplingDecl_UNType">
		<rdfs:label>samplingDecl</rdfs:label>
	<rdfs:comment>(sampling declaration) – Contains a prose description of the rationale and methods used in sampling texts in the creation of a corpus or collection.</rdfs:comment>
	</owl:DatatypeProperty>
	<owl:DatatypeProperty rdf:ID="scoreFormat__NS_scoreFormat_UNType">
		<rdfs:label>scoreFormat</rdfs:label>
	<rdfs:comment>Describes the type of score used to represent a musical composition (e.g., short score, full score, condensed score, close score, etc.).</rdfs:comment>
	</owl:DatatypeProperty>
	<owl:DatatypeProperty rdf:ID="segmentation__NS_segmentation_UNType">
		<rdfs:label>segmentation</rdfs:label>
	<rdfs:comment>Describes the principles according to which the musical text has been segmented, for example into movements, sections, etc.</rdfs:comment>
	</owl:DatatypeProperty>
	<owl:DatatypeProperty rdf:ID="seriesStmt__NS_seriesStmt_UNType">
		<rdfs:label>seriesStmt</rdfs:label>
	<rdfs:comment>(series statement) – Groups information about the series, if any, to which a publication belongs.</rdfs:comment>
	</owl:DatatypeProperty>
	<owl:DatatypeProperty rdf:ID="soundChan__NS_soundChan_UNType">
		<rdfs:label>soundChan</rdfs:label>
	<rdfs:comment>(sound channels) – Reflects the number of apparent sound channels in the playback of a recording (monaural, stereophonic, quadraphonic, etc.).</rdfs:comment>
	</owl:DatatypeProperty>
	<owl:DatatypeProperty rdf:ID="source__NS_source_UNType">
		<rdfs:label>source</rdfs:label>
	<rdfs:comment>A bibliographic description of a source used in the creation of the electronic file.</rdfs:comment>
	</owl:DatatypeProperty>
	<owl:DatatypeProperty rdf:ID="sourceDesc__NS_sourceDesc_UNType">
		<rdfs:label>sourceDesc</rdfs:label>
	<rdfs:comment>(source description) – A container for the descriptions of the source(s) used in the creation of the electronic file.</rdfs:comment>
	</owl:DatatypeProperty>
	<owl:DatatypeProperty rdf:ID="specRepro__NS_specRepro_UNType">
		<rdfs:label>specRepro</rdfs:label>
	<rdfs:comment>(special reproduction characteristic) – The equalization system, noise reduction system, etc. used in making the recording (e.g., NAB, DBX, Dolby, etc.).</rdfs:comment>
	</owl:DatatypeProperty>
	<owl:DatatypeProperty rdf:ID="stdVals__NS_stdVals_UNType">
		<rdfs:label>stdVals</rdfs:label>
	<rdfs:comment>(standard values) – Specifies the format used when standardized date or number values are supplied.</rdfs:comment>
	</owl:DatatypeProperty>
	<owl:DatatypeProperty rdf:ID="sysReq__NS_sysReq_UNType">
		<rdfs:label>sysReq</rdfs:label>
	<rdfs:comment>(system requirements) – System requirements for using the electronic item.</rdfs:comment>
	</owl:DatatypeProperty>
	<owl:DatatypeProperty rdf:ID="term__NS_term_UNType">
		<rdfs:label>term</rdfs:label>
	<rdfs:comment>Keyword or phrase which describes a resource.</rdfs:comment>
	</owl:DatatypeProperty>
	<owl:DatatypeProperty rdf:ID="termList__NS_termList_UNType">
		<rdfs:label>termList</rdfs:label>
	<rdfs:comment>Collection of text phrases which describe a resource.</rdfs:comment>
	</owl:DatatypeProperty>
	<owl:DatatypeProperty rdf:ID="titleStmt__NS_titleStmt_UNType">
		<rdfs:label>titleStmt</rdfs:label>
	<rdfs:comment>(title statement) – Container for title and responsibility meta-data.</rdfs:comment>
	</owl:DatatypeProperty>
	<owl:DatatypeProperty rdf:ID="trackConfig__NS_trackConfig_UNType">
		<rdfs:label>trackConfig</rdfs:label>
	<rdfs:comment>(track configuration) – Number of physical/input tracks on a sound medium (e.g., eight track, twelve track).</rdfs:comment>
	</owl:DatatypeProperty>
	<owl:DatatypeProperty rdf:ID="treatHist__NS_treatHist_UNType">
		<rdfs:label>treatHist</rdfs:label>
	<rdfs:comment>(treatment history) – A record of the treatment the item has undergone (e.g., de-acidification, restoration, etc.).</rdfs:comment>
	</owl:DatatypeProperty>
	<owl:DatatypeProperty rdf:ID="treatSched__NS_treatSched_UNType">
		<rdfs:label>treatSched</rdfs:label>
	<rdfs:comment>(treatment scheduled) – Scheduled treatment, e.g. de-acidification, restoration, etc., for an item.</rdfs:comment>
	</owl:DatatypeProperty>
	<owl:DatatypeProperty rdf:ID="unpub__NS_unpub_UNType">
		<rdfs:label>unpub</rdfs:label>
	<rdfs:comment>(unpublished) – Used to explicitly indicate that a bibliographic resource is unpublished.</rdfs:comment>
	</owl:DatatypeProperty>
	<owl:DatatypeProperty rdf:ID="useRestrict__NS_useRestrict_UNType">
		<rdfs:label>useRestrict</rdfs:label>
	<rdfs:comment>(usage restrictions) – Container for information about the conditions that affect use of a bibliographic item after access has been granted.</rdfs:comment>
	</owl:DatatypeProperty>
	<owl:DatatypeProperty rdf:ID="watermark__NS_watermark_UNType">
		<rdfs:label>watermark</rdfs:label>
	<rdfs:comment>Contains a description of a watermark or similar device.</rdfs:comment>
	</owl:DatatypeProperty>
	<owl:DatatypeProperty rdf:ID="work__NS_work_UNType">
		<rdfs:label>work</rdfs:label>
	<rdfs:comment>Provides a detailed description of a work, specifically its history, language use, and high-level musical attributes: key, tempo, meter, medium of performance, and intended duration.</rdfs:comment>
	</owl:DatatypeProperty>
	<owl:DatatypeProperty rdf:ID="workDesc__NS_workDesc_UNType">
		<rdfs:label>workDesc</rdfs:label>
	<rdfs:comment>(work description) – Grouping mechanism for information describing non-bibliographic aspects of a text.</rdfs:comment>
	</owl:DatatypeProperty>
	<owl:DatatypeProperty rdf:ID="arpeg__NS_arpeg_UNType">
		<rdfs:label>arpeg</rdfs:label>
	<rdfs:comment>(arpeggiation) – Indicates that the notes of a chord are to be performed successively rather than simultaneously, usually from lowest to highest. Sometimes called a &quot;roll&quot;.</rdfs:comment>
	</owl:DatatypeProperty>
	<owl:DatatypeProperty rdf:ID="beam__NS_beam_UNType">
		<rdfs:label>beam</rdfs:label>
	<rdfs:comment>A container for a series of explicitly beamed events that begins and ends entirely within a measure.</rdfs:comment>
	</owl:DatatypeProperty>
	<owl:DatatypeProperty rdf:ID="beamSpan__NS_beamSpan_UNType">
		<rdfs:label>beamSpan</rdfs:label>
	<rdfs:comment>(beam span) – Alternative element for explicitly encoding beams, particularly those which extend across bar lines.</rdfs:comment>
	</owl:DatatypeProperty>
	<owl:DatatypeProperty rdf:ID="beatRpt__NS_beatRpt_UNType">
		<rdfs:label>beatRpt</rdfs:label>
	<rdfs:comment>(beat repeat) – An indication that material on a preceding beat should be repeated.</rdfs:comment>
	</owl:DatatypeProperty>
	<owl:DatatypeProperty rdf:ID="bend__NS_bend_UNType">
		<rdfs:label>bend</rdfs:label>
	<rdfs:comment>A variation in pitch (often micro-tonal) upwards or downwards during the course of a note.</rdfs:comment>
	</owl:DatatypeProperty>
	<owl:DatatypeProperty rdf:ID="breath__NS_breath_UNType">
		<rdfs:label>breath</rdfs:label>
	<rdfs:comment>(breath mark) – A indication of a point at which the performer on an instrument requiring breath (including the voice) may breathe.</rdfs:comment>
	</owl:DatatypeProperty>
	<owl:DatatypeProperty rdf:ID="bTrem__NS_bTrem_UNType">
		<rdfs:label>bTrem</rdfs:label>
	<rdfs:comment>(bowed tremolo) – A rapid alternation on a single pitch or chord.</rdfs:comment>
	</owl:DatatypeProperty>
	<owl:DatatypeProperty rdf:ID="fermata__NS_fermata_UNType">
		<rdfs:label>fermata</rdfs:label>
	<rdfs:comment>An indication placed over a note or rest to indicate that it should be held longer than its written value. May also occur over a bar line to indicate the end of a phrase or section. Sometimes called a 'hold' or 'pause'.</rdfs:comment>
	</owl:DatatypeProperty>
	<owl:DatatypeProperty rdf:ID="fTrem__NS_fTrem_UNType">
		<rdfs:label>fTrem</rdfs:label>
	<rdfs:comment>(fingered tremolo) – A rapid alternation between a pair of notes (or chords or perhaps between a note and a chord) that are (usually) farther apart than a major second.</rdfs:comment>
	</owl:DatatypeProperty>
	<owl:DatatypeProperty rdf:ID="gliss__NS_gliss_UNType">
		<rdfs:label>gliss</rdfs:label>
	<rdfs:comment>(glissando) – A continuous or sliding movement from one pitch to another, usually indicated by a straight or wavy line.</rdfs:comment>
	</owl:DatatypeProperty>
	<owl:DatatypeProperty rdf:ID="hairpin__NS_hairpin_UNType">
		<rdfs:label>hairpin</rdfs:label>
	<rdfs:comment>Indicates continuous dynamics expressed on the score as wedge-shaped graphics, e.g. &lt; and &gt;.</rdfs:comment>
	</owl:DatatypeProperty>
	<owl:DatatypeProperty rdf:ID="halfmRpt__NS_halfmRpt_UNType">
		<rdfs:label>halfmRpt</rdfs:label>
	<rdfs:comment>(half-measure repeat) – A half-measure repeat in any meter.</rdfs:comment>
	</owl:DatatypeProperty>
	<owl:DatatypeProperty rdf:ID="harpPedal__NS_harpPedal_UNType">
		<rdfs:label>harpPedal</rdfs:label>
	<rdfs:comment>(harp pedal) – Harp pedal diagram.</rdfs:comment>
	</owl:DatatypeProperty>
	<owl:DatatypeProperty rdf:ID="measure__NS_measure_UNType">
		<rdfs:label>measure</rdfs:label>
	<rdfs:comment>Unit of musical time consisting of a fixed number of note-values of a given type, as determined by the prevailing meter, and delimited in musical notation by bar lines.</rdfs:comment>
	</owl:DatatypeProperty>
	<owl:DatatypeProperty rdf:ID="meterSig__NS_meterSig_UNType">
		<rdfs:label>meterSig</rdfs:label>
	<rdfs:comment>(meter signature) – Written meter signature.</rdfs:comment>
	</owl:DatatypeProperty>
	<owl:DatatypeProperty rdf:ID="meterSigGrp__NS_meterSigGrp_UNType">
		<rdfs:label>meterSigGrp</rdfs:label>
	<rdfs:comment>(meter signature group) – Used to capture alternating, interchanging, and mixed meter signatures.</rdfs:comment>
	</owl:DatatypeProperty>
	<owl:DatatypeProperty rdf:ID="mRest__NS_mRest_UNType">
		<rdfs:label>mRest</rdfs:label>
	<rdfs:comment>(measure rest) – Complete measure rest in any meter. </rdfs:comment>
	</owl:DatatypeProperty>
	<owl:DatatypeProperty rdf:ID="mRpt__NS_mRpt_UNType">
		<rdfs:label>mRpt</rdfs:label>
	<rdfs:comment>(measure repeat) – An indication that the previous measure should be repeated.</rdfs:comment>
	</owl:DatatypeProperty>
	<owl:DatatypeProperty rdf:ID="mRpt2__NS_mRpt2_UNType">
		<rdfs:label>mRpt2</rdfs:label>
	<rdfs:comment>(2-measure repeat) – An indication that the previous two measures should be repeated.</rdfs:comment>
	</owl:DatatypeProperty>
	<owl:DatatypeProperty rdf:ID="mSpace__NS_mSpace_UNType">
		<rdfs:label>mSpace</rdfs:label>
	<rdfs:comment>(measure space) – A measure containing only empty space in any meter.</rdfs:comment>
	</owl:DatatypeProperty>
	<owl:DatatypeProperty rdf:ID="multiRest__NS_multiRest_UNType">
		<rdfs:label>multiRest</rdfs:label>
	<rdfs:comment>(multiple rest) – Multiple measures of rest compressed into a single symbol, frequently found in performer parts.</rdfs:comment>
	</owl:DatatypeProperty>
	<owl:DatatypeProperty rdf:ID="multiRpt__NS_multiRpt_UNType">
		<rdfs:label>multiRpt</rdfs:label>
	<rdfs:comment>(multiple repeat) – Multiple repeated measures.</rdfs:comment>
	</owl:DatatypeProperty>
	<owl:DatatypeProperty rdf:ID="octave__NS_octave_UNType">
		<rdfs:label>octave</rdfs:label>
	<rdfs:comment>An indication that a passage should be performed one or more octaves above or below its written pitch.</rdfs:comment>
	</owl:DatatypeProperty>
	<owl:DatatypeProperty rdf:ID="ossia__NS_ossia_UNType">
		<rdfs:label>ossia</rdfs:label>
	<rdfs:comment>An alternate notational version *present in the source being transcribed*.</rdfs:comment>
	</owl:DatatypeProperty>
	<owl:DatatypeProperty rdf:ID="pedal__NS_pedal_UNType">
		<rdfs:label>pedal</rdfs:label>
	<rdfs:comment>Piano pedal mark.</rdfs:comment>
	</owl:DatatypeProperty>
	<owl:DatatypeProperty rdf:ID="reh__NS_reh_UNType">
		<rdfs:label>reh</rdfs:label>
	<rdfs:comment>(rehearsal mark) – In an orchestral score and its corresponding parts, a mark indicating a convenient point from which to resume rehearsal after a break.</rdfs:comment>
	</owl:DatatypeProperty>
	<owl:DatatypeProperty rdf:ID="slur__NS_slur_UNType">
		<rdfs:label>slur</rdfs:label>
	<rdfs:comment>Indication of 1) a &quot;unified melodic idea&quot; or 2) performance technique.</rdfs:comment>
	</owl:DatatypeProperty>
	<owl:DatatypeProperty rdf:ID="tie__NS_tie_UNType">
		<rdfs:label>tie</rdfs:label>
	<rdfs:comment>An indication that two notes of the same pitch form a single note with their combined rhythmic values.</rdfs:comment>
	</owl:DatatypeProperty>
	<owl:DatatypeProperty rdf:ID="tuplet__NS_tuplet_UNType">
		<rdfs:label>tuplet</rdfs:label>
	<rdfs:comment>A group of notes with &quot;irregular&quot; (sometimes called &quot;irrational&quot;) rhythmic values, for example, three notes in the time normally occupied by two or nine in the time of five.</rdfs:comment>
	</owl:DatatypeProperty>
	<owl:DatatypeProperty rdf:ID="tupletSpan__NS_tupletSpan_UNType">
		<rdfs:label>tupletSpan</rdfs:label>
	<rdfs:comment>(tuplet span) – Alternative element for encoding tuplets, especially useful for tuplets that extend across bar lines.</rdfs:comment>
	</owl:DatatypeProperty>
	<owl:DatatypeProperty rdf:ID="ligature__NS_ligature_UNType">
		<rdfs:label>ligature</rdfs:label>
	<rdfs:comment>A mensural notation symbol that combines two or more notes into a single sign.</rdfs:comment>
	</owl:DatatypeProperty>
	<owl:DatatypeProperty rdf:ID="mensur__NS_mensur_UNType">
		<rdfs:label>mensur</rdfs:label>
	<rdfs:comment>(mensuration) – Collects information about the metrical relationship between a note value and the next smaller value; that is, either triple or duple.</rdfs:comment>
	</owl:DatatypeProperty>
	<owl:DatatypeProperty rdf:ID="proport__NS_proport_UNType">
		<rdfs:label>proport</rdfs:label>
	<rdfs:comment>(proportion) – Description of note duration as arithmetic ratio.</rdfs:comment>
	</owl:DatatypeProperty>
	<owl:DatatypeProperty rdf:ID="ineume__NS_ineume_UNType">
		<rdfs:label>ineume</rdfs:label>
	<rdfs:comment>(interrupted neume) – A graphically interrupted neume; that is, a neume which is logically a single entity but is written using multiple signs.</rdfs:comment>
	</owl:DatatypeProperty>
	<owl:DatatypeProperty rdf:ID="syllable__NS_syllable_UNType">
		<rdfs:label>syllable</rdfs:label>
	<rdfs:comment>Neume notation can be thought of as &quot;neumed text&quot;. Therefore, the syllable element provides high-level organization in this repertoire.</rdfs:comment>
	</owl:DatatypeProperty>
	<owl:DatatypeProperty rdf:ID="uneume__NS_uneume_UNType">
		<rdfs:label>uneume</rdfs:label>
	<rdfs:comment>(uninterrupted neume) – A graphically-uninterrupted neume sign.</rdfs:comment>
	</owl:DatatypeProperty>
	<owl:DatatypeProperty rdf:ID="mordent__NS_mordent_UNType">
		<rdfs:label>mordent</rdfs:label>
	<rdfs:comment>An ornament indicating rapid alternation of the main note with a secondary note, usually a step below, but sometimes a step above. </rdfs:comment>
	</owl:DatatypeProperty>
	<owl:DatatypeProperty rdf:ID="trill__NS_trill_UNType">
		<rdfs:label>trill</rdfs:label>
	<rdfs:comment>Rapid alternation of a note with another (usually at the interval of a second above).</rdfs:comment>
	</owl:DatatypeProperty>
	<owl:DatatypeProperty rdf:ID="turn__NS_turn_UNType">
		<rdfs:label>turn</rdfs:label>
	<rdfs:comment>An ornament consisting of four notes — the upper neighbor of the written note, the written note, the lower neighbor, and the written note.</rdfs:comment>
	</owl:DatatypeProperty>
	<owl:DatatypeProperty rdf:ID="meiCorpus__NS_meiCorpus_UNType">
		<rdfs:label>meiCorpus</rdfs:label>
	<rdfs:comment>(MEI corpus) – A group of related MEI documents, consisting of a header for the group, and one or more &lt;mei&gt; elements, each with its own complete header.</rdfs:comment>
	</owl:DatatypeProperty>
	<owl:DatatypeProperty rdf:ID="app__NS_app_UNType">
		<rdfs:label>app</rdfs:label>
	<rdfs:comment>(apparatus) – Contains one or more alternative encodings.</rdfs:comment>
	</owl:DatatypeProperty>
	<owl:DatatypeProperty rdf:ID="lem__NS_lem_UNType">
		<rdfs:label>lem</rdfs:label>
	<rdfs:comment>(lemma) – Contains the lemma, or base text, of a textual variation.</rdfs:comment>
	</owl:DatatypeProperty>
	<owl:DatatypeProperty rdf:ID="rdg__NS_rdg_UNType">
		<rdfs:label>rdg</rdfs:label>
	<rdfs:comment>(reading) – Contains a single reading within a textual variation.</rdfs:comment>
	</owl:DatatypeProperty>
	<owl:DatatypeProperty rdf:ID="abbr__NS_abbr_UNType">
		<rdfs:label>abbr</rdfs:label>
	<rdfs:comment>(abbreviation) – A generic element for 1) a shortened form of a word, including an acronym or 2) a shorthand notation.</rdfs:comment>
	</owl:DatatypeProperty>
	<owl:DatatypeProperty rdf:ID="add__NS_add_UNType">
		<rdfs:label>add</rdfs:label>
	<rdfs:comment>(addition) – Marks an addition to the text.</rdfs:comment>
	</owl:DatatypeProperty>
	<owl:DatatypeProperty rdf:ID="choice__NS_choice_UNType">
		<rdfs:label>choice</rdfs:label>
	<rdfs:comment>Groups a number of alternative encodings for the same point in a text.</rdfs:comment>
	</owl:DatatypeProperty>
	<owl:DatatypeProperty rdf:ID="corr__NS_corr_UNType">
		<rdfs:label>corr</rdfs:label>
	<rdfs:comment>(correction) – Contains the correct form of an apparent erroneous passage.</rdfs:comment>
	</owl:DatatypeProperty>
	<owl:DatatypeProperty rdf:ID="cpMark__NS_cpMark_UNType">
		<rdfs:label>cpMark</rdfs:label>
	<rdfs:comment>(copy/colla parte mark) – A verbal or graphical indication to copy musical material written elsewhere.</rdfs:comment>
	</owl:DatatypeProperty>
	<owl:DatatypeProperty rdf:ID="damage__NS_damage_UNType">
		<rdfs:label>damage</rdfs:label>
	<rdfs:comment>Contains an area of damage to the physical medium.</rdfs:comment>
	</owl:DatatypeProperty>
	<owl:DatatypeProperty rdf:ID="del__NS_del_UNType">
		<rdfs:label>del</rdfs:label>
	<rdfs:comment>(deletion) – Contains information deleted, marked as deleted, or otherwise indicated as superfluous or spurious in the copy text by an author, scribe, annotator, or corrector.</rdfs:comment>
	</owl:DatatypeProperty>
	<owl:DatatypeProperty rdf:ID="expan__NS_expan_UNType">
		<rdfs:label>expan</rdfs:label>
	<rdfs:comment>(expansion) – Contains the expansion of an abbreviation.</rdfs:comment>
	</owl:DatatypeProperty>
	<owl:DatatypeProperty rdf:ID="gap__NS_gap_UNType">
		<rdfs:label>gap</rdfs:label>
	<rdfs:comment>Indicates a point where material has been omitted in a transcription, whether as part of sampling practice or for editorial reasons described in the MEI header.</rdfs:comment>
	</owl:DatatypeProperty>
	<owl:DatatypeProperty rdf:ID="handShift__NS_handShift_UNType">
		<rdfs:label>handShift</rdfs:label>
	<rdfs:comment>Marks the beginning of a passage written in a new hand, or of a change in the scribe, writing style, ink or character of the document hand.</rdfs:comment>
	</owl:DatatypeProperty>
	<owl:DatatypeProperty rdf:ID="orig__NS_orig_UNType">
		<rdfs:label>orig</rdfs:label>
	<rdfs:comment>(original) – Contains material which is marked as following the original, rather than being normalized or corrected.</rdfs:comment>
	</owl:DatatypeProperty>
	<owl:DatatypeProperty rdf:ID="reg__NS_reg_UNType">
		<rdfs:label>reg</rdfs:label>
	<rdfs:comment>(regularization) – Contains material which has been regularized or normalized in some sense.</rdfs:comment>
	</owl:DatatypeProperty>
	<owl:DatatypeProperty rdf:ID="restore__NS_restore_UNType">
		<rdfs:label>restore</rdfs:label>
	<rdfs:comment>Indicates restoration of material to an earlier state by cancellation of an editorial or authorial marking or instruction.</rdfs:comment>
	</owl:DatatypeProperty>
	<owl:DatatypeProperty rdf:ID="sic__NS_sic_UNType">
		<rdfs:label>sic</rdfs:label>
	<rdfs:comment>Contains apparently incorrect or inaccurate material.</rdfs:comment>
	</owl:DatatypeProperty>
	<owl:DatatypeProperty rdf:ID="subst__NS_subst_UNType">
		<rdfs:label>subst</rdfs:label>
	<rdfs:comment>(substitution) – Groups transcriptional elements when the combination is to be regarded as a single intervention in the text.</rdfs:comment>
	</owl:DatatypeProperty>
	<owl:DatatypeProperty rdf:ID="supplied__NS_supplied_UNType">
		<rdfs:label>supplied</rdfs:label>
	<rdfs:comment>Contains material supplied by the transcriber or editor for any reason.</rdfs:comment>
	</owl:DatatypeProperty>
	<owl:DatatypeProperty rdf:ID="unclear__NS_unclear_UNType">
		<rdfs:label>unclear</rdfs:label>
	<rdfs:comment>Contains material that cannot be transcribed with certainty because it is illegible or inaudible in the source.</rdfs:comment>
	</owl:DatatypeProperty>
	<owl:DatatypeProperty rdf:ID="facsimile__NS_facsimile_UNType">
		<rdfs:label>facsimile</rdfs:label>
	<rdfs:comment>Contains a representation of some written source in the form of a set of images rather than as transcribed or encoded text.</rdfs:comment>
	</owl:DatatypeProperty>
	<owl:DatatypeProperty rdf:ID="surface__NS_surface_UNType">
		<rdfs:label>surface</rdfs:label>
	<rdfs:comment>Defines a writing surface in terms of a rectangular coordinate space, optionally grouping one or more graphic representations of that space, and rectangular zones of interest within it.</rdfs:comment>
	</owl:DatatypeProperty>
	<owl:DatatypeProperty rdf:ID="zone__NS_zone_UNType">
		<rdfs:label>zone</rdfs:label>
	<rdfs:comment>Defines an area of interest within a surface or graphic file.</rdfs:comment>
	</owl:DatatypeProperty>
	<owl:DatatypeProperty rdf:ID="fig__NS_fig_UNType">
		<rdfs:label>fig</rdfs:label>
	<rdfs:comment>(figure) – Groups elements representing or containing graphic information such as an illustration or figure.</rdfs:comment>
	</owl:DatatypeProperty>
	<owl:DatatypeProperty rdf:ID="figDesc__NS_figDesc_UNType">
		<rdfs:label>figDesc</rdfs:label>
	<rdfs:comment>(figure description) – Contains a brief prose description of the appearance or content of a graphic figure, for use when documenting an image without displaying it.</rdfs:comment>
	</owl:DatatypeProperty>
	<owl:DatatypeProperty rdf:ID="graphic__NS_graphic_UNType">
		<rdfs:label>graphic</rdfs:label>
	<rdfs:comment>Indicates the location of an inline graphic.</rdfs:comment>
	</owl:DatatypeProperty>
	<owl:DatatypeProperty rdf:ID="table__NS_table_UNType">
		<rdfs:label>table</rdfs:label>
	<rdfs:comment>Contains text displayed in tabular form.</rdfs:comment>
	</owl:DatatypeProperty>
	<owl:DatatypeProperty rdf:ID="td__NS_td_UNType">
		<rdfs:label>td</rdfs:label>
	<rdfs:comment>(table data) – Designates a table cell that contains data as opposed to a cell that contains column or row heading information.</rdfs:comment>
	</owl:DatatypeProperty>
	<owl:DatatypeProperty rdf:ID="th__NS_th_UNType">
		<rdfs:label>th</rdfs:label>
	<rdfs:comment>(table header) – Designates a table cell containing column or row heading information as opposed to one containing data.</rdfs:comment>
	</owl:DatatypeProperty>
	<owl:DatatypeProperty rdf:ID="tr__NS_tr_UNType">
		<rdfs:label>tr</rdfs:label>
	<rdfs:comment>(table row) – A formatting element that contains one or more cells (intersection of a row and a column) in a &lt;table&gt;.</rdfs:comment>
	</owl:DatatypeProperty>
	<owl:DatatypeProperty rdf:ID="barre__NS_barre_UNType">
		<rdfs:label>barre</rdfs:label>
	<rdfs:comment>An indication of fingering in a chord tablature grid.</rdfs:comment>
	</owl:DatatypeProperty>
	<owl:DatatypeProperty rdf:ID="chordDef__NS_chordDef_UNType">
		<rdfs:label>chordDef</rdfs:label>
	<rdfs:comment>(chord definition) – Chord tablature definition.</rdfs:comment>
	</owl:DatatypeProperty>
	<owl:DatatypeProperty rdf:ID="chordMember__NS_chordMember_UNType">
		<rdfs:label>chordMember</rdfs:label>
	<rdfs:comment>An individual pitch in a chord defined by a &lt;chordDef&gt; element.</rdfs:comment>
	</owl:DatatypeProperty>
	<owl:DatatypeProperty rdf:ID="chordTable__NS_chordTable_UNType">
		<rdfs:label>chordTable</rdfs:label>
	<rdfs:comment>Chord/tablature look-up table.</rdfs:comment>
	</owl:DatatypeProperty>
	<owl:DatatypeProperty rdf:ID="f__NS_f_UNType">
		<rdfs:label>f</rdfs:label>
	<rdfs:comment>(figure) – Single element of a figured bass indication.</rdfs:comment>
	</owl:DatatypeProperty>
	<owl:DatatypeProperty rdf:ID="fb__NS_fb_UNType">
		<rdfs:label>fb</rdfs:label>
	<rdfs:comment>(figured bass) – Symbols added to a bass line that indicate harmony. Used to improvise a chordal accompaniment. Sometimes called Generalbass, thoroughbass, or basso continuo.</rdfs:comment>
	</owl:DatatypeProperty>
	<owl:DatatypeProperty rdf:ID="harm__NS_harm_UNType">
		<rdfs:label>harm</rdfs:label>
	<rdfs:comment>(harmony) – An indication of harmony, e.g., chord names, tablature grids, harmonic analysis, figured bass.</rdfs:comment>
	</owl:DatatypeProperty>
	<owl:DatatypeProperty rdf:ID="lyrics__NS_lyrics_UNType">
		<rdfs:label>lyrics</rdfs:label>
	<rdfs:comment>Vocally performed 'text' of a musical composition, such as a song or opera.</rdfs:comment>
	</owl:DatatypeProperty>
	<owl:DatatypeProperty rdf:ID="verse__NS_verse_UNType">
		<rdfs:label>verse</rdfs:label>
	<rdfs:comment>Lyric verse.</rdfs:comment>
	</owl:DatatypeProperty>
	<owl:DatatypeProperty rdf:ID="cc__NS_cc_UNType">
		<rdfs:label>cc</rdfs:label>
	<rdfs:comment>(control change) – MIDI parameter/control change.</rdfs:comment>
	</owl:DatatypeProperty>
	<owl:DatatypeProperty rdf:ID="chan__NS_chan_UNType">
		<rdfs:label>chan</rdfs:label>
	<rdfs:comment>(channel) – MIDI channel assignment.</rdfs:comment>
	</owl:DatatypeProperty>
	<owl:DatatypeProperty rdf:ID="chanPr__NS_chanPr_UNType">
		<rdfs:label>chanPr</rdfs:label>
	<rdfs:comment>(channel pressure) – MIDI channel pressure/after touch.</rdfs:comment>
	</owl:DatatypeProperty>
	<owl:DatatypeProperty rdf:ID="cue__NS_cue_UNType">
		<rdfs:label>cue</rdfs:label>
	<rdfs:comment>MIDI cue point.</rdfs:comment>
	</owl:DatatypeProperty>
	<owl:DatatypeProperty rdf:ID="hex__NS_hex_UNType">
		<rdfs:label>hex</rdfs:label>
	<rdfs:comment>Arbitrary MIDI data in hexadecimal form.</rdfs:comment>
	</owl:DatatypeProperty>
	<owl:DatatypeProperty rdf:ID="instrDef__NS_instrDef_UNType">
		<rdfs:label>instrDef</rdfs:label>
	<rdfs:comment>(instrument definition) – MIDI instrument declaration.</rdfs:comment>
	</owl:DatatypeProperty>
	<owl:DatatypeProperty rdf:ID="instrGrp__NS_instrGrp_UNType">
		<rdfs:label>instrGrp</rdfs:label>
	<rdfs:comment>(instrument group) – Collects MIDI instrument definitions.</rdfs:comment>
	</owl:DatatypeProperty>
	<owl:DatatypeProperty rdf:ID="metaText__NS_metaText_UNType">
		<rdfs:label>metaText</rdfs:label>
	<rdfs:comment>MIDI text meta-event.</rdfs:comment>
	</owl:DatatypeProperty>
	<owl:DatatypeProperty rdf:ID="midi__NS_midi_UNType">
		<rdfs:label>midi</rdfs:label>
	<rdfs:comment>Container for elements that contain information useful when generating MIDI output.</rdfs:comment>
	</owl:DatatypeProperty>
	<owl:DatatypeProperty rdf:ID="noteOff__NS_noteOff_UNType">
		<rdfs:label>noteOff</rdfs:label>
	<rdfs:comment>MIDI note-off event.</rdfs:comment>
	</owl:DatatypeProperty>
	<owl:DatatypeProperty rdf:ID="noteOn__NS_noteOn_UNType">
		<rdfs:label>noteOn</rdfs:label>
	<rdfs:comment>MIDI note-on event.</rdfs:comment>
	</owl:DatatypeProperty>
	<owl:DatatypeProperty rdf:ID="port__NS_port_UNType">
		<rdfs:label>port</rdfs:label>
	<rdfs:comment>MIDI port.</rdfs:comment>
	</owl:DatatypeProperty>
	<owl:DatatypeProperty rdf:ID="prog__NS_prog_UNType">
		<rdfs:label>prog</rdfs:label>
	<rdfs:comment>(program) – MIDI program change.</rdfs:comment>
	</owl:DatatypeProperty>
	<owl:DatatypeProperty rdf:ID="seqNum__NS_seqNum_UNType">
		<rdfs:label>seqNum</rdfs:label>
	<rdfs:comment>(sequence number) – MIDI sequence number.</rdfs:comment>
	</owl:DatatypeProperty>
	<owl:DatatypeProperty rdf:ID="trkName__NS_trkName_UNType">
		<rdfs:label>trkName</rdfs:label>
	<rdfs:comment>(track name) – MIDI track/sequence name.</rdfs:comment>
	</owl:DatatypeProperty>
	<owl:DatatypeProperty rdf:ID="vel__NS_vel_UNType">
		<rdfs:label>vel</rdfs:label>
	<rdfs:comment>(velocity) – MIDI Note-on/off velocity.</rdfs:comment>
	</owl:DatatypeProperty>
	<owl:DatatypeProperty rdf:ID="addName__NS_addName_UNType">
		<rdfs:label>addName</rdfs:label>
	<rdfs:comment>(additional name) – Contains an additional name component, such as a nickname, epithet, or alias, or any other descriptive phrase used within a personal name.</rdfs:comment>
	</owl:DatatypeProperty>
	<owl:DatatypeProperty rdf:ID="bloc__NS_bloc_UNType">
		<rdfs:label>bloc</rdfs:label>
	<rdfs:comment>Contains the name of a geo-political unit consisting of two or more nation states or countries.</rdfs:comment>
	</owl:DatatypeProperty>
	<owl:DatatypeProperty rdf:ID="corpName__NS_corpName_UNType">
		<rdfs:label>corpName</rdfs:label>
	<rdfs:comment>(corporate name) – Identifies an organization or group of people that acts as a single entity.</rdfs:comment>
	</owl:DatatypeProperty>
	<owl:DatatypeProperty rdf:ID="country__NS_country_UNType">
		<rdfs:label>country</rdfs:label>
	<rdfs:comment>Contains the name of a geo-political unit, such as a nation, country, colony, or commonwealth, larger than or administratively superior to a region and smaller than a bloc.</rdfs:comment>
	</owl:DatatypeProperty>
	<owl:DatatypeProperty rdf:ID="district__NS_district_UNType">
		<rdfs:label>district</rdfs:label>
	<rdfs:comment>Contains the name of any kind of subdivision of a settlement, such as a parish, ward, or other administrative or geographic unit.</rdfs:comment>
	</owl:DatatypeProperty>
	<owl:DatatypeProperty rdf:ID="famName__NS_famName_UNType">
		<rdfs:label>famName</rdfs:label>
	<rdfs:comment>(family name) – Contains a family (inherited) name, as opposed to a given, baptismal, or nick name.</rdfs:comment>
	</owl:DatatypeProperty>
	<owl:DatatypeProperty rdf:ID="foreName__NS_foreName_UNType">
		<rdfs:label>foreName</rdfs:label>
	<rdfs:comment>Contains a forename, given or baptismal name.</rdfs:comment>
	</owl:DatatypeProperty>
	<owl:DatatypeProperty rdf:ID="genName__NS_genName_UNType">
		<rdfs:label>genName</rdfs:label>
	<rdfs:comment>(generational name component) – Contains a name component used to distinguish otherwise similar names on the basis of the relative ages or generations of the persons named.</rdfs:comment>
	</owl:DatatypeProperty>
	<owl:DatatypeProperty rdf:ID="geogFeat__NS_geogFeat_UNType">
		<rdfs:label>geogFeat</rdfs:label>
	<rdfs:comment>(geographical feature name) – Contains a common noun identifying a geographical feature.</rdfs:comment>
	</owl:DatatypeProperty>
	<owl:DatatypeProperty rdf:ID="geogName__NS_geogName_UNType">
		<rdfs:label>geogName</rdfs:label>
	<rdfs:comment>(geographic name) – The proper noun designation for a place, natural feature, or political jurisdiction.</rdfs:comment>
	</owl:DatatypeProperty>
	<owl:DatatypeProperty rdf:ID="nameLink__NS_nameLink_UNType">
		<rdfs:label>nameLink</rdfs:label>
	<rdfs:comment>(name link) – Contains a connecting phrase or link used within a name but not regarded as part of it, such as &quot;van der&quot; or &quot;of&quot;, &quot;from&quot;, etc.</rdfs:comment>
	</owl:DatatypeProperty>
	<owl:DatatypeProperty rdf:ID="periodName__NS_periodName_UNType">
		<rdfs:label>periodName</rdfs:label>
	<rdfs:comment>(period name) – A label that describes a period of time, such as 'Baroque' or '3rd Style period'.</rdfs:comment>
	</owl:DatatypeProperty>
	<owl:DatatypeProperty rdf:ID="persName__NS_persName_UNType">
		<rdfs:label>persName</rdfs:label>
	<rdfs:comment>(personal name) – Designation for an individual, including any or all of that individual's forenames, surnames, honorific titles, and added names.</rdfs:comment>
	</owl:DatatypeProperty>
	<owl:DatatypeProperty rdf:ID="postBox__NS_postBox_UNType">
		<rdfs:label>postBox</rdfs:label>
	<rdfs:comment>(postal box or post office box) contains a number or other identifier for some postal delivery point other than a street address.</rdfs:comment>
	</owl:DatatypeProperty>
	<owl:DatatypeProperty rdf:ID="postCode__NS_postCode_UNType">
		<rdfs:label>postCode</rdfs:label>
	<rdfs:comment>(postal code) contains a numerical or alphanumeric code used as part of a postal address to simplify sorting or delivery of mail.</rdfs:comment>
	</owl:DatatypeProperty>
	<owl:DatatypeProperty rdf:ID="region__NS_region_UNType">
		<rdfs:label>region</rdfs:label>
	<rdfs:comment>Contains the name of an administrative unit such as a state, province, or county, larger than a settlement, but smaller than a country.</rdfs:comment>
	</owl:DatatypeProperty>
	<owl:DatatypeProperty rdf:ID="roleName__NS_roleName_UNType">
		<rdfs:label>roleName</rdfs:label>
	<rdfs:comment>(role name) – Contains a name component which indicates that the referent has a particular role or position in society, such as an official title or rank.</rdfs:comment>
	</owl:DatatypeProperty>
	<owl:DatatypeProperty rdf:ID="settlement__NS_settlement_UNType">
		<rdfs:label>settlement</rdfs:label>
	<rdfs:comment>Contains the name of a settlement such as a city, town, or village identified as a single geo-political or administrative unit.</rdfs:comment>
	</owl:DatatypeProperty>
	<owl:DatatypeProperty rdf:ID="street__NS_street_UNType">
		<rdfs:label>street</rdfs:label>
	<rdfs:comment>full street address including any name or number identifying a building as well as the name of the street or route on which it is located.</rdfs:comment>
	</owl:DatatypeProperty>
	<owl:DatatypeProperty rdf:ID="styleName__NS_styleName_UNType">
		<rdfs:label>styleName</rdfs:label>
	<rdfs:comment>(style name) – A label for a characteristic style of writing or performance, such as 'bebop' or 'rock-n-roll'.</rdfs:comment>
	</owl:DatatypeProperty>
	<owl:DatatypeProperty rdf:ID="avFile__NS_avFile_UNType">
		<rdfs:label>avFile</rdfs:label>
	<rdfs:comment>(audio/video file) – References an external digital audio or video file.</rdfs:comment>
	</owl:DatatypeProperty>
	<owl:DatatypeProperty rdf:ID="clip__NS_clip_UNType">
		<rdfs:label>clip</rdfs:label>
	<rdfs:comment>Defines a time segment of interest within a recording or within a digital audio or video file.</rdfs:comment>
	</owl:DatatypeProperty>
	<owl:DatatypeProperty rdf:ID="performance__NS_performance_UNType">
		<rdfs:label>performance</rdfs:label>
	<rdfs:comment>A presentation of one or more musical works.</rdfs:comment>
	</owl:DatatypeProperty>
	<owl:DatatypeProperty rdf:ID="recording__NS_recording_UNType">
		<rdfs:label>recording</rdfs:label>
	<rdfs:comment>A recorded performance.</rdfs:comment>
	</owl:DatatypeProperty>
	<owl:DatatypeProperty rdf:ID="when__NS_when_UNType">
		<rdfs:label>when</rdfs:label>
	<rdfs:comment>Indicates a point in time either absolutely (using the absolute attribute), or relative to another when element (using the since, interval and inttype attributes).</rdfs:comment>
	</owl:DatatypeProperty>
	<owl:DatatypeProperty rdf:ID="ptr__NS_ptr_UNType">
		<rdfs:label>ptr</rdfs:label>
	<rdfs:comment>(pointer) – Defines a pointer to another location, using only attributes to describe the destination.</rdfs:comment>
	</owl:DatatypeProperty>
	<owl:DatatypeProperty rdf:ID="ref__NS_ref_UNType">
		<rdfs:label>ref</rdfs:label>
	<rdfs:comment>(reference) – Defines a reference to another location that may contain text and sub-elements to describe the destination.</rdfs:comment>
	</owl:DatatypeProperty>
	<owl:DatatypeProperty rdf:ID="back__NS_back_UNType">
		<rdfs:label>back</rdfs:label>
	<rdfs:comment>(back matter) – Contains any appendixes, advertisements, indexes, etc. following the main body of a musical text.</rdfs:comment>
	</owl:DatatypeProperty>
	<owl:DatatypeProperty rdf:ID="front__NS_front_UNType">
		<rdfs:label>front</rdfs:label>
	<rdfs:comment>(front matter) – Bundles prefatory text found before the start of the musical text.</rdfs:comment>
	</owl:DatatypeProperty>
	<owl:DatatypeProperty rdf:ID="l__NS_l_UNType">
		<rdfs:label>l</rdfs:label>
	<rdfs:comment>(line of text) – Contains a single line of text within a line group.</rdfs:comment>
	</owl:DatatypeProperty>
	<owl:DatatypeProperty rdf:ID="lg__NS_lg_UNType">
		<rdfs:label>lg</rdfs:label>
	<rdfs:comment>(line group) – May be used for any section of text that is organized as a group of lines; however, it is most often used for a group of verse lines functioning as a formal unit, e.g. a stanza, refrain, verse paragraph, etc.</rdfs:comment>
	</owl:DatatypeProperty>
	<owl:DatatypeProperty rdf:ID="li__NS_li_UNType">
		<rdfs:label>li</rdfs:label>
	<rdfs:comment>(list item) – Single item in a &lt;list&gt;.</rdfs:comment>
	</owl:DatatypeProperty>
	<owl:DatatypeProperty rdf:ID="list__NS_list_UNType">
		<rdfs:label>list</rdfs:label>
	<rdfs:comment>A formatting element that contains a series of items separated from one another and arranged in a linear, often vertical, sequence.</rdfs:comment>
	</owl:DatatypeProperty>
	<owl:DatatypeProperty rdf:ID="quote__NS_quote_UNType">
		<rdfs:label>quote</rdfs:label>
	<rdfs:comment>(block quote) – A formatting element that designates an extended quotation; that is, a passage attributed to a source external to the text and normally set off from the text by spacing or other typographic distinction.</rdfs:comment>
	</owl:DatatypeProperty>
	<owl:DatatypeProperty rdf:ID="anchoredText__NS_anchoredText_UNType">
		<rdfs:label>anchoredText</rdfs:label>
	<rdfs:comment>Container for text that is fixed to a particular page location, regardless of changes made to the layout of the measures around it.</rdfs:comment>
	</owl:DatatypeProperty>
	<owl:DatatypeProperty rdf:ID="curve__NS_curve_UNType">
		<rdfs:label>curve</rdfs:label>
	<rdfs:comment>A curved line that cannot be represented by a more specific element, such as a slur.</rdfs:comment>
	</owl:DatatypeProperty>
	<owl:DatatypeProperty rdf:ID="line__NS_line_UNType">
		<rdfs:label>line</rdfs:label>
	<rdfs:comment>A visual line that cannot be represented by a more specific; i.e., semantic, element.</rdfs:comment>
	</owl:DatatypeProperty>
	<owl:DatatypeProperty rdf:ID="mapping__NS_mapping_UNType">
		<rdfs:label>mapping</rdfs:label>
	<rdfs:comment>One or more characters which are related to the parent symbol in some respect, as specified by the type attribute.</rdfs:comment>
	</owl:DatatypeProperty>
	<owl:DatatypeProperty rdf:ID="propName__NS_propName_UNType">
		<rdfs:label>propName</rdfs:label>
	<rdfs:comment>(property name) – Name of a property of the symbol.</rdfs:comment>
	</owl:DatatypeProperty>
	<owl:DatatypeProperty rdf:ID="propValue__NS_propValue_UNType">
		<rdfs:label>propValue</rdfs:label>
	<rdfs:comment>(property value) – A single property value.</rdfs:comment>
	</owl:DatatypeProperty>
	<owl:DatatypeProperty rdf:ID="symbol__NS_symbol_UNType">
		<rdfs:label>symbol</rdfs:label>
	<rdfs:comment>A reference to a previously defined symbol.</rdfs:comment>
	</owl:DatatypeProperty>
	<owl:DatatypeProperty rdf:ID="symbolDef__NS_symbolDef_UNType">
		<rdfs:label>symbolDef</rdfs:label>
	<rdfs:comment>(symbol definition) – Declaration of an individual symbol in a symbolTable.</rdfs:comment>
	</owl:DatatypeProperty>
	<owl:DatatypeProperty rdf:ID="symName__NS_symName_UNType">
		<rdfs:label>symName</rdfs:label>
	<rdfs:comment>(symbol name) – Contains the name of a symbol, expressed following Unicode conventions.</rdfs:comment>
	</owl:DatatypeProperty>
	<owl:DatatypeProperty rdf:ID="symProp__NS_symProp_UNType">
		<rdfs:label>symProp</rdfs:label>
	<rdfs:comment>(symbol property) – Provides a name and value for some property of the parent symbol.</rdfs:comment>
	</owl:DatatypeProperty>
	<owl:DatatypeProperty rdf:ID="symbolTable__NS_symbolTable_UNType">
		<rdfs:label>symbolTable</rdfs:label>
	<rdfs:comment>Contains a set of user-defined symbols.</rdfs:comment>
	</owl:DatatypeProperty>
	<owl:DatatypeProperty rdf:ID="vecTrans__NS_vecTrans_UNType">
		<rdfs:label>vecTrans</rdfs:label>
	<rdfs:comment>Encodes Vector Transcoding of Musical Measures for Modal Monodies</rdfs:comment>
	</owl:DatatypeProperty>
	<owl:DatatypeProperty rdf:ID="mrmr__NS_mrmr_UNType">
		<rdfs:label>mrmr</rdfs:label>
	<rdfs:comment>Encodes the Morphophonological Rythmic and Melodic Rewriting of a musical Sequence</rdfs:comment>
	</owl:DatatypeProperty>
	<owl:DatatypeProperty rdf:ID="phonoRealization__NS_phonoRealization_UNType">
		<rdfs:label>phonoRealization</rdfs:label>
	<rdfs:comment>Encodes the Phonological Realization of a Musical Sequence</rdfs:comment>
	</owl:DatatypeProperty>
	<owl:DatatypeProperty rdf:ID="notationtype_att.notationtype.attribute.notationtype__mei_data.NOTATIONTYPE">
		<rdfs:range rdf:resource="&datatypes;data.NOTATIONTYPE"/>
		<rdfs:label>notationtype</rdfs:label>
	<rdfs:comment>Contains classification of the notation contained or described by the element bearing this attribute.</rdfs:comment>
	</owl:DatatypeProperty>
	<owl:DatatypeProperty rdf:ID="notationsubtype_att.notationtype.attribute.notationsubtype__xs_NMTOKEN">
		<rdfs:range rdf:resource="&xs;NMTOKEN"/>
		<rdfs:label>notationsubtype</rdfs:label>
	<rdfs:comment>Provides any sub-classification of the notation contained or described by the element, additional to that given by its notationtype attribute.</rdfs:comment>
	</owl:DatatypeProperty>
	<rdfs:Datatype rdf:ID="NS_func_att.accid.log.attribute.func_UNType">
		<owl:equivalentClass><rdfs:Datatype>
		<owl:onDatatype rdf:resource="&xs;token"/><owl:withRestrictions rdf:parseType="Collection"><rdf:Description><xs:enumeration>caution</xs:enumeration></rdf:Description><rdf:Description><xs:enumeration>edit</xs:enumeration></rdf:Description></owl:withRestrictions></rdfs:Datatype></owl:equivalentClass></rdfs:Datatype>
	<owl:DatatypeProperty rdf:ID="func_att.accid.log.attribute.func__NS_func_att.accid.log.attribute.func_UNType">
		<rdfs:range rdf:resource="#NS_func_att.accid.log.attribute.func_UNType"/>
		<rdfs:label>func</rdfs:label>
	<rdfs:comment>Records the function of an accidental.</rdfs:comment>
	</owl:DatatypeProperty>
	<owl:DatatypeProperty rdf:ID="accid_att.accidental.attribute.accid__mei_data.ACCIDENTAL.EXPLICIT">
		<rdfs:range rdf:resource="&datatypes;data.ACCIDENTAL.EXPLICIT"/>
		<rdfs:label>accid</rdfs:label>
	<rdfs:comment>Captures a written accidental.</rdfs:comment>
	</owl:DatatypeProperty>
	<owl:DatatypeProperty rdf:ID="accid.ges_att.accidental.performed.attribute.accid.ges__mei_data.ACCIDENTAL.IMPLICIT">
		<rdfs:range rdf:resource="&datatypes;data.ACCIDENTAL.IMPLICIT"/>
		<rdfs:label>accid.ges</rdfs:label>
	<rdfs:comment>Records the performed pitch inflection.</rdfs:comment>
	</owl:DatatypeProperty>
	<rdfs:Datatype rdf:ID="NS_artic_att.articulation.attribute.artic_UNType">
		<owl:equivalentClass><rdfs:Datatype>
		<owl:onDatatype rdf:resource="artic_att.articulation.attribute.artic_NS_artic_att.articulation.attribute.artic_UNType_UNType"/><owl:withRestrictions rdf:parseType="Collection"><rdf:Description><xs:minLength>1</xs:minLength></rdf:Description></owl:withRestrictions></rdfs:Datatype></owl:equivalentClass></rdfs:Datatype>
	<rdfs:Datatype rdf:ID="artic_att.articulation.attribute.artic_NS_artic_att.articulation.attribute.artic_UNType_UNType">
		<owl:equivalentClass><rdfs:Datatype>
		<owl:oneOf><rdf:Description><rdf:type rdf:resource="#List"/><rdf:first>mei:data.ARTICULATION</rdf:first><rdf:rest rdf:resource="#nil"/></rdf:Description></owl:oneOf></rdfs:Datatype></owl:equivalentClass></rdfs:Datatype>
	<owl:DatatypeProperty rdf:ID="artic_att.articulation.attribute.artic__NS_artic_att.articulation.attribute.artic_UNType">
		<rdfs:range rdf:resource="#NS_artic_att.articulation.attribute.artic_UNType"/>
		<rdfs:label>artic</rdfs:label>
	<rdfs:comment>Encodes the written articulation(s). Articulations are normally encoded in order from the note head outward; that is, away from the stem. See additional notes at att.vis.note. Only articulations should be encoded in the artic attribute; for example, fingerings should be encoded using the &lt;fingering&gt; element.</rdfs:comment>
	</owl:DatatypeProperty>
	<rdfs:Datatype rdf:ID="NS_artic.ges_att.articulation.performed.attribute.artic.ges_UNType">
		<owl:equivalentClass><rdfs:Datatype>
		<owl:onDatatype rdf:resource="artic.ges_att.articulation.performed.attribute.artic.ges_NS_artic.ges_att.articulation.performed.attribute.artic.ges_UNType_UNType"/><owl:withRestrictions rdf:parseType="Collection"><rdf:Description><xs:minLength>1</xs:minLength></rdf:Description></owl:withRestrictions></rdfs:Datatype></owl:equivalentClass></rdfs:Datatype>
	<rdfs:Datatype rdf:ID="artic.ges_att.articulation.performed.attribute.artic.ges_NS_artic.ges_att.articulation.performed.attribute.artic.ges_UNType_UNType">
		<owl:equivalentClass><rdfs:Datatype>
		<owl:oneOf><rdf:Description><rdf:type rdf:resource="#List"/><rdf:first>mei:data.ARTICULATION</rdf:first><rdf:rest rdf:resource="#nil"/></rdf:Description></owl:oneOf></rdfs:Datatype></owl:equivalentClass></rdfs:Datatype>
	<owl:DatatypeProperty rdf:ID="artic.ges_att.articulation.performed.attribute.artic.ges__NS_artic.ges_att.articulation.performed.attribute.artic.ges_UNType">
		<rdfs:range rdf:resource="#NS_artic.ges_att.articulation.performed.attribute.artic.ges_UNType"/>
		<rdfs:label>artic.ges</rdfs:label>
	<rdfs:comment>Records performed articulation that differs from the written value.</rdfs:comment>
	</owl:DatatypeProperty>
	<owl:DatatypeProperty rdf:ID="dots_att.augmentdots.attribute.dots__mei_data.AUGMENTDOT">
		<rdfs:range rdf:resource="&datatypes;data.AUGMENTDOT"/>
		<rdfs:label>dots</rdfs:label>
	<rdfs:comment>Records the number of augmentation dots required by a dotted duration.</rdfs:comment>
	</owl:DatatypeProperty>
	<owl:DatatypeProperty rdf:ID="authority_att.authorized.attribute.authority__xs_string">
		<rdfs:range rdf:resource="&xs;string"/>
		<rdfs:label>authority</rdfs:label>
	<rdfs:comment>A name or label associated with the controlled vocabulary from which the value is taken.</rdfs:comment>
	</owl:DatatypeProperty>
	<owl:DatatypeProperty rdf:ID="authURI_att.authorized.attribute.authURI__mei_data.URI">
		<rdfs:range rdf:resource="&datatypes;data.URI"/>
		<rdfs:label>authURI</rdfs:label>
	<rdfs:comment>The web-accessible location of the controlled vocabulary from which the value is taken.</rdfs:comment>
	</owl:DatatypeProperty>
	<owl:DatatypeProperty rdf:ID="form_att.barLine.log.attribute.form__mei_data.BARRENDITION">
		<rdfs:range rdf:resource="&datatypes;data.BARRENDITION"/>
		<rdfs:label>form</rdfs:label>
	<rdfs:comment>Records the appearance and usually the function of the bar line.</rdfs:comment>
	</owl:DatatypeProperty>
	<owl:DatatypeProperty rdf:ID="barplace_att.barplacement.attribute.barplace__mei_data.BARPLACE">
		<rdfs:range rdf:resource="&datatypes;data.BARPLACE"/>
		<rdfs:label>barplace</rdfs:label>
	<rdfs:comment>Records the location of a bar line.</rdfs:comment>
	</owl:DatatypeProperty>
	<owl:DatatypeProperty rdf:ID="taktplace_att.barplacement.attribute.taktplace__mei_data.STAFFLOC">
		<rdfs:range rdf:resource="&datatypes;data.STAFFLOC"/>
		<rdfs:label>taktplace</rdfs:label>
	<rdfs:comment>If takt bar lines are to be used, then the taktplace attribute may be used to denote the staff location of the shortened bar line. The location may include staff lines, spaces, and the spaces directly above and below the staff. The value ranges between 0 (just below the staff) to 2 * number of staff lines (directly above the staff). For example, on a 5-line staff the lines would be numbered 1,3,5,7, and 9 while the spaces would be numbered 0,2,4,6,8,10. For example, a value of '9' puts the bar line through the top line of a 5-line staff.</rdfs:comment>
	</owl:DatatypeProperty>
	<owl:DatatypeProperty rdf:ID="beam.color_att.beaming.vis.attribute.beam.color__mei_data.COLOR">
		<rdfs:range rdf:resource="&datatypes;data.COLOR"/>
		<rdfs:label>beam.color</rdfs:label>
	<rdfs:comment>Color of beams, including those associated with tuplets.</rdfs:comment>
	</owl:DatatypeProperty>
	<rdfs:Datatype rdf:ID="NS_beam.rend_att.beaming.vis.attribute.beam.rend_UNType">
		<owl:equivalentClass><rdfs:Datatype>
		<owl:onDatatype rdf:resource="&xs;token"/><owl:withRestrictions rdf:parseType="Collection"><rdf:Description><xs:enumeration>acc</xs:enumeration></rdf:Description><rdf:Description><xs:enumeration>rit</xs:enumeration></rdf:Description><rdf:Description><xs:enumeration>norm</xs:enumeration></rdf:Description></owl:withRestrictions></rdfs:Datatype></owl:equivalentClass></rdfs:Datatype>
	<owl:DatatypeProperty rdf:ID="beam.rend_att.beaming.vis.attribute.beam.rend__NS_beam.rend_att.beaming.vis.attribute.beam.rend_UNType">
		<rdfs:range rdf:resource="#NS_beam.rend_att.beaming.vis.attribute.beam.rend_UNType"/>
		<rdfs:label>beam.rend</rdfs:label>
	<rdfs:comment>Encodes whether a beam is &quot;feathered&quot; and in which direction.</rdfs:comment>
	</owl:DatatypeProperty>
	<owl:DatatypeProperty rdf:ID="beam.slope_att.beaming.vis.attribute.beam.slope__xs_decimal">
		<rdfs:range rdf:resource="&xs;decimal"/>
		<rdfs:label>beam.slope</rdfs:label>
	<rdfs:comment>Captures beam slope.</rdfs:comment>
	</owl:DatatypeProperty>
	<owl:DatatypeProperty rdf:ID="analog_att.bibl.attribute.analog__xs_string">
		<rdfs:range rdf:resource="&xs;string"/>
		<rdfs:label>analog</rdfs:label>
	<rdfs:comment>Contains a reference to a field or element in another descriptive encoding system to which this MEI element is comparable.</rdfs:comment>
	</owl:DatatypeProperty>
	<owl:DatatypeProperty rdf:ID="calendar_att.calendared.attribute.calendar__xs_NMTOKEN">
		<rdfs:range rdf:resource="&xs;NMTOKEN"/>
		<rdfs:label>calendar</rdfs:label>
	<rdfs:comment>Indicates the calendar system to which a date belongs, for example, Gregorian, Julian, Roman, Mosaic, Revolutionary, Islamic, etc.</rdfs:comment>
	</owl:DatatypeProperty>
	<rdfs:Datatype rdf:ID="NS_codedval_att.canonical.attribute.codedval_UNType">
		<owl:equivalentClass><rdfs:Datatype>
		<owl:onDatatype rdf:resource="codedval_att.canonical.attribute.codedval_NS_codedval_att.canonical.attribute.codedval_UNType_UNType"/><owl:withRestrictions rdf:parseType="Collection"><rdf:Description><xs:minLength>1</xs:minLength></rdf:Description></owl:withRestrictions></rdfs:Datatype></owl:equivalentClass></rdfs:Datatype>
	<rdfs:Datatype rdf:ID="codedval_att.canonical.attribute.codedval_NS_codedval_att.canonical.attribute.codedval_UNType_UNType">
		<owl:equivalentClass><rdfs:Datatype>
		<owl:oneOf><rdf:Description><rdf:type rdf:resource="#List"/><rdf:first>xs:NMTOKEN</rdf:first><rdf:rest rdf:resource="#nil"/></rdf:Description></owl:oneOf></rdfs:Datatype></owl:equivalentClass></rdfs:Datatype>
	<owl:DatatypeProperty rdf:ID="codedval_att.canonical.attribute.codedval__NS_codedval_att.canonical.attribute.codedval_UNType">
		<rdfs:range rdf:resource="#NS_codedval_att.canonical.attribute.codedval_UNType"/>
		<rdfs:label>codedval</rdfs:label>
	<rdfs:comment>a value that represents or identifies the element content. May serve as a primary key in a web-accessible database identified by the authURI attribute.</rdfs:comment>
	</owl:DatatypeProperty>
	<owl:DatatypeProperty rdf:ID="cluster_att.chord.vis.attribute.cluster__mei_data.CLUSTER">
		<rdfs:range rdf:resource="&datatypes;data.CLUSTER"/>
		<rdfs:label>cluster</rdfs:label>
	<rdfs:comment>Indicates a single, alternative note head should be displayed instead of individual note heads. The highest and lowest notes of the chord usually indicate the upper and lower boundaries of the cluster note head.</rdfs:comment>
	</owl:DatatypeProperty>
	<owl:DatatypeProperty rdf:ID="classcode_att.classcodeident.attribute.classcode__mei_data.URI">
		<rdfs:range rdf:resource="&datatypes;data.URI"/>
		<rdfs:label>classcode</rdfs:label>
	<rdfs:comment>Contains a reference to the controlled vocabulary from which the term is drawn. The value must match the value of an ID attribute on a classCode element given elsewhere in the document.</rdfs:comment>
	</owl:DatatypeProperty>
	<owl:DatatypeProperty rdf:ID="cautionary_att.clef.log.attribute.cautionary__mei_data.BOOLEAN">
		<rdfs:range rdf:resource="&datatypes;data.BOOLEAN"/>
		<rdfs:label>cautionary</rdfs:label>
	<rdfs:comment>Records the function of the clef. A &quot;cautionary&quot; clef does not change the following pitches.</rdfs:comment>
	</owl:DatatypeProperty>
	<owl:DatatypeProperty rdf:ID="clef.shape_att.cleffing.log.attribute.clef.shape__mei_data.CLEFSHAPE">
		<rdfs:range rdf:resource="&datatypes;data.CLEFSHAPE"/>
		<rdfs:label>clef.shape</rdfs:label>
	<rdfs:comment>Encodes a value for the clef symbol.</rdfs:comment>
	</owl:DatatypeProperty>
	<owl:DatatypeProperty rdf:ID="clef.line_att.cleffing.log.attribute.clef.line__mei_data.CLEFLINE">
		<rdfs:range rdf:resource="&datatypes;data.CLEFLINE"/>
		<rdfs:label>clef.line</rdfs:label>
	<rdfs:comment>Contains a default value for the position of the clef. The value must be in the range between 1 and the number of lines on the staff. The numbering of lines starts with the lowest line of the staff.</rdfs:comment>
	</owl:DatatypeProperty>
	<owl:DatatypeProperty rdf:ID="clef.dis_att.cleffing.log.attribute.clef.dis__mei_data.OCTAVE.DIS">
		<rdfs:range rdf:resource="&datatypes;data.OCTAVE.DIS"/>
		<rdfs:label>clef.dis</rdfs:label>
	<rdfs:comment>Records the amount of octave displacement to be applied to the clef.</rdfs:comment>
	</owl:DatatypeProperty>
	<owl:DatatypeProperty rdf:ID="clef.dis.place_att.cleffing.log.attribute.clef.dis.place__mei_data.PLACE">
		<rdfs:range rdf:resource="&datatypes;data.PLACE"/>
		<rdfs:label>clef.dis.place</rdfs:label>
	<rdfs:comment>Records the direction of octave displacement to be applied to the clef.</rdfs:comment>
	</owl:DatatypeProperty>
	<owl:DatatypeProperty rdf:ID="clef.color_att.cleffing.vis.attribute.clef.color__mei_data.COLOR">
		<rdfs:range rdf:resource="&datatypes;data.COLOR"/>
		<rdfs:label>clef.color</rdfs:label>
	<rdfs:comment>Describes the color of the clef.</rdfs:comment>
	</owl:DatatypeProperty>
	<owl:DatatypeProperty rdf:ID="clef.visible_att.cleffing.vis.attribute.clef.visible__mei_data.BOOLEAN">
		<rdfs:range rdf:resource="&datatypes;data.BOOLEAN"/>
		<rdfs:label>clef.visible</rdfs:label>
	<rdfs:comment>Determines whether the clef is to be displayed.</rdfs:comment>
	</owl:DatatypeProperty>
	<owl:DatatypeProperty rdf:ID="shape_att.clefshape.attribute.shape__mei_data.CLEFSHAPE">
		<rdfs:range rdf:resource="&datatypes;data.CLEFSHAPE"/>
		<rdfs:label>shape</rdfs:label>
	<rdfs:comment>Describes a clef's shape.</rdfs:comment>
	</owl:DatatypeProperty>
	<owl:DatatypeProperty rdf:ID="color_att.color.attribute.color__mei_data.COLOR">
		<rdfs:range rdf:resource="&datatypes;data.COLOR"/>
		<rdfs:label>color</rdfs:label>
	<rdfs:comment>Used to indicate visual appearance. Do not confuse this with the musical term 'color' as used in pre-CMN notation.</rdfs:comment>
	</owl:DatatypeProperty>
	<owl:DatatypeProperty rdf:ID="colored_att.coloration.attribute.colored__mei_data.BOOLEAN">
		<rdfs:range rdf:resource="&datatypes;data.BOOLEAN"/>
		<rdfs:label>colored</rdfs:label>
	<rdfs:comment>Indicates this feature is 'colored'; that is, it is a participant in a change in rhythmic values. In mensural notation, coloration is indicated by colored notes (red, black, etc.) where void notes would otherwise occur. In CMN, coloration is indicated by an inverse color; that is, the note head is void when it would otherwise be filled and vice versa.</rdfs:comment>
	</owl:DatatypeProperty>
	<owl:DatatypeProperty rdf:ID="n_att.common.attribute.n__">
		<rdfs:label>n</rdfs:label>
	<rdfs:comment>Provides a number-like designation for an element.</rdfs:comment>
	</owl:DatatypeProperty>
	<owl:DatatypeProperty rdf:ID="label_att.commonPart.attribute.label__xs_string">
		<rdfs:range rdf:resource="&xs;string"/>
		<rdfs:label>label</rdfs:label>
	<rdfs:comment>Provides a name or label for an element. The value may be any string.</rdfs:comment>
	</owl:DatatypeProperty>
	<owl:DatatypeProperty rdf:ID="ulx_att.coordinated.attribute.ulx__xs_nonNegativeInteger">
		<rdfs:range rdf:resource="&xs;nonNegativeInteger"/>
		<rdfs:label>ulx</rdfs:label>
	<rdfs:comment>Indicates the upper-left corner x coordinate.</rdfs:comment>
	</owl:DatatypeProperty>
	<owl:DatatypeProperty rdf:ID="uly_att.coordinated.attribute.uly__xs_nonNegativeInteger">
		<rdfs:range rdf:resource="&xs;nonNegativeInteger"/>
		<rdfs:label>uly</rdfs:label>
	<rdfs:comment>Indicates the upper-left corner y coordinate.</rdfs:comment>
	</owl:DatatypeProperty>
	<owl:DatatypeProperty rdf:ID="lrx_att.coordinated.attribute.lrx__xs_nonNegativeInteger">
		<rdfs:range rdf:resource="&xs;nonNegativeInteger"/>
		<rdfs:label>lrx</rdfs:label>
	<rdfs:comment>Indicates the lower-right corner x coordinate.</rdfs:comment>
	</owl:DatatypeProperty>
	<owl:DatatypeProperty rdf:ID="lry_att.coordinated.attribute.lry__xs_nonNegativeInteger">
		<rdfs:range rdf:resource="&xs;nonNegativeInteger"/>
		<rdfs:label>lry</rdfs:label>
	<rdfs:comment>Indicates the lower-left corner x coordinate.</rdfs:comment>
	</owl:DatatypeProperty>
	<rdfs:Datatype rdf:ID="NS_bezier_att.curvature.attribute.bezier_UNType">
		<owl:equivalentClass><rdfs:Datatype>
		<owl:onDatatype rdf:resource="bezier_att.curvature.attribute.bezier_NS_bezier_att.curvature.attribute.bezier_UNType_UNType"/><owl:withRestrictions rdf:parseType="Collection"><rdf:Description><xs:minLength>2</xs:minLength></rdf:Description></owl:withRestrictions></rdfs:Datatype></owl:equivalentClass></rdfs:Datatype>
	<rdfs:Datatype rdf:ID="bezier_att.curvature.attribute.bezier_NS_bezier_att.curvature.attribute.bezier_UNType_UNType">
		<owl:equivalentClass><rdfs:Datatype>
		<owl:oneOf><rdf:Description><rdf:type rdf:resource="#List"/><rdf:first>NS_bezier_att.curvature.attribute.bezier_UNType_bezier_att.curvature.attribute.bezier_NS_bezier_att.curvature.attribute.bezier_UNType_UNType_UNType</rdf:first><rdf:rest rdf:resource="#nil"/></rdf:Description></owl:oneOf></rdfs:Datatype></owl:equivalentClass></rdfs:Datatype>
	<rdfs:Datatype rdf:ID="NS_bezier_att.curvature.attribute.bezier_UNType_bezier_att.curvature.attribute.bezier_NS_bezier_att.curvature.attribute.bezier_UNType_UNType_UNType">
		<owl:equivalentClass><rdfs:Datatype>
		<owl:unionOf rdf:parseType="Collection"><rdf:Description rdf:about="xs:decimal"/><rdf:Description rdf:about="xs:decimal"/></owl:unionOf></rdfs:Datatype></owl:equivalentClass></rdfs:Datatype>
	<owl:DatatypeProperty rdf:ID="bezier_att.curvature.attribute.bezier__NS_bezier_att.curvature.attribute.bezier_UNType">
		<rdfs:range rdf:resource="#NS_bezier_att.curvature.attribute.bezier_UNType"/>
		<rdfs:label>bezier</rdfs:label>
	<rdfs:comment>Records the placement of Bezier control points as a series of pairs of space-separated values; e.g., 19 45 -32 118.</rdfs:comment>
	</owl:DatatypeProperty>
	<rdfs:Datatype rdf:ID="NS_bulge_att.curvature.attribute.bulge_UNType">
		<owl:equivalentClass><rdfs:Datatype>
		<owl:onDatatype rdf:resource="bulge_att.curvature.attribute.bulge_NS_bulge_att.curvature.attribute.bulge_UNType_UNType"/><owl:withRestrictions rdf:parseType="Collection"><rdf:Description><xs:minLength>2</xs:minLength></rdf:Description></owl:withRestrictions></rdfs:Datatype></owl:equivalentClass></rdfs:Datatype>
	<rdfs:Datatype rdf:ID="bulge_att.curvature.attribute.bulge_NS_bulge_att.curvature.attribute.bulge_UNType_UNType">
		<owl:equivalentClass><rdfs:Datatype>
		<owl:oneOf><rdf:Description><rdf:type rdf:resource="#List"/><rdf:first>NS_bulge_att.curvature.attribute.bulge_UNType_bulge_att.curvature.attribute.bulge_NS_bulge_att.curvature.attribute.bulge_UNType_UNType_UNType</rdf:first><rdf:rest rdf:resource="#nil"/></rdf:Description></owl:oneOf></rdfs:Datatype></owl:equivalentClass></rdfs:Datatype>
	<rdfs:Datatype rdf:ID="NS_bulge_att.curvature.attribute.bulge_UNType_bulge_att.curvature.attribute.bulge_NS_bulge_att.curvature.attribute.bulge_UNType_UNType_UNType">
		<owl:equivalentClass><rdfs:Datatype>
		<owl:unionOf rdf:parseType="Collection"><rdf:Description rdf:about="xs:decimal"/><rdf:Description rdf:about="mei:data.PERCENT"/></owl:unionOf></rdfs:Datatype></owl:equivalentClass></rdfs:Datatype>
	<owl:DatatypeProperty rdf:ID="bulge_att.curvature.attribute.bulge__NS_bulge_att.curvature.attribute.bulge_UNType">
		<rdfs:range rdf:resource="#NS_bulge_att.curvature.attribute.bulge_UNType"/>
		<rdfs:label>bulge</rdfs:label>
	<rdfs:comment>Describes a curve as one or more pairs of values with respect to an imaginary line connecting the starting and ending points of the curve. The first value captures a distance to the left (positive value) or right (negative value) of the line, expressed in virtual units. The second value of each pair represents a point along the line, expressed as a percentage of the line's length. N.B. An MEI virtual unit (VU) is half the distance between adjacent staff lines.</rdfs:comment>
	</owl:DatatypeProperty>
	<rdfs:Datatype rdf:ID="NS_curvedir_att.curvature.attribute.curvedir_UNType">
		<owl:equivalentClass><rdfs:Datatype>
		<owl:onDatatype rdf:resource="&xs;token"/><owl:withRestrictions rdf:parseType="Collection"><rdf:Description><xs:enumeration>above</xs:enumeration></rdf:Description><rdf:Description><xs:enumeration>below</xs:enumeration></rdf:Description><rdf:Description><xs:enumeration>mixed</xs:enumeration></rdf:Description></owl:withRestrictions></rdfs:Datatype></owl:equivalentClass></rdfs:Datatype>
	<owl:DatatypeProperty rdf:ID="curvedir_att.curvature.attribute.curvedir__NS_curvedir_att.curvature.attribute.curvedir_UNType">
		<rdfs:range rdf:resource="#NS_curvedir_att.curvature.attribute.curvedir_UNType"/>
		<rdfs:label>curvedir</rdfs:label>
	<rdfs:comment>Describes a curve with a generic term indicating the direction of curvature.</rdfs:comment>
	</owl:DatatypeProperty>
	<owl:DatatypeProperty rdf:ID="lform_att.curverend.attribute.lform__mei_data.LINEFORM">
		<rdfs:range rdf:resource="&datatypes;data.LINEFORM"/>
		<rdfs:label>lform</rdfs:label>
	<rdfs:comment>Describes the line style of a curve.</rdfs:comment>
	</owl:DatatypeProperty>
	<owl:DatatypeProperty rdf:ID="lwidth_att.curverend.attribute.lwidth__mei_data.LINEWIDTH">
		<rdfs:range rdf:resource="&datatypes;data.LINEWIDTH"/>
		<rdfs:label>lwidth</rdfs:label>
	<rdfs:comment>Width of a curved line.</rdfs:comment>
	</owl:DatatypeProperty>
	<owl:DatatypeProperty rdf:ID="target_att.custos.log.attribute.target__mei_data.URI">
		<rdfs:range rdf:resource="&datatypes;data.URI"/>
		<rdfs:label>target</rdfs:label>
	<rdfs:comment>Encodes the target note when its pitch differs from the pitch at which the custos appears.</rdfs:comment>
	</owl:DatatypeProperty>
	<owl:DatatypeProperty rdf:ID="enddate_att.datable.attribute.enddate__mei_data.ISODATE">
		<rdfs:range rdf:resource="&datatypes;data.ISODATE"/>
		<rdfs:label>enddate</rdfs:label>
	<rdfs:comment>Contains the end point of a date range in standard ISO form.</rdfs:comment>
	</owl:DatatypeProperty>
	<owl:DatatypeProperty rdf:ID="isodate_att.datable.attribute.isodate__mei_data.ISODATE">
		<rdfs:range rdf:resource="&datatypes;data.ISODATE"/>
		<rdfs:label>isodate</rdfs:label>
	<rdfs:comment>Provides the value of a textual date in standard ISO form.</rdfs:comment>
	</owl:DatatypeProperty>
	<owl:DatatypeProperty rdf:ID="notafter_att.datable.attribute.notafter__mei_data.ISODATE">
		<rdfs:range rdf:resource="&datatypes;data.ISODATE"/>
		<rdfs:label>notafter</rdfs:label>
	<rdfs:comment>Contains an upper boundary for an uncertain date in standard ISO form.</rdfs:comment>
	</owl:DatatypeProperty>
	<owl:DatatypeProperty rdf:ID="notbefore_att.datable.attribute.notbefore__mei_data.ISODATE">
		<rdfs:range rdf:resource="&datatypes;data.ISODATE"/>
		<rdfs:label>notbefore</rdfs:label>
	<rdfs:comment>Contains a lower boundary, in standard ISO form, for an uncertain date.</rdfs:comment>
	</owl:DatatypeProperty>
	<owl:DatatypeProperty rdf:ID="startdate_att.datable.attribute.startdate__mei_data.ISODATE">
		<rdfs:range rdf:resource="&datatypes;data.ISODATE"/>
		<rdfs:label>startdate</rdfs:label>
	<rdfs:comment>Contains the starting point of a date range in standard ISO form.</rdfs:comment>
	</owl:DatatypeProperty>
	<rdfs:Datatype rdf:ID="NS_data_att.datapointing.attribute.data_UNType">
		<owl:equivalentClass><rdfs:Datatype>
		<owl:onDatatype rdf:resource="data_att.datapointing.attribute.data_NS_data_att.datapointing.attribute.data_UNType_UNType"/><owl:withRestrictions rdf:parseType="Collection"><rdf:Description><xs:minLength>1</xs:minLength></rdf:Description></owl:withRestrictions></rdfs:Datatype></owl:equivalentClass></rdfs:Datatype>
	<rdfs:Datatype rdf:ID="data_att.datapointing.attribute.data_NS_data_att.datapointing.attribute.data_UNType_UNType">
		<owl:equivalentClass><rdfs:Datatype>
		<owl:oneOf><rdf:Description><rdf:type rdf:resource="#List"/><rdf:first>mei:data.URI</rdf:first><rdf:rest rdf:resource="#nil"/></rdf:Description></owl:oneOf></rdfs:Datatype></owl:equivalentClass></rdfs:Datatype>
	<owl:DatatypeProperty rdf:ID="data_att.datapointing.attribute.data__NS_data_att.datapointing.attribute.data_UNType">
		<rdfs:range rdf:resource="#NS_data_att.datapointing.attribute.data_UNType"/>
		<rdfs:label>data</rdfs:label>
	<rdfs:comment>Used to link metadata elements to one or more data-containing elements.</rdfs:comment>
	</owl:DatatypeProperty>
	<rdfs:Datatype rdf:ID="NS_decls_att.declaring.attribute.decls_UNType">
		<owl:equivalentClass><rdfs:Datatype>
		<owl:onDatatype rdf:resource="decls_att.declaring.attribute.decls_NS_decls_att.declaring.attribute.decls_UNType_UNType"/><owl:withRestrictions rdf:parseType="Collection"><rdf:Description><xs:minLength>1</xs:minLength></rdf:Description></owl:withRestrictions></rdfs:Datatype></owl:equivalentClass></rdfs:Datatype>
	<rdfs:Datatype rdf:ID="decls_att.declaring.attribute.decls_NS_decls_att.declaring.attribute.decls_UNType_UNType">
		<owl:equivalentClass><rdfs:Datatype>
		<owl:oneOf><rdf:Description><rdf:type rdf:resource="#List"/><rdf:first>mei:data.URI</rdf:first><rdf:rest rdf:resource="#nil"/></rdf:Description></owl:oneOf></rdfs:Datatype></owl:equivalentClass></rdfs:Datatype>
	<owl:DatatypeProperty rdf:ID="decls_att.declaring.attribute.decls__NS_decls_att.declaring.attribute.decls_UNType">
		<rdfs:range rdf:resource="#NS_decls_att.declaring.attribute.decls_UNType"/>
		<rdfs:label>decls</rdfs:label>
	<rdfs:comment>Identifies one or more metadata elements within the header, which are understood to apply to the element bearing this attribute and its content.</rdfs:comment>
	</owl:DatatypeProperty>
	<owl:DatatypeProperty rdf:ID="dynam.dist_att.distances.attribute.dynam.dist__mei_data.MEASUREMENTREL">
		<rdfs:range rdf:resource="&datatypes;data.MEASUREMENTREL"/>
		<rdfs:label>dynam.dist</rdfs:label>
	<rdfs:comment>Records the default distance from the staff for dynamic marks.</rdfs:comment>
	</owl:DatatypeProperty>
	<owl:DatatypeProperty rdf:ID="harm.dist_att.distances.attribute.harm.dist__mei_data.MEASUREMENTREL">
		<rdfs:range rdf:resource="&datatypes;data.MEASUREMENTREL"/>
		<rdfs:label>harm.dist</rdfs:label>
	<rdfs:comment>Records the default distance from the staff of harmonic indications, such as guitar chord grids or functional labels.</rdfs:comment>
	</owl:DatatypeProperty>
	<owl:DatatypeProperty rdf:ID="text.dist_att.distances.attribute.text.dist__mei_data.MEASUREMENTREL">
		<rdfs:range rdf:resource="&datatypes;data.MEASUREMENTREL"/>
		<rdfs:label>text.dist</rdfs:label>
	<rdfs:comment>Determines how far from the staff to render text elements.</rdfs:comment>
	</owl:DatatypeProperty>
	<rdfs:Datatype rdf:ID="NS_form_att.dot.log.attribute.form_UNType">
		<owl:equivalentClass><rdfs:Datatype>
		<owl:onDatatype rdf:resource="&xs;token"/><owl:withRestrictions rdf:parseType="Collection"><rdf:Description><xs:enumeration>aug</xs:enumeration></rdf:Description><rdf:Description><xs:enumeration>div</xs:enumeration></rdf:Description></owl:withRestrictions></rdfs:Datatype></owl:equivalentClass></rdfs:Datatype>
	<owl:DatatypeProperty rdf:ID="form_att.dot.log.attribute.form__NS_form_att.dot.log.attribute.form_UNType">
		<rdfs:range rdf:resource="#NS_form_att.dot.log.attribute.form_UNType"/>
		<rdfs:label>form</rdfs:label>
	<rdfs:comment>Records the function of the dot.</rdfs:comment>
	</owl:DatatypeProperty>
	<rdfs:Datatype rdf:ID="NS_dur_att.duration.additive.attribute.dur_UNType">
		<owl:equivalentClass><rdfs:Datatype>
		<owl:onDatatype rdf:resource="dur_att.duration.additive.attribute.dur_NS_dur_att.duration.additive.attribute.dur_UNType_UNType"/><owl:withRestrictions rdf:parseType="Collection"><rdf:Description><xs:minLength>1</xs:minLength></rdf:Description></owl:withRestrictions></rdfs:Datatype></owl:equivalentClass></rdfs:Datatype>
	<rdfs:Datatype rdf:ID="dur_att.duration.additive.attribute.dur_NS_dur_att.duration.additive.attribute.dur_UNType_UNType">
		<owl:equivalentClass><rdfs:Datatype>
		<owl:oneOf><rdf:Description><rdf:type rdf:resource="#List"/><rdf:first>mei:data.DURATION.additive</rdf:first><rdf:rest rdf:resource="#nil"/></rdf:Description></owl:oneOf></rdfs:Datatype></owl:equivalentClass></rdfs:Datatype>
	<owl:DatatypeProperty rdf:ID="dur_att.duration.additive.attribute.dur__NS_dur_att.duration.additive.attribute.dur_UNType">
		<rdfs:range rdf:resource="#NS_dur_att.duration.additive.attribute.dur_UNType"/>
		<rdfs:label>dur</rdfs:label>
	<rdfs:comment>Records duration using optionally dotted, relative durational values provided by the data.DURATION datatype. When the duration is &quot;irrational&quot;, as is sometimes the case with tuplets, multiple space-separated values that add up to the total duration may be used. When dotted values are present, the dots attribute must be ignored.</rdfs:comment>
	</owl:DatatypeProperty>
	<owl:DatatypeProperty rdf:ID="dur.default_att.duration.default.attribute.dur.default__mei_data.DURATION">
		<rdfs:range rdf:resource="&datatypes;data.DURATION"/>
		<rdfs:label>dur.default</rdfs:label>
	<rdfs:comment>Contains a default duration in those situations when the first note, rest, chord, etc. in a measure does not have a duration specified.</rdfs:comment>
	</owl:DatatypeProperty>
	<owl:DatatypeProperty rdf:ID="num.default_att.duration.default.attribute.num.default__xs_positiveInteger">
		<rdfs:range rdf:resource="&xs;positiveInteger"/>
		<rdfs:label>num.default</rdfs:label>
	<rdfs:comment>Along with numbase.default, describes the default duration as a ratio. num.default is the first value in the ratio.</rdfs:comment>
	</owl:DatatypeProperty>
	<owl:DatatypeProperty rdf:ID="numbase.default_att.duration.default.attribute.numbase.default__xs_positiveInteger">
		<rdfs:range rdf:resource="&xs;positiveInteger"/>
		<rdfs:label>numbase.default</rdfs:label>
	<rdfs:comment>Along with num.default, describes the default duration as a ratio. numbase.default is the second value in the ratio.</rdfs:comment>
	</owl:DatatypeProperty>
	<owl:DatatypeProperty rdf:ID="dur_att.duration.musical.attribute.dur__mei_data.DURATION">
		<rdfs:range rdf:resource="&datatypes;data.DURATION"/>
		<rdfs:label>dur</rdfs:label>
	<rdfs:comment>Records the duration of a feature using the relative durational values provided by the data.DURATION datatype.</rdfs:comment>
	</owl:DatatypeProperty>
	<owl:DatatypeProperty rdf:ID="dur.ges_att.duration.performed.attribute.dur.ges__mei_data.DURATION.gestural">
		<rdfs:range rdf:resource="&datatypes;data.DURATION.gestural"/>
		<rdfs:label>dur.ges</rdfs:label>
	<rdfs:comment>Records performed duration information that differs from the written duration. Its value may be expressed in several forms; that is, ppq (MIDI clicks and MusicXML 'divisions'), Humdrum **recip values, beats, seconds, or mensural duration values.</rdfs:comment>
	</owl:DatatypeProperty>
	<owl:DatatypeProperty rdf:ID="num_att.duration.ratio.attribute.num__xs_positiveInteger">
		<rdfs:range rdf:resource="&xs;positiveInteger"/>
		<rdfs:label>num</rdfs:label>
	<rdfs:comment>Along with numbase, describes duration as a ratio. num is the first value in the ratio, while numbase is the second.</rdfs:comment>
	</owl:DatatypeProperty>
	<owl:DatatypeProperty rdf:ID="numbase_att.duration.ratio.attribute.numbase__xs_positiveInteger">
		<rdfs:range rdf:resource="&xs;positiveInteger"/>
		<rdfs:label>numbase</rdfs:label>
	<rdfs:comment>Along with num, describes duration as a ratio. num is the first value in the ratio, while numbase is the second.</rdfs:comment>
	</owl:DatatypeProperty>
	<owl:DatatypeProperty rdf:ID="enclose_att.enclosingchars.attribute.enclose__mei_data.ENCLOSURE">
		<rdfs:range rdf:resource="&datatypes;data.ENCLOSURE"/>
		<rdfs:label>enclose</rdfs:label>
	<rdfs:comment>Records the characters often used to mark accidentals, articulations, and sometimes notes as having a cautionary or editorial function. For an example of cautionary accidentals enclosed in parentheses, see Read, p. 131, ex. 9-14.</rdfs:comment>
	</owl:DatatypeProperty>
	<rdfs:Datatype rdf:ID="NS_ending.rend_att.endings.attribute.ending.rend_UNType">
		<owl:equivalentClass><rdfs:Datatype>
		<owl:onDatatype rdf:resource="&xs;token"/><owl:withRestrictions rdf:parseType="Collection"><rdf:Description><xs:enumeration>top</xs:enumeration></rdf:Description><rdf:Description><xs:enumeration>barred</xs:enumeration></rdf:Description><rdf:Description><xs:enumeration>grouped</xs:enumeration></rdf:Description></owl:withRestrictions></rdfs:Datatype></owl:equivalentClass></rdfs:Datatype>
	<owl:DatatypeProperty rdf:ID="ending.rend_att.endings.attribute.ending.rend__NS_ending.rend_att.endings.attribute.ending.rend_UNType">
		<rdfs:range rdf:resource="#NS_ending.rend_att.endings.attribute.ending.rend_UNType"/>
		<rdfs:label>ending.rend</rdfs:label>
	<rdfs:comment>Describes where ending marks should be displayed.</rdfs:comment>
	</owl:DatatypeProperty>
	<owl:DatatypeProperty rdf:ID="extender_att.extender.attribute.extender__mei_data.BOOLEAN">
		<rdfs:range rdf:resource="&datatypes;data.BOOLEAN"/>
		<rdfs:label>extender</rdfs:label>
	<rdfs:comment>Indicates the presence of an extension symbol, typically a line.</rdfs:comment>
	</owl:DatatypeProperty>
	<owl:DatatypeProperty rdf:ID="fermata_att.fermatapresent.attribute.fermata__mei_data.PLACE">
		<rdfs:range rdf:resource="&datatypes;data.PLACE"/>
		<rdfs:label>fermata</rdfs:label>
	<rdfs:comment>Indicates the attachment of a fermata to this element. If visual information about the fermata needs to be recorded, then a &lt;fermata&gt; element should be employed instead.</rdfs:comment>
	</owl:DatatypeProperty>
	<owl:DatatypeProperty rdf:ID="nonfiling_att.filing.attribute.nonfiling__xs_positiveInteger">
		<rdfs:range rdf:resource="&xs;positiveInteger"/>
		<rdfs:label>nonfiling</rdfs:label>
	<rdfs:comment>Holds the number of initial characters (such as those constituing an article or preposition) that should not be used for sorting a title or name.</rdfs:comment>
	</owl:DatatypeProperty>
	<owl:DatatypeProperty rdf:ID="level_att.grpSym.log.attribute.level__xs_positiveInteger">
		<rdfs:range rdf:resource="&xs;positiveInteger"/>
		<rdfs:label>level</rdfs:label>
	<rdfs:comment>Indicates the nesting level of staff grouping symbols.</rdfs:comment>
	</owl:DatatypeProperty>
	<owl:DatatypeProperty rdf:ID="hand_att.handident.attribute.hand__mei_data.URI">
		<rdfs:range rdf:resource="&datatypes;data.URI"/>
		<rdfs:label>hand</rdfs:label>
	<rdfs:comment>Signifies the hand responsible for an action. The value must be the ID of a &lt;hand&gt; element declared in the header.</rdfs:comment>
	</owl:DatatypeProperty>
	<owl:DatatypeProperty rdf:ID="height_att.height.attribute.height__mei_data.MEASUREMENTABS">
		<rdfs:range rdf:resource="&datatypes;data.MEASUREMENTABS"/>
		<rdfs:label>height</rdfs:label>
	<rdfs:comment>Measurement of the vertical dimension of an entity.</rdfs:comment>
	</owl:DatatypeProperty>
	<owl:DatatypeProperty rdf:ID="halign_att.horizontalalign.attribute.halign__mei_data.HORIZONTALALIGNMENT">
		<rdfs:range rdf:resource="&datatypes;data.HORIZONTALALIGNMENT"/>
		<rdfs:label>halign</rdfs:label>
	<rdfs:comment>Records horizontal alignment.</rdfs:comment>
	</owl:DatatypeProperty>
	<owl:DatatypeProperty rdf:ID="instr_att.instrumentident.attribute.instr__mei_data.URI">
		<rdfs:range rdf:resource="&datatypes;data.URI"/>
		<rdfs:label>instr</rdfs:label>
	<rdfs:comment>Provides a way of pointing to a MIDI instrument definition. It must contain the ID of an &lt;instrDef&gt; element elsewhere in the document.</rdfs:comment>
	</owl:DatatypeProperty>
	<owl:DatatypeProperty rdf:ID="mimetype_att.internetmedia.attribute.mimetype__xs_string">
		<rdfs:range rdf:resource="&xs;string"/>
		<rdfs:label>mimetype</rdfs:label>
	<rdfs:comment>Specifies the applicable MIME (multimedia internet mail extension) type. The value should be a valid MIME media type defined by the Internet Engineering Task Force in RFC 2046.</rdfs:comment>
	</owl:DatatypeProperty>
	<rdfs:Datatype rdf:ID="NS_join_att.joined.attribute.join_UNType">
		<owl:equivalentClass><rdfs:Datatype>
		<owl:onDatatype rdf:resource="join_att.joined.attribute.join_NS_join_att.joined.attribute.join_UNType_UNType"/><owl:withRestrictions rdf:parseType="Collection"><rdf:Description><xs:minLength>1</xs:minLength></rdf:Description></owl:withRestrictions></rdfs:Datatype></owl:equivalentClass></rdfs:Datatype>
	<rdfs:Datatype rdf:ID="join_att.joined.attribute.join_NS_join_att.joined.attribute.join_UNType_UNType">
		<owl:equivalentClass><rdfs:Datatype>
		<owl:oneOf><rdf:Description><rdf:type rdf:resource="#List"/><rdf:first>mei:data.URI</rdf:first><rdf:rest rdf:resource="#nil"/></rdf:Description></owl:oneOf></rdfs:Datatype></owl:equivalentClass></rdfs:Datatype>
	<owl:DatatypeProperty rdf:ID="join_att.joined.attribute.join__NS_join_att.joined.attribute.join_UNType">
		<rdfs:range rdf:resource="#NS_join_att.joined.attribute.join_UNType"/>
		<rdfs:label>join</rdfs:label>
	<rdfs:comment>Used for linking visually separate entities that form a single logical entity, for example, multiple slurs broken across a system break that form a single musical phrase. Also used to indicate a measure which metrically completes the current one. Record the identifiers of the separately encoded components, excluding the one carrying the attribute.</rdfs:comment>
	</owl:DatatypeProperty>
	<owl:DatatypeProperty rdf:ID="sig_att.keySig.log.attribute.sig__mei_data.KEYSIGNATURE">
		<rdfs:range rdf:resource="&datatypes;data.KEYSIGNATURE"/>
		<rdfs:label>sig</rdfs:label>
	<rdfs:comment>Indicates where the key lies in the circle of fifths.</rdfs:comment>
	</owl:DatatypeProperty>
	<rdfs:Datatype rdf:ID="NS_sig.mixed_att.keySig.log.attribute.sig.mixed_UNType">
		<owl:equivalentClass><rdfs:Datatype>
		<owl:onDatatype rdf:resource="sig.mixed_att.keySig.log.attribute.sig.mixed_NS_sig.mixed_att.keySig.log.attribute.sig.mixed_UNType_UNType"/><owl:withRestrictions rdf:parseType="Collection"><rdf:Description><xs:minLength>1</xs:minLength></rdf:Description></owl:withRestrictions></rdfs:Datatype></owl:equivalentClass></rdfs:Datatype>
	<rdfs:Datatype rdf:ID="sig.mixed_att.keySig.log.attribute.sig.mixed_NS_sig.mixed_att.keySig.log.attribute.sig.mixed_UNType_UNType">
		<owl:equivalentClass><rdfs:Datatype>
		<owl:oneOf><rdf:Description><rdf:type rdf:resource="#List"/><rdf:first>mei:data.KEYSIGTOKEN</rdf:first><rdf:rest rdf:resource="#nil"/></rdf:Description></owl:oneOf></rdfs:Datatype></owl:equivalentClass></rdfs:Datatype>
	<owl:DatatypeProperty rdf:ID="sig.mixed_att.keySig.log.attribute.sig.mixed__NS_sig.mixed_att.keySig.log.attribute.sig.mixed_UNType">
		<rdfs:range rdf:resource="#NS_sig.mixed_att.keySig.log.attribute.sig.mixed_UNType"/>
		<rdfs:label>sig.mixed</rdfs:label>
	<rdfs:comment>Mixed key signatures, e.g. those consisting of a mixture of flats and sharps (Read, p. 143, ex. 9-39), and key signatures with unorthodox placement of the accidentals (Read, p. 141) must be indicated by setting the key.sig attribute to 'mixed' and providing explicit key signature information in the key.sig.mixed attribute or in the &lt;keySig&gt; element. It is intended that key.sig.mixed contain a series of tokens with each token containing pitch name, accidental, and octave, such as 'a4 c5s e5f' that indicate what key accidentals should be rendered and where they should be placed.</rdfs:comment>
	</owl:DatatypeProperty>
	<owl:DatatypeProperty rdf:ID="mode_att.keySig.log.attribute.mode__mei_data.MODE">
		<rdfs:range rdf:resource="&datatypes;data.MODE"/>
		<rdfs:label>mode</rdfs:label>
	<rdfs:comment>Indicates major, minor, or other tonality.</rdfs:comment>
	</owl:DatatypeProperty>
	<owl:DatatypeProperty rdf:ID="sig.showchange_att.keySig.vis.attribute.sig.showchange__mei_data.BOOLEAN">
		<rdfs:range rdf:resource="&datatypes;data.BOOLEAN"/>
		<rdfs:label>sig.showchange</rdfs:label>
	<rdfs:comment>Determines whether cautionary accidentals should be displayed at a key change.</rdfs:comment>
	</owl:DatatypeProperty>
	<owl:DatatypeProperty rdf:ID="key.accid_att.keySigDefault.log.attribute.key.accid__mei_data.ACCIDENTAL.IMPLICIT">
		<rdfs:range rdf:resource="&datatypes;data.ACCIDENTAL.IMPLICIT"/>
		<rdfs:label>key.accid</rdfs:label>
	<rdfs:comment>Contains an accidental for the tonic key, if one is required, e.g., if key.pname equals 'c' and key.accid equals 's', then a tonic of C# is indicated.</rdfs:comment>
	</owl:DatatypeProperty>
	<owl:DatatypeProperty rdf:ID="key.mode_att.keySigDefault.log.attribute.key.mode__mei_data.MODE">
		<rdfs:range rdf:resource="&datatypes;data.MODE"/>
		<rdfs:label>key.mode</rdfs:label>
	<rdfs:comment>Indicates major, minor, or other tonality.</rdfs:comment>
	</owl:DatatypeProperty>
	<owl:DatatypeProperty rdf:ID="key.pname_att.keySigDefault.log.attribute.key.pname__mei_data.PITCHNAME">
		<rdfs:range rdf:resource="&datatypes;data.PITCHNAME"/>
		<rdfs:label>key.pname</rdfs:label>
	<rdfs:comment>Holds the pitch name of the tonic key, e.g. 'c' for the key of C.</rdfs:comment>
	</owl:DatatypeProperty>
	<owl:DatatypeProperty rdf:ID="key.sig_att.keySigDefault.log.attribute.key.sig__mei_data.KEYSIGNATURE">
		<rdfs:range rdf:resource="&datatypes;data.KEYSIGNATURE"/>
		<rdfs:label>key.sig</rdfs:label>
	<rdfs:comment>Indicates where the key lies in the circle of fifths.</rdfs:comment>
	</owl:DatatypeProperty>
	<rdfs:Datatype rdf:ID="NS_key.sig.mixed_att.keySigDefault.log.attribute.key.sig.mixed_UNType">
		<owl:equivalentClass><rdfs:Datatype>
		<owl:onDatatype rdf:resource="key.sig.mixed_att.keySigDefault.log.attribute.key.sig.mixed_NS_key.sig.mixed_att.keySigDefault.log.attribute.key.sig.mixed_UNType_UNType"/><owl:withRestrictions rdf:parseType="Collection"><rdf:Description><xs:minLength>1</xs:minLength></rdf:Description></owl:withRestrictions></rdfs:Datatype></owl:equivalentClass></rdfs:Datatype>
	<rdfs:Datatype rdf:ID="key.sig.mixed_att.keySigDefault.log.attribute.key.sig.mixed_NS_key.sig.mixed_att.keySigDefault.log.attribute.key.sig.mixed_UNType_UNType">
		<owl:equivalentClass><rdfs:Datatype>
		<owl:oneOf><rdf:Description><rdf:type rdf:resource="#List"/><rdf:first>mei:data.KEYSIGTOKEN</rdf:first><rdf:rest rdf:resource="#nil"/></rdf:Description></owl:oneOf></rdfs:Datatype></owl:equivalentClass></rdfs:Datatype>
	<owl:DatatypeProperty rdf:ID="key.sig.mixed_att.keySigDefault.log.attribute.key.sig.mixed__NS_key.sig.mixed_att.keySigDefault.log.attribute.key.sig.mixed_UNType">
		<rdfs:range rdf:resource="#NS_key.sig.mixed_att.keySigDefault.log.attribute.key.sig.mixed_UNType"/>
		<rdfs:label>key.sig.mixed</rdfs:label>
	<rdfs:comment>Mixed key signatures, e.g. those consisting of a mixture of flats and sharps (Read, p. 143, ex. 9-39), and key signatures with unorthodox placement of the accidentals (Read, p. 141) must be indicated by setting the key.sig attribute to 'mixed' and providing explicit key signature information in the key.sig.mixed attribute or in the &lt;keySig&gt; element. It is intended that key.sig.mixed contain a series of tokens with each token containing pitch name, accidental, and octave, such as 'a4 c5s e5f' that indicate what key accidentals should be rendered and where they should be placed.</rdfs:comment>
	</owl:DatatypeProperty>
	<owl:DatatypeProperty rdf:ID="key.sig.show_att.keySigDefault.vis.attribute.key.sig.show__mei_data.BOOLEAN">
		<rdfs:range rdf:resource="&datatypes;data.BOOLEAN"/>
		<rdfs:label>key.sig.show</rdfs:label>
	<rdfs:comment>Indicates whether the key signature should be displayed.</rdfs:comment>
	</owl:DatatypeProperty>
	<owl:DatatypeProperty rdf:ID="key.sig.showchange_att.keySigDefault.vis.attribute.key.sig.showchange__mei_data.BOOLEAN">
		<rdfs:range rdf:resource="&datatypes;data.BOOLEAN"/>
		<rdfs:label>key.sig.showchange</rdfs:label>
	<rdfs:comment>Determines whether cautionary accidentals should be displayed at a key change.</rdfs:comment>
	</owl:DatatypeProperty>
	<owl:DatatypeProperty rdf:ID="label.abbr_att.labels.addl.attribute.label.abbr__xs_string">
		<rdfs:range rdf:resource="&xs;string"/>
		<rdfs:label>label.abbr</rdfs:label>
	<rdfs:comment>Provides a label for a group of staves on pages after the first page. Usually, this label takes an abbreviated form.</rdfs:comment>
	</owl:DatatypeProperty>
	<owl:DatatypeProperty rdf:ID="translit_att.lang.attribute.translit__xs_NMTOKEN">
		<rdfs:range rdf:resource="&xs;NMTOKEN"/>
		<rdfs:label>translit</rdfs:label>
	<rdfs:comment>Specifies the transliteration technique used.</rdfs:comment>
	</owl:DatatypeProperty>
	<owl:DatatypeProperty rdf:ID="def_att.layer.log.attribute.def__mei_data.URI">
		<rdfs:range rdf:resource="&datatypes;data.URI"/>
		<rdfs:label>def</rdfs:label>
	<rdfs:comment>Provides a mechanism for linking the layer to a layerDef element.</rdfs:comment>
	</owl:DatatypeProperty>
	<rdfs:Datatype rdf:ID="NS_layer_att.layerident.attribute.layer_UNType">
		<owl:equivalentClass><rdfs:Datatype>
		<owl:onDatatype rdf:resource="layer_att.layerident.attribute.layer_NS_layer_att.layerident.attribute.layer_UNType_UNType"/><owl:withRestrictions rdf:parseType="Collection"><rdf:Description><xs:minLength>1</xs:minLength></rdf:Description></owl:withRestrictions></rdfs:Datatype></owl:equivalentClass></rdfs:Datatype>
	<rdfs:Datatype rdf:ID="layer_att.layerident.attribute.layer_NS_layer_att.layerident.attribute.layer_UNType_UNType">
		<owl:equivalentClass><rdfs:Datatype>
		<owl:oneOf><rdf:Description><rdf:type rdf:resource="#List"/><rdf:first>xs:positiveInteger</rdf:first><rdf:rest rdf:resource="#nil"/></rdf:Description></owl:oneOf></rdfs:Datatype></owl:equivalentClass></rdfs:Datatype>
	<owl:DatatypeProperty rdf:ID="layer_att.layerident.attribute.layer__NS_layer_att.layerident.attribute.layer_UNType">
		<rdfs:range rdf:resource="#NS_layer_att.layerident.attribute.layer_UNType"/>
		<rdfs:label>layer</rdfs:label>
	<rdfs:comment>Identifies the layer to which a feature applies.</rdfs:comment>
	</owl:DatatypeProperty>
	<owl:DatatypeProperty rdf:ID="form_att.line.vis.attribute.form__mei_data.LINEFORM">
		<rdfs:range rdf:resource="&datatypes;data.LINEFORM"/>
		<rdfs:label>form</rdfs:label>
	<rdfs:comment>Visual form of the line.</rdfs:comment>
	</owl:DatatypeProperty>
	<owl:DatatypeProperty rdf:ID="width_att.line.vis.attribute.width__mei_data.LINEWIDTH">
		<rdfs:range rdf:resource="&datatypes;data.LINEWIDTH"/>
		<rdfs:label>width</rdfs:label>
	<rdfs:comment>Width of the line.</rdfs:comment>
	</owl:DatatypeProperty>
	<owl:DatatypeProperty rdf:ID="endsym_att.line.vis.attribute.endsym__mei_data.LINESTARTENDSYMBOL">
		<rdfs:range rdf:resource="&datatypes;data.LINESTARTENDSYMBOL"/>
		<rdfs:label>endsym</rdfs:label>
	<rdfs:comment>Symbol rendered at end of line.</rdfs:comment>
	</owl:DatatypeProperty>
	<owl:DatatypeProperty rdf:ID="endsymsize_att.line.vis.attribute.endsymsize__mei_data.LINESTARTENDSYMBOLSIZE">
		<rdfs:range rdf:resource="&datatypes;data.LINESTARTENDSYMBOLSIZE"/>
		<rdfs:label>endsymsize</rdfs:label>
	<rdfs:comment>Holds the relative size of the line-end symbol.</rdfs:comment>
	</owl:DatatypeProperty>
	<owl:DatatypeProperty rdf:ID="startsym_att.line.vis.attribute.startsym__mei_data.LINESTARTENDSYMBOL">
		<rdfs:range rdf:resource="&datatypes;data.LINESTARTENDSYMBOL"/>
		<rdfs:label>startsym</rdfs:label>
	<rdfs:comment>Symbol rendered at start of line.</rdfs:comment>
	</owl:DatatypeProperty>
	<owl:DatatypeProperty rdf:ID="startsymsize_att.line.vis.attribute.startsymsize__mei_data.LINESTARTENDSYMBOLSIZE">
		<rdfs:range rdf:resource="&datatypes;data.LINESTARTENDSYMBOLSIZE"/>
		<rdfs:label>startsymsize</rdfs:label>
	<rdfs:comment>Holds the relative size of the line-start symbol.</rdfs:comment>
	</owl:DatatypeProperty>
	<owl:DatatypeProperty rdf:ID="line_att.lineloc.attribute.line__mei_data.CLEFLINE">
		<rdfs:range rdf:resource="&datatypes;data.CLEFLINE"/>
		<rdfs:label>line</rdfs:label>
	<rdfs:comment>Indicates the line upon which a feature stands. The value must be in the range between 1 and the number of lines on the staff. The numbering of lines starts with the lowest line of the staff.</rdfs:comment>
	</owl:DatatypeProperty>
	<owl:DatatypeProperty rdf:ID="lendsym_att.linerend.attribute.lendsym__mei_data.LINESTARTENDSYMBOL">
		<rdfs:range rdf:resource="&datatypes;data.LINESTARTENDSYMBOL"/>
		<rdfs:label>lendsym</rdfs:label>
	<rdfs:comment>Symbol rendered at end of line.</rdfs:comment>
	</owl:DatatypeProperty>
	<owl:DatatypeProperty rdf:ID="lendsymsize_att.linerend.attribute.lendsymsize__mei_data.LINESTARTENDSYMBOLSIZE">
		<rdfs:range rdf:resource="&datatypes;data.LINESTARTENDSYMBOLSIZE"/>
		<rdfs:label>lendsymsize</rdfs:label>
	<rdfs:comment>Holds the relative size of the line-end symbol.</rdfs:comment>
	</owl:DatatypeProperty>
	<owl:DatatypeProperty rdf:ID="lstartsym_att.linerend.attribute.lstartsym__mei_data.LINESTARTENDSYMBOL">
		<rdfs:range rdf:resource="&datatypes;data.LINESTARTENDSYMBOL"/>
		<rdfs:label>lstartsym</rdfs:label>
	<rdfs:comment>Symbol rendered at start of line.</rdfs:comment>
	</owl:DatatypeProperty>
	<owl:DatatypeProperty rdf:ID="lstartsymsize_att.linerend.attribute.lstartsymsize__mei_data.LINESTARTENDSYMBOLSIZE">
		<rdfs:range rdf:resource="&datatypes;data.LINESTARTENDSYMBOLSIZE"/>
		<rdfs:label>lstartsymsize</rdfs:label>
	<rdfs:comment>Holds the relative size of the line-start symbol.</rdfs:comment>
	</owl:DatatypeProperty>
	<owl:DatatypeProperty rdf:ID="lform_att.linerend.base.attribute.lform__mei_data.LINEFORM">
		<rdfs:range rdf:resource="&datatypes;data.LINEFORM"/>
		<rdfs:label>lform</rdfs:label>
	<rdfs:comment>Describes the line style of a line.</rdfs:comment>
	</owl:DatatypeProperty>
	<owl:DatatypeProperty rdf:ID="lwidth_att.linerend.base.attribute.lwidth__mei_data.LINEWIDTH">
		<rdfs:range rdf:resource="&datatypes;data.LINEWIDTH"/>
		<rdfs:label>lwidth</rdfs:label>
	<rdfs:comment>Width of a line.</rdfs:comment>
	</owl:DatatypeProperty>
	<owl:DatatypeProperty rdf:ID="lyric.align_att.lyricstyle.attribute.lyric.align__mei_data.MEASUREMENTREL">
		<rdfs:range rdf:resource="&datatypes;data.MEASUREMENTREL"/>
		<rdfs:label>lyric.align</rdfs:label>
	<rdfs:comment>Describes the alignment of lyric syllables associated with a note or chord.</rdfs:comment>
	</owl:DatatypeProperty>
	<owl:DatatypeProperty rdf:ID="lyric.fam_att.lyricstyle.attribute.lyric.fam__mei_data.FONTFAMILY">
		<rdfs:range rdf:resource="&datatypes;data.FONTFAMILY"/>
		<rdfs:label>lyric.fam</rdfs:label>
	<rdfs:comment>Sets the font family default value for lyrics.</rdfs:comment>
	</owl:DatatypeProperty>
	<owl:DatatypeProperty rdf:ID="lyric.name_att.lyricstyle.attribute.lyric.name__mei_data.FONTNAME">
		<rdfs:range rdf:resource="&datatypes;data.FONTNAME"/>
		<rdfs:label>lyric.name</rdfs:label>
	<rdfs:comment>Sets the font name default value for lyrics.</rdfs:comment>
	</owl:DatatypeProperty>
	<owl:DatatypeProperty rdf:ID="lyric.size_att.lyricstyle.attribute.lyric.size__mei_data.FONTSIZE">
		<rdfs:range rdf:resource="&datatypes;data.FONTSIZE"/>
		<rdfs:label>lyric.size</rdfs:label>
	<rdfs:comment>Sets the default font size value for lyrics.</rdfs:comment>
	</owl:DatatypeProperty>
	<owl:DatatypeProperty rdf:ID="lyric.style_att.lyricstyle.attribute.lyric.style__mei_data.FONTSTYLE">
		<rdfs:range rdf:resource="&datatypes;data.FONTSTYLE"/>
		<rdfs:label>lyric.style</rdfs:label>
	<rdfs:comment>Sets the default font style value for lyrics.</rdfs:comment>
	</owl:DatatypeProperty>
	<owl:DatatypeProperty rdf:ID="lyric.weight_att.lyricstyle.attribute.lyric.weight__mei_data.FONTWEIGHT">
		<rdfs:range rdf:resource="&datatypes;data.FONTWEIGHT"/>
		<rdfs:label>lyric.weight</rdfs:label>
	<rdfs:comment>Sets the default font weight value for lyrics.</rdfs:comment>
	</owl:DatatypeProperty>
	<owl:DatatypeProperty rdf:ID="left_att.measure.log.attribute.left__mei_data.BARRENDITION">
		<rdfs:range rdf:resource="&datatypes;data.BARRENDITION"/>
		<rdfs:label>left</rdfs:label>
	<rdfs:comment>Indicates the visual rendition of the left bar line. It is present here only for facilitation of translation from legacy encodings which use it. Usually, it can be safely ignored.</rdfs:comment>
	</owl:DatatypeProperty>
	<owl:DatatypeProperty rdf:ID="right_att.measure.log.attribute.right__mei_data.BARRENDITION">
		<rdfs:range rdf:resource="&datatypes;data.BARRENDITION"/>
		<rdfs:label>right</rdfs:label>
	<rdfs:comment>Indicates the function of the right bar line and is structurally important.</rdfs:comment>
	</owl:DatatypeProperty>
	<rdfs:Datatype rdf:ID="NS_unit_att.measurement.attribute.unit_UNType">
		<owl:equivalentClass><rdfs:Datatype>
		<owl:unionOf rdf:parseType="Collection"><rdf:Description rdf:about="xs:NMTOKEN"/></owl:unionOf></rdfs:Datatype></owl:equivalentClass></rdfs:Datatype>
	<owl:DatatypeProperty rdf:ID="unit_att.measurement.attribute.unit__NS_unit_att.measurement.attribute.unit_UNType">
		<rdfs:range rdf:resource="#NS_unit_att.measurement.attribute.unit_UNType"/>
		<rdfs:label>unit</rdfs:label>
	<rdfs:comment>Indicates the unit of measurement.
Suggested values include: 1] byte; 2] char; 3] cm; 4] in; 5] issue; 6] mm; 7] page; 8] pc; 9] pt; 10] px; 11] record; 12] vol; 13] vu</rdfs:comment>
	</owl:DatatypeProperty>
	<owl:DatatypeProperty rdf:ID="mnum.visible_att.measurenumbers.attribute.mnum.visible__mei_data.BOOLEAN">
		<rdfs:range rdf:resource="&datatypes;data.BOOLEAN"/>
		<rdfs:label>mnum.visible</rdfs:label>
	<rdfs:comment>Indicates whether measure numbers should be displayed.</rdfs:comment>
	</owl:DatatypeProperty>
	<owl:DatatypeProperty rdf:ID="begin_att.mediabounds.attribute.begin__">
		<rdfs:label>begin</rdfs:label>
	<rdfs:comment>Specifies a point where the relevant content begins. A numerical value must be less and a time value must be earlier than that given by the end attribute.</rdfs:comment>
	</owl:DatatypeProperty>
	<owl:DatatypeProperty rdf:ID="end_att.mediabounds.attribute.end__">
		<rdfs:label>end</rdfs:label>
	<rdfs:comment>Specifies a point where the relevant content ends. If not specified, the end of the content is assumed to be the end point. A numerical value must be greater and a time value must be later than that given by the begin attribute.</rdfs:comment>
	</owl:DatatypeProperty>
	<owl:DatatypeProperty rdf:ID="betype_att.mediabounds.attribute.betype__mei_data.BETYPE">
		<rdfs:range rdf:resource="&datatypes;data.BETYPE"/>
		<rdfs:label>betype</rdfs:label>
	<rdfs:comment>Type of values used in the begin/end attributes. The begin and end attributes can only be interpreted meaningfully in conjunction with this attribute.</rdfs:comment>
	</owl:DatatypeProperty>
	<owl:DatatypeProperty rdf:ID="medium_att.medium.attribute.medium__xs_string">
		<rdfs:range rdf:resource="&xs;string"/>
		<rdfs:label>medium</rdfs:label>
	<rdfs:comment>Describes the writing medium.</rdfs:comment>
	</owl:DatatypeProperty>
	<rdfs:Datatype rdf:ID="NS_meiversion_att.meiversion.attribute.meiversion_UNType">
		<owl:equivalentClass><rdfs:Datatype>
		<owl:onDatatype rdf:resource="&xs;token"/><owl:withRestrictions rdf:parseType="Collection"><rdf:Description><xs:enumeration>3.0.0</xs:enumeration></rdf:Description></owl:withRestrictions></rdfs:Datatype></owl:equivalentClass></rdfs:Datatype>
	<owl:DatatypeProperty rdf:ID="meiversion_att.meiversion.attribute.meiversion__NS_meiversion_att.meiversion.attribute.meiversion_UNType">
		<rdfs:range rdf:resource="#NS_meiversion_att.meiversion.attribute.meiversion_UNType"/>
		<rdfs:label>meiversion</rdfs:label>
	<rdfs:comment>Specifies a generic MEI version label.</rdfs:comment>
	</owl:DatatypeProperty>
	<owl:DatatypeProperty rdf:ID="dot_att.mensur.log.attribute.dot__mei_data.BOOLEAN">
		<rdfs:range rdf:resource="&datatypes;data.BOOLEAN"/>
		<rdfs:label>dot</rdfs:label>
	<rdfs:comment>Specifies whether a dot is to be added to the base symbol.</rdfs:comment>
	</owl:DatatypeProperty>
	<owl:DatatypeProperty rdf:ID="sign_att.mensur.log.attribute.sign__mei_data.MENSURATIONSIGN">
		<rdfs:range rdf:resource="&datatypes;data.MENSURATIONSIGN"/>
		<rdfs:label>sign</rdfs:label>
	<rdfs:comment>The base symbol in the mensuration sign/time signature of mensural notation.</rdfs:comment>
	</owl:DatatypeProperty>
	<rdfs:Datatype rdf:ID="NS_metcon_att.meterconformance.attribute.metcon_UNType">
		<owl:equivalentClass><rdfs:Datatype>
		<owl:onDatatype rdf:resource="&xs;token"/><owl:withRestrictions rdf:parseType="Collection"><rdf:Description><xs:enumeration>c</xs:enumeration></rdf:Description><rdf:Description><xs:enumeration>i</xs:enumeration></rdf:Description><rdf:Description><xs:enumeration>o</xs:enumeration></rdf:Description></owl:withRestrictions></rdfs:Datatype></owl:equivalentClass></rdfs:Datatype>
	<owl:DatatypeProperty rdf:ID="metcon_att.meterconformance.attribute.metcon__NS_metcon_att.meterconformance.attribute.metcon_UNType">
		<rdfs:range rdf:resource="#NS_metcon_att.meterconformance.attribute.metcon_UNType"/>
		<rdfs:label>metcon</rdfs:label>
	<rdfs:comment>Indicates the relationship between the content of a staff or layer and the prevailing meter.</rdfs:comment>
	</owl:DatatypeProperty>
	<owl:DatatypeProperty rdf:ID="metcon_att.meterconformance.bar.attribute.metcon__mei_data.BOOLEAN">
		<rdfs:range rdf:resource="&datatypes;data.BOOLEAN"/>
		<rdfs:label>metcon</rdfs:label>
	<rdfs:comment>Indicates the relationship between the content of a measure and the prevailing meter.</rdfs:comment>
	</owl:DatatypeProperty>
	<owl:DatatypeProperty rdf:ID="control_att.meterconformance.bar.attribute.control__mei_data.BOOLEAN">
		<rdfs:range rdf:resource="&datatypes;data.BOOLEAN"/>
		<rdfs:label>control</rdfs:label>
	<rdfs:comment>Indicates whether or not a bar line is &quot;controlling&quot;; that is, if it indicates a point of alignment across all the parts. Bar lines within a score are usually controlling; that is, they &quot;line up&quot;. Bar lines within parts may or may not be controlling. When applied to &lt;measure&gt;, this attribute indicates the nature of the right barline but not the left.</rdfs:comment>
	</owl:DatatypeProperty>
	<rdfs:Datatype rdf:ID="NS_count_att.meterSig.log.attribute.count_UNType">
		<owl:equivalentClass><rdfs:Datatype>
		<owl:onDatatype rdf:resource="&xs;string"/><owl:withRestrictions rdf:parseType="Collection"><rdf:Description><xs:pattern>\d+(\.\d+)?(\s*\+\s*\d+(\.\d+)?)*</xs:pattern></rdf:Description></owl:withRestrictions></rdfs:Datatype></owl:equivalentClass></rdfs:Datatype>
	<owl:DatatypeProperty rdf:ID="count_att.meterSig.log.attribute.count__NS_count_att.meterSig.log.attribute.count_UNType">
		<rdfs:range rdf:resource="#NS_count_att.meterSig.log.attribute.count_UNType"/>
		<rdfs:label>count</rdfs:label>
	<rdfs:comment>Captures the number of beats in a measure, that is, the top number of the meter signature. It must contain a decimal number or an additive expression that evaluates to a decimal number, such as 2+3.</rdfs:comment>
	</owl:DatatypeProperty>
	<owl:DatatypeProperty rdf:ID="sym_att.meterSig.log.attribute.sym__mei_data.METERSIGN">
		<rdfs:range rdf:resource="&datatypes;data.METERSIGN"/>
		<rdfs:label>sym</rdfs:label>
	<rdfs:comment>Indicates the use of a meter symbol instead of a numeric meter signature, that is, 'C' for common time or 'C' with a slash for cut time.</rdfs:comment>
	</owl:DatatypeProperty>
	<owl:DatatypeProperty rdf:ID="unit_att.meterSig.log.attribute.unit__xs_decimal">
		<rdfs:range rdf:resource="&xs;decimal"/>
		<rdfs:label>unit</rdfs:label>
	<rdfs:comment>Contains the number indicating the beat unit, that is, the bottom number of the meter signature.</rdfs:comment>
	</owl:DatatypeProperty>
	<rdfs:Datatype rdf:ID="NS_form_att.meterSig.vis.attribute.form_UNType">
		<owl:equivalentClass><rdfs:Datatype>
		<owl:onDatatype rdf:resource="&xs;token"/><owl:withRestrictions rdf:parseType="Collection"><rdf:Description><xs:enumeration>num</xs:enumeration></rdf:Description><rdf:Description><xs:enumeration>denomsym</xs:enumeration></rdf:Description><rdf:Description><xs:enumeration>norm</xs:enumeration></rdf:Description><rdf:Description><xs:enumeration>invis</xs:enumeration></rdf:Description></owl:withRestrictions></rdfs:Datatype></owl:equivalentClass></rdfs:Datatype>
	<owl:DatatypeProperty rdf:ID="form_att.meterSig.vis.attribute.form__NS_form_att.meterSig.vis.attribute.form_UNType">
		<rdfs:range rdf:resource="#NS_form_att.meterSig.vis.attribute.form_UNType"/>
		<rdfs:label>form</rdfs:label>
	<rdfs:comment>Contains an indication of how the meter signature should be rendered.</rdfs:comment>
	</owl:DatatypeProperty>
	<rdfs:Datatype rdf:ID="NS_meter.count_att.meterSigDefault.log.attribute.meter.count_UNType">
		<owl:equivalentClass><rdfs:Datatype>
		<owl:onDatatype rdf:resource="&xs;string"/><owl:withRestrictions rdf:parseType="Collection"><rdf:Description><xs:pattern>\d+(\.\d+)?(\s*\+\s*\d+(\.\d+)?)*</xs:pattern></rdf:Description></owl:withRestrictions></rdfs:Datatype></owl:equivalentClass></rdfs:Datatype>
	<owl:DatatypeProperty rdf:ID="meter.count_att.meterSigDefault.log.attribute.meter.count__NS_meter.count_att.meterSigDefault.log.attribute.meter.count_UNType">
		<rdfs:range rdf:resource="#NS_meter.count_att.meterSigDefault.log.attribute.meter.count_UNType"/>
		<rdfs:label>meter.count</rdfs:label>
	<rdfs:comment>Captures the number of beats in a measure, that is, the top number of the meter signature. It must contain a decimal number or an additive expression that evaluates to a decimal number, such as 2+3.</rdfs:comment>
	</owl:DatatypeProperty>
	<owl:DatatypeProperty rdf:ID="meter.unit_att.meterSigDefault.log.attribute.meter.unit__xs_decimal">
		<rdfs:range rdf:resource="&xs;decimal"/>
		<rdfs:label>meter.unit</rdfs:label>
	<rdfs:comment>Contains the number indicating the beat unit, that is, the bottom number of the meter signature.</rdfs:comment>
	</owl:DatatypeProperty>
	<rdfs:Datatype rdf:ID="NS_meter.rend_att.meterSigDefault.vis.attribute.meter.rend_UNType">
		<owl:equivalentClass><rdfs:Datatype>
		<owl:onDatatype rdf:resource="&xs;token"/><owl:withRestrictions rdf:parseType="Collection"><rdf:Description><xs:enumeration>num</xs:enumeration></rdf:Description><rdf:Description><xs:enumeration>denomsym</xs:enumeration></rdf:Description><rdf:Description><xs:enumeration>norm</xs:enumeration></rdf:Description><rdf:Description><xs:enumeration>invis</xs:enumeration></rdf:Description></owl:withRestrictions></rdfs:Datatype></owl:equivalentClass></rdfs:Datatype>
	<owl:DatatypeProperty rdf:ID="meter.rend_att.meterSigDefault.vis.attribute.meter.rend__NS_meter.rend_att.meterSigDefault.vis.attribute.meter.rend_UNType">
		<rdfs:range rdf:resource="#NS_meter.rend_att.meterSigDefault.vis.attribute.meter.rend_UNType"/>
		<rdfs:label>meter.rend</rdfs:label>
	<rdfs:comment>Contains an indication of how the meter signature should be rendered.</rdfs:comment>
	</owl:DatatypeProperty>
	<owl:DatatypeProperty rdf:ID="meter.showchange_att.meterSigDefault.vis.attribute.meter.showchange__mei_data.BOOLEAN">
		<rdfs:range rdf:resource="&datatypes;data.BOOLEAN"/>
		<rdfs:label>meter.showchange</rdfs:label>
	<rdfs:comment>Determines whether a new meter signature should be displayed when the meter signature changes.</rdfs:comment>
	</owl:DatatypeProperty>
	<owl:DatatypeProperty rdf:ID="meter.sym_att.meterSigDefault.vis.attribute.meter.sym__mei_data.METERSIGN">
		<rdfs:range rdf:resource="&datatypes;data.METERSIGN"/>
		<rdfs:label>meter.sym</rdfs:label>
	<rdfs:comment>Indicates the use of a meter symbol instead of a numeric meter signature, that is, 'C' for common time or 'C' with a slash for cut time.</rdfs:comment>
	</owl:DatatypeProperty>
	<owl:DatatypeProperty rdf:ID="mm_att.mmtempo.attribute.mm__mei_data.TEMPOVALUE">
		<rdfs:range rdf:resource="&datatypes;data.TEMPOVALUE"/>
		<rdfs:label>mm</rdfs:label>
	<rdfs:comment>Used to describe tempo in terms of beats (often the meter signature denominator) per minute, ala M.M. (Maezel's Metronome). Do not confuse this attribute with midi.bpm or midi.mspb. In MIDI, a beat is always defined as a quarter note, *not the numerator of the time signature or the metronomic indication*.</rdfs:comment>
	</owl:DatatypeProperty>
	<owl:DatatypeProperty rdf:ID="mm.unit_att.mmtempo.attribute.mm.unit__mei_data.DURATION">
		<rdfs:range rdf:resource="&datatypes;data.DURATION"/>
		<rdfs:label>mm.unit</rdfs:label>
	<rdfs:comment>Captures the metronomic unit.</rdfs:comment>
	</owl:DatatypeProperty>
	<owl:DatatypeProperty rdf:ID="mm.dots_att.mmtempo.attribute.mm.dots__mei_data.AUGMENTDOT">
		<rdfs:range rdf:resource="&datatypes;data.AUGMENTDOT"/>
		<rdfs:label>mm.dots</rdfs:label>
	<rdfs:comment>Records the number of augmentation dots required by a dotted metronome unit.</rdfs:comment>
	</owl:DatatypeProperty>
	<owl:DatatypeProperty rdf:ID="multi.number_att.multinummeasures.attribute.multi.number__mei_data.BOOLEAN">
		<rdfs:range rdf:resource="&datatypes;data.BOOLEAN"/>
		<rdfs:label>multi.number</rdfs:label>
	<rdfs:comment>Indicates whether programmatically calculated counts of multiple measures of rest (mRest) and whole measure repeats (mRpt) in parts should be rendered.</rdfs:comment>
	</owl:DatatypeProperty>
	<owl:DatatypeProperty rdf:ID="nymref_att.name.attribute.nymref__mei_data.URI">
		<rdfs:range rdf:resource="&datatypes;data.URI"/>
		<rdfs:label>nymref</rdfs:label>
	<rdfs:comment>Used to record a pointer to the regularized form of the name elsewhere in the document.</rdfs:comment>
	</owl:DatatypeProperty>
	<owl:DatatypeProperty rdf:ID="role_att.name.attribute.role__">
		<rdfs:label>role</rdfs:label>
	<rdfs:comment>Used to specify further information about the entity referenced by this name, for example, the occupation of a person or the status of a place. Use a standard value whenever possible.</rdfs:comment>
	</owl:DatatypeProperty>
	<owl:DatatypeProperty rdf:ID="music.name_att.notationstyle.attribute.music.name__mei_data.MUSICFONT">
		<rdfs:range rdf:resource="&datatypes;data.MUSICFONT"/>
		<rdfs:label>music.name</rdfs:label>
	<rdfs:comment>Sets the default music font name.</rdfs:comment>
	</owl:DatatypeProperty>
	<owl:DatatypeProperty rdf:ID="music.size_att.notationstyle.attribute.music.size__mei_data.FONTSIZE">
		<rdfs:range rdf:resource="&datatypes;data.FONTSIZE"/>
		<rdfs:label>music.size</rdfs:label>
	<rdfs:comment>Sets the default music font size.</rdfs:comment>
	</owl:DatatypeProperty>
	<owl:DatatypeProperty rdf:ID="oct.ges_att.note.ges.attribute.oct.ges__mei_data.OCTAVE">
		<rdfs:range rdf:resource="&datatypes;data.OCTAVE"/>
		<rdfs:label>oct.ges</rdfs:label>
	<rdfs:comment>Records performed octave information that differs from the written value.</rdfs:comment>
	</owl:DatatypeProperty>
	<owl:DatatypeProperty rdf:ID="pname.ges_att.note.ges.attribute.pname.ges__mei_data.PITCHNAME.GES">
		<rdfs:range rdf:resource="&datatypes;data.PITCHNAME.GES"/>
		<rdfs:label>pname.ges</rdfs:label>
	<rdfs:comment>Contains a performed pitch name that differs from the written value.</rdfs:comment>
	</owl:DatatypeProperty>
	<owl:DatatypeProperty rdf:ID="pnum_att.note.ges.attribute.pnum__mei_data.PITCHNUMBER">
		<rdfs:range rdf:resource="&datatypes;data.PITCHNUMBER"/>
		<rdfs:label>pnum</rdfs:label>
	<rdfs:comment>Holds a pitch-to-number mapping, a base-40 or MIDI note number, for example.</rdfs:comment>
	</owl:DatatypeProperty>
	<owl:DatatypeProperty rdf:ID="head.color_att.noteheads.attribute.head.color__mei_data.COLOR">
		<rdfs:range rdf:resource="&datatypes;data.COLOR"/>
		<rdfs:label>head.color</rdfs:label>
	<rdfs:comment>Captures the overall color of a notehead.</rdfs:comment>
	</owl:DatatypeProperty>
	<owl:DatatypeProperty rdf:ID="head.fill_att.noteheads.attribute.head.fill__mei_data.FILL">
		<rdfs:range rdf:resource="&datatypes;data.FILL"/>
		<rdfs:label>head.fill</rdfs:label>
	<rdfs:comment>Describes how/if the notehead is filled.</rdfs:comment>
	</owl:DatatypeProperty>
	<owl:DatatypeProperty rdf:ID="head.fillcolor_att.noteheads.attribute.head.fillcolor__mei_data.COLOR">
		<rdfs:range rdf:resource="&datatypes;data.COLOR"/>
		<rdfs:label>head.fillcolor</rdfs:label>
	<rdfs:comment>Captures the fill color of a notehead if different from the overall note color.</rdfs:comment>
	</owl:DatatypeProperty>
	<rdfs:Datatype rdf:ID="NS_head.mod_att.noteheads.attribute.head.mod_UNType">
		<owl:equivalentClass><rdfs:Datatype>
		<owl:onDatatype rdf:resource="head.mod_att.noteheads.attribute.head.mod_NS_head.mod_att.noteheads.attribute.head.mod_UNType_UNType"/><owl:withRestrictions rdf:parseType="Collection"><rdf:Description><xs:minLength>1</xs:minLength></rdf:Description></owl:withRestrictions></rdfs:Datatype></owl:equivalentClass></rdfs:Datatype>
	<rdfs:Datatype rdf:ID="head.mod_att.noteheads.attribute.head.mod_NS_head.mod_att.noteheads.attribute.head.mod_UNType_UNType">
		<owl:equivalentClass><rdfs:Datatype>
		<owl:oneOf><rdf:Description><rdf:type rdf:resource="#List"/><rdf:first>mei:data.NOTEHEADMODIFIER</rdf:first><rdf:rest rdf:resource="#nil"/></rdf:Description></owl:oneOf></rdfs:Datatype></owl:equivalentClass></rdfs:Datatype>
	<owl:DatatypeProperty rdf:ID="head.mod_att.noteheads.attribute.head.mod__NS_head.mod_att.noteheads.attribute.head.mod_UNType">
		<rdfs:range rdf:resource="#NS_head.mod_att.noteheads.attribute.head.mod_UNType"/>
		<rdfs:label>head.mod</rdfs:label>
	<rdfs:comment>Records any additional symbols applied to the notehead.</rdfs:comment>
	</owl:DatatypeProperty>
	<owl:DatatypeProperty rdf:ID="head.rotation_att.noteheads.attribute.head.rotation__mei_data.ROTATION">
		<rdfs:range rdf:resource="&datatypes;data.ROTATION"/>
		<rdfs:label>head.rotation</rdfs:label>
	<rdfs:comment>Describes rotation applied to the basic notehead shape. A positive value rotates the notehead in a counter-clockwise fashion, while negative values produce clockwise rotation.</rdfs:comment>
	</owl:DatatypeProperty>
	<owl:DatatypeProperty rdf:ID="head.shape_att.noteheads.attribute.head.shape__mei_data.HEADSHAPE">
		<rdfs:range rdf:resource="&datatypes;data.HEADSHAPE"/>
		<rdfs:label>head.shape</rdfs:label>
	<rdfs:comment>Used to override the head shape normally used for the given duration.</rdfs:comment>
	</owl:DatatypeProperty>
	<owl:DatatypeProperty rdf:ID="head.visible_att.noteheads.attribute.head.visible__mei_data.BOOLEAN">
		<rdfs:range rdf:resource="&datatypes;data.BOOLEAN"/>
		<rdfs:label>head.visible</rdfs:label>
	<rdfs:comment>Indicates if a feature should be rendered when the notation is presented graphically or sounded when it is presented in an aural form.</rdfs:comment>
	</owl:DatatypeProperty>
	<owl:DatatypeProperty rdf:ID="oct_att.octave.attribute.oct__mei_data.OCTAVE">
		<rdfs:range rdf:resource="&datatypes;data.OCTAVE"/>
		<rdfs:label>oct</rdfs:label>
	<rdfs:comment>Captures written octave information.</rdfs:comment>
	</owl:DatatypeProperty>
	<owl:DatatypeProperty rdf:ID="octave.default_att.octavedefault.attribute.octave.default__mei_data.OCTAVE">
		<rdfs:range rdf:resource="&datatypes;data.OCTAVE"/>
		<rdfs:label>octave.default</rdfs:label>
	<rdfs:comment>Contains a default octave specification for use when the first note, rest, chord, etc. in a measure does not have an octave value specified.</rdfs:comment>
	</owl:DatatypeProperty>
	<owl:DatatypeProperty rdf:ID="dis_att.octavedisplacement.attribute.dis__mei_data.OCTAVE.DIS">
		<rdfs:range rdf:resource="&datatypes;data.OCTAVE.DIS"/>
		<rdfs:label>dis</rdfs:label>
	<rdfs:comment>Records the amount of octave displacement.</rdfs:comment>
	</owl:DatatypeProperty>
	<owl:DatatypeProperty rdf:ID="dis.place_att.octavedisplacement.attribute.dis.place__mei_data.PLACE">
		<rdfs:range rdf:resource="&datatypes;data.PLACE"/>
		<rdfs:label>dis.place</rdfs:label>
	<rdfs:comment>Records the direction of octave displacement.</rdfs:comment>
	</owl:DatatypeProperty>
	<owl:DatatypeProperty rdf:ID="ontheline_att.onelinestaff.attribute.ontheline__mei_data.BOOLEAN">
		<rdfs:range rdf:resource="&datatypes;data.BOOLEAN"/>
		<rdfs:label>ontheline</rdfs:label>
	<rdfs:comment>Determines the placement of notes on a 1-line staff. A value of 'true' places all notes on the line, while a value of 'false' places stems-up notes above the line and stems-down notes below the line.</rdfs:comment>
	</owl:DatatypeProperty>
	<owl:DatatypeProperty rdf:ID="optimize_att.optimization.attribute.optimize__mei_data.BOOLEAN">
		<rdfs:range rdf:resource="&datatypes;data.BOOLEAN"/>
		<rdfs:label>optimize</rdfs:label>
	<rdfs:comment>Indicates whether staves without notes, rests, etc. should be displayed. When the value is 'true', empty staves are displayed.</rdfs:comment>
	</owl:DatatypeProperty>
	<rdfs:Datatype rdf:ID="NS_origin.layer_att.origin.layerident.attribute.origin.layer_UNType">
		<owl:equivalentClass><rdfs:Datatype>
		<owl:onDatatype rdf:resource="origin.layer_att.origin.layerident.attribute.origin.layer_NS_origin.layer_att.origin.layerident.attribute.origin.layer_UNType_UNType"/><owl:withRestrictions rdf:parseType="Collection"><rdf:Description><xs:minLength>1</xs:minLength></rdf:Description></owl:withRestrictions></rdfs:Datatype></owl:equivalentClass></rdfs:Datatype>
	<rdfs:Datatype rdf:ID="origin.layer_att.origin.layerident.attribute.origin.layer_NS_origin.layer_att.origin.layerident.attribute.origin.layer_UNType_UNType">
		<owl:equivalentClass><rdfs:Datatype>
		<owl:oneOf><rdf:Description><rdf:type rdf:resource="#List"/><rdf:first>xs:positiveInteger</rdf:first><rdf:rest rdf:resource="#nil"/></rdf:Description></owl:oneOf></rdfs:Datatype></owl:equivalentClass></rdfs:Datatype>
	<owl:DatatypeProperty rdf:ID="origin.layer_att.origin.layerident.attribute.origin.layer__NS_origin.layer_att.origin.layerident.attribute.origin.layer_UNType">
		<rdfs:range rdf:resource="#NS_origin.layer_att.origin.layerident.attribute.origin.layer_UNType"/>
		<rdfs:label>origin.layer</rdfs:label>
	<rdfs:comment>identifies the layer on which referenced notation occurs.</rdfs:comment>
	</owl:DatatypeProperty>
	<rdfs:Datatype rdf:ID="NS_origin.staff_att.origin.staffident.attribute.origin.staff_UNType">
		<owl:equivalentClass><rdfs:Datatype>
		<owl:onDatatype rdf:resource="origin.staff_att.origin.staffident.attribute.origin.staff_NS_origin.staff_att.origin.staffident.attribute.origin.staff_UNType_UNType"/><owl:withRestrictions rdf:parseType="Collection"><rdf:Description><xs:minLength>1</xs:minLength></rdf:Description></owl:withRestrictions></rdfs:Datatype></owl:equivalentClass></rdfs:Datatype>
	<rdfs:Datatype rdf:ID="origin.staff_att.origin.staffident.attribute.origin.staff_NS_origin.staff_att.origin.staffident.attribute.origin.staff_UNType_UNType">
		<owl:equivalentClass><rdfs:Datatype>
		<owl:oneOf><rdf:Description><rdf:type rdf:resource="#List"/><rdf:first>xs:positiveInteger</rdf:first><rdf:rest rdf:resource="#nil"/></rdf:Description></owl:oneOf></rdfs:Datatype></owl:equivalentClass></rdfs:Datatype>
	<owl:DatatypeProperty rdf:ID="origin.staff_att.origin.staffident.attribute.origin.staff__NS_origin.staff_att.origin.staffident.attribute.origin.staff_UNType">
		<rdfs:range rdf:resource="#NS_origin.staff_att.origin.staffident.attribute.origin.staff_UNType"/>
		<rdfs:label>origin.staff</rdfs:label>
	<rdfs:comment>signifies the staff on which referenced notation occurs. Defaults to the same value as the local staff. Mandatory when applicable.</rdfs:comment>
	</owl:DatatypeProperty>
	<owl:DatatypeProperty rdf:ID="origin.startid_att.origin.startendid.attribute.origin.startid__mei_data.URI">
		<rdfs:range rdf:resource="&datatypes;data.URI"/>
		<rdfs:label>origin.startid</rdfs:label>
	<rdfs:comment>indicates the first element in a sequence of events.</rdfs:comment>
	</owl:DatatypeProperty>
	<owl:DatatypeProperty rdf:ID="origin.endid_att.origin.startendid.attribute.origin.endid__mei_data.URI">
		<rdfs:range rdf:resource="&datatypes;data.URI"/>
		<rdfs:label>origin.endid</rdfs:label>
	<rdfs:comment>indicates the final element in a sequence of events.</rdfs:comment>
	</owl:DatatypeProperty>
	<owl:DatatypeProperty rdf:ID="origin.tstamp_att.origin.timestamp.musical.attribute.origin.tstamp__mei_data.MEASUREBEATOFFSET">
		<rdfs:range rdf:resource="&datatypes;data.MEASUREBEATOFFSET"/>
		<rdfs:label>origin.tstamp</rdfs:label>
	<rdfs:comment>encodes the starting point of musical material in terms of musical time, i.e., a (potentially negative) count of measures plus a beat location.</rdfs:comment>
	</owl:DatatypeProperty>
	<owl:DatatypeProperty rdf:ID="origin.tstamp2_att.origin.timestamp.musical.attribute.origin.tstamp2__mei_data.MEASUREBEAT">
		<rdfs:range rdf:resource="&datatypes;data.MEASUREBEAT"/>
		<rdfs:label>origin.tstamp2</rdfs:label>
	<rdfs:comment>encodes the ending point of musical material in terms of musical time, i.e., a count of measures plus a beat location. The values are relative to the measure identified by @origin.tstamp.</rdfs:comment>
	</owl:DatatypeProperty>
	<owl:DatatypeProperty rdf:ID="num_att.pad.log.attribute.num__xs_decimal">
		<rdfs:range rdf:resource="&xs;decimal"/>
		<rdfs:label>num</rdfs:label>
	<rdfs:comment>Amount of &quot;padding&quot; to be added, in interline units; that is, in units of 1/2 the distance between adjacent staff lines.</rdfs:comment>
	</owl:DatatypeProperty>
	<owl:DatatypeProperty rdf:ID="page.height_att.pages.attribute.page.height__mei_data.MEASUREMENTABS">
		<rdfs:range rdf:resource="&datatypes;data.MEASUREMENTABS"/>
		<rdfs:label>page.height</rdfs:label>
	<rdfs:comment>Specifies the height of the page; may be expressed in real-world units or staff steps.</rdfs:comment>
	</owl:DatatypeProperty>
	<owl:DatatypeProperty rdf:ID="page.width_att.pages.attribute.page.width__mei_data.MEASUREMENTABS">
		<rdfs:range rdf:resource="&datatypes;data.MEASUREMENTABS"/>
		<rdfs:label>page.width</rdfs:label>
	<rdfs:comment>Describes the width of the page; may be expressed in real-world units or staff steps.</rdfs:comment>
	</owl:DatatypeProperty>
	<owl:DatatypeProperty rdf:ID="page.topmar_att.pages.attribute.page.topmar__mei_data.MEASUREMENTABS">
		<rdfs:range rdf:resource="&datatypes;data.MEASUREMENTABS"/>
		<rdfs:label>page.topmar</rdfs:label>
	<rdfs:comment>Indicates the amount of whitespace at the top of a page.</rdfs:comment>
	</owl:DatatypeProperty>
	<owl:DatatypeProperty rdf:ID="page.botmar_att.pages.attribute.page.botmar__mei_data.MEASUREMENTABS">
		<rdfs:range rdf:resource="&datatypes;data.MEASUREMENTABS"/>
		<rdfs:label>page.botmar</rdfs:label>
	<rdfs:comment>Indicates the amount of whitespace at the bottom of a page.</rdfs:comment>
	</owl:DatatypeProperty>
	<owl:DatatypeProperty rdf:ID="page.leftmar_att.pages.attribute.page.leftmar__mei_data.MEASUREMENTABS">
		<rdfs:range rdf:resource="&datatypes;data.MEASUREMENTABS"/>
		<rdfs:label>page.leftmar</rdfs:label>
	<rdfs:comment>Indicates the amount of whitespace at the left side of a page.</rdfs:comment>
	</owl:DatatypeProperty>
	<owl:DatatypeProperty rdf:ID="page.rightmar_att.pages.attribute.page.rightmar__mei_data.MEASUREMENTABS">
		<rdfs:range rdf:resource="&datatypes;data.MEASUREMENTABS"/>
		<rdfs:label>page.rightmar</rdfs:label>
	<rdfs:comment>Indicates the amount of whitespace at the right side of a page.</rdfs:comment>
	</owl:DatatypeProperty>
	<owl:DatatypeProperty rdf:ID="page.panels_att.pages.attribute.page.panels__mei_data.PAGE.PANELS">
		<rdfs:range rdf:resource="&datatypes;data.PAGE.PANELS"/>
		<rdfs:label>page.panels</rdfs:label>
	<rdfs:comment>Indicates the number of logical pages to be rendered on a single physical page.</rdfs:comment>
	</owl:DatatypeProperty>
	<owl:DatatypeProperty rdf:ID="page.scale_att.pages.attribute.page.scale__mei_data.PGSCALE">
		<rdfs:range rdf:resource="&datatypes;data.PGSCALE"/>
		<rdfs:label>page.scale</rdfs:label>
	<rdfs:comment>Indicates how the page should be scaled when rendered.</rdfs:comment>
	</owl:DatatypeProperty>
	<rdfs:Datatype rdf:ID="NS_folium_att.pb.vis.attribute.folium_UNType">
		<owl:equivalentClass><rdfs:Datatype>
		<owl:onDatatype rdf:resource="&xs;token"/><owl:withRestrictions rdf:parseType="Collection"><rdf:Description><xs:enumeration>verso</xs:enumeration></rdf:Description><rdf:Description><xs:enumeration>recto</xs:enumeration></rdf:Description></owl:withRestrictions></rdfs:Datatype></owl:equivalentClass></rdfs:Datatype>
	<owl:DatatypeProperty rdf:ID="folium_att.pb.vis.attribute.folium__NS_folium_att.pb.vis.attribute.folium_UNType">
		<rdfs:range rdf:resource="#NS_folium_att.pb.vis.attribute.folium_UNType"/>
		<rdfs:label>folium</rdfs:label>
	<rdfs:comment>States the side of a leaf (as in a manuscript) on which the content following the &lt;pb&gt; element occurs.</rdfs:comment>
	</owl:DatatypeProperty>
	<owl:DatatypeProperty rdf:ID="pname_att.pitch.attribute.pname__mei_data.PITCHNAME">
		<rdfs:range rdf:resource="&datatypes;data.PITCHNAME"/>
		<rdfs:label>pname</rdfs:label>
	<rdfs:comment>Contains a written pitch name.</rdfs:comment>
	</owl:DatatypeProperty>
	<owl:DatatypeProperty rdf:ID="place_att.placement.attribute.place__mei_data.STAFFREL">
		<rdfs:range rdf:resource="&datatypes;data.STAFFREL"/>
		<rdfs:label>place</rdfs:label>
	<rdfs:comment>Captures the placement of the item with respect to the staff with which it is associated.</rdfs:comment>
	</owl:DatatypeProperty>
	<rdfs:Datatype rdf:ID="NS_plist_att.plist.attribute.plist_UNType">
		<owl:equivalentClass><rdfs:Datatype>
		<owl:onDatatype rdf:resource="plist_att.plist.attribute.plist_NS_plist_att.plist.attribute.plist_UNType_UNType"/><owl:withRestrictions rdf:parseType="Collection"><rdf:Description><xs:minLength>1</xs:minLength></rdf:Description></owl:withRestrictions></rdfs:Datatype></owl:equivalentClass></rdfs:Datatype>
	<rdfs:Datatype rdf:ID="plist_att.plist.attribute.plist_NS_plist_att.plist.attribute.plist_UNType_UNType">
		<owl:equivalentClass><rdfs:Datatype>
		<owl:oneOf><rdf:Description><rdf:type rdf:resource="#List"/><rdf:first>mei:data.URI</rdf:first><rdf:rest rdf:resource="#nil"/></rdf:Description></owl:oneOf></rdfs:Datatype></owl:equivalentClass></rdfs:Datatype>
	<owl:DatatypeProperty rdf:ID="plist_att.plist.attribute.plist__NS_plist_att.plist.attribute.plist_UNType">
		<rdfs:range rdf:resource="#NS_plist_att.plist.attribute.plist_UNType"/>
		<rdfs:label>plist</rdfs:label>
	<rdfs:comment>Contains a space separated list of references that identify active participants in a collection/relationship, such as notes under a phrase mark; that is, the entities pointed &quot;from&quot;.</rdfs:comment>
	</owl:DatatypeProperty>
	<rdfs:Datatype rdf:ID="NS_target_att.pointing.attribute.target_UNType">
		<owl:equivalentClass><rdfs:Datatype>
		<owl:onDatatype rdf:resource="target_att.pointing.attribute.target_NS_target_att.pointing.attribute.target_UNType_UNType"/><owl:withRestrictions rdf:parseType="Collection"><rdf:Description><xs:minLength>1</xs:minLength></rdf:Description></owl:withRestrictions></rdfs:Datatype></owl:equivalentClass></rdfs:Datatype>
	<rdfs:Datatype rdf:ID="target_att.pointing.attribute.target_NS_target_att.pointing.attribute.target_UNType_UNType">
		<owl:equivalentClass><rdfs:Datatype>
		<owl:oneOf><rdf:Description><rdf:type rdf:resource="#List"/><rdf:first>mei:data.URI</rdf:first><rdf:rest rdf:resource="#nil"/></rdf:Description></owl:oneOf></rdfs:Datatype></owl:equivalentClass></rdfs:Datatype>
	<owl:DatatypeProperty rdf:ID="target_att.pointing.attribute.target__NS_target_att.pointing.attribute.target_UNType">
		<rdfs:range rdf:resource="#NS_target_att.pointing.attribute.target_UNType"/>
		<rdfs:label>target</rdfs:label>
	<rdfs:comment>Allows the use of one or more previously-undeclared URIs to identify passive participants in a relationship; that is, the entities pointed &quot;to&quot;.</rdfs:comment>
	</owl:DatatypeProperty>
	<owl:DatatypeProperty rdf:ID="targettype_att.pointing.attribute.targettype__xs_NMTOKEN">
		<rdfs:range rdf:resource="&xs;NMTOKEN"/>
		<rdfs:label>targettype</rdfs:label>
	<rdfs:comment>Characterization of target resource(s) using any convenient classification scheme or typology.</rdfs:comment>
	</owl:DatatypeProperty>
	<rdfs:Datatype rdf:ID="NS_quantity_att.quantity.attribute.quantity_UNType">
		<owl:equivalentClass><rdfs:Datatype>
		<owl:onDatatype rdf:resource="&xs;decimal"/><owl:withRestrictions rdf:parseType="Collection"><rdf:Description><xs:minInclusive>0</xs:minInclusive></rdf:Description></owl:withRestrictions></rdfs:Datatype></owl:equivalentClass></rdfs:Datatype>
	<owl:DatatypeProperty rdf:ID="quantity_att.quantity.attribute.quantity__NS_quantity_att.quantity.attribute.quantity_UNType">
		<rdfs:range rdf:resource="#NS_quantity_att.quantity.attribute.quantity_UNType"/>
		<rdfs:label>quantity</rdfs:label>
	<rdfs:comment>Numeric value capturing a measurement or count. Can only be interpreted in combination with the unit or currency attribute.</rdfs:comment>
	</owl:DatatypeProperty>
	<owl:DatatypeProperty rdf:ID="size_att.relativesize.attribute.size__mei_data.SIZE">
		<rdfs:range rdf:resource="&datatypes;data.SIZE"/>
		<rdfs:label>size</rdfs:label>
	<rdfs:comment>Describes the relative size of a feature.</rdfs:comment>
	</owl:DatatypeProperty>
	<rdfs:Datatype rdf:ID="NS_resp_att.responsibility.attribute.resp_UNType">
		<owl:equivalentClass><rdfs:Datatype>
		<owl:onDatatype rdf:resource="resp_att.responsibility.attribute.resp_NS_resp_att.responsibility.attribute.resp_UNType_UNType"/><owl:withRestrictions rdf:parseType="Collection"><rdf:Description><xs:minLength>1</xs:minLength></rdf:Description></owl:withRestrictions></rdfs:Datatype></owl:equivalentClass></rdfs:Datatype>
	<rdfs:Datatype rdf:ID="resp_att.responsibility.attribute.resp_NS_resp_att.responsibility.attribute.resp_UNType_UNType">
		<owl:equivalentClass><rdfs:Datatype>
		<owl:oneOf><rdf:Description><rdf:type rdf:resource="#List"/><rdf:first>mei:data.URI</rdf:first><rdf:rest rdf:resource="#nil"/></rdf:Description></owl:oneOf></rdfs:Datatype></owl:equivalentClass></rdfs:Datatype>
	<owl:DatatypeProperty rdf:ID="resp_att.responsibility.attribute.resp__NS_resp_att.responsibility.attribute.resp_UNType">
		<rdfs:range rdf:resource="#NS_resp_att.responsibility.attribute.resp_UNType"/>
		<rdfs:label>resp</rdfs:label>
	<rdfs:comment>Indicates the agent(s) responsible for some aspect of the text's creation, transcription, editing, or encoding. Its value must point to one or more identifiers declared in the document header.</rdfs:comment>
	</owl:DatatypeProperty>
	<rdfs:Datatype rdf:ID="NS_form_att.sb.vis.attribute.form_UNType">
		<owl:equivalentClass><rdfs:Datatype>
		<owl:onDatatype rdf:resource="&xs;token"/><owl:withRestrictions rdf:parseType="Collection"><rdf:Description><xs:enumeration>hash</xs:enumeration></rdf:Description></owl:withRestrictions></rdfs:Datatype></owl:equivalentClass></rdfs:Datatype>
	<owl:DatatypeProperty rdf:ID="form_att.sb.vis.attribute.form__NS_form_att.sb.vis.attribute.form_UNType">
		<rdfs:range rdf:resource="#NS_form_att.sb.vis.attribute.form_UNType"/>
		<rdfs:label>form</rdfs:label>
	<rdfs:comment>Indicates whether hash marks should be rendered between systems. See Read, p. 436, ex. 26-3.</rdfs:comment>
	</owl:DatatypeProperty>
	<owl:DatatypeProperty rdf:ID="scale_att.scalable.attribute.scale__mei_data.PERCENT">
		<rdfs:range rdf:resource="&datatypes;data.PERCENT"/>
		<rdfs:label>scale</rdfs:label>
	<rdfs:comment>Scale factor to be applied to the feature to make it the desired display size.</rdfs:comment>
	</owl:DatatypeProperty>
	<owl:DatatypeProperty rdf:ID="tune.pname_att.scoreDef.ges.attribute.tune.pname__mei_data.PITCHNAME">
		<rdfs:range rdf:resource="&datatypes;data.PITCHNAME"/>
		<rdfs:label>tune.pname</rdfs:label>
	<rdfs:comment>Holds the pitch name of a tuning reference pitch.</rdfs:comment>
	</owl:DatatypeProperty>
	<owl:DatatypeProperty rdf:ID="tune.Hz_att.scoreDef.ges.attribute.tune.Hz__xs_decimal">
		<rdfs:range rdf:resource="&xs;decimal"/>
		<rdfs:label>tune.Hz</rdfs:label>
	<rdfs:comment>Holds a value for cycles per second, i.e., Hertz, for a tuning reference pitch.</rdfs:comment>
	</owl:DatatypeProperty>
	<owl:DatatypeProperty rdf:ID="tune.temper_att.scoreDef.ges.attribute.tune.temper__mei_data.TEMPERAMENT">
		<rdfs:range rdf:resource="&datatypes;data.TEMPERAMENT"/>
		<rdfs:label>tune.temper</rdfs:label>
	<rdfs:comment>Provides an indication of the tuning system, 'just', for example.</rdfs:comment>
	</owl:DatatypeProperty>
	<rdfs:Datatype rdf:ID="NS_vu.height_att.scoreDef.vis.attribute.vu.height_UNType">
		<owl:equivalentClass><rdfs:Datatype>
		<owl:onDatatype rdf:resource="&xs;token"/><owl:withRestrictions rdf:parseType="Collection"><rdf:Description><xs:pattern>\d+(\.\d+)?(cm|mm|in|pt|pc)</xs:pattern></rdf:Description></owl:withRestrictions></rdfs:Datatype></owl:equivalentClass></rdfs:Datatype>
	<owl:DatatypeProperty rdf:ID="vu.height_att.scoreDef.vis.attribute.vu.height__NS_vu.height_att.scoreDef.vis.attribute.vu.height_UNType">
		<rdfs:range rdf:resource="#NS_vu.height_att.scoreDef.vis.attribute.vu.height_UNType"/>
		<rdfs:label>vu.height</rdfs:label>
	<rdfs:comment>Defines the height of a &quot;virtual unit&quot; (vu) in terms of real-world units. A single vu is half the distance between the vertical center point of a staff line and that of an adjacent staff line.</rdfs:comment>
	</owl:DatatypeProperty>
	<owl:DatatypeProperty rdf:ID="restart_att.section.vis.attribute.restart__mei_data.BOOLEAN">
		<rdfs:range rdf:resource="&datatypes;data.BOOLEAN"/>
		<rdfs:label>restart</rdfs:label>
	<rdfs:comment>Indicates that staves begin again with this section.</rdfs:comment>
	</owl:DatatypeProperty>
	<owl:DatatypeProperty rdf:ID="seq_att.sequence.attribute.seq__xs_positiveInteger">
		<rdfs:range rdf:resource="&xs;positiveInteger"/>
		<rdfs:label>seq</rdfs:label>
	<rdfs:comment>Used to assign a sequence number related to the order in which the encoded features carrying this attribute are believed to have occurred.</rdfs:comment>
	</owl:DatatypeProperty>
	<owl:DatatypeProperty rdf:ID="slash_att.slashcount.attribute.slash__mei_data.SLASH">
		<rdfs:range rdf:resource="&datatypes;data.SLASH"/>
		<rdfs:label>slash</rdfs:label>
	<rdfs:comment>Indicates the number of slashes present.</rdfs:comment>
	</owl:DatatypeProperty>
	<rdfs:Datatype rdf:ID="NS_slur_att.slurpresent.attribute.slur_UNType">
		<owl:equivalentClass><rdfs:Datatype>
		<owl:onDatatype rdf:resource="slur_att.slurpresent.attribute.slur_NS_slur_att.slurpresent.attribute.slur_UNType_UNType"/><owl:withRestrictions rdf:parseType="Collection"><rdf:Description><xs:minLength>1</xs:minLength></rdf:Description></owl:withRestrictions></rdfs:Datatype></owl:equivalentClass></rdfs:Datatype>
	<rdfs:Datatype rdf:ID="slur_att.slurpresent.attribute.slur_NS_slur_att.slurpresent.attribute.slur_UNType_UNType">
		<owl:equivalentClass><rdfs:Datatype>
		<owl:oneOf><rdf:Description><rdf:type rdf:resource="#List"/><rdf:first>mei:data.SLUR</rdf:first><rdf:rest rdf:resource="#nil"/></rdf:Description></owl:oneOf></rdfs:Datatype></owl:equivalentClass></rdfs:Datatype>
	<owl:DatatypeProperty rdf:ID="slur_att.slurpresent.attribute.slur__NS_slur_att.slurpresent.attribute.slur_UNType">
		<rdfs:range rdf:resource="#NS_slur_att.slurpresent.attribute.slur_UNType"/>
		<rdfs:label>slur</rdfs:label>
	<rdfs:comment>Indicates that this element participates in a slur. If visual information about the slur needs to be recorded, then a &lt;slur&gt; element should be employed.</rdfs:comment>
	</owl:DatatypeProperty>
	<owl:DatatypeProperty rdf:ID="compressable_att.space.vis.attribute.compressable__mei_data.BOOLEAN">
		<rdfs:range rdf:resource="&datatypes;data.BOOLEAN"/>
		<rdfs:label>compressable</rdfs:label>
	<rdfs:comment>Indicates whether a space is 'compressible', i.e., if it may be removed at the discretion of processing software.</rdfs:comment>
	</owl:DatatypeProperty>
	<owl:DatatypeProperty rdf:ID="spacing.packexp_att.spacing.attribute.spacing.packexp__xs_decimal">
		<rdfs:range rdf:resource="&xs;decimal"/>
		<rdfs:label>spacing.packexp</rdfs:label>
	<rdfs:comment>Describes a note's spacing relative to its time value.</rdfs:comment>
	</owl:DatatypeProperty>
	<owl:DatatypeProperty rdf:ID="spacing.packfact_att.spacing.attribute.spacing.packfact__xs_decimal">
		<rdfs:range rdf:resource="&xs;decimal"/>
		<rdfs:label>spacing.packfact</rdfs:label>
	<rdfs:comment>Describes the note spacing of output.</rdfs:comment>
	</owl:DatatypeProperty>
	<owl:DatatypeProperty rdf:ID="spacing.staff_att.spacing.attribute.spacing.staff__mei_data.MEASUREMENTREL">
		<rdfs:range rdf:resource="&datatypes;data.MEASUREMENTREL"/>
		<rdfs:label>spacing.staff</rdfs:label>
	<rdfs:comment>Specifies the minimum amount of space between adjacent staves in the same system; measured from the bottom line of the staff above to the top line of the staff below.</rdfs:comment>
	</owl:DatatypeProperty>
	<rdfs:Datatype rdf:ID="NS_spacing.system_att.spacing.attribute.spacing.system_UNType">
		<owl:equivalentClass><rdfs:Datatype>
		<owl:onDatatype rdf:resource="spacing.system_att.spacing.attribute.spacing.system_NS_spacing.system_att.spacing.attribute.spacing.system_UNType_UNType"/><owl:withRestrictions rdf:parseType="Collection"><rdf:Description><xs:minLength>1</xs:minLength></rdf:Description><rdf:Description><xs:maxLength>2</xs:maxLength></rdf:Description></owl:withRestrictions></rdfs:Datatype></owl:equivalentClass></rdfs:Datatype>
	<rdfs:Datatype rdf:ID="spacing.system_att.spacing.attribute.spacing.system_NS_spacing.system_att.spacing.attribute.spacing.system_UNType_UNType">
		<owl:equivalentClass><rdfs:Datatype>
		<owl:oneOf><rdf:Description><rdf:type rdf:resource="#List"/><rdf:first>NS_spacing.system_att.spacing.attribute.spacing.system_UNType_spacing.system_att.spacing.attribute.spacing.system_NS_spacing.system_att.spacing.attribute.spacing.system_UNType_UNType_UNType</rdf:first><rdf:rest rdf:resource="#nil"/></rdf:Description></owl:oneOf></rdfs:Datatype></owl:equivalentClass></rdfs:Datatype>
	<rdfs:Datatype rdf:ID="NS_spacing.system_att.spacing.attribute.spacing.system_UNType_spacing.system_att.spacing.attribute.spacing.system_NS_spacing.system_att.spacing.attribute.spacing.system_UNType_UNType_UNType">
		<owl:equivalentClass><rdfs:Datatype>
		<owl:unionOf rdf:parseType="Collection"><rdf:Description rdf:about="mei:data.MEASUREMENTREL"/><rdf:Description rdf:about="mei:data.MEASUREMENTREL"/></owl:unionOf></rdfs:Datatype></owl:equivalentClass></rdfs:Datatype>
	<owl:DatatypeProperty rdf:ID="spacing.system_att.spacing.attribute.spacing.system__NS_spacing.system_att.spacing.attribute.spacing.system_UNType">
		<rdfs:range rdf:resource="#NS_spacing.system_att.spacing.attribute.spacing.system_UNType"/>
		<rdfs:label>spacing.system</rdfs:label>
	<rdfs:comment>Describes the space between adjacent systems; a pair of space-separated values (minimum and maximum, respectively) provides a range between which a rendering system-supplied value may fall, while a single value indicates a fixed amount of space; that is, the minimum and maximum values are equal.</rdfs:comment>
	</owl:DatatypeProperty>
	<owl:DatatypeProperty rdf:ID="def_att.staff.log.attribute.def__mei_data.URI">
		<rdfs:range rdf:resource="&datatypes;data.URI"/>
		<rdfs:label>def</rdfs:label>
	<rdfs:comment>Provides a mechanism for linking the staff to a staffDef element.</rdfs:comment>
	</owl:DatatypeProperty>
	<owl:DatatypeProperty rdf:ID="grid.show_att.staffDef.vis.attribute.grid.show__mei_data.BOOLEAN">
		<rdfs:range rdf:resource="&datatypes;data.BOOLEAN"/>
		<rdfs:label>grid.show</rdfs:label>
	<rdfs:comment>Determines whether to display guitar chord grids.</rdfs:comment>
	</owl:DatatypeProperty>
	<owl:DatatypeProperty rdf:ID="layerscheme_att.staffDef.vis.attribute.layerscheme__mei_data.LAYERSCHEME">
		<rdfs:range rdf:resource="&datatypes;data.LAYERSCHEME"/>
		<rdfs:label>layerscheme</rdfs:label>
	<rdfs:comment>Indicates the number of layers and their stem directions.</rdfs:comment>
	</owl:DatatypeProperty>
	<owl:DatatypeProperty rdf:ID="lines_att.staffDef.vis.attribute.lines__xs_positiveInteger">
		<rdfs:range rdf:resource="&xs;positiveInteger"/>
		<rdfs:label>lines</rdfs:label>
	<rdfs:comment>Indicates the number of staff lines.</rdfs:comment>
	</owl:DatatypeProperty>
	<rdfs:Datatype rdf:ID="NS_lines.color_att.staffDef.vis.attribute.lines.color_UNType">
		<owl:equivalentClass><rdfs:Datatype>
		<owl:onDatatype rdf:resource="lines.color_att.staffDef.vis.attribute.lines.color_NS_lines.color_att.staffDef.vis.attribute.lines.color_UNType_UNType"/><owl:withRestrictions rdf:parseType="Collection"><rdf:Description><xs:minLength>1</xs:minLength></rdf:Description></owl:withRestrictions></rdfs:Datatype></owl:equivalentClass></rdfs:Datatype>
	<rdfs:Datatype rdf:ID="lines.color_att.staffDef.vis.attribute.lines.color_NS_lines.color_att.staffDef.vis.attribute.lines.color_UNType_UNType">
		<owl:equivalentClass><rdfs:Datatype>
		<owl:oneOf><rdf:Description><rdf:type rdf:resource="#List"/><rdf:first>mei:data.COLOR</rdf:first><rdf:rest rdf:resource="#nil"/></rdf:Description></owl:oneOf></rdfs:Datatype></owl:equivalentClass></rdfs:Datatype>
	<owl:DatatypeProperty rdf:ID="lines.color_att.staffDef.vis.attribute.lines.color__NS_lines.color_att.staffDef.vis.attribute.lines.color_UNType">
		<rdfs:range rdf:resource="#NS_lines.color_att.staffDef.vis.attribute.lines.color_UNType"/>
		<rdfs:label>lines.color</rdfs:label>
	<rdfs:comment>Captures the colors of the staff lines. The value is structured; that is, it should have the same number of space-separated RGB values as the number of lines indicated by the lines attribute. A line can be made invisible by assigning it the same RGB value as the background, usually white.</rdfs:comment>
	</owl:DatatypeProperty>
	<owl:DatatypeProperty rdf:ID="lines.visible_att.staffDef.vis.attribute.lines.visible__mei_data.BOOLEAN">
		<rdfs:range rdf:resource="&datatypes;data.BOOLEAN"/>
		<rdfs:label>lines.visible</rdfs:label>
	<rdfs:comment>Records whether all staff lines are visible.</rdfs:comment>
	</owl:DatatypeProperty>
	<owl:DatatypeProperty rdf:ID="spacing_att.staffDef.vis.attribute.spacing__mei_data.MEASUREMENTREL">
		<rdfs:range rdf:resource="&datatypes;data.MEASUREMENTREL"/>
		<rdfs:label>spacing</rdfs:label>
	<rdfs:comment>Records the absolute distance (as opposed to the relative distances recorded in &lt;scoreDef&gt; elements) between this staff and the preceding one in the same system. This value is meaningless for the first staff in a system since the spacing.system attribute indicates the spacing between systems.</rdfs:comment>
	</owl:DatatypeProperty>
	<rdfs:Datatype rdf:ID="NS_symbol_att.staffgroupingsym.attribute.symbol_UNType">
		<owl:equivalentClass><rdfs:Datatype>
		<owl:onDatatype rdf:resource="&xs;token"/><owl:withRestrictions rdf:parseType="Collection"><rdf:Description><xs:enumeration>brace</xs:enumeration></rdf:Description><rdf:Description><xs:enumeration>bracket</xs:enumeration></rdf:Description><rdf:Description><xs:enumeration>bracketsq</xs:enumeration></rdf:Description><rdf:Description><xs:enumeration>line</xs:enumeration></rdf:Description><rdf:Description><xs:enumeration>none</xs:enumeration></rdf:Description></owl:withRestrictions></rdfs:Datatype></owl:equivalentClass></rdfs:Datatype>
	<owl:DatatypeProperty rdf:ID="symbol_att.staffgroupingsym.attribute.symbol__NS_symbol_att.staffgroupingsym.attribute.symbol_UNType">
		<rdfs:range rdf:resource="#NS_symbol_att.staffgroupingsym.attribute.symbol_UNType"/>
		<rdfs:label>symbol</rdfs:label>
	<rdfs:comment>Specifies the symbol used to group a set of staves.</rdfs:comment>
	</owl:DatatypeProperty>
	<owl:DatatypeProperty rdf:ID="barthru_att.staffGrp.vis.attribute.barthru__mei_data.BOOLEAN">
		<rdfs:range rdf:resource="&datatypes;data.BOOLEAN"/>
		<rdfs:label>barthru</rdfs:label>
	<rdfs:comment>Indicates whether bar lines go across the space between staves (true) or are only drawn across the lines of each staff (false).</rdfs:comment>
	</owl:DatatypeProperty>
	<rdfs:Datatype rdf:ID="NS_staff_att.staffident.attribute.staff_UNType">
		<owl:equivalentClass><rdfs:Datatype>
		<owl:onDatatype rdf:resource="staff_att.staffident.attribute.staff_NS_staff_att.staffident.attribute.staff_UNType_UNType"/><owl:withRestrictions rdf:parseType="Collection"><rdf:Description><xs:minLength>1</xs:minLength></rdf:Description></owl:withRestrictions></rdfs:Datatype></owl:equivalentClass></rdfs:Datatype>
	<rdfs:Datatype rdf:ID="staff_att.staffident.attribute.staff_NS_staff_att.staffident.attribute.staff_UNType_UNType">
		<owl:equivalentClass><rdfs:Datatype>
		<owl:oneOf><rdf:Description><rdf:type rdf:resource="#List"/><rdf:first>xs:positiveInteger</rdf:first><rdf:rest rdf:resource="#nil"/></rdf:Description></owl:oneOf></rdfs:Datatype></owl:equivalentClass></rdfs:Datatype>
	<owl:DatatypeProperty rdf:ID="staff_att.staffident.attribute.staff__NS_staff_att.staffident.attribute.staff_UNType">
		<rdfs:range rdf:resource="#NS_staff_att.staffident.attribute.staff_UNType"/>
		<rdfs:label>staff</rdfs:label>
	<rdfs:comment>Signifies the staff on which a notated event occurs or to which a control event applies. Mandatory when applicable.</rdfs:comment>
	</owl:DatatypeProperty>
	<owl:DatatypeProperty rdf:ID="loc_att.staffloc.attribute.loc__mei_data.STAFFLOC">
		<rdfs:range rdf:resource="&datatypes;data.STAFFLOC"/>
		<rdfs:label>loc</rdfs:label>
	<rdfs:comment>Holds the staff location of the feature.</rdfs:comment>
	</owl:DatatypeProperty>
	<owl:DatatypeProperty rdf:ID="ploc_att.staffloc.pitched.attribute.ploc__mei_data.PITCHNAME">
		<rdfs:range rdf:resource="&datatypes;data.PITCHNAME"/>
		<rdfs:label>ploc</rdfs:label>
	<rdfs:comment>Captures staff location in terms of written pitch name.</rdfs:comment>
	</owl:DatatypeProperty>
	<owl:DatatypeProperty rdf:ID="oloc_att.staffloc.pitched.attribute.oloc__mei_data.OCTAVE">
		<rdfs:range rdf:resource="&datatypes;data.OCTAVE"/>
		<rdfs:label>oloc</rdfs:label>
	<rdfs:comment>Records staff location in terms of written octave.</rdfs:comment>
	</owl:DatatypeProperty>
	<owl:DatatypeProperty rdf:ID="endid_att.startendid.attribute.endid__mei_data.URI">
		<rdfs:range rdf:resource="&datatypes;data.URI"/>
		<rdfs:label>endid</rdfs:label>
	<rdfs:comment>Indicates the final element in a sequence of events to which the feature applies.</rdfs:comment>
	</owl:DatatypeProperty>
	<owl:DatatypeProperty rdf:ID="startid_att.startid.attribute.startid__mei_data.URI">
		<rdfs:range rdf:resource="&datatypes;data.URI"/>
		<rdfs:label>startid</rdfs:label>
	<rdfs:comment>Holds a reference to the first element in a sequence of events to which the feature applies.</rdfs:comment>
	</owl:DatatypeProperty>
	<owl:DatatypeProperty rdf:ID="stem.dir_att.stems.attribute.stem.dir__mei_data.STEMDIRECTION">
		<rdfs:range rdf:resource="&datatypes;data.STEMDIRECTION"/>
		<rdfs:label>stem.dir</rdfs:label>
	<rdfs:comment>Describes the direction of a stem.</rdfs:comment>
	</owl:DatatypeProperty>
	<owl:DatatypeProperty rdf:ID="stem.len_att.stems.attribute.stem.len__mei_data.MEASUREMENTABS">
		<rdfs:range rdf:resource="&datatypes;data.MEASUREMENTABS"/>
		<rdfs:label>stem.len</rdfs:label>
	<rdfs:comment>Encodes the stem length.</rdfs:comment>
	</owl:DatatypeProperty>
	<owl:DatatypeProperty rdf:ID="stem.mod_att.stems.attribute.stem.mod__mei_data.STEMMODIFIER">
		<rdfs:range rdf:resource="&datatypes;data.STEMMODIFIER"/>
		<rdfs:label>stem.mod</rdfs:label>
	<rdfs:comment>Encodes any stem &quot;modifiers&quot;; that is, symbols rendered on the stem, such as tremolo or Sprechstimme indicators.</rdfs:comment>
	</owl:DatatypeProperty>
	<owl:DatatypeProperty rdf:ID="stem.pos_att.stems.attribute.stem.pos__mei_data.STEMPOSITION">
		<rdfs:range rdf:resource="&datatypes;data.STEMPOSITION"/>
		<rdfs:label>stem.pos</rdfs:label>
	<rdfs:comment>Records the position of the stem in relation to the note head(s).</rdfs:comment>
	</owl:DatatypeProperty>
	<owl:DatatypeProperty rdf:ID="stem.x_att.stems.attribute.stem.x__xs_decimal">
		<rdfs:range rdf:resource="&xs;decimal"/>
		<rdfs:label>stem.x</rdfs:label>
	<rdfs:comment>Records the output x coordinate of the stem's attachment point.</rdfs:comment>
	</owl:DatatypeProperty>
	<owl:DatatypeProperty rdf:ID="stem.y_att.stems.attribute.stem.y__xs_decimal">
		<rdfs:range rdf:resource="&xs;decimal"/>
		<rdfs:label>stem.y</rdfs:label>
	<rdfs:comment>Records the output y coordinate of the stem's attachment point.</rdfs:comment>
	</owl:DatatypeProperty>
	<rdfs:Datatype rdf:ID="NS_con_att.syl.log.attribute.con_UNType">
		<owl:equivalentClass><rdfs:Datatype>
		<owl:onDatatype rdf:resource="&xs;token"/><owl:withRestrictions rdf:parseType="Collection"><rdf:Description><xs:enumeration>s</xs:enumeration></rdf:Description><rdf:Description><xs:enumeration>d</xs:enumeration></rdf:Description><rdf:Description><xs:enumeration>u</xs:enumeration></rdf:Description><rdf:Description><xs:enumeration>t</xs:enumeration></rdf:Description><rdf:Description><xs:enumeration>c</xs:enumeration></rdf:Description><rdf:Description><xs:enumeration>v</xs:enumeration></rdf:Description><rdf:Description><xs:enumeration>i</xs:enumeration></rdf:Description><rdf:Description><xs:enumeration>b</xs:enumeration></rdf:Description></owl:withRestrictions></rdfs:Datatype></owl:equivalentClass></rdfs:Datatype>
	<owl:DatatypeProperty rdf:ID="con_att.syl.log.attribute.con__NS_con_att.syl.log.attribute.con_UNType">
		<rdfs:range rdf:resource="#NS_con_att.syl.log.attribute.con_UNType"/>
		<rdfs:label>con</rdfs:label>
	<rdfs:comment>Describes the symbols typically used to indicate breaks between syllables and their functions.</rdfs:comment>
	</owl:DatatypeProperty>
	<rdfs:Datatype rdf:ID="NS_wordpos_att.syl.log.attribute.wordpos_UNType">
		<owl:equivalentClass><rdfs:Datatype>
		<owl:onDatatype rdf:resource="&xs;token"/><owl:withRestrictions rdf:parseType="Collection"><rdf:Description><xs:enumeration>i</xs:enumeration></rdf:Description><rdf:Description><xs:enumeration>m</xs:enumeration></rdf:Description><rdf:Description><xs:enumeration>t</xs:enumeration></rdf:Description></owl:withRestrictions></rdfs:Datatype></owl:equivalentClass></rdfs:Datatype>
	<owl:DatatypeProperty rdf:ID="wordpos_att.syl.log.attribute.wordpos__NS_wordpos_att.syl.log.attribute.wordpos_UNType">
		<rdfs:range rdf:resource="#NS_wordpos_att.syl.log.attribute.wordpos_UNType"/>
		<rdfs:label>wordpos</rdfs:label>
	<rdfs:comment>Records the position of a syllable within a word.</rdfs:comment>
	</owl:DatatypeProperty>
	<owl:DatatypeProperty rdf:ID="syl_att.syltext.attribute.syl__xs_string">
		<rdfs:range rdf:resource="&xs;string"/>
		<rdfs:label>syl</rdfs:label>
	<rdfs:comment>Holds an associated sung text syllable.</rdfs:comment>
	</owl:DatatypeProperty>
	<owl:DatatypeProperty rdf:ID="system.leftline_att.systems.attribute.system.leftline__mei_data.BOOLEAN">
		<rdfs:range rdf:resource="&datatypes;data.BOOLEAN"/>
		<rdfs:label>system.leftline</rdfs:label>
	<rdfs:comment>Indicates whether the staves are joined at the left by a continuous line. The default value is &quot;true&quot;. Do not confuse this with the heavy vertical line used as a grouping symbol.</rdfs:comment>
	</owl:DatatypeProperty>
	<owl:DatatypeProperty rdf:ID="system.leftmar_att.systems.attribute.system.leftmar__mei_data.MEASUREMENTABS">
		<rdfs:range rdf:resource="&datatypes;data.MEASUREMENTABS"/>
		<rdfs:label>system.leftmar</rdfs:label>
	<rdfs:comment>Describes the amount of whitespace at the left system margin relative to page.leftmar.</rdfs:comment>
	</owl:DatatypeProperty>
	<owl:DatatypeProperty rdf:ID="system.rightmar_att.systems.attribute.system.rightmar__mei_data.MEASUREMENTABS">
		<rdfs:range rdf:resource="&datatypes;data.MEASUREMENTABS"/>
		<rdfs:label>system.rightmar</rdfs:label>
	<rdfs:comment>Describes the amount of whitespace at the right system margin relative to page.rightmar.</rdfs:comment>
	</owl:DatatypeProperty>
	<owl:DatatypeProperty rdf:ID="system.topmar_att.systems.attribute.system.topmar__mei_data.MEASUREMENTABS">
		<rdfs:range rdf:resource="&datatypes;data.MEASUREMENTABS"/>
		<rdfs:label>system.topmar</rdfs:label>
	<rdfs:comment>Describes the distance from page's top edge to the first system; used for first page only.</rdfs:comment>
	</owl:DatatypeProperty>
	<rdfs:Datatype rdf:ID="NS_evaluate_att.targeteval.attribute.evaluate_UNType">
		<owl:equivalentClass><rdfs:Datatype>
		<owl:onDatatype rdf:resource="&xs;token"/><owl:withRestrictions rdf:parseType="Collection"><rdf:Description><xs:enumeration>all</xs:enumeration></rdf:Description><rdf:Description><xs:enumeration>one</xs:enumeration></rdf:Description><rdf:Description><xs:enumeration>none</xs:enumeration></rdf:Description></owl:withRestrictions></rdfs:Datatype></owl:equivalentClass></rdfs:Datatype>
	<owl:DatatypeProperty rdf:ID="evaluate_att.targeteval.attribute.evaluate__NS_evaluate_att.targeteval.attribute.evaluate_UNType">
		<rdfs:range rdf:resource="#NS_evaluate_att.targeteval.attribute.evaluate_UNType"/>
		<rdfs:label>evaluate</rdfs:label>
	<rdfs:comment>Specifies the intended meaning when a participant in a relationship is itself a pointer.</rdfs:comment>
	</owl:DatatypeProperty>
	<rdfs:Datatype rdf:ID="NS_func_att.tempo.log.attribute.func_UNType">
		<owl:equivalentClass><rdfs:Datatype>
		<owl:onDatatype rdf:resource="&xs;token"/><owl:withRestrictions rdf:parseType="Collection"><rdf:Description><xs:enumeration>continuous</xs:enumeration></rdf:Description><rdf:Description><xs:enumeration>instantaneous</xs:enumeration></rdf:Description><rdf:Description><xs:enumeration>metricmod</xs:enumeration></rdf:Description><rdf:Description><xs:enumeration>precedente</xs:enumeration></rdf:Description></owl:withRestrictions></rdfs:Datatype></owl:equivalentClass></rdfs:Datatype>
	<owl:DatatypeProperty rdf:ID="func_att.tempo.log.attribute.func__NS_func_att.tempo.log.attribute.func_UNType">
		<rdfs:range rdf:resource="#NS_func_att.tempo.log.attribute.func_UNType"/>
		<rdfs:label>func</rdfs:label>
	<rdfs:comment>Records the function of a tempo indication.</rdfs:comment>
	</owl:DatatypeProperty>
	<owl:DatatypeProperty rdf:ID="text.fam_att.textstyle.attribute.text.fam__mei_data.FONTFAMILY">
		<rdfs:range rdf:resource="&datatypes;data.FONTFAMILY"/>
		<rdfs:label>text.fam</rdfs:label>
	<rdfs:comment>Provides a default value for the font family name of text (other than lyrics) when this information is not provided on the individual elements.</rdfs:comment>
	</owl:DatatypeProperty>
	<owl:DatatypeProperty rdf:ID="text.name_att.textstyle.attribute.text.name__mei_data.FONTNAME">
		<rdfs:range rdf:resource="&datatypes;data.FONTNAME"/>
		<rdfs:label>text.name</rdfs:label>
	<rdfs:comment>Provides a default value for the font name of text (other than lyrics) when this information is not provided on the individual elements.</rdfs:comment>
	</owl:DatatypeProperty>
	<owl:DatatypeProperty rdf:ID="text.size_att.textstyle.attribute.text.size__mei_data.FONTSIZE">
		<rdfs:range rdf:resource="&datatypes;data.FONTSIZE"/>
		<rdfs:label>text.size</rdfs:label>
	<rdfs:comment>Provides a default value for the font size of text (other than lyrics) when this information is not provided on the individual elements.</rdfs:comment>
	</owl:DatatypeProperty>
	<owl:DatatypeProperty rdf:ID="text.style_att.textstyle.attribute.text.style__mei_data.FONTSTYLE">
		<rdfs:range rdf:resource="&datatypes;data.FONTSTYLE"/>
		<rdfs:label>text.style</rdfs:label>
	<rdfs:comment>Provides a default value for the font style of text (other than lyrics) when this information is not provided on the individual elements.</rdfs:comment>
	</owl:DatatypeProperty>
	<owl:DatatypeProperty rdf:ID="text.weight_att.textstyle.attribute.text.weight__mei_data.FONTWEIGHT">
		<rdfs:range rdf:resource="&datatypes;data.FONTWEIGHT"/>
		<rdfs:label>text.weight</rdfs:label>
	<rdfs:comment>Provides a default value for the font weight for text (other than lyrics) when this information is not provided on the individual elements.</rdfs:comment>
	</owl:DatatypeProperty>
	<rdfs:Datatype rdf:ID="NS_tie_att.tiepresent.attribute.tie_UNType">
		<owl:equivalentClass><rdfs:Datatype>
		<owl:onDatatype rdf:resource="tie_att.tiepresent.attribute.tie_NS_tie_att.tiepresent.attribute.tie_UNType_UNType"/><owl:withRestrictions rdf:parseType="Collection"><rdf:Description><xs:minLength>1</xs:minLength></rdf:Description></owl:withRestrictions></rdfs:Datatype></owl:equivalentClass></rdfs:Datatype>
	<rdfs:Datatype rdf:ID="tie_att.tiepresent.attribute.tie_NS_tie_att.tiepresent.attribute.tie_UNType_UNType">
		<owl:equivalentClass><rdfs:Datatype>
		<owl:oneOf><rdf:Description><rdf:type rdf:resource="#List"/><rdf:first>mei:data.TIE</rdf:first><rdf:rest rdf:resource="#nil"/></rdf:Description></owl:oneOf></rdfs:Datatype></owl:equivalentClass></rdfs:Datatype>
	<owl:DatatypeProperty rdf:ID="tie_att.tiepresent.attribute.tie__NS_tie_att.tiepresent.attribute.tie_UNType">
		<rdfs:range rdf:resource="#NS_tie_att.tiepresent.attribute.tie_UNType"/>
		<rdfs:label>tie</rdfs:label>
	<rdfs:comment>Indicates that this element participates in a tie. If visual information about the tie needs to be recorded, then a &lt;tie&gt; element should be employed.</rdfs:comment>
	</owl:DatatypeProperty>
	<owl:DatatypeProperty rdf:ID="tstamp_att.timestamp.musical.attribute.tstamp__mei_data.BEAT">
		<rdfs:range rdf:resource="&datatypes;data.BEAT"/>
		<rdfs:label>tstamp</rdfs:label>
	<rdfs:comment>Encodes the onset time in terms of musical time, i.e., beats[.fractional_beat_part].</rdfs:comment>
	</owl:DatatypeProperty>
	<owl:DatatypeProperty rdf:ID="tstamp.ges_att.timestamp.performed.attribute.tstamp.ges__mei_data.DURATION.gestural">
		<rdfs:range rdf:resource="&datatypes;data.DURATION.gestural"/>
		<rdfs:label>tstamp.ges</rdfs:label>
	<rdfs:comment>Captures performed onset time in several forms; that is, ppq (MIDI clicks and MusicXML 'divisions'), Humdrum **recip values, beats, seconds, or mensural duration values.</rdfs:comment>
	</owl:DatatypeProperty>
	<owl:DatatypeProperty rdf:ID="tstamp.real_att.timestamp.performed.attribute.tstamp.real__mei_data.ISOTIME">
		<rdfs:range rdf:resource="&datatypes;data.ISOTIME"/>
		<rdfs:label>tstamp.real</rdfs:label>
	<rdfs:comment>Used to record the onset time in terms of ISO time.</rdfs:comment>
	</owl:DatatypeProperty>
	<owl:DatatypeProperty rdf:ID="tstamp2_att.timestamp2.musical.attribute.tstamp2__mei_data.MEASUREBEAT">
		<rdfs:range rdf:resource="&datatypes;data.MEASUREBEAT"/>
		<rdfs:label>tstamp2</rdfs:label>
	<rdfs:comment>Encodes the ending point of an event in terms of musical time, i.e., a count of measures plus a beat location.</rdfs:comment>
	</owl:DatatypeProperty>
	<owl:DatatypeProperty rdf:ID="trans.diat_att.transposition.attribute.trans.diat__xs_decimal">
		<rdfs:range rdf:resource="&xs;decimal"/>
		<rdfs:label>trans.diat</rdfs:label>
	<rdfs:comment>Records the amount of diatonic pitch shift, e.g., C to C♯ = 0, C to D♭ = 1, necessary to calculate the sounded pitch from the written one.</rdfs:comment>
	</owl:DatatypeProperty>
	<owl:DatatypeProperty rdf:ID="trans.semi_att.transposition.attribute.trans.semi__xs_decimal">
		<rdfs:range rdf:resource="&xs;decimal"/>
		<rdfs:label>trans.semi</rdfs:label>
	<rdfs:comment>Records the amount of pitch shift in semitones, e.g., C to C♯ = 1, C to D♭ = 1, necessary to calculate the sounded pitch from the written one.</rdfs:comment>
	</owl:DatatypeProperty>
	<rdfs:Datatype rdf:ID="NS_tuplet_att.tupletpresent.attribute.tuplet_UNType">
		<owl:equivalentClass><rdfs:Datatype>
		<owl:onDatatype rdf:resource="tuplet_att.tupletpresent.attribute.tuplet_NS_tuplet_att.tupletpresent.attribute.tuplet_UNType_UNType"/><owl:withRestrictions rdf:parseType="Collection"><rdf:Description><xs:minLength>1</xs:minLength></rdf:Description></owl:withRestrictions></rdfs:Datatype></owl:equivalentClass></rdfs:Datatype>
	<rdfs:Datatype rdf:ID="tuplet_att.tupletpresent.attribute.tuplet_NS_tuplet_att.tupletpresent.attribute.tuplet_UNType_UNType">
		<owl:equivalentClass><rdfs:Datatype>
		<owl:oneOf><rdf:Description><rdf:type rdf:resource="#List"/><rdf:first>mei:data.TUPLET</rdf:first><rdf:rest rdf:resource="#nil"/></rdf:Description></owl:oneOf></rdfs:Datatype></owl:equivalentClass></rdfs:Datatype>
	<owl:DatatypeProperty rdf:ID="tuplet_att.tupletpresent.attribute.tuplet__NS_tuplet_att.tupletpresent.attribute.tuplet_UNType">
		<rdfs:range rdf:resource="#NS_tuplet_att.tupletpresent.attribute.tuplet_UNType"/>
		<rdfs:label>tuplet</rdfs:label>
	<rdfs:comment>Indicates that this feature participates in a tuplet. If visual information about the tuplet needs to be recorded, then a &lt;tuplet&gt; element should be employed.</rdfs:comment>
	</owl:DatatypeProperty>
	<owl:DatatypeProperty rdf:ID="type_att.typed.attribute.type__xs_NMTOKEN">
		<rdfs:range rdf:resource="&xs;NMTOKEN"/>
		<rdfs:label>type</rdfs:label>
	<rdfs:comment>Characterizes the element in some sense, using any convenient classification scheme or typology.</rdfs:comment>
	</owl:DatatypeProperty>
	<owl:DatatypeProperty rdf:ID="subtype_att.typed.attribute.subtype__xs_NMTOKEN">
		<rdfs:range rdf:resource="&xs;NMTOKEN"/>
		<rdfs:label>subtype</rdfs:label>
	<rdfs:comment>Provide any sub-classification for the element, additional to that given by its type attribute.</rdfs:comment>
	</owl:DatatypeProperty>
	<owl:DatatypeProperty rdf:ID="fontfam_att.typography.attribute.fontfam__mei_data.FONTFAMILY">
		<rdfs:range rdf:resource="&datatypes;data.FONTFAMILY"/>
		<rdfs:label>fontfam</rdfs:label>
	<rdfs:comment>Contains the name of a font-family.</rdfs:comment>
	</owl:DatatypeProperty>
	<owl:DatatypeProperty rdf:ID="fontname_att.typography.attribute.fontname__mei_data.FONTNAME">
		<rdfs:range rdf:resource="&datatypes;data.FONTNAME"/>
		<rdfs:label>fontname</rdfs:label>
	<rdfs:comment>Holds the name of a font.</rdfs:comment>
	</owl:DatatypeProperty>
	<owl:DatatypeProperty rdf:ID="fontsize_att.typography.attribute.fontsize__mei_data.FONTSIZE">
		<rdfs:range rdf:resource="&datatypes;data.FONTSIZE"/>
		<rdfs:label>fontsize</rdfs:label>
	<rdfs:comment>Indicates the size of a font expressed in printers' points, i.e., 1/72nd of an inch, relative terms, e.g., &quot;small&quot;, &quot;larger&quot;, etc., or percentage values relative to &quot;normal&quot; size, e.g., &quot;125%&quot;. </rdfs:comment>
	</owl:DatatypeProperty>
	<owl:DatatypeProperty rdf:ID="fontstyle_att.typography.attribute.fontstyle__mei_data.FONTSTYLE">
		<rdfs:range rdf:resource="&datatypes;data.FONTSTYLE"/>
		<rdfs:label>fontstyle</rdfs:label>
	<rdfs:comment>Records the style of a font, i.e, italic, oblique, or normal.</rdfs:comment>
	</owl:DatatypeProperty>
	<owl:DatatypeProperty rdf:ID="fontweight_att.typography.attribute.fontweight__mei_data.FONTWEIGHT">
		<rdfs:range rdf:resource="&datatypes;data.FONTWEIGHT"/>
		<rdfs:label>fontweight</rdfs:label>
	<rdfs:comment>Used to indicate bold type.</rdfs:comment>
	</owl:DatatypeProperty>
	<owl:DatatypeProperty rdf:ID="visible_att.visibility.attribute.visible__mei_data.BOOLEAN">
		<rdfs:range rdf:resource="&datatypes;data.BOOLEAN"/>
		<rdfs:label>visible</rdfs:label>
	<rdfs:comment>Indicates if a feature should be rendered when the notation is presented graphically or sounded when it is presented in an aural form.</rdfs:comment>
	</owl:DatatypeProperty>
	<owl:DatatypeProperty rdf:ID="ho_att.visualoffset.ho.attribute.ho__mei_data.MEASUREMENTREL">
		<rdfs:range rdf:resource="&datatypes;data.MEASUREMENTREL"/>
		<rdfs:label>ho</rdfs:label>
	<rdfs:comment>Records a horizontal adjustment to a feature's programmatically-determined location in terms of staff interline distance; that is, in units of 1/2 the distance between adjacent staff lines.</rdfs:comment>
	</owl:DatatypeProperty>
	<owl:DatatypeProperty rdf:ID="to_att.visualoffset.to.attribute.to__mei_data.TSTAMPOFFSET">
		<rdfs:range rdf:resource="&datatypes;data.TSTAMPOFFSET"/>
		<rdfs:label>to</rdfs:label>
	<rdfs:comment>Records a timestamp adjustment of a feature's programmatically-determined location in terms of musical time; that is, beats.</rdfs:comment>
	</owl:DatatypeProperty>
	<owl:DatatypeProperty rdf:ID="vo_att.visualoffset.vo.attribute.vo__mei_data.MEASUREMENTREL">
		<rdfs:range rdf:resource="&datatypes;data.MEASUREMENTREL"/>
		<rdfs:label>vo</rdfs:label>
	<rdfs:comment>Records the vertical adjustment of a feature's programmatically-determined location in terms of staff interline distance; that is, in units of 1/2 the distance between adjacent staff lines.</rdfs:comment>
	</owl:DatatypeProperty>
	<owl:DatatypeProperty rdf:ID="startho_att.visualoffset2.ho.attribute.startho__mei_data.MEASUREMENTREL">
		<rdfs:range rdf:resource="&datatypes;data.MEASUREMENTREL"/>
		<rdfs:label>startho</rdfs:label>
	<rdfs:comment>Records the horizontal adjustment of a feature's programmatically-determined start point.</rdfs:comment>
	</owl:DatatypeProperty>
	<owl:DatatypeProperty rdf:ID="endho_att.visualoffset2.ho.attribute.endho__mei_data.MEASUREMENTREL">
		<rdfs:range rdf:resource="&datatypes;data.MEASUREMENTREL"/>
		<rdfs:label>endho</rdfs:label>
	<rdfs:comment>Records the horizontal adjustment of a feature's programmatically-determined end point.</rdfs:comment>
	</owl:DatatypeProperty>
	<owl:DatatypeProperty rdf:ID="startto_att.visualoffset2.to.attribute.startto__mei_data.TSTAMPOFFSET">
		<rdfs:range rdf:resource="&datatypes;data.TSTAMPOFFSET"/>
		<rdfs:label>startto</rdfs:label>
	<rdfs:comment>Records a timestamp adjustment of a feature's programmatically-determined start point.</rdfs:comment>
	</owl:DatatypeProperty>
	<owl:DatatypeProperty rdf:ID="endto_att.visualoffset2.to.attribute.endto__mei_data.TSTAMPOFFSET">
		<rdfs:range rdf:resource="&datatypes;data.TSTAMPOFFSET"/>
		<rdfs:label>endto</rdfs:label>
	<rdfs:comment>Records a timestamp adjustment of a feature's programmatically-determined end point.</rdfs:comment>
	</owl:DatatypeProperty>
	<owl:DatatypeProperty rdf:ID="startvo_att.visualoffset2.vo.attribute.startvo__mei_data.MEASUREMENTREL">
		<rdfs:range rdf:resource="&datatypes;data.MEASUREMENTREL"/>
		<rdfs:label>startvo</rdfs:label>
	<rdfs:comment>Records a vertical adjustment of a feature's programmatically-determined start point.</rdfs:comment>
	</owl:DatatypeProperty>
	<owl:DatatypeProperty rdf:ID="endvo_att.visualoffset2.vo.attribute.endvo__mei_data.MEASUREMENTREL">
		<rdfs:range rdf:resource="&datatypes;data.MEASUREMENTREL"/>
		<rdfs:label>endvo</rdfs:label>
	<rdfs:comment>Records a vertical adjustment of a feature's programmatically-determined end point.</rdfs:comment>
	</owl:DatatypeProperty>
	<owl:DatatypeProperty rdf:ID="width_att.width.attribute.width__mei_data.MEASUREMENTABS">
		<rdfs:range rdf:resource="&datatypes;data.MEASUREMENTABS"/>
		<rdfs:label>width</rdfs:label>
	<rdfs:comment>Measurement of the horizontal dimension of an entity.</rdfs:comment>
	</owl:DatatypeProperty>
	<owl:DatatypeProperty rdf:ID="x_att.xy.attribute.x__xs_decimal">
		<rdfs:range rdf:resource="&xs;decimal"/>
		<rdfs:label>x</rdfs:label>
	<rdfs:comment>Encodes an x coordinate for a feature in an output coordinate system. When it is necessary to record the placement of a feature in a facsimile image, use the facs attribute.</rdfs:comment>
	</owl:DatatypeProperty>
	<owl:DatatypeProperty rdf:ID="y_att.xy.attribute.y__xs_decimal">
		<rdfs:range rdf:resource="&xs;decimal"/>
		<rdfs:label>y</rdfs:label>
	<rdfs:comment>Encodes an y coordinate for a feature in an output coordinate system. When it is necessary to record the placement of a feature in a facsimile image, use the facs attribute.</rdfs:comment>
	</owl:DatatypeProperty>
	<owl:DatatypeProperty rdf:ID="x2_att.xy2.attribute.x2__xs_decimal">
		<rdfs:range rdf:resource="&xs;decimal"/>
		<rdfs:label>x2</rdfs:label>
	<rdfs:comment>Encodes the optional 2nd x coordinate.</rdfs:comment>
	</owl:DatatypeProperty>
	<owl:DatatypeProperty rdf:ID="y2_att.xy2.attribute.y2__xs_decimal">
		<rdfs:range rdf:resource="&xs;decimal"/>
		<rdfs:label>y2</rdfs:label>
	<rdfs:comment>Encodes the optional 2nd y coordinate.</rdfs:comment>
	</owl:DatatypeProperty>
	<rdfs:Datatype rdf:ID="NS_method_att.regularmethod.attribute.method_UNType">
		<owl:equivalentClass><rdfs:Datatype>
		<owl:onDatatype rdf:resource="&xs;token"/><owl:withRestrictions rdf:parseType="Collection"><rdf:Description><xs:enumeration>silent</xs:enumeration></rdf:Description><rdf:Description><xs:enumeration>tags</xs:enumeration></rdf:Description></owl:withRestrictions></rdfs:Datatype></owl:equivalentClass></rdfs:Datatype>
	<owl:DatatypeProperty rdf:ID="method_att.regularmethod.attribute.method__NS_method_att.regularmethod.attribute.method_UNType">
		<rdfs:range rdf:resource="#NS_method_att.regularmethod.attribute.method_UNType"/>
		<rdfs:label>method</rdfs:label>
	<rdfs:comment>Indicates the method employed to mark corrections and normalizations.</rdfs:comment>
	</owl:DatatypeProperty>
	<rdfs:Datatype rdf:ID="NS_order_att.arpeg.log.attribute.order_UNType">
		<owl:equivalentClass><rdfs:Datatype>
		<owl:onDatatype rdf:resource="&xs;token"/><owl:withRestrictions rdf:parseType="Collection"><rdf:Description><xs:enumeration>up</xs:enumeration></rdf:Description><rdf:Description><xs:enumeration>down</xs:enumeration></rdf:Description><rdf:Description><xs:enumeration>nonarp</xs:enumeration></rdf:Description></owl:withRestrictions></rdfs:Datatype></owl:equivalentClass></rdfs:Datatype>
	<owl:DatatypeProperty rdf:ID="order_att.arpeg.log.attribute.order__NS_order_att.arpeg.log.attribute.order_UNType">
		<rdfs:range rdf:resource="#NS_order_att.arpeg.log.attribute.order_UNType"/>
		<rdfs:label>order</rdfs:label>
	<rdfs:comment>Describes the direction in which an arpeggio is to be performed.</rdfs:comment>
	</owl:DatatypeProperty>
	<owl:DatatypeProperty rdf:ID="arrow_att.arpeg.vis.attribute.arrow__mei_data.BOOLEAN">
		<rdfs:range rdf:resource="&datatypes;data.BOOLEAN"/>
		<rdfs:label>arrow</rdfs:label>
	<rdfs:comment>Indicates if an arrowhead is to be drawn as part of the arpeggiation symbol.</rdfs:comment>
	</owl:DatatypeProperty>
	<rdfs:Datatype rdf:ID="NS_beam_att.beamed.attribute.beam_UNType">
		<owl:equivalentClass><rdfs:Datatype>
		<owl:onDatatype rdf:resource="beam_att.beamed.attribute.beam_NS_beam_att.beamed.attribute.beam_UNType_UNType"/><owl:withRestrictions rdf:parseType="Collection"><rdf:Description><xs:minLength>1</xs:minLength></rdf:Description></owl:withRestrictions></rdfs:Datatype></owl:equivalentClass></rdfs:Datatype>
	<rdfs:Datatype rdf:ID="beam_att.beamed.attribute.beam_NS_beam_att.beamed.attribute.beam_UNType_UNType">
		<owl:equivalentClass><rdfs:Datatype>
		<owl:oneOf><rdf:Description><rdf:type rdf:resource="#List"/><rdf:first>mei:data.BEAM</rdf:first><rdf:rest rdf:resource="#nil"/></rdf:Description></owl:oneOf></rdfs:Datatype></owl:equivalentClass></rdfs:Datatype>
	<owl:DatatypeProperty rdf:ID="beam_att.beamed.attribute.beam__NS_beam_att.beamed.attribute.beam_UNType">
		<rdfs:range rdf:resource="#NS_beam_att.beamed.attribute.beam_UNType"/>
		<rdfs:label>beam</rdfs:label>
	<rdfs:comment>Indicates that this event is &quot;under a beam&quot;.</rdfs:comment>
	</owl:DatatypeProperty>
	<owl:DatatypeProperty rdf:ID="beam.with_att.beamedwith.attribute.beam.with__mei_data.OTHERSTAFF">
		<rdfs:range rdf:resource="&datatypes;data.OTHERSTAFF"/>
		<rdfs:label>beam.with</rdfs:label>
	<rdfs:comment>In the case of cross-staff beams, the beam.with attribute is used to indicate which staff the beam is connected to; that is, the staff above or the staff below.</rdfs:comment>
	</owl:DatatypeProperty>
	<owl:DatatypeProperty rdf:ID="beam.group_att.beaming.log.attribute.beam.group__xs_string">
		<rdfs:range rdf:resource="&xs;string"/>
		<rdfs:label>beam.group</rdfs:label>
	<rdfs:comment>Provides an example of how automated beaming (including secondary beams) is to be performed.</rdfs:comment>
	</owl:DatatypeProperty>
	<owl:DatatypeProperty rdf:ID="beam.rests_att.beaming.log.attribute.beam.rests__mei_data.BOOLEAN">
		<rdfs:range rdf:resource="&datatypes;data.BOOLEAN"/>
		<rdfs:label>beam.rests</rdfs:label>
	<rdfs:comment>Indicates whether automatically-drawn beams should include rests shorter than a quarter note duration.</rdfs:comment>
	</owl:DatatypeProperty>
	<rdfs:Datatype rdf:ID="NS_form_att.beamrend.attribute.form_UNType">
		<owl:equivalentClass><rdfs:Datatype>
		<owl:onDatatype rdf:resource="&xs;token"/><owl:withRestrictions rdf:parseType="Collection"><rdf:Description><xs:enumeration>acc</xs:enumeration></rdf:Description><rdf:Description><xs:enumeration>mixed</xs:enumeration></rdf:Description><rdf:Description><xs:enumeration>rit</xs:enumeration></rdf:Description><rdf:Description><xs:enumeration>norm</xs:enumeration></rdf:Description></owl:withRestrictions></rdfs:Datatype></owl:equivalentClass></rdfs:Datatype>
	<owl:DatatypeProperty rdf:ID="form_att.beamrend.attribute.form__NS_form_att.beamrend.attribute.form_UNType">
		<rdfs:range rdf:resource="#NS_form_att.beamrend.attribute.form_UNType"/>
		<rdfs:label>form</rdfs:label>
	<rdfs:comment>Captures whether a beam is &quot;feathered&quot; and in which direction.</rdfs:comment>
	</owl:DatatypeProperty>
	<owl:DatatypeProperty rdf:ID="slope_att.beamrend.attribute.slope__xs_decimal">
		<rdfs:range rdf:resource="&xs;decimal"/>
		<rdfs:label>slope</rdfs:label>
	<rdfs:comment>Records the slope of the beam.</rdfs:comment>
	</owl:DatatypeProperty>
	<owl:DatatypeProperty rdf:ID="breaksec_att.beamsecondary.attribute.breaksec__xs_positiveInteger">
		<rdfs:range rdf:resource="&xs;positiveInteger"/>
		<rdfs:label>breaksec</rdfs:label>
	<rdfs:comment>Presence of this attribute indicates that the secondary beam should be broken following this note/chord. The value of the attribute records the number of beams which should remain unbroken.</rdfs:comment>
	</owl:DatatypeProperty>
	<owl:DatatypeProperty rdf:ID="beatDef_att.beatRpt.log.attribute.beatDef__mei_data.DURATION.gestural">
		<rdfs:range rdf:resource="&datatypes;data.DURATION.gestural"/>
		<rdfs:label>beatDef</rdfs:label>
	<rdfs:comment>Indicates the performed duration represented by the beatRpt symbol.</rdfs:comment>
	</owl:DatatypeProperty>
	<owl:DatatypeProperty rdf:ID="form_att.beatRpt.vis.attribute.form__mei_data.BEATRPT.REND">
		<rdfs:range rdf:resource="&datatypes;data.BEATRPT.REND"/>
		<rdfs:label>form</rdfs:label>
	<rdfs:comment>Indicates the number of slashes required to render the appropriate beat repeat symbol. When a single beat is repeated, consisting of a single note or chord, it is indicated by a single thick, slanting slash; therefore, the value '1' should be used. The following values should be used when the beat is divided into even notes: 4ths or 8ths=1, 16ths=2, 32nds=3, 64ths=4, 128ths=5. When the beat is comprised of mixed duration values, the symbol is always rendered as 2 slashes and 2 dots.</rdfs:comment>
	</owl:DatatypeProperty>
	<owl:DatatypeProperty rdf:ID="amount_att.bend.ges.attribute.amount__mei_data.BEND.AMOUNT">
		<rdfs:range rdf:resource="&datatypes;data.BEND.AMOUNT"/>
		<rdfs:label>amount</rdfs:label>
	<rdfs:comment>Records the amount of detuning. The decimal values should be rendered as a fraction (or an integer plus a fraction) along with the bend symbol.</rdfs:comment>
	</owl:DatatypeProperty>
	<rdfs:Datatype rdf:ID="NS_form_att.bTrem.log.attribute.form_UNType">
		<owl:equivalentClass><rdfs:Datatype>
		<owl:onDatatype rdf:resource="&xs;token"/><owl:withRestrictions rdf:parseType="Collection"><rdf:Description><xs:enumeration>meas</xs:enumeration></rdf:Description><rdf:Description><xs:enumeration>unmeas</xs:enumeration></rdf:Description></owl:withRestrictions></rdfs:Datatype></owl:equivalentClass></rdfs:Datatype>
	<owl:DatatypeProperty rdf:ID="form_att.bTrem.log.attribute.form__NS_form_att.bTrem.log.attribute.form_UNType">
		<rdfs:range rdf:resource="#NS_form_att.bTrem.log.attribute.form_UNType"/>
		<rdfs:label>form</rdfs:label>
	<rdfs:comment>Indicates whether the tremolo is measured or unmeasured.</rdfs:comment>
	</owl:DatatypeProperty>
	<rdfs:Datatype rdf:ID="NS_cutout_att.cutout.attribute.cutout_UNType">
		<owl:equivalentClass><rdfs:Datatype>
		<owl:onDatatype rdf:resource="&xs;token"/><owl:withRestrictions rdf:parseType="Collection"><rdf:Description><xs:enumeration>cutout</xs:enumeration></rdf:Description></owl:withRestrictions></rdfs:Datatype></owl:equivalentClass></rdfs:Datatype>
	<owl:DatatypeProperty rdf:ID="cutout_att.cutout.attribute.cutout__NS_cutout_att.cutout.attribute.cutout_UNType">
		<rdfs:range rdf:resource="#NS_cutout_att.cutout.attribute.cutout_UNType"/>
		<rdfs:label>cutout</rdfs:label>
	<rdfs:comment>&quot;Cut-out&quot; style indicated for this measure.</rdfs:comment>
	</owl:DatatypeProperty>
	<owl:DatatypeProperty rdf:ID="expand_att.expandable.attribute.expand__mei_data.BOOLEAN">
		<rdfs:range rdf:resource="&datatypes;data.BOOLEAN"/>
		<rdfs:label>expand</rdfs:label>
	<rdfs:comment>Indicates whether to render a repeat symbol or the source material to which it refers. A value of 'true' renders the source material, while 'false' displays the repeat symbol.</rdfs:comment>
	</owl:DatatypeProperty>
	<rdfs:Datatype rdf:ID="NS_form_att.fermata.vis.attribute.form_UNType">
		<owl:equivalentClass><rdfs:Datatype>
		<owl:onDatatype rdf:resource="&xs;token"/><owl:withRestrictions rdf:parseType="Collection"><rdf:Description><xs:enumeration>inv</xs:enumeration></rdf:Description><rdf:Description><xs:enumeration>norm</xs:enumeration></rdf:Description></owl:withRestrictions></rdfs:Datatype></owl:equivalentClass></rdfs:Datatype>
	<owl:DatatypeProperty rdf:ID="form_att.fermata.vis.attribute.form__NS_form_att.fermata.vis.attribute.form_UNType">
		<rdfs:range rdf:resource="#NS_form_att.fermata.vis.attribute.form_UNType"/>
		<rdfs:label>form</rdfs:label>
	<rdfs:comment>Describes the visual appearance of the fermata; that is, whether it occurs as upright or inverted.</rdfs:comment>
	</owl:DatatypeProperty>
	<rdfs:Datatype rdf:ID="NS_shape_att.fermata.vis.attribute.shape_UNType">
		<owl:equivalentClass><rdfs:Datatype>
		<owl:onDatatype rdf:resource="&xs;token"/><owl:withRestrictions rdf:parseType="Collection"><rdf:Description><xs:enumeration>curved</xs:enumeration></rdf:Description><rdf:Description><xs:enumeration>square</xs:enumeration></rdf:Description><rdf:Description><xs:enumeration>angular</xs:enumeration></rdf:Description></owl:withRestrictions></rdfs:Datatype></owl:equivalentClass></rdfs:Datatype>
	<owl:DatatypeProperty rdf:ID="shape_att.fermata.vis.attribute.shape__NS_shape_att.fermata.vis.attribute.shape_UNType">
		<rdfs:range rdf:resource="#NS_shape_att.fermata.vis.attribute.shape_UNType"/>
		<rdfs:label>shape</rdfs:label>
	<rdfs:comment>Describes the visual appearance of the fermata; that is, whether it has a curved, square, or angular shape.</rdfs:comment>
	</owl:DatatypeProperty>
	<rdfs:Datatype rdf:ID="NS_form_att.fTrem.log.attribute.form_UNType">
		<owl:equivalentClass><rdfs:Datatype>
		<owl:onDatatype rdf:resource="&xs;token"/><owl:withRestrictions rdf:parseType="Collection"><rdf:Description><xs:enumeration>meas</xs:enumeration></rdf:Description><rdf:Description><xs:enumeration>unmeas</xs:enumeration></rdf:Description></owl:withRestrictions></rdfs:Datatype></owl:equivalentClass></rdfs:Datatype>
	<owl:DatatypeProperty rdf:ID="form_att.fTrem.log.attribute.form__NS_form_att.fTrem.log.attribute.form_UNType">
		<rdfs:range rdf:resource="#NS_form_att.fTrem.log.attribute.form_UNType"/>
		<rdfs:label>form</rdfs:label>
	<rdfs:comment>Describes the style of the tremolo.</rdfs:comment>
	</owl:DatatypeProperty>
	<owl:DatatypeProperty rdf:ID="grace_att.graced.attribute.grace__mei_data.GRACE">
		<rdfs:range rdf:resource="&datatypes;data.GRACE"/>
		<rdfs:label>grace</rdfs:label>
	<rdfs:comment>Marks a note or chord as a &quot;grace&quot; (without a definitive written duration) and records from which other note/chord it should &quot;steal&quot; time.</rdfs:comment>
	</owl:DatatypeProperty>
	<owl:DatatypeProperty rdf:ID="grace.time_att.graced.attribute.grace.time__mei_data.PERCENT">
		<rdfs:range rdf:resource="&datatypes;data.PERCENT"/>
		<rdfs:label>grace.time</rdfs:label>
	<rdfs:comment>Records the amount of time to be &quot;stolen&quot; from a non-grace note/chord.</rdfs:comment>
	</owl:DatatypeProperty>
	<rdfs:Datatype rdf:ID="NS_form_att.hairpin.log.attribute.form_UNType">
		<owl:equivalentClass><rdfs:Datatype>
		<owl:onDatatype rdf:resource="&xs;token"/><owl:withRestrictions rdf:parseType="Collection"><rdf:Description><xs:enumeration>cres</xs:enumeration></rdf:Description><rdf:Description><xs:enumeration>dim</xs:enumeration></rdf:Description></owl:withRestrictions></rdfs:Datatype></owl:equivalentClass></rdfs:Datatype>
	<owl:DatatypeProperty rdf:ID="form_att.hairpin.log.attribute.form__NS_form_att.hairpin.log.attribute.form_UNType">
		<rdfs:range rdf:resource="#NS_form_att.hairpin.log.attribute.form_UNType"/>
		<rdfs:label>form</rdfs:label>
	<rdfs:comment>Captures the visual rendition and function of the hairpin; that is, whether it indicates an increase or a decrease in volume.</rdfs:comment>
	</owl:DatatypeProperty>
	<owl:DatatypeProperty rdf:ID="niente_att.hairpin.log.attribute.niente__mei_data.BOOLEAN">
		<rdfs:range rdf:resource="&datatypes;data.BOOLEAN"/>
		<rdfs:label>niente</rdfs:label>
	<rdfs:comment>Indicates that the hairpin starts from or ends in silence. Often rendered as a small circle attached to the closed end of the hairpin. See Gould, p. 108.</rdfs:comment>
	</owl:DatatypeProperty>
	<owl:DatatypeProperty rdf:ID="opening_att.hairpin.vis.attribute.opening__mei_data.MEASUREMENTABS">
		<rdfs:range rdf:resource="&datatypes;data.MEASUREMENTABS"/>
		<rdfs:label>opening</rdfs:label>
	<rdfs:comment>Specifies the distance between the lines at the open end of a hairpin dynamic mark.</rdfs:comment>
	</owl:DatatypeProperty>
	<rdfs:Datatype rdf:ID="NS_c_att.harpPedal.log.attribute.c_UNType">
		<owl:equivalentClass><rdfs:Datatype>
		<owl:onDatatype rdf:resource="&xs;token"/><owl:withRestrictions rdf:parseType="Collection"><rdf:Description><xs:enumeration>f</xs:enumeration></rdf:Description><rdf:Description><xs:enumeration>n</xs:enumeration></rdf:Description><rdf:Description><xs:enumeration>s</xs:enumeration></rdf:Description></owl:withRestrictions></rdfs:Datatype></owl:equivalentClass></rdfs:Datatype>
	<owl:DatatypeProperty rdf:ID="c_att.harpPedal.log.attribute.c__NS_c_att.harpPedal.log.attribute.c_UNType">
		<rdfs:range rdf:resource="#NS_c_att.harpPedal.log.attribute.c_UNType"/>
		<rdfs:label>c</rdfs:label>
	<rdfs:comment>Indicates the pedal setting for the harp's C strings.</rdfs:comment>
	</owl:DatatypeProperty>
	<rdfs:Datatype rdf:ID="NS_d_att.harpPedal.log.attribute.d_UNType">
		<owl:equivalentClass><rdfs:Datatype>
		<owl:onDatatype rdf:resource="&xs;token"/><owl:withRestrictions rdf:parseType="Collection"><rdf:Description><xs:enumeration>f</xs:enumeration></rdf:Description><rdf:Description><xs:enumeration>n</xs:enumeration></rdf:Description><rdf:Description><xs:enumeration>s</xs:enumeration></rdf:Description></owl:withRestrictions></rdfs:Datatype></owl:equivalentClass></rdfs:Datatype>
	<owl:DatatypeProperty rdf:ID="d_att.harpPedal.log.attribute.d__NS_d_att.harpPedal.log.attribute.d_UNType">
		<rdfs:range rdf:resource="#NS_d_att.harpPedal.log.attribute.d_UNType"/>
		<rdfs:label>d</rdfs:label>
	<rdfs:comment>Indicates the pedal setting for the harp's D strings.</rdfs:comment>
	</owl:DatatypeProperty>
	<rdfs:Datatype rdf:ID="NS_e_att.harpPedal.log.attribute.e_UNType">
		<owl:equivalentClass><rdfs:Datatype>
		<owl:onDatatype rdf:resource="&xs;token"/><owl:withRestrictions rdf:parseType="Collection"><rdf:Description><xs:enumeration>f</xs:enumeration></rdf:Description><rdf:Description><xs:enumeration>n</xs:enumeration></rdf:Description><rdf:Description><xs:enumeration>s</xs:enumeration></rdf:Description></owl:withRestrictions></rdfs:Datatype></owl:equivalentClass></rdfs:Datatype>
	<owl:DatatypeProperty rdf:ID="e_att.harpPedal.log.attribute.e__NS_e_att.harpPedal.log.attribute.e_UNType">
		<rdfs:range rdf:resource="#NS_e_att.harpPedal.log.attribute.e_UNType"/>
		<rdfs:label>e</rdfs:label>
	<rdfs:comment>Indicates the pedal setting for the harp's E strings.</rdfs:comment>
	</owl:DatatypeProperty>
	<rdfs:Datatype rdf:ID="NS_f_att.harpPedal.log.attribute.f_UNType">
		<owl:equivalentClass><rdfs:Datatype>
		<owl:onDatatype rdf:resource="&xs;token"/><owl:withRestrictions rdf:parseType="Collection"><rdf:Description><xs:enumeration>f</xs:enumeration></rdf:Description><rdf:Description><xs:enumeration>n</xs:enumeration></rdf:Description><rdf:Description><xs:enumeration>s</xs:enumeration></rdf:Description></owl:withRestrictions></rdfs:Datatype></owl:equivalentClass></rdfs:Datatype>
	<owl:DatatypeProperty rdf:ID="f_att.harpPedal.log.attribute.f__NS_f_att.harpPedal.log.attribute.f_UNType">
		<rdfs:range rdf:resource="#NS_f_att.harpPedal.log.attribute.f_UNType"/>
		<rdfs:label>f</rdfs:label>
	<rdfs:comment>Indicates the pedal setting for the harp's F strings.</rdfs:comment>
	</owl:DatatypeProperty>
	<rdfs:Datatype rdf:ID="NS_g_att.harpPedal.log.attribute.g_UNType">
		<owl:equivalentClass><rdfs:Datatype>
		<owl:onDatatype rdf:resource="&xs;token"/><owl:withRestrictions rdf:parseType="Collection"><rdf:Description><xs:enumeration>f</xs:enumeration></rdf:Description><rdf:Description><xs:enumeration>n</xs:enumeration></rdf:Description><rdf:Description><xs:enumeration>s</xs:enumeration></rdf:Description></owl:withRestrictions></rdfs:Datatype></owl:equivalentClass></rdfs:Datatype>
	<owl:DatatypeProperty rdf:ID="g_att.harpPedal.log.attribute.g__NS_g_att.harpPedal.log.attribute.g_UNType">
		<rdfs:range rdf:resource="#NS_g_att.harpPedal.log.attribute.g_UNType"/>
		<rdfs:label>g</rdfs:label>
	<rdfs:comment>Indicates the pedal setting for the harp's G strings.</rdfs:comment>
	</owl:DatatypeProperty>
	<rdfs:Datatype rdf:ID="NS_a_att.harpPedal.log.attribute.a_UNType">
		<owl:equivalentClass><rdfs:Datatype>
		<owl:onDatatype rdf:resource="&xs;token"/><owl:withRestrictions rdf:parseType="Collection"><rdf:Description><xs:enumeration>f</xs:enumeration></rdf:Description><rdf:Description><xs:enumeration>n</xs:enumeration></rdf:Description><rdf:Description><xs:enumeration>s</xs:enumeration></rdf:Description></owl:withRestrictions></rdfs:Datatype></owl:equivalentClass></rdfs:Datatype>
	<owl:DatatypeProperty rdf:ID="a_att.harpPedal.log.attribute.a__NS_a_att.harpPedal.log.attribute.a_UNType">
		<rdfs:range rdf:resource="#NS_a_att.harpPedal.log.attribute.a_UNType"/>
		<rdfs:label>a</rdfs:label>
	<rdfs:comment>Indicates the pedal setting for the harp's A strings.</rdfs:comment>
	</owl:DatatypeProperty>
	<rdfs:Datatype rdf:ID="NS_b_att.harpPedal.log.attribute.b_UNType">
		<owl:equivalentClass><rdfs:Datatype>
		<owl:onDatatype rdf:resource="&xs;token"/><owl:withRestrictions rdf:parseType="Collection"><rdf:Description><xs:enumeration>f</xs:enumeration></rdf:Description><rdf:Description><xs:enumeration>n</xs:enumeration></rdf:Description><rdf:Description><xs:enumeration>s</xs:enumeration></rdf:Description></owl:withRestrictions></rdfs:Datatype></owl:equivalentClass></rdfs:Datatype>
	<owl:DatatypeProperty rdf:ID="b_att.harpPedal.log.attribute.b__NS_b_att.harpPedal.log.attribute.b_UNType">
		<rdfs:range rdf:resource="#NS_b_att.harpPedal.log.attribute.b_UNType"/>
		<rdfs:label>b</rdfs:label>
	<rdfs:comment>Indicates the pedal setting for the harp's B strings.</rdfs:comment>
	</owl:DatatypeProperty>
	<owl:DatatypeProperty rdf:ID="lv_att.lvpresent.attribute.lv__mei_data.BOOLEAN">
		<rdfs:range rdf:resource="&datatypes;data.BOOLEAN"/>
		<rdfs:label>lv</rdfs:label>
	<rdfs:comment>Indicates the attachment of an l.v. (laissez vibrer) sign to this element.</rdfs:comment>
	</owl:DatatypeProperty>
	<rdfs:Datatype rdf:ID="NS_func_att.meterSigGrp.log.attribute.func_UNType">
		<owl:equivalentClass><rdfs:Datatype>
		<owl:onDatatype rdf:resource="&xs;token"/><owl:withRestrictions rdf:parseType="Collection"><rdf:Description><xs:enumeration>alternating</xs:enumeration></rdf:Description><rdf:Description><xs:enumeration>interchanging</xs:enumeration></rdf:Description><rdf:Description><xs:enumeration>mixed</xs:enumeration></rdf:Description></owl:withRestrictions></rdfs:Datatype></owl:equivalentClass></rdfs:Datatype>
	<owl:DatatypeProperty rdf:ID="func_att.meterSigGrp.log.attribute.func__NS_func_att.meterSigGrp.log.attribute.func_UNType">
		<rdfs:range rdf:resource="#NS_func_att.meterSigGrp.log.attribute.func_UNType"/>
		<rdfs:label>func</rdfs:label>
	<rdfs:comment>Function of the meter signature group.</rdfs:comment>
	</owl:DatatypeProperty>
	<owl:DatatypeProperty rdf:ID="block_att.multiRest.vis.attribute.block__mei_data.BOOLEAN">
		<rdfs:range rdf:resource="&datatypes;data.BOOLEAN"/>
		<rdfs:label>block</rdfs:label>
	<rdfs:comment>When the block attribute is used, combinations of the 1, 2, and 4 measure rest forms (Read, p. 104) should be rendered instead of the modern form or an alternative symbol.</rdfs:comment>
	</owl:DatatypeProperty>
	<owl:DatatypeProperty rdf:ID="gliss_att.note.ges.cmn.attribute.gliss__mei_data.GLISSANDO">
		<rdfs:range rdf:resource="&datatypes;data.GLISSANDO"/>
		<rdfs:label>gliss</rdfs:label>
	<rdfs:comment>Indicates that this element participates in a glissando.</rdfs:comment>
	</owl:DatatypeProperty>
	<owl:DatatypeProperty rdf:ID="num_att.numbered.attribute.num__xs_positiveInteger">
		<rdfs:range rdf:resource="&xs;positiveInteger"/>
		<rdfs:label>num</rdfs:label>
	<rdfs:comment>Records a number or count accompanying a notational feature.</rdfs:comment>
	</owl:DatatypeProperty>
	<owl:DatatypeProperty rdf:ID="num.place_att.numberplacement.attribute.num.place__mei_data.PLACE">
		<rdfs:range rdf:resource="&datatypes;data.PLACE"/>
		<rdfs:label>num.place</rdfs:label>
	<rdfs:comment>States where the tuplet number will be placed in relation to the note heads.</rdfs:comment>
	</owl:DatatypeProperty>
	<owl:DatatypeProperty rdf:ID="num.visible_att.numberplacement.attribute.num.visible__mei_data.BOOLEAN">
		<rdfs:range rdf:resource="&datatypes;data.BOOLEAN"/>
		<rdfs:label>num.visible</rdfs:label>
	<rdfs:comment>Determines if the tuplet number is visible.</rdfs:comment>
	</owl:DatatypeProperty>
	<rdfs:Datatype rdf:ID="NS_coll_att.octave.log.attribute.coll_UNType">
		<owl:equivalentClass><rdfs:Datatype>
		<owl:onDatatype rdf:resource="&xs;token"/><owl:withRestrictions rdf:parseType="Collection"><rdf:Description><xs:enumeration>coll</xs:enumeration></rdf:Description></owl:withRestrictions></rdfs:Datatype></owl:equivalentClass></rdfs:Datatype>
	<owl:DatatypeProperty rdf:ID="coll_att.octave.log.attribute.coll__NS_coll_att.octave.log.attribute.coll_UNType">
		<rdfs:range rdf:resource="#NS_coll_att.octave.log.attribute.coll_UNType"/>
		<rdfs:label>coll</rdfs:label>
	<rdfs:comment>Indicates whether the octave displacement should be performed simultaneously with the written notes, i.e., &quot;coll' ottava&quot;. Unlike other octave signs which are indicated by broken lines, coll' ottava typically uses an unbroken line or a series of longer broken lines, ending with a short vertical stroke. See Read, p. 47-48.</rdfs:comment>
	</owl:DatatypeProperty>
	<rdfs:Datatype rdf:ID="NS_dir_att.pedal.log.attribute.dir_UNType">
		<owl:equivalentClass><rdfs:Datatype>
		<owl:onDatatype rdf:resource="&xs;token"/><owl:withRestrictions rdf:parseType="Collection"><rdf:Description><xs:enumeration>down</xs:enumeration></rdf:Description><rdf:Description><xs:enumeration>up</xs:enumeration></rdf:Description><rdf:Description><xs:enumeration>half</xs:enumeration></rdf:Description><rdf:Description><xs:enumeration>bounce</xs:enumeration></rdf:Description></owl:withRestrictions></rdfs:Datatype></owl:equivalentClass></rdfs:Datatype>
	<owl:DatatypeProperty rdf:ID="dir_att.pedal.log.attribute.dir__NS_dir_att.pedal.log.attribute.dir_UNType">
		<rdfs:range rdf:resource="#NS_dir_att.pedal.log.attribute.dir_UNType"/>
		<rdfs:label>dir</rdfs:label>
	<rdfs:comment>Records the position of the piano damper pedal.</rdfs:comment>
	</owl:DatatypeProperty>
	<rdfs:Datatype rdf:ID="NS_form_att.pedal.vis.attribute.form_UNType">
		<owl:equivalentClass><rdfs:Datatype>
		<owl:onDatatype rdf:resource="&xs;token"/><owl:withRestrictions rdf:parseType="Collection"><rdf:Description><xs:enumeration>line</xs:enumeration></rdf:Description><rdf:Description><xs:enumeration>pedstar</xs:enumeration></rdf:Description><rdf:Description><xs:enumeration>altpedstar</xs:enumeration></rdf:Description></owl:withRestrictions></rdfs:Datatype></owl:equivalentClass></rdfs:Datatype>
	<owl:DatatypeProperty rdf:ID="form_att.pedal.vis.attribute.form__NS_form_att.pedal.vis.attribute.form_UNType">
		<rdfs:range rdf:resource="#NS_form_att.pedal.vis.attribute.form_UNType"/>
		<rdfs:label>form</rdfs:label>
	<rdfs:comment>Determines whether piano pedal marks should be rendered as lines or as terms.</rdfs:comment>
	</owl:DatatypeProperty>
	<rdfs:Datatype rdf:ID="NS_pedal.style_att.pianopedals.attribute.pedal.style_UNType">
		<owl:equivalentClass><rdfs:Datatype>
		<owl:onDatatype rdf:resource="&xs;token"/><owl:withRestrictions rdf:parseType="Collection"><rdf:Description><xs:enumeration>line</xs:enumeration></rdf:Description><rdf:Description><xs:enumeration>pedstar</xs:enumeration></rdf:Description><rdf:Description><xs:enumeration>altpedstar</xs:enumeration></rdf:Description></owl:withRestrictions></rdfs:Datatype></owl:equivalentClass></rdfs:Datatype>
	<owl:DatatypeProperty rdf:ID="pedal.style_att.pianopedals.attribute.pedal.style__NS_pedal.style_att.pianopedals.attribute.pedal.style_UNType">
		<rdfs:range rdf:resource="#NS_pedal.style_att.pianopedals.attribute.pedal.style_UNType"/>
		<rdfs:label>pedal.style</rdfs:label>
	<rdfs:comment>Determines whether piano pedal marks should be rendered as lines or as terms.</rdfs:comment>
	</owl:DatatypeProperty>
	<rdfs:Datatype rdf:ID="NS_reh.enclose_att.rehearsal.attribute.reh.enclose_UNType">
		<owl:equivalentClass><rdfs:Datatype>
		<owl:onDatatype rdf:resource="&xs;token"/><owl:withRestrictions rdf:parseType="Collection"><rdf:Description><xs:enumeration>box</xs:enumeration></rdf:Description><rdf:Description><xs:enumeration>circle</xs:enumeration></rdf:Description><rdf:Description><xs:enumeration>none</xs:enumeration></rdf:Description></owl:withRestrictions></rdfs:Datatype></owl:equivalentClass></rdfs:Datatype>
	<owl:DatatypeProperty rdf:ID="reh.enclose_att.rehearsal.attribute.reh.enclose__NS_reh.enclose_att.rehearsal.attribute.reh.enclose_UNType">
		<rdfs:range rdf:resource="#NS_reh.enclose_att.rehearsal.attribute.reh.enclose_UNType"/>
		<rdfs:label>reh.enclose</rdfs:label>
	<rdfs:comment>Describes the enclosing shape for rehearsal marks.</rdfs:comment>
	</owl:DatatypeProperty>
	<owl:DatatypeProperty rdf:ID="grid.show_att.scoreDef.vis.cmn.attribute.grid.show__mei_data.BOOLEAN">
		<rdfs:range rdf:resource="&datatypes;data.BOOLEAN"/>
		<rdfs:label>grid.show</rdfs:label>
	<rdfs:comment>Determines whether to display guitar chord grids.</rdfs:comment>
	</owl:DatatypeProperty>
	<owl:DatatypeProperty rdf:ID="slur.lform_att.slurrend.attribute.slur.lform__mei_data.LINEFORM">
		<rdfs:range rdf:resource="&datatypes;data.LINEFORM"/>
		<rdfs:label>slur.lform</rdfs:label>
	</owl:DatatypeProperty>
	<owl:DatatypeProperty rdf:ID="slur.lwidth_att.slurrend.attribute.slur.lwidth__mei_data.LINEWIDTH">
		<rdfs:range rdf:resource="&datatypes;data.LINEWIDTH"/>
		<rdfs:label>slur.lwidth</rdfs:label>
	</owl:DatatypeProperty>
	<owl:DatatypeProperty rdf:ID="stem.with_att.stems.cmn.attribute.stem.with__mei_data.OTHERSTAFF">
		<rdfs:range rdf:resource="&datatypes;data.OTHERSTAFF"/>
		<rdfs:label>stem.with</rdfs:label>
	<rdfs:comment>Contains an indication of which staff a note or chord that logically belongs to the current staff should be visually placed on; that is, the one above or the one below.</rdfs:comment>
	</owl:DatatypeProperty>
	<owl:DatatypeProperty rdf:ID="tie.lform_att.tierend.attribute.tie.lform__mei_data.LINEFORM">
		<rdfs:range rdf:resource="&datatypes;data.LINEFORM"/>
		<rdfs:label>tie.lform</rdfs:label>
	</owl:DatatypeProperty>
	<owl:DatatypeProperty rdf:ID="tie.lwidth_att.tierend.attribute.tie.lwidth__mei_data.LINEWIDTH">
		<rdfs:range rdf:resource="&datatypes;data.LINEWIDTH"/>
		<rdfs:label>tie.lwidth</rdfs:label>
	</owl:DatatypeProperty>
	<owl:DatatypeProperty rdf:ID="measperf_att.tremmeasured.attribute.measperf__mei_data.DURATION.cmn">
		<rdfs:range rdf:resource="&datatypes;data.DURATION.cmn"/>
		<rdfs:label>measperf</rdfs:label>
	<rdfs:comment>The performed duration of an individual note in a measured tremolo.</rdfs:comment>
	</owl:DatatypeProperty>
	<owl:DatatypeProperty rdf:ID="bracket.place_att.tuplet.vis.attribute.bracket.place__mei_data.PLACE">
		<rdfs:range rdf:resource="&datatypes;data.PLACE"/>
		<rdfs:label>bracket.place</rdfs:label>
	<rdfs:comment>Used to state where a tuplet bracket will be placed in relation to the note heads.</rdfs:comment>
	</owl:DatatypeProperty>
	<owl:DatatypeProperty rdf:ID="bracket.visible_att.tuplet.vis.attribute.bracket.visible__mei_data.BOOLEAN">
		<rdfs:range rdf:resource="&datatypes;data.BOOLEAN"/>
		<rdfs:label>bracket.visible</rdfs:label>
	<rdfs:comment>States whether a bracket should be rendered with a tuplet.</rdfs:comment>
	</owl:DatatypeProperty>
	<owl:DatatypeProperty rdf:ID="dur.visible_att.tuplet.vis.attribute.dur.visible__mei_data.BOOLEAN">
		<rdfs:range rdf:resource="&datatypes;data.BOOLEAN"/>
		<rdfs:label>dur.visible</rdfs:label>
	<rdfs:comment>Determines if the tuplet duration is visible.</rdfs:comment>
	</owl:DatatypeProperty>
	<rdfs:Datatype rdf:ID="NS_num.format_att.tuplet.vis.attribute.num.format_UNType">
		<owl:equivalentClass><rdfs:Datatype>
		<owl:onDatatype rdf:resource="&xs;token"/><owl:withRestrictions rdf:parseType="Collection"><rdf:Description><xs:enumeration>count</xs:enumeration></rdf:Description><rdf:Description><xs:enumeration>ratio</xs:enumeration></rdf:Description></owl:withRestrictions></rdfs:Datatype></owl:equivalentClass></rdfs:Datatype>
	<owl:DatatypeProperty rdf:ID="num.format_att.tuplet.vis.attribute.num.format__NS_num.format_att.tuplet.vis.attribute.num.format_UNType">
		<rdfs:range rdf:resource="#NS_num.format_att.tuplet.vis.attribute.num.format_UNType"/>
		<rdfs:label>num.format</rdfs:label>
	<rdfs:comment>Controls how the num:numbase ratio is to be displayed.</rdfs:comment>
	</owl:DatatypeProperty>
	<owl:DatatypeProperty rdf:ID="form_att.ligature.log.attribute.form__mei_data.LIGATUREFORM">
		<rdfs:range rdf:resource="&datatypes;data.LIGATUREFORM"/>
		<rdfs:label>form</rdfs:label>
	<rdfs:comment>Provides an indication of the function of the ligature.</rdfs:comment>
	</owl:DatatypeProperty>
	<rdfs:Datatype rdf:ID="NS_form_att.mensur.vis.attribute.form_UNType">
		<owl:equivalentClass><rdfs:Datatype>
		<owl:onDatatype rdf:resource="&xs;token"/><owl:withRestrictions rdf:parseType="Collection"><rdf:Description><xs:enumeration>horizontal</xs:enumeration></rdf:Description><rdf:Description><xs:enumeration>vertical</xs:enumeration></rdf:Description></owl:withRestrictions></rdfs:Datatype></owl:equivalentClass></rdfs:Datatype>
	<owl:DatatypeProperty rdf:ID="form_att.mensur.vis.attribute.form__NS_form_att.mensur.vis.attribute.form_UNType">
		<rdfs:range rdf:resource="#NS_form_att.mensur.vis.attribute.form_UNType"/>
		<rdfs:label>form</rdfs:label>
	<rdfs:comment>Indicates whether the base symbol is written vertically or horizontally.</rdfs:comment>
	</owl:DatatypeProperty>
	<owl:DatatypeProperty rdf:ID="orient_att.mensur.vis.attribute.orient__mei_data.ORIENTATION">
		<rdfs:range rdf:resource="&datatypes;data.ORIENTATION"/>
		<rdfs:label>orient</rdfs:label>
	<rdfs:comment>Describes the rotation or reflection of the base symbol.</rdfs:comment>
	</owl:DatatypeProperty>
	<owl:DatatypeProperty rdf:ID="mensur.dot_att.mensural.log.attribute.mensur.dot__mei_data.BOOLEAN">
		<rdfs:range rdf:resource="&datatypes;data.BOOLEAN"/>
		<rdfs:label>mensur.dot</rdfs:label>
	<rdfs:comment>Determines if a dot is to be added to the base symbol.</rdfs:comment>
	</owl:DatatypeProperty>
	<owl:DatatypeProperty rdf:ID="mensur.sign_att.mensural.log.attribute.mensur.sign__mei_data.MENSURATIONSIGN">
		<rdfs:range rdf:resource="&datatypes;data.MENSURATIONSIGN"/>
		<rdfs:label>mensur.sign</rdfs:label>
	<rdfs:comment>The base symbol in the mensuration sign/time signature of mensural notation.</rdfs:comment>
	</owl:DatatypeProperty>
	<owl:DatatypeProperty rdf:ID="mensur.slash_att.mensural.log.attribute.mensur.slash__xs_positiveInteger">
		<rdfs:range rdf:resource="&xs;positiveInteger"/>
		<rdfs:label>mensur.slash</rdfs:label>
	<rdfs:comment>Indicates the number lines added to the mensuration sign. For example, one slash is added for what we now call 'alla breve'.</rdfs:comment>
	</owl:DatatypeProperty>
	<owl:DatatypeProperty rdf:ID="proport.num_att.mensural.log.attribute.proport.num__xs_positiveInteger">
		<rdfs:range rdf:resource="&xs;positiveInteger"/>
		<rdfs:label>proport.num</rdfs:label>
	<rdfs:comment>Together, proport.num and proport.numbase specify a proportional change as a ratio, e.g., 1:3. Proport.num is for the first value in the ratio.</rdfs:comment>
	</owl:DatatypeProperty>
	<owl:DatatypeProperty rdf:ID="proport.numbase_att.mensural.log.attribute.proport.numbase__xs_positiveInteger">
		<rdfs:range rdf:resource="&xs;positiveInteger"/>
		<rdfs:label>proport.numbase</rdfs:label>
	<rdfs:comment>Together, proport.num and proport.numbase specify a proportional change as a ratio, e.g., 1:3. Proport.numbase is for the second value in the ratio.</rdfs:comment>
	</owl:DatatypeProperty>
	<owl:DatatypeProperty rdf:ID="modusmaior_att.mensural.shared.attribute.modusmaior__mei_data.MODUSMAIOR">
		<rdfs:range rdf:resource="&datatypes;data.MODUSMAIOR"/>
		<rdfs:label>modusmaior</rdfs:label>
	<rdfs:comment>Describes the maxima-long relationship.</rdfs:comment>
	</owl:DatatypeProperty>
	<owl:DatatypeProperty rdf:ID="modusminor_att.mensural.shared.attribute.modusminor__mei_data.MODUSMINOR">
		<rdfs:range rdf:resource="&datatypes;data.MODUSMINOR"/>
		<rdfs:label>modusminor</rdfs:label>
	<rdfs:comment>Describes the long-breve relationship.</rdfs:comment>
	</owl:DatatypeProperty>
	<owl:DatatypeProperty rdf:ID="prolatio_att.mensural.shared.attribute.prolatio__mei_data.PROLATIO">
		<rdfs:range rdf:resource="&datatypes;data.PROLATIO"/>
		<rdfs:label>prolatio</rdfs:label>
	<rdfs:comment>Describes the semibreve-minim relationship.</rdfs:comment>
	</owl:DatatypeProperty>
	<owl:DatatypeProperty rdf:ID="tempus_att.mensural.shared.attribute.tempus__mei_data.TEMPUS">
		<rdfs:range rdf:resource="&datatypes;data.TEMPUS"/>
		<rdfs:label>tempus</rdfs:label>
	<rdfs:comment>Describes the breve-semibreve relationship.</rdfs:comment>
	</owl:DatatypeProperty>
	<owl:DatatypeProperty rdf:ID="mensur.color_att.mensural.vis.attribute.mensur.color__mei_data.COLOR">
		<rdfs:range rdf:resource="&datatypes;data.COLOR"/>
		<rdfs:label>mensur.color</rdfs:label>
	<rdfs:comment>Records the color of the mensuration sign. Do not confuse this with the musical term 'color' as used in pre-CMN notation.</rdfs:comment>
	</owl:DatatypeProperty>
	<rdfs:Datatype rdf:ID="NS_mensur.form_att.mensural.vis.attribute.mensur.form_UNType">
		<owl:equivalentClass><rdfs:Datatype>
		<owl:onDatatype rdf:resource="&xs;token"/><owl:withRestrictions rdf:parseType="Collection"><rdf:Description><xs:enumeration>horizontal</xs:enumeration></rdf:Description><rdf:Description><xs:enumeration>vertical</xs:enumeration></rdf:Description></owl:withRestrictions></rdfs:Datatype></owl:equivalentClass></rdfs:Datatype>
	<owl:DatatypeProperty rdf:ID="mensur.form_att.mensural.vis.attribute.mensur.form__NS_mensur.form_att.mensural.vis.attribute.mensur.form_UNType">
		<rdfs:range rdf:resource="#NS_mensur.form_att.mensural.vis.attribute.mensur.form_UNType"/>
		<rdfs:label>mensur.form</rdfs:label>
	<rdfs:comment>Indicates whether the base symbol is written vertically or horizontally.</rdfs:comment>
	</owl:DatatypeProperty>
	<owl:DatatypeProperty rdf:ID="mensur.loc_att.mensural.vis.attribute.mensur.loc__mei_data.STAFFLOC">
		<rdfs:range rdf:resource="&datatypes;data.STAFFLOC"/>
		<rdfs:label>mensur.loc</rdfs:label>
	<rdfs:comment>Holds the staff location of the mensuration sign.</rdfs:comment>
	</owl:DatatypeProperty>
	<owl:DatatypeProperty rdf:ID="mensur.orient_att.mensural.vis.attribute.mensur.orient__mei_data.ORIENTATION">
		<rdfs:range rdf:resource="&datatypes;data.ORIENTATION"/>
		<rdfs:label>mensur.orient</rdfs:label>
	<rdfs:comment>Describes the rotation or reflection of the base symbol.</rdfs:comment>
	</owl:DatatypeProperty>
	<owl:DatatypeProperty rdf:ID="mensur.size_att.mensural.vis.attribute.mensur.size__mei_data.SIZE">
		<rdfs:range rdf:resource="&datatypes;data.SIZE"/>
		<rdfs:label>mensur.size</rdfs:label>
	<rdfs:comment>Describes the relative size of the mensuration sign.</rdfs:comment>
	</owl:DatatypeProperty>
	<rdfs:Datatype rdf:ID="NS_lig_att.note.log.mensural.attribute.lig_UNType">
		<owl:equivalentClass><rdfs:Datatype>
		<owl:onDatatype rdf:resource="&xs;token"/><owl:withRestrictions rdf:parseType="Collection"><rdf:Description><xs:enumeration>recta</xs:enumeration></rdf:Description><rdf:Description><xs:enumeration>obliqua</xs:enumeration></rdf:Description></owl:withRestrictions></rdfs:Datatype></owl:equivalentClass></rdfs:Datatype>
	<owl:DatatypeProperty rdf:ID="lig_att.note.log.mensural.attribute.lig__NS_lig_att.note.log.mensural.attribute.lig_UNType">
		<rdfs:range rdf:resource="#NS_lig_att.note.log.mensural.attribute.lig_UNType"/>
		<rdfs:label>lig</rdfs:label>
	<rdfs:comment>Indicates this element's participation in a ligature.</rdfs:comment>
	</owl:DatatypeProperty>
	<owl:DatatypeProperty rdf:ID="spaces_att.rest.vis.mensural.attribute.spaces__xs_positiveInteger">
		<rdfs:range rdf:resource="&xs;positiveInteger"/>
		<rdfs:label>spaces</rdfs:label>
	<rdfs:comment>States how many spaces are covered by the rest.</rdfs:comment>
	</owl:DatatypeProperty>
	<owl:DatatypeProperty rdf:ID="form_att.ineume.log.attribute.form__mei_data.INEUMEFORM">
		<rdfs:range rdf:resource="&datatypes;data.INEUMEFORM"/>
		<rdfs:label>form</rdfs:label>
	<rdfs:comment>Provides a subclass or functional label for the neume.</rdfs:comment>
	</owl:DatatypeProperty>
	<owl:DatatypeProperty rdf:ID="name_att.ineume.log.attribute.name__mei_data.INEUMENAME">
		<rdfs:range rdf:resource="&datatypes;data.INEUMENAME"/>
		<rdfs:label>name</rdfs:label>
	<rdfs:comment>Records the name of the neume.</rdfs:comment>
	</owl:DatatypeProperty>
	<owl:DatatypeProperty rdf:ID="form_att.uneume.log.attribute.form__mei_data.UNEUMEFORM">
		<rdfs:range rdf:resource="&datatypes;data.UNEUMEFORM"/>
		<rdfs:label>form</rdfs:label>
	<rdfs:comment>Provides a subclass or functional label for the neume.</rdfs:comment>
	</owl:DatatypeProperty>
	<owl:DatatypeProperty rdf:ID="name_att.uneume.log.attribute.name__mei_data.UNEUMENAME">
		<rdfs:range rdf:resource="&datatypes;data.UNEUMENAME"/>
		<rdfs:label>name</rdfs:label>
	<rdfs:comment>Records the name of the neume.</rdfs:comment>
	</owl:DatatypeProperty>
	<owl:DatatypeProperty rdf:ID="copyof_att.common.anl.attribute.copyof__mei_data.URI">
		<rdfs:range rdf:resource="&datatypes;data.URI"/>
		<rdfs:label>copyof</rdfs:label>
	<rdfs:comment>Points to an element of which the current element is a copy.</rdfs:comment>
	</owl:DatatypeProperty>
	<rdfs:Datatype rdf:ID="NS_corresp_att.common.anl.attribute.corresp_UNType">
		<owl:equivalentClass><rdfs:Datatype>
		<owl:onDatatype rdf:resource="corresp_att.common.anl.attribute.corresp_NS_corresp_att.common.anl.attribute.corresp_UNType_UNType"/><owl:withRestrictions rdf:parseType="Collection"><rdf:Description><xs:minLength>1</xs:minLength></rdf:Description></owl:withRestrictions></rdfs:Datatype></owl:equivalentClass></rdfs:Datatype>
	<rdfs:Datatype rdf:ID="corresp_att.common.anl.attribute.corresp_NS_corresp_att.common.anl.attribute.corresp_UNType_UNType">
		<owl:equivalentClass><rdfs:Datatype>
		<owl:oneOf><rdf:Description><rdf:type rdf:resource="#List"/><rdf:first>mei:data.URI</rdf:first><rdf:rest rdf:resource="#nil"/></rdf:Description></owl:oneOf></rdfs:Datatype></owl:equivalentClass></rdfs:Datatype>
	<owl:DatatypeProperty rdf:ID="corresp_att.common.anl.attribute.corresp__NS_corresp_att.common.anl.attribute.corresp_UNType">
		<rdfs:range rdf:resource="#NS_corresp_att.common.anl.attribute.corresp_UNType"/>
		<rdfs:label>corresp</rdfs:label>
	<rdfs:comment>Used to point to other elements that correspond to this one in a generic fashion.</rdfs:comment>
	</owl:DatatypeProperty>
	<rdfs:Datatype rdf:ID="NS_next_att.common.anl.attribute.next_UNType">
		<owl:equivalentClass><rdfs:Datatype>
		<owl:onDatatype rdf:resource="next_att.common.anl.attribute.next_NS_next_att.common.anl.attribute.next_UNType_UNType"/><owl:withRestrictions rdf:parseType="Collection"><rdf:Description><xs:minLength>1</xs:minLength></rdf:Description></owl:withRestrictions></rdfs:Datatype></owl:equivalentClass></rdfs:Datatype>
	<rdfs:Datatype rdf:ID="next_att.common.anl.attribute.next_NS_next_att.common.anl.attribute.next_UNType_UNType">
		<owl:equivalentClass><rdfs:Datatype>
		<owl:oneOf><rdf:Description><rdf:type rdf:resource="#List"/><rdf:first>mei:data.URI</rdf:first><rdf:rest rdf:resource="#nil"/></rdf:Description></owl:oneOf></rdfs:Datatype></owl:equivalentClass></rdfs:Datatype>
	<owl:DatatypeProperty rdf:ID="next_att.common.anl.attribute.next__NS_next_att.common.anl.attribute.next_UNType">
		<rdfs:range rdf:resource="#NS_next_att.common.anl.attribute.next_UNType"/>
		<rdfs:label>next</rdfs:label>
	<rdfs:comment>Used to point to the next event(s) in a user-defined collection.</rdfs:comment>
	</owl:DatatypeProperty>
	<rdfs:Datatype rdf:ID="NS_prev_att.common.anl.attribute.prev_UNType">
		<owl:equivalentClass><rdfs:Datatype>
		<owl:onDatatype rdf:resource="prev_att.common.anl.attribute.prev_NS_prev_att.common.anl.attribute.prev_UNType_UNType"/><owl:withRestrictions rdf:parseType="Collection"><rdf:Description><xs:minLength>1</xs:minLength></rdf:Description></owl:withRestrictions></rdfs:Datatype></owl:equivalentClass></rdfs:Datatype>
	<rdfs:Datatype rdf:ID="prev_att.common.anl.attribute.prev_NS_prev_att.common.anl.attribute.prev_UNType_UNType">
		<owl:equivalentClass><rdfs:Datatype>
		<owl:oneOf><rdf:Description><rdf:type rdf:resource="#List"/><rdf:first>mei:data.URI</rdf:first><rdf:rest rdf:resource="#nil"/></rdf:Description></owl:oneOf></rdfs:Datatype></owl:equivalentClass></rdfs:Datatype>
	<owl:DatatypeProperty rdf:ID="prev_att.common.anl.attribute.prev__NS_prev_att.common.anl.attribute.prev_UNType">
		<rdfs:range rdf:resource="#NS_prev_att.common.anl.attribute.prev_UNType"/>
		<rdfs:label>prev</rdfs:label>
	<rdfs:comment>Points to the previous event(s) in a user-defined collection.</rdfs:comment>
	</owl:DatatypeProperty>
	<rdfs:Datatype rdf:ID="NS_sameas_att.common.anl.attribute.sameas_UNType">
		<owl:equivalentClass><rdfs:Datatype>
		<owl:onDatatype rdf:resource="sameas_att.common.anl.attribute.sameas_NS_sameas_att.common.anl.attribute.sameas_UNType_UNType"/><owl:withRestrictions rdf:parseType="Collection"><rdf:Description><xs:minLength>1</xs:minLength></rdf:Description></owl:withRestrictions></rdfs:Datatype></owl:equivalentClass></rdfs:Datatype>
	<rdfs:Datatype rdf:ID="sameas_att.common.anl.attribute.sameas_NS_sameas_att.common.anl.attribute.sameas_UNType_UNType">
		<owl:equivalentClass><rdfs:Datatype>
		<owl:oneOf><rdf:Description><rdf:type rdf:resource="#List"/><rdf:first>mei:data.URI</rdf:first><rdf:rest rdf:resource="#nil"/></rdf:Description></owl:oneOf></rdfs:Datatype></owl:equivalentClass></rdfs:Datatype>
	<owl:DatatypeProperty rdf:ID="sameas_att.common.anl.attribute.sameas__NS_sameas_att.common.anl.attribute.sameas_UNType">
		<rdfs:range rdf:resource="#NS_sameas_att.common.anl.attribute.sameas_UNType"/>
		<rdfs:label>sameas</rdfs:label>
	<rdfs:comment>Points to an element that is the same as the current element but is not a literal copy of the current element.</rdfs:comment>
	</owl:DatatypeProperty>
	<rdfs:Datatype rdf:ID="NS_synch_att.common.anl.attribute.synch_UNType">
		<owl:equivalentClass><rdfs:Datatype>
		<owl:onDatatype rdf:resource="synch_att.common.anl.attribute.synch_NS_synch_att.common.anl.attribute.synch_UNType_UNType"/><owl:withRestrictions rdf:parseType="Collection"><rdf:Description><xs:minLength>1</xs:minLength></rdf:Description></owl:withRestrictions></rdfs:Datatype></owl:equivalentClass></rdfs:Datatype>
	<rdfs:Datatype rdf:ID="synch_att.common.anl.attribute.synch_NS_synch_att.common.anl.attribute.synch_UNType_UNType">
		<owl:equivalentClass><rdfs:Datatype>
		<owl:oneOf><rdf:Description><rdf:type rdf:resource="#List"/><rdf:first>mei:data.URI</rdf:first><rdf:rest rdf:resource="#nil"/></rdf:Description></owl:oneOf></rdfs:Datatype></owl:equivalentClass></rdfs:Datatype>
	<owl:DatatypeProperty rdf:ID="synch_att.common.anl.attribute.synch__NS_synch_att.common.anl.attribute.synch_UNType">
		<rdfs:range rdf:resource="#NS_synch_att.common.anl.attribute.synch_UNType"/>
		<rdfs:label>synch</rdfs:label>
	<rdfs:comment>Points to elements that are synchronous with the current element.</rdfs:comment>
	</owl:DatatypeProperty>
	<owl:DatatypeProperty rdf:ID="deg_att.harmonicfunction.attribute.deg__mei_data.SCALEDEGREE">
		<rdfs:range rdf:resource="&datatypes;data.SCALEDEGREE"/>
		<rdfs:label>deg</rdfs:label>
	<rdfs:comment>Captures relative scale degree information using Humdrum **deg syntax -- an optional indicator of melodic approach (^ = ascending approach, v = descending approach), a scale degree value (1 = tonic ... 7 = leading tone), and an optional indication of chromatic alteration. The amount of chromatic alternation is not indicated.</rdfs:comment>
	</owl:DatatypeProperty>
	<rdfs:Datatype rdf:ID="NS_inth_att.intervalharmonic.attribute.inth_UNType">
		<owl:equivalentClass><rdfs:Datatype>
		<owl:onDatatype rdf:resource="inth_att.intervalharmonic.attribute.inth_NS_inth_att.intervalharmonic.attribute.inth_UNType_UNType"/><owl:withRestrictions rdf:parseType="Collection"><rdf:Description><xs:minLength>1</xs:minLength></rdf:Description></owl:withRestrictions></rdfs:Datatype></owl:equivalentClass></rdfs:Datatype>
	<rdfs:Datatype rdf:ID="inth_att.intervalharmonic.attribute.inth_NS_inth_att.intervalharmonic.attribute.inth_UNType_UNType">
		<owl:equivalentClass><rdfs:Datatype>
		<owl:oneOf><rdf:Description><rdf:type rdf:resource="#List"/><rdf:first>mei:data.INTERVAL.HARMONIC</rdf:first><rdf:rest rdf:resource="#nil"/></rdf:Description></owl:oneOf></rdfs:Datatype></owl:equivalentClass></rdfs:Datatype>
	<owl:DatatypeProperty rdf:ID="inth_att.intervalharmonic.attribute.inth__NS_inth_att.intervalharmonic.attribute.inth_UNType">
		<rdfs:range rdf:resource="#NS_inth_att.intervalharmonic.attribute.inth_UNType"/>
		<rdfs:label>inth</rdfs:label>
	<rdfs:comment>Encodes the harmonic interval between pitches occurring at the same time.</rdfs:comment>
	</owl:DatatypeProperty>
	<owl:DatatypeProperty rdf:ID="intm_att.intervalmelodic.attribute.intm__mei_data.INTERVAL.MELODIC">
		<rdfs:range rdf:resource="&datatypes;data.INTERVAL.MELODIC"/>
		<rdfs:label>intm</rdfs:label>
	<rdfs:comment>Encodes the melodic interval from the previous pitch. The value may be a general directional indication (u, d, s), an indication of diatonic interval direction, quality, and size, or a precise numeric value in half steps.</rdfs:comment>
	</owl:DatatypeProperty>
	<owl:DatatypeProperty rdf:ID="mfunc_att.melodicfunction.attribute.mfunc__mei_data.MELODICFUNCTION">
		<rdfs:range rdf:resource="&datatypes;data.MELODICFUNCTION"/>
		<rdfs:label>mfunc</rdfs:label>
	<rdfs:comment>Describes melodic function using Humdrum **embel syntax.</rdfs:comment>
	</owl:DatatypeProperty>
	<owl:DatatypeProperty rdf:ID="pclass_att.pitchclass.attribute.pclass__mei_data.PITCHCLASS">
		<rdfs:range rdf:resource="&datatypes;data.PITCHCLASS"/>
		<rdfs:label>pclass</rdfs:label>
	<rdfs:comment>Holds pitch class information.</rdfs:comment>
	</owl:DatatypeProperty>
	<owl:DatatypeProperty rdf:ID="psolfa_att.solfa.attribute.psolfa__xs_NMTOKEN">
		<rdfs:range rdf:resource="&xs;NMTOKEN"/>
		<rdfs:label>psolfa</rdfs:label>
	<rdfs:comment>Contains sol-fa designation, e.g., do, re, mi, etc., in either a fixed or movable Do system.</rdfs:comment>
	</owl:DatatypeProperty>
	<rdfs:Datatype rdf:ID="NS_form_att.mordent.log.attribute.form_UNType">
		<owl:equivalentClass><rdfs:Datatype>
		<owl:onDatatype rdf:resource="&xs;token"/><owl:withRestrictions rdf:parseType="Collection"><rdf:Description><xs:enumeration>inv</xs:enumeration></rdf:Description><rdf:Description><xs:enumeration>norm</xs:enumeration></rdf:Description></owl:withRestrictions></rdfs:Datatype></owl:equivalentClass></rdfs:Datatype>
	<owl:DatatypeProperty rdf:ID="form_att.mordent.log.attribute.form__NS_form_att.mordent.log.attribute.form_UNType">
		<rdfs:range rdf:resource="#NS_form_att.mordent.log.attribute.form_UNType"/>
		<rdfs:label>form</rdfs:label>
	<rdfs:comment>Traditionally, the 'normal' mordent is written as a short wavy line with a vertical line through it and the inverted mordent is written without the vertical line. However, the meaning of these signs is sometimes reversed. See Read, p. 245-246. Another attribute in the visual domain would be necessary in order to be completely explicit about which visual symbol is actually to be rendered.</rdfs:comment>
	</owl:DatatypeProperty>
	<owl:DatatypeProperty rdf:ID="long_att.mordent.log.attribute.long__mei_data.BOOLEAN">
		<rdfs:range rdf:resource="&datatypes;data.BOOLEAN"/>
		<rdfs:label>long</rdfs:label>
	<rdfs:comment>When the long attribute is set to 'yes', a double or long mordent, consisting of 5 notes, is indicated.</rdfs:comment>
	</owl:DatatypeProperty>
	<rdfs:Datatype rdf:ID="NS_ornam_att.ornam.attribute.ornam_UNType">
		<owl:equivalentClass><rdfs:Datatype>
		<owl:onDatatype rdf:resource="ornam_att.ornam.attribute.ornam_NS_ornam_att.ornam.attribute.ornam_UNType_UNType"/><owl:withRestrictions rdf:parseType="Collection"><rdf:Description><xs:minLength>1</xs:minLength></rdf:Description></owl:withRestrictions></rdfs:Datatype></owl:equivalentClass></rdfs:Datatype>
	<rdfs:Datatype rdf:ID="ornam_att.ornam.attribute.ornam_NS_ornam_att.ornam.attribute.ornam_UNType_UNType">
		<owl:equivalentClass><rdfs:Datatype>
		<owl:oneOf><rdf:Description><rdf:type rdf:resource="#List"/><rdf:first>mei:data.ORNAM.cmn</rdf:first><rdf:rest rdf:resource="#nil"/></rdf:Description></owl:oneOf></rdfs:Datatype></owl:equivalentClass></rdfs:Datatype>
	<owl:DatatypeProperty rdf:ID="ornam_att.ornam.attribute.ornam__NS_ornam_att.ornam.attribute.ornam_UNType">
		<rdfs:range rdf:resource="#NS_ornam_att.ornam.attribute.ornam_UNType"/>
		<rdfs:label>ornam</rdfs:label>
	<rdfs:comment>Indicates that this element has an attached ornament. If visual information about the ornament is needed, then one of the elements that represents an ornament (mordent, trill, or turn) should be employed.</rdfs:comment>
	</owl:DatatypeProperty>
	<owl:DatatypeProperty rdf:ID="accidupper_att.ornamentaccid.attribute.accidupper__mei_data.ACCIDENTAL.EXPLICIT">
		<rdfs:range rdf:resource="&datatypes;data.ACCIDENTAL.EXPLICIT"/>
		<rdfs:label>accidupper</rdfs:label>
	<rdfs:comment>Records the written accidental associated with an upper neighboring note.</rdfs:comment>
	</owl:DatatypeProperty>
	<owl:DatatypeProperty rdf:ID="accidlower_att.ornamentaccid.attribute.accidlower__mei_data.ACCIDENTAL.EXPLICIT">
		<rdfs:range rdf:resource="&datatypes;data.ACCIDENTAL.EXPLICIT"/>
		<rdfs:label>accidlower</rdfs:label>
	<rdfs:comment>Records the written accidental associated with a lower neighboring note.</rdfs:comment>
	</owl:DatatypeProperty>
	<owl:DatatypeProperty rdf:ID="delayed_att.turn.log.attribute.delayed__mei_data.BOOLEAN">
		<rdfs:range rdf:resource="&datatypes;data.BOOLEAN"/>
		<rdfs:label>delayed</rdfs:label>
	<rdfs:comment>When the delayed attribute is set to 'true', the turn begins on the second half of the beat. See Read, p. 246.</rdfs:comment>
	</owl:DatatypeProperty>
	<rdfs:Datatype rdf:ID="NS_form_att.turn.log.attribute.form_UNType">
		<owl:equivalentClass><rdfs:Datatype>
		<owl:onDatatype rdf:resource="&xs;token"/><owl:withRestrictions rdf:parseType="Collection"><rdf:Description><xs:enumeration>inv</xs:enumeration></rdf:Description><rdf:Description><xs:enumeration>norm</xs:enumeration></rdf:Description></owl:withRestrictions></rdfs:Datatype></owl:equivalentClass></rdfs:Datatype>
	<owl:DatatypeProperty rdf:ID="form_att.turn.log.attribute.form__NS_form_att.turn.log.attribute.form_UNType">
		<rdfs:range rdf:resource="#NS_form_att.turn.log.attribute.form_UNType"/>
		<rdfs:label>form</rdfs:label>
	<rdfs:comment>Indicates the style of the turn.</rdfs:comment>
	</owl:DatatypeProperty>
	<owl:DatatypeProperty rdf:ID="cause_att.crit.attribute.cause__xs_NMTOKEN">
		<rdfs:range rdf:resource="&xs;NMTOKEN"/>
		<rdfs:label>cause</rdfs:label>
	<rdfs:comment>Classifies the cause for the variant reading, according to any appropriate typology of possible origins.</rdfs:comment>
	</owl:DatatypeProperty>
	<rdfs:Datatype rdf:ID="NS_source_att.source.attribute.source_UNType">
		<owl:equivalentClass><rdfs:Datatype>
		<owl:onDatatype rdf:resource="source_att.source.attribute.source_NS_source_att.source.attribute.source_UNType_UNType"/><owl:withRestrictions rdf:parseType="Collection"><rdf:Description><xs:minLength>1</xs:minLength></rdf:Description></owl:withRestrictions></rdfs:Datatype></owl:equivalentClass></rdfs:Datatype>
	<rdfs:Datatype rdf:ID="source_att.source.attribute.source_NS_source_att.source.attribute.source_UNType_UNType">
		<owl:equivalentClass><rdfs:Datatype>
		<owl:oneOf><rdf:Description><rdf:type rdf:resource="#List"/><rdf:first>mei:data.URI</rdf:first><rdf:rest rdf:resource="#nil"/></rdf:Description></owl:oneOf></rdfs:Datatype></owl:equivalentClass></rdfs:Datatype>
	<owl:DatatypeProperty rdf:ID="source_att.source.attribute.source__NS_source_att.source.attribute.source_UNType">
		<rdfs:range rdf:resource="#NS_source_att.source.attribute.source_UNType"/>
		<rdfs:label>source</rdfs:label>
	<rdfs:comment>Contains a list of one or more pointers indicating the sources which attest to a given reading. Each value should correspond to the ID of a &lt;source&gt; element located in the document header.</rdfs:comment>
	</owl:DatatypeProperty>
	<owl:DatatypeProperty rdf:ID="agent_att.agentident.attribute.agent__xs_string">
		<rdfs:range rdf:resource="&xs;string"/>
		<rdfs:label>agent</rdfs:label>
	<rdfs:comment>Signifies the causative agent of damage, illegibility, or other loss of original text.</rdfs:comment>
	</owl:DatatypeProperty>
	<owl:DatatypeProperty rdf:ID="cert_att.evidence.attribute.cert__mei_data.CERTAINTY">
		<rdfs:range rdf:resource="&datatypes;data.CERTAINTY"/>
		<rdfs:label>cert</rdfs:label>
	<rdfs:comment>Signifies the degree of certainty or precision associated with a feature.</rdfs:comment>
	</owl:DatatypeProperty>
	<owl:DatatypeProperty rdf:ID="evidence_att.evidence.attribute.evidence__xs_NMTOKEN">
		<rdfs:range rdf:resource="&xs;NMTOKEN"/>
		<rdfs:label>evidence</rdfs:label>
	<rdfs:comment>Indicates the nature of the evidence supporting the reliability or accuracy of the intervention or interpretation. Suggested values include: 'internal', 'external', 'conjecture'.</rdfs:comment>
	</owl:DatatypeProperty>
	<owl:DatatypeProperty rdf:ID="extent_att.extent.attribute.extent__xs_string">
		<rdfs:range rdf:resource="&xs;string"/>
		<rdfs:label>extent</rdfs:label>
	<rdfs:comment>Indicates the extent of damage or omission.</rdfs:comment>
	</owl:DatatypeProperty>
	<owl:DatatypeProperty rdf:ID="reason_att.reasonident.attribute.reason__xs_string">
		<rdfs:range rdf:resource="&xs;string"/>
		<rdfs:label>reason</rdfs:label>
	<rdfs:comment>Holds a short phrase describing the reason for missing textual material (gap), why material is supplied (supplied), or why transcription is difficult (unclear).</rdfs:comment>
	</owl:DatatypeProperty>
	<rdfs:Datatype rdf:ID="NS_facs_att.facsimile.attribute.facs_UNType">
		<owl:equivalentClass><rdfs:Datatype>
		<owl:onDatatype rdf:resource="facs_att.facsimile.attribute.facs_NS_facs_att.facsimile.attribute.facs_UNType_UNType"/><owl:withRestrictions rdf:parseType="Collection"><rdf:Description><xs:minLength>1</xs:minLength></rdf:Description></owl:withRestrictions></rdfs:Datatype></owl:equivalentClass></rdfs:Datatype>
	<rdfs:Datatype rdf:ID="facs_att.facsimile.attribute.facs_NS_facs_att.facsimile.attribute.facs_UNType_UNType">
		<owl:equivalentClass><rdfs:Datatype>
		<owl:oneOf><rdf:Description><rdf:type rdf:resource="#List"/><rdf:first>mei:data.URI</rdf:first><rdf:rest rdf:resource="#nil"/></rdf:Description></owl:oneOf></rdfs:Datatype></owl:equivalentClass></rdfs:Datatype>
	<owl:DatatypeProperty rdf:ID="facs_att.facsimile.attribute.facs__NS_facs_att.facsimile.attribute.facs_UNType">
		<rdfs:range rdf:resource="#NS_facs_att.facsimile.attribute.facs_UNType"/>
		<rdfs:label>facs</rdfs:label>
	<rdfs:comment>Permits the current element to reference a facsimile surface or image zone which corresponds to it.</rdfs:comment>
	</owl:DatatypeProperty>
	<owl:DatatypeProperty rdf:ID="colspan_att.tabular.attribute.colspan__xs_positiveInteger">
		<rdfs:range rdf:resource="&xs;positiveInteger"/>
		<rdfs:label>colspan</rdfs:label>
	<rdfs:comment>The number of columns spanned by this cell.</rdfs:comment>
	</owl:DatatypeProperty>
	<owl:DatatypeProperty rdf:ID="rowspan_att.tabular.attribute.rowspan__xs_positiveInteger">
		<rdfs:range rdf:resource="&xs;positiveInteger"/>
		<rdfs:label>rowspan</rdfs:label>
	<rdfs:comment>The number of rows spanned by this cell.</rdfs:comment>
	</owl:DatatypeProperty>
	<owl:DatatypeProperty rdf:ID="fret_att.fretlocation.attribute.fret__mei_data.FRET">
		<rdfs:range rdf:resource="&datatypes;data.FRET"/>
		<rdfs:label>fret</rdfs:label>
	<rdfs:comment>Records the location at which a string should be stopped against a fret.</rdfs:comment>
	</owl:DatatypeProperty>
	<owl:DatatypeProperty rdf:ID="chordref_att.harm.log.attribute.chordref__mei_data.URI">
		<rdfs:range rdf:resource="&datatypes;data.URI"/>
		<rdfs:label>chordref</rdfs:label>
	<rdfs:comment>Contains a reference to a &lt;chordDef&gt; element elsewhere in the document.</rdfs:comment>
	</owl:DatatypeProperty>
	<rdfs:Datatype rdf:ID="NS_rendgrid_att.harm.vis.attribute.rendgrid_UNType">
		<owl:equivalentClass><rdfs:Datatype>
		<owl:onDatatype rdf:resource="&xs;token"/><owl:withRestrictions rdf:parseType="Collection"><rdf:Description><xs:enumeration>grid</xs:enumeration></rdf:Description><rdf:Description><xs:enumeration>gridtext</xs:enumeration></rdf:Description><rdf:Description><xs:enumeration>text</xs:enumeration></rdf:Description></owl:withRestrictions></rdfs:Datatype></owl:equivalentClass></rdfs:Datatype>
	<owl:DatatypeProperty rdf:ID="rendgrid_att.harm.vis.attribute.rendgrid__NS_rendgrid_att.harm.vis.attribute.rendgrid_UNType">
		<rdfs:range rdf:resource="#NS_rendgrid_att.harm.vis.attribute.rendgrid_UNType"/>
		<rdfs:label>rendgrid</rdfs:label>
	<rdfs:comment>Describes how the harmonic indication should be rendered.</rdfs:comment>
	</owl:DatatypeProperty>
	<owl:DatatypeProperty rdf:ID="refrain_att.verse.log.attribute.refrain__mei_data.BOOLEAN">
		<rdfs:range rdf:resource="&datatypes;data.BOOLEAN"/>
		<rdfs:label>refrain</rdfs:label>
	<rdfs:comment>Used to indicate a common, usually centered, refrain.</rdfs:comment>
	</owl:DatatypeProperty>
	<owl:DatatypeProperty rdf:ID="rhythm_att.verse.log.attribute.rhythm__xs_string">
		<rdfs:range rdf:resource="&xs;string"/>
		<rdfs:label>rhythm</rdfs:label>
	<rdfs:comment>Used to specify a rhythm for the lyric syllables that differs from that of the notes on the staff, e.g. '4,4,4,4' when the rhythm of the notes is '4.,8,4.,8'.</rdfs:comment>
	</owl:DatatypeProperty>
	<owl:DatatypeProperty rdf:ID="midi.channel_att.channelized.attribute.midi.channel__mei_data.MIDICHANNEL">
		<rdfs:range rdf:resource="&datatypes;data.MIDICHANNEL"/>
		<rdfs:label>midi.channel</rdfs:label>
	<rdfs:comment>Records a MIDI channel value.</rdfs:comment>
	</owl:DatatypeProperty>
	<owl:DatatypeProperty rdf:ID="midi.duty_att.channelized.attribute.midi.duty__mei_data.PERCENT">
		<rdfs:range rdf:resource="&datatypes;data.PERCENT"/>
		<rdfs:label>midi.duty</rdfs:label>
	<rdfs:comment>Specifies the 'on' part of the duty cycle as a percentage of a note's duration.</rdfs:comment>
	</owl:DatatypeProperty>
	<owl:DatatypeProperty rdf:ID="midi.port_att.channelized.attribute.midi.port__mei_data.MIDIVALUE">
		<rdfs:range rdf:resource="&datatypes;data.MIDIVALUE"/>
		<rdfs:label>midi.port</rdfs:label>
	<rdfs:comment>Sets the MIDI port value.</rdfs:comment>
	</owl:DatatypeProperty>
	<owl:DatatypeProperty rdf:ID="midi.track_att.channelized.attribute.midi.track__xs_positiveInteger">
		<rdfs:range rdf:resource="&xs;positiveInteger"/>
		<rdfs:label>midi.track</rdfs:label>
	<rdfs:comment>Sets the MIDI track.</rdfs:comment>
	</owl:DatatypeProperty>
	<owl:DatatypeProperty rdf:ID="midi.instrnum_att.midiinstrument.attribute.midi.instrnum__mei_data.MIDIVALUE">
		<rdfs:range rdf:resource="&datatypes;data.MIDIVALUE"/>
		<rdfs:label>midi.instrnum</rdfs:label>
	<rdfs:comment>Sets the MIDI instrument number.</rdfs:comment>
	</owl:DatatypeProperty>
	<owl:DatatypeProperty rdf:ID="midi.instrname_att.midiinstrument.attribute.midi.instrname__mei_data.MIDINAMES">
		<rdfs:range rdf:resource="&datatypes;data.MIDINAMES"/>
		<rdfs:label>midi.instrname</rdfs:label>
	<rdfs:comment>Provides a General MIDI label for the MIDI instrument.</rdfs:comment>
	</owl:DatatypeProperty>
	<owl:DatatypeProperty rdf:ID="midi.pan_att.midiinstrument.attribute.midi.pan__mei_data.MIDIVALUE">
		<rdfs:range rdf:resource="&datatypes;data.MIDIVALUE"/>
		<rdfs:label>midi.pan</rdfs:label>
	<rdfs:comment>Sets the instrument's position in a stereo field. Values of 0 and 1 both pan left, 127 pans right, and 64 pans to the center.</rdfs:comment>
	</owl:DatatypeProperty>
	<owl:DatatypeProperty rdf:ID="midi.volume_att.midiinstrument.attribute.midi.volume__mei_data.MIDIVALUE">
		<rdfs:range rdf:resource="&datatypes;data.MIDIVALUE"/>
		<rdfs:label>midi.volume</rdfs:label>
	<rdfs:comment>Sets the instrument's volume.</rdfs:comment>
	</owl:DatatypeProperty>
	<owl:DatatypeProperty rdf:ID="num_att.midinumber.attribute.num__mei_data.MIDIVALUE">
		<rdfs:range rdf:resource="&datatypes;data.MIDIVALUE"/>
		<rdfs:label>num</rdfs:label>
	<rdfs:comment>MIDI number in the range set by data.MIDIVALUE.</rdfs:comment>
	</owl:DatatypeProperty>
	<owl:DatatypeProperty rdf:ID="midi.bpm_att.miditempo.attribute.midi.bpm__mei_data.MIDIBPM">
		<rdfs:range rdf:resource="&datatypes;data.MIDIBPM"/>
		<rdfs:label>midi.bpm</rdfs:label>
	<rdfs:comment>Captures the number of *quarter notes* per minute. In MIDI, a beat is always defined as a quarter note, *not the numerator of the time signature or the metronomic indication*.</rdfs:comment>
	</owl:DatatypeProperty>
	<owl:DatatypeProperty rdf:ID="midi.mspb_att.miditempo.attribute.midi.mspb__mei_data.MIDIMSPB">
		<rdfs:range rdf:resource="&datatypes;data.MIDIMSPB"/>
		<rdfs:label>midi.mspb</rdfs:label>
	<rdfs:comment>Records the number of microseconds per *quarter note*. In MIDI, a beat is always defined as a quarter note, *not the numerator of the time signature or the metronomic indication*. At 120 quarter notes per minute, each quarter note will last 500,000 microseconds.</rdfs:comment>
	</owl:DatatypeProperty>
	<owl:DatatypeProperty rdf:ID="val_att.midivalue.attribute.val__mei_data.MIDIVALUE">
		<rdfs:range rdf:resource="&datatypes;data.MIDIVALUE"/>
		<rdfs:label>val</rdfs:label>
	<rdfs:comment>MIDI number.</rdfs:comment>
	</owl:DatatypeProperty>
	<owl:DatatypeProperty rdf:ID="val2_att.midivalue2.attribute.val2__mei_data.MIDIVALUE">
		<rdfs:range rdf:resource="&datatypes;data.MIDIVALUE"/>
		<rdfs:label>val2</rdfs:label>
	<rdfs:comment>MIDI number.</rdfs:comment>
	</owl:DatatypeProperty>
	<owl:DatatypeProperty rdf:ID="vel_att.midivelocity.attribute.vel__mei_data.MIDIVALUE">
		<rdfs:range rdf:resource="&datatypes;data.MIDIVALUE"/>
		<rdfs:label>vel</rdfs:label>
	<rdfs:comment>MIDI Note-on/off velocity.</rdfs:comment>
	</owl:DatatypeProperty>
	<owl:DatatypeProperty rdf:ID="ppq_att.timebase.attribute.ppq__xs_positiveInteger">
		<rdfs:range rdf:resource="&xs;positiveInteger"/>
		<rdfs:label>ppq</rdfs:label>
	<rdfs:comment>Indicates the number of pulses (sometimes referred to as ticks or divisions) per quarter note. Unlike MIDI, MEI permits different values for a score and individual staves.</rdfs:comment>
	</owl:DatatypeProperty>
	<owl:DatatypeProperty rdf:ID="when_att.alignment.attribute.when__mei_data.URI">
		<rdfs:range rdf:resource="&datatypes;data.URI"/>
		<rdfs:label>when</rdfs:label>
	<rdfs:comment>Indicates the point of occurrence of this feature along a time line. Its value must be the ID of a when element elsewhere in the document.</rdfs:comment>
	</owl:DatatypeProperty>
	<owl:DatatypeProperty rdf:ID="tab.fret_att.note.ges.tablature.attribute.tab.fret__mei_data.FRETNUMBER">
		<rdfs:range rdf:resource="&datatypes;data.FRETNUMBER"/>
		<rdfs:label>tab.fret</rdfs:label>
	<rdfs:comment>Records the fret at which a string should be stopped.</rdfs:comment>
	</owl:DatatypeProperty>
	<owl:DatatypeProperty rdf:ID="tab.string_att.note.ges.tablature.attribute.tab.string__mei_data.STRINGNUMBER">
		<rdfs:range rdf:resource="&datatypes;data.STRINGNUMBER"/>
		<rdfs:label>tab.string</rdfs:label>
	<rdfs:comment>Records which string is to be played.</rdfs:comment>
	</owl:DatatypeProperty>
	<rdfs:Datatype rdf:ID="NS_tab.strings_att.staffDef.ges.tablature.attribute.tab.strings_UNType">
		<owl:equivalentClass><rdfs:Datatype>
		<owl:onDatatype rdf:resource="tab.strings_att.staffDef.ges.tablature.attribute.tab.strings_NS_tab.strings_att.staffDef.ges.tablature.attribute.tab.strings_UNType_UNType"/><owl:withRestrictions rdf:parseType="Collection"><rdf:Description><xs:minLength>1</xs:minLength></rdf:Description></owl:withRestrictions></rdfs:Datatype></owl:equivalentClass></rdfs:Datatype>
	<rdfs:Datatype rdf:ID="tab.strings_att.staffDef.ges.tablature.attribute.tab.strings_NS_tab.strings_att.staffDef.ges.tablature.attribute.tab.strings_UNType_UNType">
		<owl:equivalentClass><rdfs:Datatype>
		<owl:oneOf><rdf:Description><rdf:type rdf:resource="#List"/><rdf:first>NS_tab.strings_att.staffDef.ges.tablature.attribute.tab.strings_UNType_tab.strings_att.staffDef.ges.tablature.attribute.tab.strings_NS_tab.strings_att.staffDef.ges.tablature.attribute.tab.strings_UNType_UNType_UNType</rdf:first><rdf:rest rdf:resource="#nil"/></rdf:Description></owl:oneOf></rdfs:Datatype></owl:equivalentClass></rdfs:Datatype>
	<rdfs:Datatype rdf:ID="NS_tab.strings_att.staffDef.ges.tablature.attribute.tab.strings_UNType_tab.strings_att.staffDef.ges.tablature.attribute.tab.strings_NS_tab.strings_att.staffDef.ges.tablature.attribute.tab.strings_UNType_UNType_UNType">
		<owl:equivalentClass><rdfs:Datatype>
		<owl:onDatatype rdf:resource="&xs;token"/><owl:withRestrictions rdf:parseType="Collection"><rdf:Description><xs:pattern>[a-g][0-9](s|f|ss|x|ff|xs|sx|ts|tf|n|nf|ns|su|sd|fu|fd|nu|nd|1qf|3qf|1qs|3qs)?([a-g][0-9](s|f|ss|x|ff|xs|sx|ts|tf|n|nf|ns|su|sd|fu|fd|nu|nd|1qf|3qf|1qs|3qs)?)*</xs:pattern></rdf:Description></owl:withRestrictions></rdfs:Datatype></owl:equivalentClass></rdfs:Datatype>
	<owl:DatatypeProperty rdf:ID="tab.strings_att.staffDef.ges.tablature.attribute.tab.strings__NS_tab.strings_att.staffDef.ges.tablature.attribute.tab.strings_UNType">
		<rdfs:range rdf:resource="#NS_tab.strings_att.staffDef.ges.tablature.attribute.tab.strings_UNType"/>
		<rdfs:label>tab.strings</rdfs:label>
	<rdfs:comment>Provides a *written* pitch and octave for each open string or course of strings.</rdfs:comment>
	</owl:DatatypeProperty>
	<owl:DatatypeProperty rdf:ID="altsym_att.altsym.attribute.altsym__mei_data.URI">
		<rdfs:range rdf:resource="&datatypes;data.URI"/>
		<rdfs:label>altsym</rdfs:label>
	<rdfs:comment>Provides a way of pointing to a user-defined symbol. It must contain an ID of a &lt;symbolDef&gt; element elsewhere in the document.</rdfs:comment>
	</owl:DatatypeProperty>
	<rdfs:Datatype rdf:ID="NS_snr_att.grammar.analysis.attribute.snr_UNType">
		<owl:equivalentClass><rdfs:Datatype>
		<owl:onDatatype rdf:resource="&xs;token"/><owl:withRestrictions rdf:parseType="Collection"><rdf:Description><xs:enumeration>\alpha</xs:enumeration></rdf:Description><rdf:Description><xs:enumeration>\beta</xs:enumeration></rdf:Description></owl:withRestrictions></rdfs:Datatype></owl:equivalentClass></rdfs:Datatype>
	<owl:DatatypeProperty rdf:ID="snr_att.grammar.analysis.attribute.snr__NS_snr_att.grammar.analysis.attribute.snr_UNType">
		<rdfs:range rdf:resource="#NS_snr_att.grammar.analysis.attribute.snr_UNType"/>
		<rdfs:label>snr</rdfs:label>
	<rdfs:comment>Syllabic Nuclear Reduction</rdfs:comment>
	</owl:DatatypeProperty>
	<rdfs:Datatype rdf:ID="NS_mnr_att.grammar.analysis.attribute.mnr_UNType">
		<owl:equivalentClass><rdfs:Datatype>
		<owl:onDatatype rdf:resource="&xs;token"/><owl:withRestrictions rdf:parseType="Collection"><rdf:Description><xs:enumeration>yes</xs:enumeration></rdf:Description><rdf:Description><xs:enumeration>no</xs:enumeration></rdf:Description></owl:withRestrictions></rdfs:Datatype></owl:equivalentClass></rdfs:Datatype>
	<owl:DatatypeProperty rdf:ID="mnr_att.grammar.analysis.attribute.mnr__NS_mnr_att.grammar.analysis.attribute.mnr_UNType">
		<rdfs:range rdf:resource="#NS_mnr_att.grammar.analysis.attribute.mnr_UNType"/>
		<rdfs:label>mnr</rdfs:label>
	<rdfs:comment>Metasyllabic Nuclear Reduction</rdfs:comment>
	</owl:DatatypeProperty>
	<owl:DatatypeProperty rdf:ID="number_att.grammar.numbering.attribute.number__xs_nonNegativeInteger">
		<rdfs:range rdf:resource="&xs;nonNegativeInteger"/>
		<rdfs:label>number</rdfs:label>
	<rdfs:comment>Number of an element used in the analysis</rdfs:comment>
	</owl:DatatypeProperty>
	</rdf:RDF>
